@prefix : <https://w3id.org/ad4gd/model/> .
@prefix qb: <http://purl.org/linked-data/cube#> .
@prefix dct: <http://purl.org/dc/terms/> .
@prefix owl: <http://www.w3.org/2002/07/owl#> .
@prefix rdf: <http://www.w3.org/1999/02/22-rdf-syntax-ns#> .
@prefix xml: <http://www.w3.org/XML/1998/namespace> .
@prefix xsd: <http://www.w3.org/2001/XMLSchema#> .
@prefix dcat: <http://www.w3.org/ns/dcat#> .
@prefix foaf: <http://xmlns.com/foaf/0.1/> .
@prefix qudt: <http://qudt.org/schema/qudt/> .
@prefix prov: <http://www.w3.org/ns/prov#> .
@prefix rdfs: <http://www.w3.org/2000/01/rdf-schema#> .
@prefix skos: <http://www.w3.org/2004/02/skos/core#> .
@prefix stat: <http://data.europa.eu/m8g/> .
@prefix schema: <https://schema.org/> .
@prefix af-inspire:	<http://inspire.ec.europa.eu/schemas/af/3.0#> .
@prefix act-inspire:	<http://inspire.ec.europa.eu/schemas/act-core/3.0#> .
@prefix foodie: <http://foodie-cloud.com/model/foodie#> .
@prefix saref4agri: <https://saref.etsi.org/saref4agri/> .
@prefix s4watr: <https://saref.etsi.org/saref4watr/> .
@prefix common: <http://portele.de/ont/inspire/baseInspire#> .
@prefix fiware: <https://smartdatamodels.org/> .
@prefix fiware-agrifood: <https://smartdatamodels.org/dataModel.Agrifood/> .
@prefix fiware-weather: <https://smartdatamodels.org/dataModel.Weather/> .
@prefix fiware-environment: <https://smartdatamodels.org/dataModel.Environment/> .
@prefix fiware-waterquality: <https://smartdatamodels.org/dataModel.WaterQuality/> .
@prefix iso19109: <http://def.seegrid.csiro.au/isotc211/iso19109/2005/feature#> .
@prefix iso19150-2: <http://def.seegrid.csiro.au/isotc211/iso19150/-2/2012/basic#> .
@prefix iso19103: <http://def.seegrid.csiro.au/isotc211/iso19103/2005/basic#> .
@prefix geo:   <http://www.opengis.net/ont/geosparql#> .
@prefix ssn: <http://www.w3.org/ns/ssn/> .
@prefix sosa: <http://www.w3.org/ns/sosa/> .
@prefix saref: <https://saref.etsi.org/core/> .
@prefix cf-feature: <http://purl.oclc.org/NET/ssnx/cf/cf-feature#> .
@prefix quantity: <http://purl.oclc.org/NET/ssnx/qu/quantity#> .
@prefix cf: <http://purl.oclc.org/NET/ssnx/cf/cf-property#> .
@prefix qu: <http://purl.oclc.org/NET/ssnx/qu/qu#> .
@prefix dim: <http://purl.oclc.org/NET/ssnx/qu/dim#> .
@prefix m3-lite: <http://purl.org/iot/vocab/m3-lite#> .
@base <https://w3id.org/ad4gd/model/> .

<https://w3id.org/ad4gd/model/gdProperty> a owl:Ontology ;
                            owl:versionIRI <https://w3id.org/ad4gd/model/gdProperty/1.0> ;
                            dct:contributor [ schema:affiliation [ foaf:name "OGC"
                                                                 ] ;
                                              foaf:name "Rob Atkinson"
                                            ] ;
                            dct:creator [ schema:affiliation [ foaf:name "PSNC"
                                                             ] ;
                                          rdfs:seeAlso <http://orcid.org/0000-0003-4289-4922> ;
                                          foaf:name "Raul Palma"
                                        ] ;
                            owl:imports <https://w3id.org/ad4gd/model/gdCommon> ;
                            dct:description "The GDProperty module is one of the modules of the AD4GD - Green Deal Information Model (GDIM). This ontology module was created by reusing and aligning well-known ontologies and vocabularies"@en ;
                            dct:rights "This vocabulary is distributed under Creative Commons Attribution 4.0 License - http://creativecommons.org/licenses/by/4.0"@en ;
                            dct:title "GDIM GDProperty"@en ;
                            rdfs:label "GDIM GDProperty" ;
                            rdfs:comment "The AD4GD - Green Deal Information Model (GDIM) is the common vocabulary in AD4GD project providing the basis for semantic interoperability across solutions related to the green deal domain"@en ;
                            owl:versionInfo "1.0" ;
                            foaf:maker [ foaf:homepage <https://ad4gd.eu/> ;
                                                      foaf:name "AD4GD project"
                                                    ] .

#################################################################
#    Annotation properties
#################################################################


#################################################################
#    Datatypes
#################################################################


#################################################################
#    Object Properties
#################################################################

###  https://saref.etsi.org/core/isControlledByDevice
saref:isControlledByDevice a owl:ObjectProperty ;
                                              rdfs:isDefinedBy <https://saref.etsi.org/core/> ;
                                              rdfs:comment "A relationship specifying the devices that can control a certain property" ;
                                              rdfs:label "is controlled by device"@en .

###  https://saref.etsi.org/core/isMeasuredByDevice
saref:isMeasuredByDevice a owl:ObjectProperty ;
                                            rdfs:isDefinedBy <https://saref.etsi.org/core/> ;
                                            rdfs:comment "A relationship specifying the devices that can measure a certain property" ;
                                            rdfs:label "is measured by device"@en .

###  https://saref.etsi.org/core/relatesToMeasurement
saref:relatesToMeasurement a owl:ObjectProperty ;
                                              rdfs:isDefinedBy <https://saref.etsi.org/core/> ;
                                              rdfs:comment "A relationship between a property and the measurements it relates to" ;
                                              rdfs:label "relates to measurement"@en .

###  https://saref.etsi.org/core/isMeasuredIn
saref:isMeasuredIn a owl:ObjectProperty ;
                                      rdfs:isDefinedBy <https://saref.etsi.org/core/> ;
                                      rdfs:comment "A relationship identifying the unit of measure used for a certain entity." ;
                                      rdfs:label "is measured in"@en .

###  https://saref.etsi.org/core/relatesToProperty
saref:relatesToProperty a owl:ObjectProperty ;
                                           rdfs:isDefinedBy <https://saref.etsi.org/core/> ;
                                           rdfs:comment "A relationship between a measurement and the property it relates to" ;
                                           rdfs:label "relates to property"@en .

###  https://saref.etsi.org/core/makesMeasurement
saref:makesMeasurement a owl:ObjectProperty ;
                                          owl:inverseOf saref:measurementMadeBy ;
                                          rdfs:isDefinedBy <https://saref.etsi.org/core/> ;
                                          rdfs:comment "A relation between a device and the measurements it makes. Such measurement will link together the value of the measurement, its unit of measure and the property to which it relates." ;
                                          rdfs:label "makes measurement"@en .

###  https://saref.etsi.org/core/measurementMadeBy
saref:measurementMadeBy a owl:ObjectProperty ;
                                           rdfs:comment "Relation between a measurement and the device that made it."@en ;
                                           rdfs:isDefinedBy <https://saref.etsi.org/core/> ;
                                           rdfs:label "measurement made by"@en .

###  https://saref.etsi.org/core/controlsProperty
saref:controlsProperty a owl:ObjectProperty ;
                                          rdfs:isDefinedBy <https://saref.etsi.org/core/> ;
                                          rdfs:comment "A relationship specifying the Property that can be controlled by a certain Device";
                                          rdfs:label "controls property"@en .

###  https://saref.etsi.org/core/measuresProperty
saref:measuresProperty a owl:ObjectProperty ;
                                          rdfs:isDefinedBy <https://saref.etsi.org/core/> ;
                                          rdfs:comment "A relationship specifying the Property that can be measured by a certain Device" ;
                                          rdfs:label "measures property"@en .

###  https://saref.etsi.org/core/hasFeatureOfInterest
saref:hasFeatureOfInterest a owl:ObjectProperty ;
                                              owl:inverseOf saref:isFeatureOfInterestOf ;
                                              rdfs:comment "Relation between a measurement and the feature of interest being measured."@en ;
                                              rdfs:isDefinedBy <https://saref.etsi.org/core/> ;
                                              rdfs:label "has feature of interest"@en .

###  https://saref.etsi.org/core/isFeatureOfInterestOf
saref:isFeatureOfInterestOf a owl:ObjectProperty ;
                                               rdfs:comment "Relation betwwen a feature of interest and the measurments that are about it."@en ;
                                               rdfs:isDefinedBy <https://saref.etsi.org/core/> ;
                                               rdfs:label "is feature of interest of"@en .

###  https://saref.etsi.org/core/hasProperty
saref:hasProperty a owl:ObjectProperty ;
                                     owl:inverseOf saref:isPropertyOf ;
                                     rdfs:comment "Relation between a feature of interest and its properties."@en ;
                                     rdfs:isDefinedBy <https://saref.etsi.org/core/> ;
                                     rdfs:label "has property"@en .

###  https://saref.etsi.org/core/isPropertyOf
saref:isPropertyOf a owl:ObjectProperty ;
                                      rdfs:comment "Relation between a property and a feature of interest in which such property appears."@en ;
                                      rdfs:isDefinedBy <https://saref.etsi.org/core/> ;
                                      rdfs:label "is property of"@en .



#################################################################
#    Data properties
#################################################################

###  https://saref.etsi.org/core/hasValue
saref:hasValue a owl:DatatypeProperty ;
                                  rdfs:isDefinedBy <https://saref.etsi.org/core/> ;
                                  rdfs:comment "A relationship defining the value of a certain property, e.g., energy or power" ;
                                  rdfs:label "has value"@en .


### https://smartdatamodels.org/dataModel.Weather/temperature
fiware-weather:temperature	a	owl:DatatypeProperty ;
        rdfs:label   		"temperature"@en ;
        rdfs:comment		"Temperature of the item. Prev: The observed air temperature (in the shade) nominally in degrees centigrade." ;
        rdfs:isDefinedBy <https://github.com/smart-data-models/dataModel.Weather/blob/master/WeatherObserved/schema.json> .

### https://smartdatamodels.org/dateObserved
fiware:dateObserved	a     owl:DatatypeProperty ;
        rdfs:range      xsd:dateTime ;
        rdfs:label   		"date observed"@en ;
        rdfs:comment		"Date of the observed entity defined by the user" ;
        rdfs:isDefinedBy <https://smart-data-models.github.io/data-models/common-schema.json#/definitions/dateObserved> .

### https://smartdatamodels.org/dataModel.Weather/weatherType
fiware-weather:weatherType	a   owl:DatatypeProperty ;
        rdfs:label   		"weatherType"@en ;
        rdfs:comment		"Text description of the weather. Prev: The observed weather type. It is represented by a comma separated list of weather statuses, for instance overcast, lightRain." ;
        rdfs:isDefinedBy <https://github.com/smart-data-models/dataModel.Weather/blob/master/weather-schema.json> .

### https://smartdatamodels.org/dataModel.Weather/dewPoint
fiware-weather:dewPoint	a      	owl:DatatypeProperty ;
        rdfs:label   		"dewPoint"@en ;
        rdfs:comment		"The dew point encoded as a number. Observed temperature to which air must be cooled to become saturated with water vapor" ;
        rdfs:isDefinedBy <https://github.com/smart-data-models/dataModel.Weather/blob/master/WeatherObserved/schema.json> .

### https://uri.fiware.org/ns/data-models#visibility
fiware-weather:visibility	a      owl:DatatypeProperty ;
        rdfs:label   		"visibility"@en ;
        rdfs:comment		"Categories of visibility. Prev: Visibility reported (veryPoor, poor, moderate, good, veryGood, excellent)" ;
        rdfs:isDefinedBy <https://github.com/smart-data-models/dataModel.Weather/blob/master/weather-schema.json> .

### https://smartdatamodels.org/dataModel.Weather/airTemperatureForecast
fiware-weather:airTemperatureForecast	a   owl:DatatypeProperty ;
        rdfs:label   		"airTemperatureForecast"@en ;
        rdfs:comment		"Forecasted value of air temperature over a certain duration in future" ;
        rdfs:isDefinedBy <https://github.com/smart-data-models/dataModel.Weather/blob/master/WeatherObserved/schema.json> .

### https://smartdatamodels.org/dataModel.Weather/relativeHumidity
fiware-weather:relativeHumidity	a	owl:DatatypeProperty ;
        rdfs:label   		"relativeHumidity"@en ;
        rdfs:comment		"Humidity in the Air. Observed instantaneous relative humidity (water vapour in air)" ;
        rdfs:isDefinedBy <https://github.com/smart-data-models/dataModel.Weather/blob/master/WeatherObserved/schema.json> .

### https://smartdatamodels.org/dataModel.Weather/precipitation
fiware-weather:precipitation	a	owl:DatatypeProperty ;
        rdfs:label   		"precipitation"@en ;
        rdfs:comment		"Amount of water rain registered. Units:'Liters per square meter'" ;
        rdfs:isDefinedBy <https://github.com/smart-data-models/dataModel.Weather/blob/master/WeatherObserved/schema.json> .

### https://smartdatamodels.org/dataModel.Weather/windDirection
fiware-weather:windDirection	a	owl:DatatypeProperty ;
        rdfs:label   		"windDirection"@en ;
        rdfs:comment		"Direction of the wind bet" ;
        rdfs:isDefinedBy <https://github.com/smart-data-models/dataModel.Weather/blob/master/weather-schema.json> .

### https://smartdatamodels.org/dataModel.Weather/windSpeed
fiware-weather:windSpeed	a      owl:DatatypeProperty ;
        rdfs:label   		"windSpeed"@en ;
        rdfs:comment		"Intensity of the wind." ;
        rdfs:isDefinedBy <https://github.com/smart-data-models/dataModel.Weather/blob/master/weather-schema.json> .

### https://smartdatamodels.org/dataModel.Weather/atmosphericPressure
fiware-weather:atmosphericPressure	a	owl:DatatypeProperty ;
        rdfs:label   		"atmosphericPressure"@en ;
        rdfs:comment		"The atmospheric pressure observed measured in Hecto Pascals. Units:'Hecto pascals'" ;
        rdfs:isDefinedBy <https://github.com/smart-data-models/dataModel.Weather/blob/master/weather-schema.json> .

### https://smartdatamodels.org/dataModel.Weather/pressureTendency
fiware-weather:pressureTendency	a	owl:DatatypeProperty ;
        rdfs:label   		"pressureTendency"@en ;
        rdfs:comment		"Is the pressure rising or falling? It can be expressed in quantitative terms or qualitative terms (raising, falling, steady)" ;
        rdfs:isDefinedBy <https://github.com/smart-data-models/dataModel.Weather/blob/master/WeatherObserved/schema.json> .

### https://smartdatamodels.org/dataModel.Weather/solarRadiation
fiware-weather:solarRadiation	a	owl:DatatypeProperty ;
        rdfs:label   		"solarRadiation"@en ;
        rdfs:comment		"The solar radiation observed measured in Watts per square. Units:'w/m2'" ;
        rdfs:isDefinedBy <https://github.com/smart-data-models/dataModel.Weather/blob/master/WeatherObserved/schema.json> .

### https://smartdatamodels.org/dataModel.Weather/illuminance
fiware-weather:illuminance	a		owl:DatatypeProperty ;
        rdfs:label   		"illuminance"@en ;
        rdfs:comment		"The illumninance observed measured in lux (lx) or lumens per square metre (cd·sr·m−2)" ;
        rdfs:isDefinedBy <https://github.com/smart-data-models/dataModel.Weather/blob/master/WeatherObserved/schema.json> .

### https://smartdatamodels.org/dataModel.Weather/streamGauge
fiware-weather:streamGauge	a		owl:DatatypeProperty ;
        rdfs:label   		"streamGauge"@en ;
        rdfs:comment		"The water level surface elevation observed by Hydrometric measurement sensors, namely a Stream Gauge expressed in centimeters. Units:'centimeters'" ;
        rdfs:isDefinedBy <https://github.com/smart-data-models/dataModel.Weather/blob/master/WeatherObserved/schema.json> .

### https://smartdatamodels.org/dataModel.Weather/snowHeight
fiware-weather:snowHeight	a      owl:DatatypeProperty ;
        rdfs:label   		"snowHeight"@en ;
        rdfs:comment		"The snow height observed by generic snow depth measurement sensors, expressed in centimeters. Units:'centimeters'" ;
        rdfs:isDefinedBy <https://github.com/smart-data-models/dataModel.Weather/blob/master/WeatherObserved/schema.json> .

### https://smartdatamodels.org/dataModel.Environment/flow
fiware-environment:flow	a      owl:DatatypeProperty ;
        rdfs:label   		"flow"@en ;
        rdfs:comment		"Water Flow observed. The unit code (text) of measurement given using the UN/CEFACAT" ;
        rdfs:isDefinedBy <https://github.com/smart-data-models/dataModel.Environment/blob/master/WaterObserved/schema.json> .

### https://smartdatamodels.org/dataModel.Environment/waterLevel
fiware-environment:waterLevel	a      owl:DatatypeProperty ;
        rdfs:label   		"waterLevel"@en ;
        rdfs:comment		"Current water level corresponding to this observation. The unit code (text) of measurement given using the UN/CEFACT Common Codes (max. 3 characters)" ;
        rdfs:isDefinedBy <https://github.com/smart-data-models/dataModel.Environment/blob/master/WaterObserved/schema.json> .        

### https://smartdatamodels.org/dataModel.Environment/waveLength
fiware-environment:waveLength	a      owl:DatatypeProperty ;
        rdfs:label   		"waveLength"@en ;
        rdfs:comment		"Wave Length observed" ;
        rdfs:isDefinedBy <https://github.com/smart-data-models/dataModel.Environment/blob/master/WaterObserved/schema.json> .                

### https://smartdatamodels.org/dataModel.Environment/swellDirection
fiware-environment:swellDirection	a      owl:DatatypeProperty ;
        rdfs:label   		"swellDirection"@en ;
        rdfs:comment		"Swells Direction observed" ;
        rdfs:isDefinedBy <https://github.com/smart-data-models/dataModel.Environment/blob/master/WaterObserved/schema.json> .

### https://smartdatamodels.org/dataModel.Environment/swellHeight
fiware-environment:swellHeight	a      owl:DatatypeProperty ;
        rdfs:label   		"swellHeight"@en ;
        rdfs:comment		"Swells height observed" ;
        rdfs:isDefinedBy <https://github.com/smart-data-models/dataModel.Environment/blob/master/WaterObserved/schema.json> .

### https://smartdatamodels.org/dataModel.Environment/swellPeriod
fiware-environment:swellPeriod	a      owl:DatatypeProperty ;
        rdfs:label   		"swellPeriod"@en ;
        rdfs:comment		"Swells period observed" ;
        rdfs:isDefinedBy <https://github.com/smart-data-models/dataModel.Environment/blob/master/WaterObserved/schema.json> .

####### chemical water properties as data properties (not recommended)
### https://smartdatamodels.org/dataModel.WaterQuality/Al
fiware-waterquality:Al  a      owl:DatatypeProperty ;
        rdfs:label   		"Al"@en ;
        rdfs:comment		"Aluminium. Concentration of aluminium" ;
        rdfs:isDefinedBy <https://github.com/smart-data-models/dataModel.WaterQuality/blob/master/WaterQualityObserved/schema.json> .

### https://smartdatamodels.org/dataModel.WaterQuality/As
fiware-waterquality:As  a      owl:DatatypeProperty ;
        rdfs:label   		"As"@en ;
        rdfs:comment		"Arsenic. Concentration of Arsenic" ;
        rdfs:isDefinedBy <https://github.com/smart-data-models/dataModel.WaterQuality/blob/master/WaterQualityObserved/schema.json> .

### https://smartdatamodels.org/dataModel.WaterQuality/B
fiware-waterquality:B  a      owl:DatatypeProperty ;
        rdfs:label   		"B"@en ;
        rdfs:comment		"Boron. Concentration of Boron" ;
        rdfs:isDefinedBy <https://github.com/smart-data-models/dataModel.WaterQuality/blob/master/WaterQualityObserved/schema.json> .

### https://smartdatamodels.org/dataModel.WaterQuality/Ba
fiware-waterquality:Ba  a      owl:DatatypeProperty ;
        rdfs:label   		"Ba"@en ;
        rdfs:comment		"Barium. Concentration of Barium" ;
        rdfs:isDefinedBy <https://github.com/smart-data-models/dataModel.WaterQuality/blob/master/WaterQualityObserved/schema.json> .

### https://smartdatamodels.org/dataModel.WaterQuality/Cd
fiware-waterquality:Cd  a      owl:DatatypeProperty ;
        rdfs:label   		"Cd"@en ;
        rdfs:comment		"Cadmium. Concentration of Cadmium" ;
        rdfs:isDefinedBy <https://github.com/smart-data-models/dataModel.WaterQuality/blob/master/WaterQualityObserved/schema.json> .

### https://smartdatamodels.org/dataModel.WaterQuality/Chla
fiware-waterquality:Chla  a      owl:DatatypeProperty ;
        rdfs:label   		"Chla"@en ;
        rdfs:comment		"Concentration of chlorophyll A" ;
        rdfs:isDefinedBy <https://github.com/smart-data-models/dataModel.WaterQuality/blob/master/WaterQualityObserved/schema.json> .

### https://smartdatamodels.org/dataModel.WaterQuality/Cl-
fiware-waterquality:Cl-  a      owl:DatatypeProperty ;
        rdfs:label   		"Cl-"@en ;
        rdfs:comment		"Concentration of chlorides" ;
        rdfs:isDefinedBy <https://github.com/smart-data-models/dataModel.WaterQuality/blob/master/WaterQualityObserved/schema.json> . 

### https://smartdatamodels.org/dataModel.WaterQuality/Cr
fiware-waterquality:Cr  a      owl:DatatypeProperty ;
        rdfs:label   		"Cr"@en ;
        rdfs:comment		"Chromium. Concentration of Chromium" ;
        rdfs:isDefinedBy <https://github.com/smart-data-models/dataModel.WaterQuality/blob/master/WaterQualityObserved/schema.json> .

### https://smartdatamodels.org/dataModel.WaterQuality/Cr-III
fiware-waterquality:Cr-III  a      owl:DatatypeProperty ;
        rdfs:label   		"Cr-III"@en ;
        rdfs:comment		"Chromium III. Concentration of chromium at the oxidation state +3" ;
        rdfs:isDefinedBy <https://github.com/smart-data-models/dataModel.WaterQuality/blob/master/WaterQualityObserved/schema.json> .

### https://smartdatamodels.org/dataModel.WaterQuality/Cr-VI
fiware-waterquality:Cr-VI  a      owl:DatatypeProperty ;
        rdfs:label   		"Cr-VI"@en ;
        rdfs:comment		"Chromium VI. Concentration of chromium at the oxidation state +6" ;
        rdfs:isDefinedBy <https://github.com/smart-data-models/dataModel.WaterQuality/blob/master/WaterQualityObserved/schema.json> .

### https://smartdatamodels.org/dataModel.WaterQuality/Cu
fiware-waterquality:Cu  a      owl:DatatypeProperty ;
        rdfs:label   		"Cu"@en ;
        rdfs:comment		"Copper. Concentration of Copper" ;
        rdfs:isDefinedBy <https://github.com/smart-data-models/dataModel.WaterQuality/blob/master/WaterQualityObserved/schema.json> .

### https://smartdatamodels.org/dataModel.WaterQuality/Fe
fiware-waterquality:Fe  a      owl:DatatypeProperty ;
        rdfs:label   		"Fe"@en ;
        rdfs:comment		"Iron. Concentration of Iron" ;
        rdfs:isDefinedBy <https://github.com/smart-data-models/dataModel.WaterQuality/blob/master/WaterQualityObserved/schema.json> .

### https://smartdatamodels.org/dataModel.WaterQuality/Hg
fiware-waterquality:Hg  a      owl:DatatypeProperty ;
        rdfs:label   		"Hg"@en ;
        rdfs:comment		"Mercury. Concentration of Mercury" ;
        rdfs:isDefinedBy <https://github.com/smart-data-models/dataModel.WaterQuality/blob/master/WaterQualityObserved/schema.json> .

### https://smartdatamodels.org/dataModel.WaterQuality/N-TOT
fiware-waterquality:N-TOT  a      owl:DatatypeProperty ;
        rdfs:label   		"N-TOT"@en ;
        rdfs:comment		"Total Nitrogen. otal Nitrogen (TN) is the sum of nitrate-nitrogen (NO3-N), nitrite-nitrogen (NO2-N), ammonia-nitrogen (NH3-N) and organically bonded nitrogen" ;
        rdfs:isDefinedBy <https://github.com/smart-data-models/dataModel.WaterQuality/blob/master/WaterQualityObserved/schema.json> .  

### https://smartdatamodels.org/dataModel.WaterQuality/NH3
fiware-waterquality:NH3  a      owl:DatatypeProperty ;
        rdfs:label   		"NH3"@en ;
        rdfs:comment		"Concentration of ammonia" ;
        rdfs:isDefinedBy <https://github.com/smart-data-models/dataModel.WaterQuality/blob/master/WaterQualityObserved/schema.json> .                                                               

### https://smartdatamodels.org/dataModel.WaterQuality/NH4
fiware-waterquality:NH4  a      owl:DatatypeProperty ;
        rdfs:label   		"NH4"@en ;
        rdfs:comment		"Concentration of ammonium" ;
        rdfs:isDefinedBy <https://github.com/smart-data-models/dataModel.WaterQuality/blob/master/WaterQualityObserved/schema.json> .

### https://smartdatamodels.org/dataModel.WaterQuality/NO2
fiware-waterquality:NO2  a      owl:DatatypeProperty ;
        rdfs:label   		"NO2"@en ;
        rdfs:comment		"Nitrite nitrogen. Concentration of a sample in nitrite nitrogen" ;
        rdfs:isDefinedBy <https://github.com/smart-data-models/dataModel.WaterQuality/blob/master/WaterQualityObserved/schema.json> . 

### https://smartdatamodels.org/dataModel.WaterQuality/NO3
fiware-waterquality:NO3  a      owl:DatatypeProperty ;
        rdfs:label   		"NO3"@en ;
        rdfs:comment		"Concentration of nitrates" ;
        rdfs:isDefinedBy <https://github.com/smart-data-models/dataModel.WaterQuality/blob/master/WaterQualityObserved/schema.json> .

### https://smartdatamodels.org/dataModel.WaterQuality/Ni
fiware-waterquality:Ni  a      owl:DatatypeProperty ;
        rdfs:label   		"Ni"@en ;
        rdfs:comment		"Nickel. Concentration of Nickel" ;
        rdfs:isDefinedBy <https://github.com/smart-data-models/dataModel.WaterQuality/blob/master/WaterQualityObserved/schema.json> .

### https://smartdatamodels.org/dataModel.WaterQuality/O2
fiware-waterquality:O2  a      owl:DatatypeProperty ;
        rdfs:label   		"O2"@en ;
        rdfs:comment		"Level of free, non-compound oxygen present" ;
        rdfs:isDefinedBy <https://github.com/smart-data-models/dataModel.WaterQuality/blob/master/WaterQualityObserved/schema.json> .

### https://smartdatamodels.org/dataModel.WaterQuality/P-PO4
fiware-waterquality:P-PO4  a      owl:DatatypeProperty ;
        rdfs:label   		"P-PO4"@en ;
        rdfs:comment		"Phosphate-phosphorus. Concentration of phosphorus as phosphate" ;
        rdfs:isDefinedBy <https://github.com/smart-data-models/dataModel.WaterQuality/blob/master/WaterQualityObserved/schema.json> .                                                

### https://smartdatamodels.org/dataModel.WaterQuality/P-TOT
fiware-waterquality:P-TOT  a      owl:DatatypeProperty ;
        rdfs:label   		"P-TOT"@en ;
        rdfs:comment		"Total Phosphorus. Total phosphorus is a measure of all forms of phosphorus in the water, including dissolved and particulate, organic and inorganic" ;
        rdfs:isDefinedBy <https://github.com/smart-data-models/dataModel.WaterQuality/blob/master/WaterQualityObserved/schema.json> .

### https://smartdatamodels.org/dataModel.WaterQuality/PC
fiware-waterquality:PC  a      owl:DatatypeProperty ;
        rdfs:label   		"PC"@en ;
        rdfs:comment		"Concentration of pigment phycocyanin which can be measured to estimate cyanobacteria concentrations specifically" ;
        rdfs:isDefinedBy <https://github.com/smart-data-models/dataModel.WaterQuality/blob/master/WaterQualityObserved/schema.json> .

### https://smartdatamodels.org/dataModel.WaterQuality/PE
fiware-waterquality:PE  a      owl:DatatypeProperty ;
        rdfs:label   		"PE"@en ;
        rdfs:comment		"Concentration of pigment phycoerythrin which can be measured to estimate cyanobacteria concentrations specifically" ;
        rdfs:isDefinedBy <https://github.com/smart-data-models/dataModel.WaterQuality/blob/master/WaterQualityObserved/schema.json> .                

### https://smartdatamodels.org/dataModel.WaterQuality/PO4
fiware-waterquality:PO4  a      owl:DatatypeProperty ;
        rdfs:label   		"PO4"@en ;
        rdfs:comment		"Concentration of phosphates" ;
        rdfs:isDefinedBy <https://github.com/smart-data-models/dataModel.WaterQuality/blob/master/WaterQualityObserved/schema.json> .

### https://smartdatamodels.org/dataModel.WaterQuality/Pb
fiware-waterquality:Pb  a      owl:DatatypeProperty ;
        rdfs:label   		"Pb"@en ;
        rdfs:comment		"Lead. Concentration of lead" ;
        rdfs:isDefinedBy <https://github.com/smart-data-models/dataModel.WaterQuality/blob/master/WaterQualityObserved/schema.json> .

### https://smartdatamodels.org/dataModel.WaterQuality/Se
fiware-waterquality:Se  a      owl:DatatypeProperty ;
        rdfs:label   		"Se"@en ;
        rdfs:comment		"Selenium. Concentration of Selenium" ;
        rdfs:isDefinedBy <https://github.com/smart-data-models/dataModel.WaterQuality/blob/master/WaterQualityObserved/schema.json> .

### https://smartdatamodels.org/dataModel.WaterQuality/Sn
fiware-waterquality:Sn  a      owl:DatatypeProperty ;
        rdfs:label   		"Sn"@en ;
        rdfs:comment		"Tin. Concentration of Tin" ;
        rdfs:isDefinedBy <https://github.com/smart-data-models/dataModel.WaterQuality/blob/master/WaterQualityObserved/schema.json> .

### https://smartdatamodels.org/dataModel.WaterQuality/THC
fiware-waterquality:THC  a      owl:DatatypeProperty ;
        rdfs:label   		"THC"@en ;
        rdfs:comment		"Total hydrocarbon. Concentration of total hydrocarbon" ;
        rdfs:isDefinedBy <https://github.com/smart-data-models/dataModel.WaterQuality/blob/master/WaterQualityObserved/schema.json> .

### https://smartdatamodels.org/dataModel.WaterQuality/TKN
fiware-waterquality:TKN  a      owl:DatatypeProperty ;
        rdfs:label   		"TKN"@en ;
        rdfs:comment		"Total Kjeldahl Nitrogen. A measure that determines both the organic and the inorganic forms of nitrogen" ;
        rdfs:isDefinedBy <https://github.com/smart-data-models/dataModel.WaterQuality/blob/master/WaterQualityObserved/schema.json> .

### https://smartdatamodels.org/dataModel.WaterQuality/TO
fiware-waterquality:TO  a      owl:DatatypeProperty ;
        rdfs:label   		"TO"@en ;
        rdfs:comment		"Total oil content. Concentration of oil" ;
        rdfs:isDefinedBy <https://github.com/smart-data-models/dataModel.WaterQuality/blob/master/WaterQualityObserved/schema.json> .

### https://smartdatamodels.org/dataModel.WaterQuality/Zn
fiware-waterquality:Zn  a      owl:DatatypeProperty ;
        rdfs:label   		"Zn"@en ;
        rdfs:comment		"Zinc. Concentration of Zinc" ;
        rdfs:isDefinedBy <https://github.com/smart-data-models/dataModel.WaterQuality/blob/master/WaterQualityObserved/schema.json> .

### https://smartdatamodels.org/dataModel.WaterQuality/alkalinity
fiware-waterquality:alkalinity  a      owl:DatatypeProperty ;
        rdfs:label   		"alkalinity"@en ;
        rdfs:comment		"The alkalinity of water is its acid-neutralizing capacity comprised of the total of all titratable bases" ;
        rdfs:isDefinedBy <https://github.com/smart-data-models/dataModel.WaterQuality/blob/master/WaterQualityObserved/schema.json> .

### https://smartdatamodels.org/dataModel.WaterQuality/anionic-surfactants
fiware-waterquality:anionic-surfactants  a      owl:DatatypeProperty ;
        rdfs:label   		"anionic-surfactants"@en ;
        rdfs:comment		"Concentration of anionic surfactants" ;
        rdfs:isDefinedBy <https://github.com/smart-data-models/dataModel.WaterQuality/blob/master/WaterQualityObserved/schema.json> .

### https://smartdatamodels.org/dataModel.WaterQuality/bod
fiware-waterquality:bod  a      owl:DatatypeProperty ;
        rdfs:label   		"bod"@en ;
        rdfs:comment		"Biochemical oxygen demand (BOD) is the amount of dissolved oxygen (DO) needed (i.e. demanded) by aerobic biological organisms to break down organic material present in a given water sample at certain temperature over a specific time period" ;
        rdfs:isDefinedBy <https://github.com/smart-data-models/dataModel.WaterQuality/blob/master/WaterQualityObserved/schema.json> .

### https://smartdatamodels.org/dataModel.WaterQuality/cationic-surfactants
fiware-waterquality:cationic-surfactants  a      owl:DatatypeProperty ;
        rdfs:label   		"cationic-surfactants"@en ;
        rdfs:comment		"Concentrtation of cationic surfactants" ;
        rdfs:isDefinedBy <https://github.com/smart-data-models/dataModel.WaterQuality/blob/master/WaterQualityObserved/schema.json> .

### https://smartdatamodels.org/dataModel.WaterQuality/cod
fiware-waterquality:cod  a      owl:DatatypeProperty ;
        rdfs:label   		"cod"@en ;
        rdfs:comment		"Chemical oxygen demand (COD) is an indicative measure of the amount of oxygen that can be consumed by reactions in a measured solution" ;
        rdfs:isDefinedBy <https://github.com/smart-data-models/dataModel.WaterQuality/blob/master/WaterQualityObserved/schema.json> . 

### https://smartdatamodels.org/dataModel.WaterQuality/conductance
fiware-waterquality:conductance  a      owl:DatatypeProperty ;
        rdfs:label   		"conductance"@en ;
        rdfs:comment		"Specific Conductance" ;
        rdfs:isDefinedBy <https://github.com/smart-data-models/dataModel.WaterQuality/blob/master/WaterQualityObserved/schema.json> .

### https://smartdatamodels.org/dataModel.WaterQuality/conductivity
fiware-waterquality:conductivity  a      owl:DatatypeProperty ;
        rdfs:label   		"conductivity"@en ;
        rdfs:comment		"Electrical Conductivity" ;
        rdfs:isDefinedBy <https://github.com/smart-data-models/dataModel.WaterQuality/blob/master/WaterQualityObserved/schema.json> .

### https://smartdatamodels.org/dataModel.WaterQuality/enterococci
fiware-waterquality:enterococci  a      owl:DatatypeProperty ;
        rdfs:label   		"enterococci"@en ;
        rdfs:comment		"Concentration of Enterococci" ;
        rdfs:isDefinedBy <https://github.com/smart-data-models/dataModel.WaterQuality/blob/master/WaterQualityObserved/schema.json> .

### https://smartdatamodels.org/dataModel.WaterQuality/escherichiaColi
fiware-waterquality:escherichiaColi  a      owl:DatatypeProperty ;
        rdfs:label   		"escherichiaColi"@en ;
        rdfs:comment		"Concentration of Escherichia coli" ;
        rdfs:isDefinedBy <https://github.com/smart-data-models/dataModel.WaterQuality/blob/master/WaterQualityObserved/schema.json> .

### https://smartdatamodels.org/dataModel.WaterQuality/fluoride
fiware-waterquality:fluoride  a      owl:DatatypeProperty ;
        rdfs:label   		"fluoride"@en ;
        rdfs:comment		"Concentration of fluoride" ;
        rdfs:isDefinedBy <https://github.com/smart-data-models/dataModel.WaterQuality/blob/master/WaterQualityObserved/schema.json> .

### https://smartdatamodels.org/dataModel.WaterQuality/non-ionic-surfactants
fiware-waterquality:non-ionic-surfactants  a      owl:DatatypeProperty ;
        rdfs:label   		"non-ionic-surfactants"@en ;
        rdfs:comment		"Concentration of non-ionic surfactants" ;
        rdfs:isDefinedBy <https://github.com/smart-data-models/dataModel.WaterQuality/blob/master/WaterQualityObserved/schema.json> .

### https://smartdatamodels.org/dataModel.WaterQuality/orp
fiware-waterquality:orp  a      owl:DatatypeProperty ;
        rdfs:label   		"orp"@en ;
        rdfs:comment		"Oxidation-Reduction potential" ;
        rdfs:isDefinedBy <https://github.com/smart-data-models/dataModel.WaterQuality/blob/master/WaterQualityObserved/schema.json> .

### https://smartdatamodels.org/dataModel.WaterQuality/pH
fiware-waterquality:pH  a      owl:DatatypeProperty ;
        rdfs:label   		"pH"@en ;
        rdfs:comment		"Acidity or basicity of an aqueous solution" ;
        rdfs:isDefinedBy <https://github.com/smart-data-models/dataModel.WaterQuality/blob/master/WaterQualityObserved/schema.json> . 

### https://smartdatamodels.org/dataModel.WaterQuality/salinity
fiware-waterquality:salinity  a      owl:DatatypeProperty ;
        rdfs:label   		"salinity"@en ;
        rdfs:comment		"Amount of salts dissolved in water" ;
        rdfs:isDefinedBy <https://github.com/smart-data-models/dataModel.WaterQuality/blob/master/WaterQualityObserved/schema.json> .

### https://smartdatamodels.org/dataModel.WaterQuality/sulphate
fiware-waterquality:sulphate  a      owl:DatatypeProperty ;
        rdfs:label   		"sulphate"@en ;
        rdfs:comment		"Concentration of sulfate" ;
        rdfs:isDefinedBy <https://github.com/smart-data-models/dataModel.WaterQuality/blob/master/WaterQualityObserved/schema.json> .

### https://smartdatamodels.org/dataModel.WaterQuality/sulphite
fiware-waterquality:sulphite  a      owl:DatatypeProperty ;
        rdfs:label   		"sulphite"@en ;
        rdfs:comment		"Concentration of sulphite" ;
        rdfs:isDefinedBy <https://github.com/smart-data-models/dataModel.WaterQuality/blob/master/WaterQualityObserved/schema.json> .

### https://smartdatamodels.org/dataModel.WaterQuality/tds
fiware-waterquality:tds  a      owl:DatatypeProperty ;
        rdfs:label   		"tds"@en ;
        rdfs:comment		"Total dissolved solids" ;
        rdfs:isDefinedBy <https://github.com/smart-data-models/dataModel.WaterQuality/blob/master/WaterQualityObserved/schema.json> .

### https://smartdatamodels.org/dataModel.WaterQuality/total-surfactants
fiware-waterquality:total-surfactants  a      owl:DatatypeProperty ;
        rdfs:label   		"total-surfactants"@en ;
        rdfs:comment		"Concentration of total surfactants" ;
        rdfs:isDefinedBy <https://github.com/smart-data-models/dataModel.WaterQuality/blob/master/WaterQualityObserved/schema.json> .

### https://smartdatamodels.org/dataModel.WaterQuality/tss
fiware-waterquality:tss  a      owl:DatatypeProperty ;
        rdfs:label   		"tss"@en ;
        rdfs:comment		"Total suspended solids" ;
        rdfs:isDefinedBy <https://github.com/smart-data-models/dataModel.WaterQuality/blob/master/WaterQualityObserved/schema.json> .

### https://smartdatamodels.org/dataModel.WaterQuality/turbidity
fiware-waterquality:turbidity  a      owl:DatatypeProperty ;
        rdfs:label   		"turbidity"@en ;
        rdfs:comment		"Amount of light scattered by particles in the water column" ;
        rdfs:isDefinedBy <https://github.com/smart-data-models/dataModel.WaterQuality/blob/master/WaterQualityObserved/schema.json> .
####### end of chemical water properties as data properties (not recommended)

### https://smartdatamodels.org/dataModel.WaterQuality/waterQualityPredictionValue
fiware-waterquality:waterQualityPredictionValue  a      owl:DatatypeProperty ;
        rdfs:label   		"waterQualityPredictionValue"@en ;
        rdfs:comment		"Describes a summary of the water quality prediction" ;
        rdfs:isDefinedBy <https://github.com/smart-data-models/dataModel.WaterQuality/blob/master/WaterQualityPredicted/schema.json> .                                                                                                                                                                       

#################################################################
#    Classes
#################################################################

###  https://saref.etsi.org/core/Property
saref:Property a owl:Class ;
                                  rdfs:subClassOf [ a owl:Restriction ;
                                                    owl:onProperty saref:isControlledByDevice ;
                                                    owl:allValuesFrom saref:Device
                                                  ] ,
                                                  [ a owl:Restriction ;
                                                    owl:onProperty saref:isMeasuredByDevice ;
                                                    owl:allValuesFrom saref:Device
                                                  ] ,
                                                  [ a owl:Restriction ;
                                                    owl:onProperty saref:isPropertyOf ;
                                                    owl:allValuesFrom saref:FeatureOfInterest
                                                  ] ,
                                                  [ a owl:Restriction ;
                                                    owl:onProperty saref:relatesToMeasurement ;
                                                    owl:allValuesFrom saref:Measurement
                                                  ] ;
                                  owl:disjointWith saref:UnitOfMeasure ;
                                  rdfs:comment "An aspect of an entity that can be observable by a sensor."@en ,
                                               "Anything that can be sensed, measured or controlled in households, common public buildings or offices. We propose here a list of properties that are relevant for the purpose of SAREF, but this list can be extended." ;
                                  rdfs:isDefinedBy <https://saref.etsi.org/core/> ;
                                  rdfs:label "Property"@en ,
                                             "Property" .

###  https://saref.etsi.org/core/Measurement
saref:Measurement a owl:Class ;
                                     rdfs:subClassOf [ a owl:Restriction ;
                                                       owl:onProperty saref:hasFeatureOfInterest ;
                                                       owl:allValuesFrom saref:FeatureOfInterest
                                                     ] ,
                                                     [ a owl:Restriction ;
                                                       owl:onProperty saref:isMeasuredIn ;
                                                       owl:allValuesFrom saref:UnitOfMeasure
                                                     ] ,
                                                     [ a owl:Restriction ;
                                                       owl:onProperty saref:relatesToProperty ;
                                                       owl:allValuesFrom saref:Property
                                                     ] ,
                                                     [ a owl:Restriction ;
                                                       owl:onProperty saref:isMeasuredIn ;
                                                       owl:qualifiedCardinality "1"^^xsd:nonNegativeInteger ;
                                                       owl:onClass saref:UnitOfMeasure
                                                     ] ,
                                                     [ a owl:Restriction ;
                                                       owl:onProperty saref:relatesToProperty ;
                                                       owl:qualifiedCardinality "1"^^xsd:nonNegativeInteger ;
                                                       owl:onClass saref:Property
                                                     ] ,
                                                     [ a owl:Restriction ;
                                                       owl:onProperty saref:hasTimestamp ;
                                                       owl:allValuesFrom xsd:dateTime
                                                     ] ,
                                                     [ a owl:Restriction ;
                                                       owl:onProperty saref:hasValue ;
                                                       owl:cardinality "1"^^xsd:nonNegativeInteger
                                                     ] ,
                                                     [ a owl:Restriction ;
                                                       owl:onProperty saref:hasValue ;
                                                       owl:qualifiedCardinality "1"^^xsd:nonNegativeInteger ;
                                                       owl:onDataRange xsd:float
                                                     ] ;
                                     owl:disjointWith saref:Property ,
                                                      saref:UnitOfMeasure ;
                                     rdfs:comment "Represents the measured value made over a property. It is also linked to the unit of measure in which the value is expressed and the timestamp of the measurement."@en ;
                                     rdfs:isDefinedBy <https://saref.etsi.org/core/> ;
                                     rdfs:label "Measurement"@en .

###  https://saref.etsi.org/core/UnitOfMeasure
saref:UnitOfMeasure a owl:Class ;
                                       rdfs:comment "The unit of measure is a standard for measurement of a quantity, such as a Property. For example,  Power is a property and Watt is a unit of power that represents a definite predetermined power: when we say 10 Watt, we actually mean 10 times the definite predetermined power called \"watt\". Our definition is based on the definition of unit of measure in the Ontology of units of Measure (OM). We propose here a list of some units of measure that are relevant for the purpose of the Smart Appliances ontology, but this list can be extended."@en ,
                                                    "The unit of measure is a standard for measurement of a quantity, such as a Property. For example,  Power is a property and Watt is a unit of power that represents a definite predetermined power: when we say 10 Watt, we actually mean 10 times the definite predetermined power called \"watt\". Our definition is based on the definition of unit of measure in the Ontology of units of Measure (OM). We propose here a list of some units of measure that are relevant for the purpose of SAREF, but this list can be extended, also using some other ontologies rather than the Ontology of units of Measure (OM)." ;
                                       rdfs:isDefinedBy <http://www.wurvoc.org/vocabularies/om-1.6/Unit_of_measure> ,
                                                        <https://saref.etsi.org/core/> ;
                                       rdfs:label "Unit of measure"@en .

###  https://saref.etsi.org/core/FeatureOfInterest
saref:FeatureOfInterest a owl:Class ;
                                           rdfs:subClassOf [ a owl:Restriction ;
                                                             owl:onProperty saref:hasProperty ;
                                                             owl:allValuesFrom saref:Property
                                                           ] ,
                                                           [ a owl:Restriction ;
                                                             owl:onProperty saref:isFeatureOfInterestOf ;
                                                             owl:allValuesFrom saref:Measurement
                                                           ] ;
                                           rdfs:comment "A feature of interest represents any real world entity from which a property is measured" ;
                                           rdfs:label "Feature of interest"@en ;
                                           rdfs:isDefinedBy <https://saref.etsi.org/core/> .

###  https://saref.etsi.org/core/Humidity
saref:Humidity a owl:Class ;
                                  rdfs:subClassOf saref:Property ;
                                  rdfs:comment "A saref:Property related to some measurements that are characterized by a certain value that is measured in a humidity unit" ;
                                  rdfs:label "Humidity"@en ;
                                  rdfs:isDefinedBy <https://saref.etsi.org/core/> .

###  https://saref.etsi.org/core/Temperature
saref:Temperature a owl:Class ;
                                     rdfs:subClassOf saref:Property ;
                                     rdfs:comment "A saref:Property related to some measurements that are characterized by a certain value that is measured in a temperature unit (degree_Celsius, degree_Fahrenheit, or degree_kelvin)" ;
                                     rdfs:label "Temperature"@en ;
                                     rdfs:isDefinedBy <https://saref.etsi.org/core/> .

###  http://purl.org/iot/vocab/m3-lite#WaterLevel
m3-lite:WaterLevel a owl:Class ;
			  rdfs:subClassOf qu:QuantityKind ;
        rdfs:comment "The height reached by the water in a reservoir, river, storage tank, or similar." ;
        rdfs:label "Water Level"@en ;
        rdfs:isDefinedBy <http://purl.org/iot/vocab/m3-lite#WaterLevel> .


###  https://saref.etsi.org/saref4watr/AcceptabilityProperty
s4watr:AcceptabilityProperty rdf:type owl:Class ;
                             rdfs:subClassOf s4watr:WaterProperty ;
                             rdfs:comment "An acceptability property is a property of water that is related to its acceptability."@en ;
                             rdfs:label "Acceptability property"@en .

###  https://saref.etsi.org/saref4watr/BacterialProperty
s4watr:BacterialProperty rdf:type owl:Class ;
                         rdfs:subClassOf s4watr:MicrobialProperty ;
                         rdfs:comment "A bacterial property is a property of water that is related to bacteria."@en ;
                         rdfs:label "Bacterial property"@en .                             

###  https://saref.etsi.org/saref4watr/ChemicalProperty
s4watr:ChemicalProperty rdf:type owl:Class ;
                        rdfs:subClassOf s4watr:WaterProperty ;
                        rdfs:comment "A chemical property is a property of water that is related to chemical components."@en ;
                        rdfs:label "ChemicalProperty"@en ;
                        rdfs:isDefinedBy <https://saref.etsi.org/saref4watr/> .

###  https://saref.etsi.org/saref4watr/EnvironmentalProperty
s4watr:EnvironmentalProperty rdf:type owl:Class ;
                             rdfs:subClassOf saref:Property ;
                             rdfs:comment "Class to group those properties related to the environment."@en ;
                             rdfs:label "Environmental property"@en ;
                             rdfs:isDefinedBy <https://saref.etsi.org/saref4watr/> .

###  https://saref.etsi.org/saref4watr/GaugingStation
s4watr:GaugingStation rdf:type owl:Class ;
                      rdfs:subClassOf s4watr:MonitoringInfrastructure ;
                      rdfs:comment "A gauging station is an infrastructure to monitor and test terrestrial bodies of water."@en ;
                      rdfs:label "Gauging station"@en ;
                      rdfs:isDefinedBy <https://saref.etsi.org/saref4watr/> .

###  https://saref.etsi.org/saref4watr/Lagoon
s4watr:Lagoon rdf:type owl:Class ;
              rdfs:subClassOf s4watr:SourceAsset ;
              rdfs:comment "A lagoon is a shallow body of water separated from a larger body of water by barrier islands or reefs."@en ;
              rdfs:label "Lagoon"@en ;
              rdfs:isDefinedBy <https://saref.etsi.org/saref4watr/> .

###  https://saref.etsi.org/saref4watr/Lake
s4watr:Lake rdf:type owl:Class ;
            rdfs:subClassOf s4watr:SourceAsset ;
            rdfs:comment "A lake is an area filled with water, localized in a basin, surrounded by land, apart from any river or other outlet that serves to feed or drain the lake."@en ;
            rdfs:label "Lake"@en ;
            rdfs:isDefinedBy <https://saref.etsi.org/saref4watr/> .                      

###  https://saref.etsi.org/saref4watr/MicrobialProperty
s4watr:MicrobialProperty rdf:type owl:Class ;
                         rdfs:subClassOf s4watr:WaterProperty ;
                         rdfs:comment "A microbial property is a property of water that is related to microbes."@en ;
                         rdfs:label "Microbial property"@en .

###  https://saref.etsi.org/saref4watr/MonitoringInfrastructure
s4watr:MonitoringInfrastructure rdf:type owl:Class ;
                                rdfs:subClassOf s4watr:WaterInfrastructure ;
                                rdfs:comment "A monitoring infrastructure is an infrastructure to monitor water."@en ;
                                rdfs:label "Monitoring infrastructure"@en .

###  https://saref.etsi.org/saref4watr/SourceAsset
s4watr:SourceAsset rdf:type owl:Class ;
                   rdfs:subClassOf s4watr:WaterAsset ;
                   rdfs:comment "A source asset is a water asset that is a natural source of water."@en ;
                   rdfs:label "Source asset"@en .

###  https://saref.etsi.org/saref4watr/TreatmentPlant
s4watr:TreatmentPlant rdf:type owl:Class ;
                      rdfs:subClassOf s4watr:WaterInfrastructure ;
                      rdfs:comment "A treatment plant is an infrastructure to improve the quality of water to make it more acceptable for a specific end-use."@en ;
                      rdfs:label "Treatment plant"@en .

###  https://saref.etsi.org/saref4watr/Water
s4watr:Water rdf:type owl:Class ;
             rdfs:subClassOf saref:FeatureOfInterest ,
                             [ rdf:type owl:Restriction ;
                               owl:onProperty saref:hasProperty ;
                               owl:allValuesFrom s4watr:WaterProperty
                             ] ;
             rdfs:comment "This class is used to define a particular quantity or body of water."@en ;
             rdfs:label "Water"@en .

###  https://saref.etsi.org/saref4watr/WaterAsset
s4watr:WaterAsset rdf:type owl:Class ;
                  rdfs:subClassOf geo:Feature ,
                                  saref:FeatureOfInterest ,
                                  ssn:System ;     
                  rdfs:comment "A water asset is a physical entity used in the process of transporting, treating, storing and distributing water."@en ;
                  rdfs:comment "A water infrastructure is a complex system and each of its subsystems may be defined as a water asset"@en ;
                  rdfs:label "Water asset"@en .

###  https://saref.etsi.org/saref4watr/WaterInfrastructure
s4watr:WaterInfrastructure rdf:type owl:Class ;
                           rdfs:subClassOf geo:Feature ,
                                           ssn:System ,
                                           saref:FeatureOfInterest ;
                           rdfs:comment "A water infrastructure is the set of facilities, services, and installations needed for water management."@en ;
                           rdfs:comment "A water infrastructure is a complex system and each of its subsystems may be defined as a water asset"@en ;
                           rdfs:label "Water infrastructure"@en .

###  https://saref.etsi.org/saref4watr/WaterProperty
s4watr:WaterProperty rdf:type owl:Class ;
                     rdfs:subClassOf saref:Property ;
                     rdfs:comment "Class to group those properties related to the water."@en ;
                     rdfs:label "Water property"@en ;
                     rdfs:isDefinedBy <https://saref.etsi.org/saref4watr/> .

### https://smartdatamodels.org/dataModel.Weather/WeatherObserved
fiware-weather:WeatherObserved	a owl:Class ;
			rdfs:label "WeatherObserved" ;
			rdfs:comment "An observation of weather conditions at a certain place and time" ;
			rdfs:isDefinedBy <https://github.com/smart-data-models/dataModel.Weather/blob/master/WeatherObserved/schema.json> .

### https://smartdatamodels.org/dataModel.Weather/WeatherForecast
fiware-weather:WeatherForecast	a owl:Class ;
			rdfs:label "WeatherForecast" ;
			rdfs:comment "A harmonised description of a Weather Forecast" ;
			rdfs:isDefinedBy <https://github.com/smart-data-models/dataModel.Weather/blob/master/WeatherForecast/schema.json> .

### https://smartdatamodels.org/dataModel.Environment/WaterObserved
fiware-environment:WaterObserved	a owl:Class ;
			rdfs:label "WaterObserved" ;
			rdfs:comment "Represents the parameters of flow, level and volume of water observed, as well as the swell information, over a fixed or variable area. This observation also includes the masses of floating objects on this area. The data collected is provided by Sensors, Cameras,Water stations positioned at specific or sensitive locations for rivers, streams, torrent, lakes, seas, etc." ;
			rdfs:isDefinedBy <https://github.com/smart-data-models/dataModel.Environment/blob/master/WaterObserved/schema.json> .

### https://smartdatamodels.org/dataModel.WaterQuality/WaterQualityObserved
fiware-waterquality:WaterQualityObserved	a owl:Class ;
			rdfs:label "WaterQualityObserved" ;
			rdfs:comment "Represents water quality parameters at a certain water mass (river, lake, sea, etc.) section" ;
			rdfs:isDefinedBy <https://github.com/smart-data-models/dataModel.WaterQuality/blob/master/WaterQualityObserved/schema.json> .

### https://smartdatamodels.org/dataModel.WaterQuality/WaterQualityPredicted
fiware-waterquality:WaterQualityPredicted	a owl:Class ;
			rdfs:label "WaterQualityPredicted" ;
			rdfs:comment "Represents predictions of water quality at a certain water mass (river, lake, sea, etc.) section" ;
			rdfs:isDefinedBy <https://github.com/smart-data-models/dataModel.WaterQuality/blob/master/WaterQualityPredicted/schema.json> .

##### Features of Interest subclasses with alignments
###  http://purl.oclc.org/NET/ssnx/cf/cf-feature#Layer
cf-feature:Layer a owl:Class ;
                 rdfs:subClassOf sosa:FeatureOfInterest ;
                 rdfs:label "Layer" ;
                 rdfs:comment "A cf-feature:Layer is something that is a ssn:FeatureOfInterest" ;
                 rdfs:isDefinedBy <http://purl.oclc.org/NET/ssnx/cf/cf-feature> .

###  http://purl.oclc.org/NET/ssnx/cf/cf-feature#Medium
cf-feature:Medium a owl:Class ;
                  rdfs:subClassOf sosa:FeatureOfInterest ;
                  rdfs:label "Medium" ;
                  rdfs:comment "A cf-feature:Medium is something that is a ssn:FeatureOfInterest" ;
                  rdfs:isDefinedBy <http://purl.oclc.org/NET/ssnx/cf/cf-feature> .

###  http://purl.oclc.org/NET/ssnx/cf/cf-feature#Precipitation
cf-feature:Precipitation a owl:Class ;
                         rdfs:subClassOf sosa:FeatureOfInterest ;
                         rdfs:label "Precipitation" ;
                         rdfs:comment "A cf-feature:Precipitation is something that is a ssn:FeatureOfInterest" ;
                         rdfs:isDefinedBy <http://purl.oclc.org/NET/ssnx/cf/cf-feature> .

###  http://purl.oclc.org/NET/ssnx/cf/cf-feature#Surface
cf-feature:Surface a owl:Class ;
                   rdfs:subClassOf sosa:FeatureOfInterest ;
                   rdfs:label "Surface" ;
                   rdfs:comment "A cf-feature:Surface is something that is a ssn:FeatureOfInterest" ;
                   rdfs:isDefinedBy <http://purl.oclc.org/NET/ssnx/cf/cf-feature> .


###  http://purl.oclc.org/NET/ssnx/cf/cf-feature#SurfaceLayer
cf-feature:SurfaceLayer a owl:Class ;
                        rdfs:subClassOf sosa:FeatureOfInterest ;
                        rdfs:label "Surface Layer" ;
                        rdfs:comment "A cf-feature:SurfaceLayer is something that is a ssn:FeatureOfInterest" ;
                        rdfs:isDefinedBy <http://purl.oclc.org/NET/ssnx/cf/cf-feature> .

###  http://purl.oclc.org/NET/ssnx/cf/cf-feature#SurfaceMedium
cf-feature:SurfaceMedium a owl:Class ;
                        rdfs:subClassOf sosa:FeatureOfInterest ;
                        rdfs:label "Surface Medium" ;
                        rdfs:comment "A cf-feature:SurfaceMedium is something that is a ssn:FeatureOfInterest" ;
                        rdfs:isDefinedBy <http://purl.oclc.org/NET/ssnx/cf/cf-feature> .
                        
###  http://purl.oclc.org/NET/ssnx/cf/cf-feature#SurfaceMediumMedium
cf-feature:SurfaceMediumMedium a owl:Class ;
                        rdfs:subClassOf sosa:FeatureOfInterest ;
                        rdfs:label "Surface Medium Medium" ;
                        rdfs:comment "A cf-feature:SurfaceMediumMedium is something that is a ssn:FeatureOfInterest" ;
                        rdfs:isDefinedBy <http://purl.oclc.org/NET/ssnx/cf/cf-feature> .                        

###  http://purl.oclc.org/NET/ssnx/cf/cf-feature#Wind
cf-feature:Wind a owl:Class ;
                rdfs:subClassOf sosa:FeatureOfInterest ;
                rdfs:label "Wind" ;
                rdfs:comment "A cf-feature:Wind is something that is a ssn:FeatureOfInterest" ;
                rdfs:isDefinedBy <http://purl.oclc.org/NET/ssnx/cf/cf-feature> .                                                            

#################################################################
#    Alignments
#################################################################

ssn:hasProperty owl:equivalentProperty saref:hasProperty .
ssn:isPropertyOf owl:equivalentProperty saref:isPropertyOf .
#ssn:Property owl:equivalentClass saref:Property .
sosa:ObservableProperty owl:equivalentClass saref:Property . 
saref:hasFeatureOfInterest owl:equivalentProperty sosa:hasFeatureOfInterest .
saref:isFeatureOfInterestOf owl:equivalentProperty sosa:isFeatureOfInterestOf .
saref:FeatureOfInterest owl:equivalentClass sosa:FeatureOfInterest .
saref:measurementMadeBy owl:equivalentProperty sosa:madeBySensor .
saref:makesMeasurement owl:equivalentProperty sosa:madeObservation .
saref:Property owl:equivalentClass qu:QuantityKind .
saref:Temperature owl:equivalentClass dim:Temperature .
#saref:Measurement owl:equivalentClass iso19103:Measure .
saref:Measurement owl:equivalentClass sosa:Observation .
saref:relatesToProperty owl:equivalentProperty sosa:observedProperty .
saref:hasTimestamp owl:equivalentProperty sosa:resultTime .
saref:hasValue owl:equivalentProperty sosa:hasSimpleResult .
saref:isMeasuredIn owl:equivalentProperty qudt:unit .
saref:UnitOfMeasure owl:equivalentClass qudt:Unit .
fiware:dateObserved rdfs:subPropertyOf saref:hasTimestamp .
fiware-weather:temperature rdfs:subPropertyOf saref:hasValue .
fiware-weather:atmosphericPressure rdfs:subPropertyOf saref:hasValue .
fiware-weather:WeatherObserved rdfs:subClassOf saref:FeatureOfInterest .
fiware-weather:WeatherForecast rdfs:subClassOf saref:FeatureOfInterest .
fiware-weather:dewPoint rdfs:subPropertyOf saref:hasValue .
fiware-weather:visibility rdfs:subPropertyOf saref:hasValue .
fiware-weather:airTemperatureForecast rdfs:subPropertyOf saref:hasValue .
fiware-weather:relativeHumidity rdfs:subPropertyOf saref:hasValue .
fiware-weather:precipitation rdfs:subPropertyOf saref:hasValue .
fiware-weather:windDirection rdfs:subPropertyOf saref:hasValue .
fiware-weather:windSpeed rdfs:subPropertyOf saref:hasValue .
fiware-weather:pressureTendency rdfs:subPropertyOf saref:hasValue .
fiware-weather:solarRadiation rdfs:subPropertyOf saref:hasValue .
fiware-weather:illuminance rdfs:subPropertyOf saref:hasValue .
fiware-weather:streamGauge rdfs:subPropertyOf saref:hasValue .
fiware-weather:snowHeight rdfs:subPropertyOf saref:hasValue .
saref:Device owl:equivalentClass ssn:System .


#################################################################
#    Individuals
#################################################################

###  http://dbpedia.org/resource/DBM
<http://dbpedia.org/resource/DBM> a owl:NamedIndividual ,
                                           saref:UnitOfMeasure ;
                                rdfs:isDefinedBy <https://en.wikipedia.org/wiki/DBm> ;
                                rdfs:comment "a unit for power measurement" ;
                                rdfs:label "decibel-milliwatts"@en .

#### units of measurements from om-2

###  http://www.ontology-of-units-of-measure.org/resource/om-2/degreeCelsius
<http://www.ontology-of-units-of-measure.org/resource/om-2/degreeCelsius> a owl:NamedIndividual ,
                                                                         saref:UnitOfMeasure ;
                                                                          rdfs:isDefinedBy <http://www.ontology-of-units-of-measure.org/resource/om-2/degreeCelsius> ;
                                                                          rdfs:comment "The degree Celsius is a unit of temperature defined as 1 kelvin." ;         
                                                                          rdfs:label "degree Celsius"@en .

###  http://www.ontology-of-units-of-measure.org/resource/om-2/millibar
<http://www.ontology-of-units-of-measure.org/resource/om-2/millibar> a owl:NamedIndividual ,
                                                                        saref:UnitOfMeasure ;
                                                                     rdfs:isDefinedBy <http://www.ontology-of-units-of-measure.org/resource/om-2/millibar> ;
                                                                      rdfs:comment "The millibar is a unit of pressure defined as 1.0e-3 bar." ;          
                                                                     rdfs:label "millibar"@en .

###  http://www.ontology-of-units-of-measure.org/resource/om-2/millimetre
<http://www.ontology-of-units-of-measure.org/resource/om-2/millimetre> a owl:NamedIndividual ,
                                                                        saref:UnitOfMeasure ;
                                                                      rdfs:isDefinedBy <http://www.ontology-of-units-of-measure.org/resource/om-2/millimetre> ;
                                                                      rdfs:comment "The millimetre is a unit of length defined as 1.0e-3 metre." ;
                                                                       rdfs:label "millimetre"@en .

###  http://www.ontology-of-units-of-measure.org/resource/om-2/millivolt
<http://www.ontology-of-units-of-measure.org/resource/om-2/millivolt> a owl:NamedIndividual ,
                                                                        saref:UnitOfMeasure ;
                                                                      rdfs:isDefinedBy <http://www.ontology-of-units-of-measure.org/resource/om-2/millivolt> ;
                                                                      rdfs:comment "The millivolt is a unit of Voltage" ;
                                                                      rdfs:label "millivolt"@en .


####### chemical water properties to be used as observed properties (recommended)

###  https://saref.etsi.org/saref4watr/Acrylamide
s4watr:Acrylamide rdf:type owl:NamedIndividual ,
                           s4watr:ChemicalProperty ;
                  rdfs:comment "Property of the water indicating its concentration of acrylamide."@en ;
                  rdfs:label "Acrylamide"@en .

###  https://saref.etsi.org/saref4watr/Aluminium
s4watr:Aluminium rdf:type owl:NamedIndividual ,
                          s4watr:ChemicalProperty ;
                 rdfs:comment "Property of the water indicating its concentration of aluminium."@en ;
                 rdfs:label "Aluminium"@en .

###  https://saref.etsi.org/saref4watr/Ammonium
s4watr:Ammonium rdf:type owl:NamedIndividual ,
                         s4watr:ChemicalProperty ;
                rdfs:comment "Property of the water indicating its concentration of ammonium."@en ;
                rdfs:label "Ammonium"@en .


###  https://saref.etsi.org/saref4watr/Antimony
s4watr:Antimony rdf:type owl:NamedIndividual ,
                         s4watr:ChemicalProperty ;
                rdfs:comment "Property of the water indicating its concentration of antimony."@en ;
                rdfs:label "Antimony"@en .


###  https://saref.etsi.org/saref4watr/AtmosphericPressure
###  duplicated term
s4watr:AtmosphericPressure rdf:type owl:NamedIndividual ,
                                    s4watr:EnvironmentalProperty ;
                           rdfs:comment "Property of the environment indicating the atmospheric pressure."@en ;
                           rdfs:label "Atmospheric pressure"@en .


###  https://saref.etsi.org/saref4watr/Arsenic
s4watr:Arsenic rdf:type owl:NamedIndividual ,
                        s4watr:ChemicalProperty ;
               rdfs:comment "Property of the water indicating its concentration of arsenic."@en ;
               rdfs:label "Arsenic"@en .

###  https://saref.etsi.org/saref4watr/Benzene
s4watr:Benzene rdf:type owl:NamedIndividual ,
                        s4watr:ChemicalProperty ;
               rdfs:comment "Property of the water indicating its concentration of benzene."@en ;
               rdfs:label "Benzene"@en .


###  https://saref.etsi.org/saref4watr/Benzoapyrene
s4watr:Benzoapyrene rdf:type owl:NamedIndividual ,
                             s4watr:ChemicalProperty ;
                    rdfs:comment "Property of the water indicating its concentration of benzo(a)pyrene."@en ;
                    rdfs:label "Benzo(a)pyrene"@en .


###  https://saref.etsi.org/saref4watr/Boron
s4watr:Boron rdf:type owl:NamedIndividual ,
                      s4watr:ChemicalProperty ;
             rdfs:comment "Property of the water indicating its concentration of boron."@en ;
             rdfs:label "Boron"@en .


###  https://saref.etsi.org/saref4watr/Bromate
s4watr:Bromate rdf:type owl:NamedIndividual ,
                        s4watr:ChemicalProperty ;
               rdfs:comment "Property of the water indicating its concentration of bromate."@en ;
               rdfs:label "Bromate"@en .


###  https://saref.etsi.org/saref4watr/Cadmium
s4watr:Cadmium rdf:type owl:NamedIndividual ,
                        s4watr:ChemicalProperty ;
               rdfs:comment "Property of the water indicating its concentration of cadmium."@en ;
               rdfs:label "Cadmium"@en .


###  https://saref.etsi.org/saref4watr/Chloride
s4watr:Chloride rdf:type owl:NamedIndividual ,
                         s4watr:ChemicalProperty ;
                rdfs:comment "Property of the water indicating its concentration of chloride."@en ;
                rdfs:label "Chloride"@en .


###  https://saref.etsi.org/saref4watr/Chromium
s4watr:Chromium rdf:type owl:NamedIndividual ,
                         s4watr:ChemicalProperty ;
                rdfs:comment "Property of the water indicating its concentration of chromium."@en ;
                rdfs:label "Chromium"@en .


###  https://saref.etsi.org/saref4watr/ClostridiumPerfringens
s4watr:ClostridiumPerfringens rdf:type owl:NamedIndividual ,
                                       s4watr:BacterialProperty ;
                              rdfs:comment "Property of the water indicating its concentration of clostridium perfringens."@en ;
                              rdfs:label "Clostridium perfringens"@en .


###  https://saref.etsi.org/saref4watr/ColiformBacteria
s4watr:ColiformBacteria rdf:type owl:NamedIndividual ,
                                 s4watr:BacterialProperty ;
                        rdfs:comment "Property of the water indicating its concentration of coliform bacteria."@en ;
                        rdfs:label "Coliform bacteria"@en .


###  https://saref.etsi.org/saref4watr/ColonyCount22C
s4watr:ColonyCount22C rdf:type owl:NamedIndividual ,
                               s4watr:BacterialProperty ;
                      rdfs:comment "Property of the water indicating its colony count at 22 ÂºC."@en ;
                      rdfs:label "Colony count at 22 Â°C"@en .


###  https://saref.etsi.org/saref4watr/ColonyCount37C
s4watr:ColonyCount37C rdf:type owl:NamedIndividual ,
                               s4watr:BacterialProperty ;
                      rdfs:comment "Property of the water indicating its colony count at 37 ÂºC."@en ;
                      rdfs:label "Colony count at 37 Â°C"@en .


###  https://saref.etsi.org/saref4watr/Colour
s4watr:Colour rdf:type owl:NamedIndividual ,
                       s4watr:AcceptabilityProperty ;
              rdfs:comment "Property of the water indicating its colour."@en ;
              rdfs:label "Colour"@en .


###  https://saref.etsi.org/saref4watr/Conductivity
###  duplicated term
s4watr:Conductivity rdf:type owl:NamedIndividual ,
                             s4watr:AcceptabilityProperty ;
                    rdfs:comment "Property of the water indicating its conductivity."@en ;
                    rdfs:label "Conductivity"@en .


###  https://saref.etsi.org/saref4watr/Copper
s4watr:Copper rdf:type owl:NamedIndividual ,
                       s4watr:ChemicalProperty ;
              rdfs:comment "Property of the water indicating its concentration of copper."@en ;
              rdfs:label "Copper"@en .


###  https://saref.etsi.org/saref4watr/Cyanide
s4watr:Cyanide rdf:type owl:NamedIndividual ,
                        s4watr:ChemicalProperty ;
               rdfs:comment "Property of the water indicating its concentration of cyanide."@en ;
               rdfs:label "Cyanide"@en .


###  https://saref.etsi.org/saref4watr/Enterococci
###  duplicated term
s4watr:Enterococci rdf:type owl:NamedIndividual ,
                            s4watr:BacterialProperty ;
                   rdfs:comment "Property of the water indicating its concentration of enterococci."@en ;
                   rdfs:label "Enterococci"@en .


###  https://saref.etsi.org/saref4watr/Epichlorohydrin
s4watr:Epichlorohydrin rdf:type owl:NamedIndividual ,
                                s4watr:ChemicalProperty ;
                       rdfs:comment "Property of the water indicating its concentration of epichlorohydrin."@en ;
                       rdfs:label "Epichlorohydrin"@en .


###  https://saref.etsi.org/saref4watr/EscherichiaColi
###  duplicated term
s4watr:EscherichiaColi rdf:type owl:NamedIndividual ,
                                s4watr:BacterialProperty ;
                       rdfs:comment "Property of the water indicating its concentration of escherichia coli."@en ;
                       rdfs:label "E. coli"@en ,
                                  "Escherichia coli"@en .


###  https://saref.etsi.org/saref4watr/ExternalTemperature
s4watr:ExternalTemperature rdf:type owl:NamedIndividual ,
                                    s4watr:EnvironmentalProperty ;
                           rdfs:comment "Property of the environment indicating the temperature."@en ;
                           rdfs:label "External temperature"@en .

###  https://saref.etsi.org/saref4watr/Fluoride
###  duplicated term
s4watr:Fluoride rdf:type owl:NamedIndividual ,
                         s4watr:ChemicalProperty ;
                rdfs:comment "Property of the water indicating its concentration of fluoride."@en ;
                rdfs:label "Fluoride"@en .


###  https://saref.etsi.org/saref4watr/Hardness
s4watr:Hardness rdf:type owl:NamedIndividual ,
                         s4watr:AcceptabilityProperty ;
                rdfs:comment "Property of the water indicating its hardness."@en ;
                rdfs:label "Hardness"@en .


###  https://saref.etsi.org/saref4watr/Humidity
###  duplicated term including case
s4watr:Humidity rdf:type owl:NamedIndividual ,
                         s4watr:EnvironmentalProperty ;
                rdfs:comment "Property of the environment indicating the humidity."@en ;
                rdfs:label "Humidity"@en .


###  https://saref.etsi.org/saref4watr/HydrogenIonConcentration
s4watr:HydrogenIonConcentration rdf:type owl:NamedIndividual ,
                                         s4watr:AcceptabilityProperty ;
                                rdfs:comment "Property of the water indicating its hydrogen ion concentration."@en ;
                                rdfs:label "Hydrogen ion concentration"@en ,
                                           "pH"@en .


###  https://saref.etsi.org/saref4watr/Iron
s4watr:Iron rdf:type owl:NamedIndividual ,
                     s4watr:ChemicalProperty ;
            rdfs:comment "Property of the water indicating its concentration of iron."@en ;
            rdfs:label "Iron"@en .


###  https://saref.etsi.org/saref4watr/Lead
s4watr:Lead rdf:type owl:NamedIndividual ,
                     s4watr:ChemicalProperty ;
            rdfs:comment "Property of the water indicating its concentration of lead."@en ;
            rdfs:label "Lead"@en .


###  https://saref.etsi.org/saref4watr/Manganese
s4watr:Manganese rdf:type owl:NamedIndividual ,
                          s4watr:ChemicalProperty ;
                 rdfs:comment "Property of the water indicating its concentration of manganese."@en ;
                 rdfs:label "Manganese"@en .


###  https://saref.etsi.org/saref4watr/Mercury
s4watr:Mercury rdf:type owl:NamedIndividual ,
                        s4watr:ChemicalProperty ;
               rdfs:comment "Property of the water indicating its concentration of mercury."@en ;
               rdfs:label "Mercury"@en .

###  https://saref.etsi.org/saref4watr/Nickel
s4watr:Nickel rdf:type owl:NamedIndividual ,
                       s4watr:ChemicalProperty ;
              rdfs:comment "Property of the water indicating its concentration of nickel."@en ;
              rdfs:label "Nickel"@en .


###  https://saref.etsi.org/saref4watr/Nitrate
s4watr:Nitrate rdf:type owl:NamedIndividual ,
                        s4watr:ChemicalProperty ;
               rdfs:comment "Property of the water indicating its concentration of nitrate."@en ;
               rdfs:label "Nitrate"@en .


###  https://saref.etsi.org/saref4watr/Nitrite
s4watr:Nitrite rdf:type owl:NamedIndividual ,
                        s4watr:ChemicalProperty ;
               rdfs:comment "Property of the water indicating its concentration of nitrite."@en ;
               rdfs:label "Nitrite"@en .


###  https://saref.etsi.org/saref4watr/Odour
s4watr:Odour rdf:type owl:NamedIndividual ,
                      s4watr:AcceptabilityProperty ;
             rdfs:comment "Property of the water indicating its odour."@en ;
             rdfs:label "Odour"@en .


###  https://saref.etsi.org/saref4watr/Oxidisability
s4watr:Oxidisability rdf:type owl:NamedIndividual ,
                              s4watr:AcceptabilityProperty ;
                     rdfs:comment "Property of the water indicating its oxidisability."@en ;
                     rdfs:label "Oxidisability"@en .


###  https://saref.etsi.org/saref4watr/Oxygen
s4watr:Oxygen rdf:type owl:NamedIndividual ,
                       s4watr:ChemicalProperty ;
              rdfs:comment "Property of the water indicating its oxygen saturation."@en ;
              rdfs:label "Oxygen"@en ,
                         "Oxygen saturation"@en ,
                         "Dissolved oxygen"@en .


###  https://saref.etsi.org/saref4watr/PolycyclicAromaticHydrocarbons
s4watr:PolycyclicAromaticHydrocarbons rdf:type owl:NamedIndividual ,
                                               s4watr:ChemicalProperty ;
                                      rdfs:comment "Property of the water indicating its concentration of polycyclic aromatic hydrocarbons."@en ;
                                      rdfs:label "Polycyclic aromatic hydrocarbons"@en .


###  https://saref.etsi.org/saref4watr/Precipitation
###  duplicated term, also with case
s4watr:Precipitation rdf:type owl:NamedIndividual ,
                              s4watr:EnvironmentalProperty ;
                     rdfs:comment "Property of the environment indicating the precipitation."@en ;
                     rdfs:label "Precipitation"@en .


###  https://saref.etsi.org/saref4watr/PseudomonasAeruginosa
s4watr:PseudomonasAeruginosa rdf:type owl:NamedIndividual ,
                                      s4watr:BacterialProperty ;
                             rdfs:comment "Property of the water indicating its concentration of pseudomonas aeruginosa."@en ;
                             rdfs:label "Pseudomonas aeruginosa"@en .

###  https://saref.etsi.org/saref4watr/Selenium
s4watr:Selenium rdf:type owl:NamedIndividual ,
                         s4watr:ChemicalProperty ;
                rdfs:comment "Property of the water indicating its concentration of selenium."@en ;
                rdfs:label "Selenium"@en .


###  https://saref.etsi.org/saref4watr/Sodium
s4watr:Sodium rdf:type owl:NamedIndividual ,
                       s4watr:ChemicalProperty ;
              rdfs:comment "Property of the water indicating its concentration of sodium."@en ;
              rdfs:label "Sodium"@en .

###  https://saref.etsi.org/saref4watr/Sulphate
###  duplicated term
s4watr:Sulphate rdf:type owl:NamedIndividual ,
                         s4watr:ChemicalProperty ;
                rdfs:comment "Property of the water indicating its concentration of sulphate."@en ;
                rdfs:label "Sulphate"@en .


###  https://saref.etsi.org/saref4watr/Taste
s4watr:Taste rdf:type owl:NamedIndividual ,
                      s4watr:AcceptabilityProperty ;
             rdfs:comment "Property of the water indicating its taste."@en ;
             rdfs:label "Taste"@en .


###  https://saref.etsi.org/saref4watr/Temperature
###  duplicted term, including case
s4watr:Temperature rdf:type owl:NamedIndividual ,
                            s4watr:AcceptabilityProperty ;
                   rdfs:comment "Property of the water indicating its temperature."@en ;
                   rdfs:label "Temperature"@en .


###  https://saref.etsi.org/saref4watr/Tetrachloroethene
s4watr:Tetrachloroethene rdf:type owl:NamedIndividual ,
                                  s4watr:ChemicalProperty ;
                         rdfs:comment "Property of the water indicating its concentration of tetrachloroethene."@en ;
                         rdfs:label "Tetrachloroethene"@en .


###  https://saref.etsi.org/saref4watr/TotalIndicativeDose
s4watr:TotalIndicativeDose rdf:type owl:NamedIndividual ,
                                    s4watr:AcceptabilityProperty ;
                           rdfs:comment "Property of the water indicating its total indicative dose."@en ;
                           rdfs:label "Total indicative dose"@en .


###  https://saref.etsi.org/saref4watr/TotalDissolvedSolids
s4watr:TotalDissolvedSolids rdf:type owl:NamedIndividual ,
                                     s4watr:AcceptabilityProperty ;
                            rdfs:comment "Property of the water indicating the dissolved combined content of all inorganic and organic substances present in a sample of water."@en ;
                            rdfs:label "Total dissolved solids"@en .


###  https://saref.etsi.org/saref4watr/TotalOrganicCarbon
s4watr:TotalOrganicCarbon rdf:type owl:NamedIndividual ,
                                   s4watr:ChemicalProperty ;
                          rdfs:comment "Property of the water indicating its concentration of total organic carbon."@en ;
                          rdfs:label "TOC"@en ,
                                     "Total organic carbon"@en .


###  https://saref.etsi.org/saref4watr/TotalSuspendedSolids
s4watr:TotalSuspendedSolids rdf:type owl:NamedIndividual ,
                                     s4watr:AcceptabilityProperty ;
                            rdfs:comment "Property of the water indicating the dry-weight of suspended particles, that are not dissolved, in a sample of water."@en ;
                            rdfs:label "Total suspended solids"@en .


###  https://saref.etsi.org/saref4watr/Trichloroethene
s4watr:Trichloroethene rdf:type owl:NamedIndividual ,
                                s4watr:ChemicalProperty ;
                       rdfs:comment "Property of the water indicating its concentration of trichloroethene."@en ;
                       rdfs:label "Trichloroethene"@en .


###  https://saref.etsi.org/saref4watr/Trihalomethanes
s4watr:Trihalomethanes rdf:type owl:NamedIndividual ,
                                s4watr:ChemicalProperty ;
                       rdfs:comment "Property of the water indicating its concentration of trihalomethanes."@en ;
                       rdfs:label "Trihalomethanes"@en .


###  https://saref.etsi.org/saref4watr/Tritium
s4watr:Tritium rdf:type owl:NamedIndividual ,
                        s4watr:ChemicalProperty ;
               rdfs:comment "Property of the water indicating its concentration of tritium."@en ;
               rdfs:label "Tritium"@en .


###  https://saref.etsi.org/saref4watr/Turbidity
###  duplicated term
s4watr:Turbidity rdf:type owl:NamedIndividual ,
                          s4watr:AcceptabilityProperty ;
                 rdfs:comment "Property of the water indicating its turbidity."@en ;
                 rdfs:label "Turbidity"@en .


###  https://saref.etsi.org/saref4watr/VinylChloride
s4watr:VinylChloride rdf:type owl:NamedIndividual ,
                              s4watr:ChemicalProperty ;
                     rdfs:comment "Property of the water indicating its concentration of vinyl chloride."@en ;
                     rdfs:label "Vinyl chloride"@en .

###  https://saref.etsi.org/saref4watr/12Dichloroethane
s4watr:12Dichloroethane rdf:type owl:NamedIndividual ,
                                 s4watr:ChemicalProperty ;
                        rdfs:comment "Property of the water indicating its concentration of 1,2-dichloroethane."@en ;
                        rdfs:label "1,2-dichloroethane"@en .

####### end of chemical water properties to be used as observed properties (recommended)

########## features of interest from cf-feature

###  http://purl.oclc.org/NET/ssnx/cf/cf-feature#water
cf-feature:water a owl:NamedIndividual ,
                          cf-feature:Medium ;
                 rdfs:label "water" ;
                 rdfs:comment "water" ;
                 rdfs:isDefinedBy <http://purl.oclc.org/NET/ssnx/cf/cf-feature> .
  
<http://purl.oclc.org/NET/ssnx/cf/cf-feature#air>
  a owl:NamedIndividual, <http://purl.oclc.org/NET/ssnx/cf/cf-feature#Medium> ;
  rdfs:label "air" ;
  rdfs:isDefinedBy <http://purl.oclc.org/NET/ssnx/cf/cf-feature> .

<http://purl.oclc.org/NET/ssnx/cf/cf-feature#cloud_base_air>
  a <http://purl.oclc.org/NET/ssnx/cf/cf-feature#SurfaceMedium> ;
  rdfs:label "cloud base air" ;
  rdfs:isDefinedBy <http://purl.oclc.org/NET/ssnx/cf/cf-feature> .

<http://purl.oclc.org/NET/ssnx/cf/cf-feature#cloud_top_air>
  a <http://purl.oclc.org/NET/ssnx/cf/cf-feature#SurfaceMedium> ;
  rdfs:label "convective cloud top air" ;  
  rdfs:isDefinedBy <http://purl.oclc.org/NET/ssnx/cf/cf-feature> .

<http://purl.oclc.org/NET/ssnx/cf/cf-feature#convective_cloud_base_air>
  a <http://purl.oclc.org/NET/ssnx/cf/cf-feature#SurfaceMedium> ;
  rdfs:label "convective cloud base air" ;  
  rdfs:isDefinedBy <http://purl.oclc.org/NET/ssnx/cf/cf-feature> .

<http://purl.oclc.org/NET/ssnx/cf/cf-feature#convective_cloud_top_air>
  a <http://purl.oclc.org/NET/ssnx/cf/cf-feature#SurfaceMedium> ;
  rdfs:label "convective cloud top air" ;  
  rdfs:isDefinedBy <http://purl.oclc.org/NET/ssnx/cf/cf-feature> .

<http://purl.oclc.org/NET/ssnx/cf/cf-feature#freezing_level_air>
  a <http://purl.oclc.org/NET/ssnx/cf/cf-feature#SurfaceMedium> ;
  rdfs:label "freezing level air" ;  
  rdfs:isDefinedBy <http://purl.oclc.org/NET/ssnx/cf/cf-feature> .

<http://purl.oclc.org/NET/ssnx/cf/cf-feature#surface_air>
  a <http://purl.oclc.org/NET/ssnx/cf/cf-feature#SurfaceMedium> ;
  rdfs:label "surface air" ;  
  rdfs:isDefinedBy <http://purl.oclc.org/NET/ssnx/cf/cf-feature> .

<http://purl.oclc.org/NET/ssnx/cf/cf-feature#tropopause_air>
  a <http://purl.oclc.org/NET/ssnx/cf/cf-feature#SurfaceMedium> ;
  rdfs:label "tropopause air" ;  
  rdfs:isDefinedBy <http://purl.oclc.org/NET/ssnx/cf/cf-feature> .

########## observed properties from cf-property
###  http://purl.oclc.org/NET/ssnx/cf/cf-property#air_density
cf:air_density a owl:NamedIndividual ,
                        dim:Density ;
               rdfs:label "air density" ;
               rdfs:comment "The amount of air in per cubic volume" ;
               rdfs:isDefinedBy <http://purl.oclc.org/NET/ssnx/cf/cf-property> .

<http://purl.oclc.org/NET/ssnx/cf/cf-property#air_potential_temperature>
  a owl:NamedIndividual, <http://purl.oclc.org/NET/ssnx/qu/dim#Temperature> ;
  rdfs:label "air potential temperature" ;
  rdfs:isDefinedBy <http://purl.oclc.org/NET/ssnx/cf/cf-property> ;
  rdfs:comment "Potential temperature is the temperature a parcel of air or sea water would have if moved adiabatically to sea level pressure." .

<http://purl.oclc.org/NET/ssnx/cf/cf-property#air_pressure>
  a owl:NamedIndividual, <http://purl.oclc.org/NET/ssnx/qu/dim#StressOrPressure> ;
  rdfs:label "air pressure" ;
  rdfs:isDefinedBy <http://purl.oclc.org/NET/ssnx/cf/cf-property> .

<http://purl.oclc.org/NET/ssnx/cf/cf-property#air_pressure_anomaly>
  a owl:NamedIndividual, <http://purl.oclc.org/NET/ssnx/qu/dim#StressOrPressure> ;
  rdfs:label "air pressure anomaly" ;
  rdfs:isDefinedBy <http://purl.oclc.org/NET/ssnx/cf/cf-property> ;
  rdfs:comment "anomaly means difference from climatology." .

<http://purl.oclc.org/NET/ssnx/cf/cf-property#air_temperature>
  a owl:NamedIndividual, <http://purl.oclc.org/NET/ssnx/qu/dim#Temperature> ;
  rdfs:label "air temperature" ;
  rdfs:isDefinedBy <http://purl.oclc.org/NET/ssnx/cf/cf-property> ;
  rdfs:comment "Air temperature is the bulk temperature of the air, not the surface (skin) temperature." .

<http://purl.oclc.org/NET/ssnx/cf/cf-property#air_temperature_anomaly>
  a owl:NamedIndividual, <http://purl.oclc.org/NET/ssnx/qu/dim#Temperature> ;
  rdfs:label "air temperature anomaly" ;
  rdfs:isDefinedBy <http://purl.oclc.org/NET/ssnx/cf/cf-property> ;
  rdfs:comment "anomaly means difference from climatology. Air temperature is the bulk temperature of the air, not the surface (skin) temperature." .

<http://purl.oclc.org/NET/ssnx/cf/cf-property#air_temperature_threshold>
  a owl:NamedIndividual, <http://purl.oclc.org/NET/ssnx/qu/dim#Temperature> ;
  rdfs:label "air temperature threshold" ;
  rdfs:isDefinedBy <http://purl.oclc.org/NET/ssnx/cf/cf-property> ;
  rdfs:comment "Air temperature is the bulk temperature of the air, not the surface (skin) temperature. Air temperature excess and deficit are calculated relative to the air temperature threshold." .

<http://purl.oclc.org/NET/ssnx/cf/cf-property#angstrom_exponent_of_ambient_aerosol_in_air>
  a owl:NamedIndividual, <http://purl.oclc.org/NET/ssnx/qu/dim#Dimensionless> ;
  rdfs:label "angstrom exponent of ambient aerosol in air" ;
  rdfs:isDefinedBy <http://purl.oclc.org/NET/ssnx/cf/cf-property> ;
  rdfs:comment " Aerosol means the suspended liquid or solid particles in air (except cloud droplets).  Ambient aerosol is aerosol that has taken up ambient water through hygroscopic growth. The extent of hygroscopic growth depends on the relative humidity and the composition of the aerosol. The Angstrom exponent appears in the formula relating aerosol optical thickness to the wavelength of incident radiation: T(lambda) = T(lambda0) * [lambda/lambda0] ** (-1 * alpha) where alpha is the Angstrom exponent, lambda is the wavelength of incident radiation, lambda0 is a reference wavelength, T(lambda) and T(lambda0) are the values of aerosol optical thickness at wavelengths lambda and lambda0, respectively." .

<http://purl.oclc.org/NET/ssnx/cf/cf-property#downward_eastward_momentum_flux_in_air>
  a owl:NamedIndividual, <http://purl.oclc.org/NET/ssnx/qu/dim#StressOrPressure> ;
  rdfs:label "downward eastward momentum flux in air" ;
  rdfs:isDefinedBy <http://purl.oclc.org/NET/ssnx/cf/cf-property> ;
  rdfs:comment "Eastward indicates a vector component which is positive when directed eastward (negative westward). Downward indicates a vector component which is positive when directed downward (negative upward). Downward eastward indicates the ZX component of a tensor. Momentum flux is dimensionally equivalent to stress and pressure. It is a tensor quantity. In accordance with common usage in geophysical disciplines, flux implies per unit area, called flux density in physics." .

<http://purl.oclc.org/NET/ssnx/cf/cf-property#downward_heat_flux_in_air>
  a owl:NamedIndividual, <http://purl.oclc.org/NET/ssnx/qu/dim#EnergyFlux> ;
  rdfs:label "downward heat flux in air" ;
  rdfs:isDefinedBy <http://purl.oclc.org/NET/ssnx/cf/cf-property> ;
  rdfs:comment "Downward indicates a vector component which is positive when directed downward (negative upward). The vertical heat flux in air is the sum of all heat fluxes i.e. radiative, latent and sensible. In accordance with common usage in geophysical disciplines, flux implies per unit area, called flux density in physics." .

<http://purl.oclc.org/NET/ssnx/cf/cf-property#downward_northward_momentum_flux_in_air>
  a owl:NamedIndividual, <http://purl.oclc.org/NET/ssnx/qu/dim#StressOrPressure> ;
  rdfs:label "downward northward momentum flux in air" ;
  rdfs:isDefinedBy <http://purl.oclc.org/NET/ssnx/cf/cf-property> ;
  rdfs:comment "Northward indicates a vector component which is positive when directed northward (negative southward). Downward indicates a vector component which is positive when directed downward (negative upward). Downward northward indicates the ZY component of a tensor. Momentum flux is dimensionally equivalent to stress and pressure. It is a tensor quantity. In accordance with common usage in geophysical disciplines, flux implies per unit area, called flux density in physics." .

<http://purl.oclc.org/NET/ssnx/cf/cf-property#downward_water_vapor_flux_in_air_due_to_diffusion>
  a owl:NamedIndividual, <http://purl.oclc.org/NET/ssnx/qu/dim#MassPerTimePerArea> ;
  rdfs:label "downward water vapor flux in air due to diffusion" ;
  rdfs:isDefinedBy <http://purl.oclc.org/NET/ssnx/cf/cf-property> ;
  rdfs:comment "The specification of a physical process by the phrase due_to_process means that the quantity named is a single term in a sum of terms which together compose the general quantity named by omitting the phrase. Downward indicates a vector component which is positive when directed downward (negative upward). In accordance with common usage in geophysical disciplines, flux implies per unit area, called flux density in physics." .

<http://purl.oclc.org/NET/ssnx/cf/cf-property#downwelling_longwave_flux_in_air>
  a owl:NamedIndividual, <http://purl.oclc.org/NET/ssnx/qu/dim#EnergyFlux> ;
  rdfs:label "downwelling longwave flux in air" ;
  rdfs:isDefinedBy <http://purl.oclc.org/NET/ssnx/cf/cf-property> ;
  rdfs:comment "longwave means longwave radiation. Downwelling radiation is radiation from above. It does not mean net downward. When thought of as being incident on a surface, a radiative flux is sometimes called irradiance. In addition, it is identical with the quantity measured by a cosine-collector light-meter and sometimes called vector irradiance. In accordance with common usage in geophysical disciplines, flux implies per unit area, called flux density in physics." .

<http://purl.oclc.org/NET/ssnx/cf/cf-property#downwelling_longwave_flux_in_air_assuming_clear_sky>
  a owl:NamedIndividual, <http://purl.oclc.org/NET/ssnx/qu/dim#EnergyFlux> ;
  rdfs:label "downwelling longwave flux in air assuming clear sky" ;
  rdfs:isDefinedBy <http://purl.oclc.org/NET/ssnx/cf/cf-property> ;
  rdfs:comment "Downwelling radiation is radiation from above. It does not mean net downward.  When thought of as being incident on a surface, a radiative flux is sometimes called irradiance.  In addition, it is identical with the quantity measured by a cosine-collector light-meter and sometimes called vector irradiance.  In accordance with common usage in geophysical disciplines, flux implies per unit area, called flux density in physics.  A phrase assuming_condition  indicates that the named quantity is the value which would obtain if all  aspects of the system were unaltered except for the assumption of the  circumstances specified by the condition.  longwave means longwave radiation. " .

<http://purl.oclc.org/NET/ssnx/cf/cf-property#downwelling_longwave_radiance_in_air>
  a owl:NamedIndividual, <http://purl.oclc.org/NET/ssnx/qu/dim#Radiance> ;
  rdfs:label "downwelling longwave radiance in air" ;
  rdfs:isDefinedBy <http://purl.oclc.org/NET/ssnx/cf/cf-property> ;
  rdfs:comment "longwave means longwave radiation. Downwelling radiation is radiation from above. It does not mean net downward. Radiance is the radiative flux in a particular direction, per unit of solid angle. The direction from which it is coming must be specified, for instance with a coordinate of zenith_angle. If the radiation does not depend on direction, a standard name of isotropic radiance should be chosen instead." .

<http://purl.oclc.org/NET/ssnx/cf/cf-property#downwelling_shortwave_flux_in_air>
  a owl:NamedIndividual, <http://purl.oclc.org/NET/ssnx/qu/dim#EnergyFlux> ;
  rdfs:label "downwelling shortwave flux in air" ;
  rdfs:isDefinedBy <http://purl.oclc.org/NET/ssnx/cf/cf-property> ;
  rdfs:comment "shortwave means shortwave radiation. Downwelling radiation is radiation from above. It does not mean net downward. When thought of as being incident on a surface, a radiative flux is sometimes called irradiance. In addition, it is identical with the quantity measured by a cosine-collector light-meter and sometimes called vector irradiance. In accordance with common usage in geophysical disciplines, flux implies per unit area, called flux density in physics." .

<http://purl.oclc.org/NET/ssnx/cf/cf-property#downwelling_shortwave_flux_in_air_assuming_clear_sky>
  a owl:NamedIndividual, <http://purl.oclc.org/NET/ssnx/qu/dim#EnergyFlux> ;
  rdfs:label "downwelling shortwave flux in air assuming clear sky" ;
  rdfs:isDefinedBy <http://purl.oclc.org/NET/ssnx/cf/cf-property> ;
  rdfs:comment "Downwelling radiation is radiation from above. It does not mean net downward.  When thought of as being incident on a surface, a radiative flux is sometimes called irradiance.  In addition, it is identical with the quantity measured by a cosine-collector light-meter and sometimes called vector irradiance.  In accordance with common usage in geophysical disciplines, flux implies per unit area, called flux density in physics.  A phrase assuming_condition  indicates that the named quantity is the value which would obtain if all  aspects of the system were unaltered except for the assumption of the  circumstances specified by the condition.  shortwave means shortwave radiation. " .

<http://purl.oclc.org/NET/ssnx/cf/cf-property#downwelling_shortwave_radiance_in_air>
  a owl:NamedIndividual, <http://purl.oclc.org/NET/ssnx/qu/dim#Radiance> ;
  rdfs:label "downwelling shortwave radiance in air" ;
  rdfs:isDefinedBy <http://purl.oclc.org/NET/ssnx/cf/cf-property> ;
  rdfs:comment "shortwave means shortwave radiation. Downwelling radiation is radiation from above. It does not mean net downward. Radiance is the radiative flux in a particular direction, per unit of solid angle. The direction from which it is coming must be specified, for instance with a coordinate of zenith_angle. If the radiation does not depend on direction, a standard name of isotropic radiance should be chosen instead." .

<http://purl.oclc.org/NET/ssnx/cf/cf-property#eastward_mass_flux_of_air>
  a owl:NamedIndividual, <http://purl.oclc.org/NET/ssnx/qu/dim#MassPerTimePerArea> ;
  rdfs:label "eastward mass flux of air" ;
  rdfs:isDefinedBy <http://purl.oclc.org/NET/ssnx/cf/cf-property> ;
  rdfs:comment "Eastward indicates a vector component which is positive when directed eastward (negative westward). In accordance with common usage in geophysical disciplines, flux implies per unit area, called flux density in physics." .

<http://purl.oclc.org/NET/ssnx/cf/cf-property#isotropic_longwave_radiance_in_air>
  a owl:NamedIndividual, <http://purl.oclc.org/NET/ssnx/qu/dim#Radiance> ;
  rdfs:label "isotropic longwave radiance in air" ;
  rdfs:isDefinedBy <http://purl.oclc.org/NET/ssnx/cf/cf-property> ;
  rdfs:comment "longwave means longwave radiation. Radiance is the radiative flux in a particular direction, per unit of solid angle. If radiation is isotropic, the radiance is independent of direction, so the direction should not be specified. If the radiation is directionally dependent, a standard name of upwelling or downwelling radiance should be chosen instead." .

<http://purl.oclc.org/NET/ssnx/cf/cf-property#isotropic_shortwave_radiance_in_air>
  a owl:NamedIndividual, <http://purl.oclc.org/NET/ssnx/qu/dim#Radiance> ;
  rdfs:label "isotropic shortwave radiance in air" ;
  rdfs:isDefinedBy <http://purl.oclc.org/NET/ssnx/cf/cf-property> ;
  rdfs:comment "shortwave means shortwave radiation. Radiance is the radiative flux in a particular direction, per unit of solid angle. If radiation is isotropic, the radiance is independent of direction, so the direction should not be specified. If the radiation is directionally dependent, a standard name of upwelling or downwelling radiance should be chosen instead." .

<http://purl.oclc.org/NET/ssnx/cf/cf-property#mass_concentration_of_acetic_acid_in_air>
  a owl:NamedIndividual, <http://purl.oclc.org/NET/ssnx/qu/dim#Density> ;
  rdfs:label "mass concentration of acetic acid in air" ;
  rdfs:isDefinedBy <http://purl.oclc.org/NET/ssnx/cf/cf-property> ;
  rdfs:comment " Mass concentration means mass per unit volume and is used in the construction mass_concentration_of_X_in_Y, where X is a material constituent of Y.  A chemical species denoted by X may be described by a single term such as 'nitrogen' or a phrase such as 'nox_expressed_as_nitrogen'. The chemical formula for acetic_acid is CH3COOH. The IUPAC name for acetic acid is ethanoic acid." .

<http://purl.oclc.org/NET/ssnx/cf/cf-property#mass_concentration_of_aceto_nitrile_in_air>
  a owl:NamedIndividual, <http://purl.oclc.org/NET/ssnx/qu/dim#Density> ;
  rdfs:label "mass concentration of aceto nitrile in air" ;
  rdfs:isDefinedBy <http://purl.oclc.org/NET/ssnx/cf/cf-property> ;
  rdfs:comment " Mass concentration means mass per unit volume and is used in the construction mass_concentration_of_X_in_Y, where X is a material constituent of Y.  A chemical species denoted by X may be described by a single term such as 'nitrogen' or a phrase such as 'nox_expressed_as_nitrogen'. The chemical formula for aceto-nitrile is CH3CN. The IUPAC name for aceto-nitrile is ethanenitrile." .

<http://purl.oclc.org/NET/ssnx/cf/cf-property#mass_concentration_of_alkanes_in_air>
  a owl:NamedIndividual, <http://purl.oclc.org/NET/ssnx/qu/dim#Density> ;
  rdfs:label "mass concentration of alkanes in air" ;
  rdfs:isDefinedBy <http://purl.oclc.org/NET/ssnx/cf/cf-property> ;
  rdfs:comment " Mass concentration means mass per unit volume and is used in the construction mass_concentration_of_X_in_Y, where X is a material constituent of Y.  A chemical species denoted by X may be described by a single term such as 'nitrogen' or a phrase such as 'nox_expressed_as_nitrogen'. Alkanes are saturated hydrocarbons, i.e. they do not contain any chemical double bonds.  Alkanes contain only hydrogen and carbon combined in the general proportions C(n)H(2n+2); alkanes is the term used in standard names to describe the group of chemical species having this common structure that are represented within a given model. The list of individual species that are included in a quantity having a group chemical standard name can vary between models.  Where possible, the data variable should be accompanied by a complete description of the species represented, for example, by using a comment attribute. Standard names exist for some individual alkane species, e.g., methane and ethane." .

<http://purl.oclc.org/NET/ssnx/cf/cf-property#mass_concentration_of_alkenes_in_air>
  a owl:NamedIndividual, <http://purl.oclc.org/NET/ssnx/qu/dim#Density> ;
  rdfs:label "mass concentration of alkenes in air" ;
  rdfs:isDefinedBy <http://purl.oclc.org/NET/ssnx/cf/cf-property> ;
  rdfs:comment " Mass concentration means mass per unit volume and is used in the construction mass_concentration_of_X_in_Y, where X is a material constituent of Y.  A chemical species denoted by X may be described by a single term such as 'nitrogen' or a phrase such as 'nox_expressed_as_nitrogen'. Alkenes are unsaturated hydrocarbons as they contain chemical double bonds between adjacent carbon atoms.  Alkenes contain only hydrogen and carbon combined in the general proportions C(n)H(2n); alkenes is the term used in standard names to describe the group of chemical species having this common structure that are represented within a given model. The list of individual species that are included in a quantity having a group chemical standard name can vary between models.  Where possible, the data variable should be accompanied by a complete description of the species represented, for example, by using a comment attribute. Standard names exist for some individual alkene species, e.g., ethene and propene." .

<http://purl.oclc.org/NET/ssnx/cf/cf-property#mass_concentration_of_alpha_hexachlorocyclohexane_in_air>
  a owl:NamedIndividual, <http://purl.oclc.org/NET/ssnx/qu/dim#Density> ;
  rdfs:label "mass concentration of alpha hexachlorocyclohexane in air" ;
  rdfs:isDefinedBy <http://purl.oclc.org/NET/ssnx/cf/cf-property> ;
  rdfs:comment " Mass concentration means mass per unit volume and is used in the construction mass_concentration_of_X_in_Y, where X is a material constituent of Y.  A chemical species denoted by X may be described by a single term such as 'nitrogen' or a phrase such as 'nox_expressed_as_nitrogen'. The chemical formula for alpha_hexachlorocyclohexane is C6H6Cl6." .

<http://purl.oclc.org/NET/ssnx/cf/cf-property#mass_concentration_of_alpha_pinene_in_air>
  a owl:NamedIndividual, <http://purl.oclc.org/NET/ssnx/qu/dim#Density> ;
  rdfs:label "mass concentration of alpha pinene in air" ;
  rdfs:isDefinedBy <http://purl.oclc.org/NET/ssnx/cf/cf-property> ;
  rdfs:comment " Mass concentration means mass per unit volume and is used in the construction mass_concentration_of_X_in_Y, where X is a material constituent of Y.  A chemical species denoted by X may be described by a single term such as 'nitrogen' or a phrase such as 'nox_expressed_as_nitrogen'. The chemical formula for alpha_pinene is C10H16. The IUPAC name for alpha-pinene is (1S,5S)-2,6,6-trimethylbicyclo[3.1.1]hept-2-ene." .

<http://purl.oclc.org/NET/ssnx/cf/cf-property#mass_concentration_of_ammonia_in_air>
  a owl:NamedIndividual, <http://purl.oclc.org/NET/ssnx/qu/dim#Density> ;
  rdfs:label "mass concentration of ammonia in air" ;
  rdfs:isDefinedBy <http://purl.oclc.org/NET/ssnx/cf/cf-property> ;
  rdfs:comment " Mass concentration means mass per unit volume and is used in the construction mass_concentration_of_X_in_Y, where X is a material constituent of Y.  A chemical species denoted by X may be described by a single term such as 'nitrogen' or a phrase such as 'nox_expressed_as_nitrogen'. The chemical formula for ammonia is NH3." .

<http://purl.oclc.org/NET/ssnx/cf/cf-property#mass_concentration_of_ammonium_dry_aerosol_in_air>
  a owl:NamedIndividual, <http://purl.oclc.org/NET/ssnx/qu/dim#Density> ;
  rdfs:label "mass concentration of ammonium dry aerosol in air" ;
  rdfs:isDefinedBy <http://purl.oclc.org/NET/ssnx/cf/cf-property> ;
  rdfs:comment " Mass concentration means mass per unit volume and is used in the construction mass_concentration_of_X_in_Y, where X is a material constituent of Y.  A chemical species denoted by X may be described by a single term such as 'nitrogen' or a phrase such as 'nox_expressed_as_nitrogen'. Aerosol means the suspended liquid or solid particles in air (except cloud droplets).  Aerosol takes up ambient water (a process known as hygroscopic growth) depending on the relative humidity and the composition of the aerosol. Dry aerosol means aerosol without water. The chemical formula for ammonium is NH4." .

<http://purl.oclc.org/NET/ssnx/cf/cf-property#mass_concentration_of_anthropogenic_nmvoc_expressed_as_carbon_in_air>
  a owl:NamedIndividual, <http://purl.oclc.org/NET/ssnx/qu/dim#Density> ;
  rdfs:label "mass concentration of anthropogenic nmvoc expressed as carbon in air" ;
  rdfs:isDefinedBy <http://purl.oclc.org/NET/ssnx/cf/cf-property> ;
  rdfs:comment " Mass concentration means mass per unit volume and is used in the construction mass_concentration_of_X_in_Y, where X is a material constituent of Y.  A chemical species denoted by X may be described by a single term such as 'nitrogen' or a phrase such as 'nox_expressed_as_nitrogen'. nmvoc means non methane volatile organic compounds. Anthropogenic means influenced, caused, or created by human activity.  The phrase 'expressed_as' is used in the construction A_expressed_as_B, where B is a chemical constituent of A. It means that the quantity indicated by the standard name is calculated solely with respect to the B contained in A, neglecting all other chemical constituents of A." .

<http://purl.oclc.org/NET/ssnx/cf/cf-property#mass_concentration_of_aromatic_compounds_in_air>
  a owl:NamedIndividual, <http://purl.oclc.org/NET/ssnx/qu/dim#Density> ;
  rdfs:label "mass concentration of aromatic compounds in air" ;
  rdfs:isDefinedBy <http://purl.oclc.org/NET/ssnx/cf/cf-property> ;
  rdfs:comment " Mass concentration means mass per unit volume and is used in the construction mass_concentration_of_X_in_Y, where X is a material constituent of Y.  A chemical species denoted by X may be described by a single term such as 'nitrogen' or a phrase such as 'nox_expressed_as_nitrogen'. Aromatic compounds in organic chemistry are compounds that contain at least one benzene ring of six carbon atoms joined by alternating single and double covalent bonds.  The simplest aromatic compound is benzene itself.  In standard names aromatic_compounds is the term used to describe the group of aromatic chemical species that  are represented within a given model.  The list of individual species that are included in a quantity having a group chemical standard name can vary between models.  Where possible, the data variable should be accompanied by a complete description of the species represented, for example, by using a comment attribute.  Standard names exist for some individual aromatic species, e.g. benzene and xylene." .

<http://purl.oclc.org/NET/ssnx/cf/cf-property#mass_concentration_of_atomic_bromine_in_air>
  a owl:NamedIndividual, <http://purl.oclc.org/NET/ssnx/qu/dim#Density> ;
  rdfs:label "mass concentration of atomic bromine in air" ;
  rdfs:isDefinedBy <http://purl.oclc.org/NET/ssnx/cf/cf-property> ;
  rdfs:comment " Mass concentration means mass per unit volume and is used in the construction mass_concentration_of_X_in_Y, where X is a material constituent of Y.  A chemical species denoted by X may be described by a single term such as 'nitrogen' or a phrase such as 'nox_expressed_as_nitrogen'. The chemical symbol for atomic bromine is Br." .

<http://purl.oclc.org/NET/ssnx/cf/cf-property#mass_concentration_of_atomic_chlorine_in_air>
  a owl:NamedIndividual, <http://purl.oclc.org/NET/ssnx/qu/dim#Density> ;
  rdfs:label "mass concentration of atomic chlorine in air" ;
  rdfs:isDefinedBy <http://purl.oclc.org/NET/ssnx/cf/cf-property> ;
  rdfs:comment " Mass concentration means mass per unit volume and is used in the construction mass_concentration_of_X_in_Y, where X is a material constituent of Y.  A chemical species denoted by X may be described by a single term such as 'nitrogen' or a phrase such as 'nox_expressed_as_nitrogen'. The chemical symbol for atomic chlorine is Cl." .

<http://purl.oclc.org/NET/ssnx/cf/cf-property#mass_concentration_of_atomic_nitrogen_in_air>
  a owl:NamedIndividual, <http://purl.oclc.org/NET/ssnx/qu/dim#Density> ;
  rdfs:label "mass concentration of atomic nitrogen in air" ;
  rdfs:isDefinedBy <http://purl.oclc.org/NET/ssnx/cf/cf-property> ;
  rdfs:comment " Mass concentration means mass per unit volume and is used in the construction mass_concentration_of_X_in_Y, where X is a material constituent of Y.  A chemical species denoted by X may be described by a single term such as 'nitrogen' or a phrase such as 'nox_expressed_as_nitrogen'. The chemical symbol for atomic nitrogen is N." .

<http://purl.oclc.org/NET/ssnx/cf/cf-property#mass_concentration_of_benzene_in_air>
  a owl:NamedIndividual, <http://purl.oclc.org/NET/ssnx/qu/dim#Density> ;
  rdfs:label "mass concentration of benzene in air" ;
  rdfs:isDefinedBy <http://purl.oclc.org/NET/ssnx/cf/cf-property> ;
  rdfs:comment " Mass concentration means mass per unit volume and is used in the construction mass_concentration_of_X_in_Y, where X is a material constituent of Y.  A chemical species denoted by X may be described by a single term such as 'nitrogen' or a phrase such as 'nox_expressed_as_nitrogen'. The chemical formula for benzene is C6H6.  Benzene is the simplest aromatic hydrocarbon and has a ring structure consisting of six carbon atoms joined by alternating single and double chemical bonds. Each carbon atom is additionally bonded to one hydrogen atom. There are standard names that refer to aromatic_compounds as a group, as well as those for individual species." .

<http://purl.oclc.org/NET/ssnx/cf/cf-property#mass_concentration_of_beta_pinene_in_air>
  a owl:NamedIndividual, <http://purl.oclc.org/NET/ssnx/qu/dim#Density> ;
  rdfs:label "mass concentration of beta pinene in air" ;
  rdfs:isDefinedBy <http://purl.oclc.org/NET/ssnx/cf/cf-property> ;
  rdfs:comment " Mass concentration means mass per unit volume and is used in the construction mass_concentration_of_X_in_Y, where X is a material constituent of Y.  A chemical species denoted by X may be described by a single term such as 'nitrogen' or a phrase such as 'nox_expressed_as_nitrogen'. The chemical formula for beta_pinene is C10H16.  The IUPAC name for beta-pinene is (1S,5S)-6,6-dimethyl-2-methylenebicyclo[3.1.1]heptane." .

<http://purl.oclc.org/NET/ssnx/cf/cf-property#mass_concentration_of_biogenic_nmvoc_expressed_as_carbon_in_air>
  a owl:NamedIndividual, <http://purl.oclc.org/NET/ssnx/qu/dim#Density> ;
  rdfs:label "mass concentration of biogenic nmvoc expressed as carbon in air" ;
  rdfs:isDefinedBy <http://purl.oclc.org/NET/ssnx/cf/cf-property> ;
  rdfs:comment " Mass concentration means mass per unit volume and is used in the construction mass_concentration_of_X_in_Y, where X is a material constituent of Y.  A chemical species denoted by X may be described by a single term such as 'nitrogen' or a phrase such as 'nox_expressed_as_nitrogen'. nmvoc means non methane volatile organic compounds. Biogenic means influenced, caused, or created by natural processes.  The phrase 'expressed_as' is used in the construction A_expressed_as_B, where B is a chemical constituent of A. It means that the quantity indicated by the standard name is calculated solely with respect to the B contained in A, neglecting all other chemical constituents of A." .

<http://purl.oclc.org/NET/ssnx/cf/cf-property#mass_concentration_of_black_carbon_dry_aerosol_in_air>
  a owl:NamedIndividual, <http://purl.oclc.org/NET/ssnx/qu/dim#Density> ;
  rdfs:label "mass concentration of black carbon dry aerosol in air" ;
  rdfs:isDefinedBy <http://purl.oclc.org/NET/ssnx/cf/cf-property> ;
  rdfs:comment " Mass concentration means mass per unit volume and is used in the construction mass_concentration_of_X_in_Y, where X is a material constituent of Y.  A chemical species denoted by X may be described by a single term such as 'nitrogen' or a phrase such as 'nox_expressed_as_nitrogen'. Aerosol means the suspended liquid or solid particles in air (except cloud droplets).  Aerosol takes up ambient water (a process known as hygroscopic growth) depending on the relative humidity and the composition of the aerosol. Dry aerosol means aerosol without water." .

<http://purl.oclc.org/NET/ssnx/cf/cf-property#mass_concentration_of_bromine_chloride_in_air>
  a owl:NamedIndividual, <http://purl.oclc.org/NET/ssnx/qu/dim#Density> ;
  rdfs:label "mass concentration of bromine chloride in air" ;
  rdfs:isDefinedBy <http://purl.oclc.org/NET/ssnx/cf/cf-property> ;
  rdfs:comment " Mass concentration means mass per unit volume and is used in the construction mass_concentration_of_X_in_Y, where X is a material constituent of Y.  A chemical species denoted by X may be described by a single term such as 'nitrogen' or a phrase such as 'nox_expressed_as_nitrogen'. The chemical formula for bromine chloride is BrCl." .

<http://purl.oclc.org/NET/ssnx/cf/cf-property#mass_concentration_of_bromine_monoxide_in_air>
  a owl:NamedIndividual, <http://purl.oclc.org/NET/ssnx/qu/dim#Density> ;
  rdfs:label "mass concentration of bromine monoxide in air" ;
  rdfs:isDefinedBy <http://purl.oclc.org/NET/ssnx/cf/cf-property> ;
  rdfs:comment " Mass concentration means mass per unit volume and is used in the construction mass_concentration_of_X_in_Y, where X is a material constituent of Y.  A chemical species denoted by X may be described by a single term such as 'nitrogen' or a phrase such as 'nox_expressed_as_nitrogen'. The chemical formula for bromine monoxide is BrO." .

<http://purl.oclc.org/NET/ssnx/cf/cf-property#mass_concentration_of_bromine_nitrate_in_air>
  a owl:NamedIndividual, <http://purl.oclc.org/NET/ssnx/qu/dim#Density> ;
  rdfs:label "mass concentration of bromine nitrate in air" ;
  rdfs:isDefinedBy <http://purl.oclc.org/NET/ssnx/cf/cf-property> ;
  rdfs:comment " Mass concentration means mass per unit volume and is used in the construction mass_concentration_of_X_in_Y, where X is a material constituent of Y.  A chemical species denoted by X may be described by a single term such as 'nitrogen' or a phrase such as 'nox_expressed_as_nitrogen'. The chemical formula for bromine nitrate is BrONO2." .

<http://purl.oclc.org/NET/ssnx/cf/cf-property#mass_concentration_of_brox_expressed_as_bromine_in_air>
  a owl:NamedIndividual, <http://purl.oclc.org/NET/ssnx/qu/dim#Density> ;
  rdfs:label "mass concentration of brox expressed as bromine in air" ;
  rdfs:isDefinedBy <http://purl.oclc.org/NET/ssnx/cf/cf-property> ;
  rdfs:comment " Mass concentration means mass per unit volume and is used in the construction mass_concentration_of_X_in_Y, where X is a material constituent of Y.  A chemical species denoted by X may be described by a single term such as 'nitrogen' or a phrase such as 'nox_expressed_as_nitrogen'. Brox  describes a family of chemical species consisting of inorganic bromine compounds with the exception of  hydrogen bromide (HBr) and bromine nitrate (BrONO2). Brox is the term used in standard names for all species belonging to the family that are represented within a given model. The list of individual species that are included in a quantity with a group chemical standard name can vary between models.  Where possible, the data variable should be accompanied by a complete description of the species represented, for example, by using a comment attribute. Inorganic bromine, sometimes referred to as Bry, describes a family of chemical species which result from the degradation of source gases containing bromine (halons, methyl bromide, VSLS) and natural inorganic bromine sources such as volcanoes, seasalt and other aerosols.  Standard names that use the term inorganic_bromine are used for quantities that contain all inorganic bromine species including HCl and ClONO2. The phrase 'expressed_as' is used in the construction A_expressed_as_B, where B is a chemical constituent of A. It means that the quantity indicated by the standard name is calculated solely with respect to the B contained in A, neglecting all other chemical constituents of A." .

<http://purl.oclc.org/NET/ssnx/cf/cf-property#mass_concentration_of_butane_in_air>
  a owl:NamedIndividual, <http://purl.oclc.org/NET/ssnx/qu/dim#Density> ;
  rdfs:label "mass concentration of butane in air" ;
  rdfs:isDefinedBy <http://purl.oclc.org/NET/ssnx/cf/cf-property> ;
  rdfs:comment " Mass concentration means mass per unit volume and is used in the construction mass_concentration_of_X_in_Y, where X is a material constituent of Y.  A chemical species denoted by X may be described by a single term such as 'nitrogen' or a phrase such as 'nox_expressed_as_nitrogen'. The chemical formula for butane is C4H10. Butane is a member of the group of hydrocarbons known as alkanes.  There are standard names for the alkane group as well as for some of the individual species." .

<http://purl.oclc.org/NET/ssnx/cf/cf-property#mass_concentration_of_carbon_dioxide_in_air>
  a owl:NamedIndividual, <http://purl.oclc.org/NET/ssnx/qu/dim#Density> ;
  rdfs:label "mass concentration of carbon dioxide in air" ;
  rdfs:isDefinedBy <http://purl.oclc.org/NET/ssnx/cf/cf-property> ;
  rdfs:comment " Mass concentration means mass per unit volume and is used in the construction mass_concentration_of_X_in_Y, where X is a material constituent of Y.  A chemical species denoted by X may be described by a single term such as 'nitrogen' or a phrase such as 'nox_expressed_as_nitrogen'. The chemical formula for carbon dioxide is CO2." .

<http://purl.oclc.org/NET/ssnx/cf/cf-property#mass_concentration_of_carbon_monoxide_in_air>
  a owl:NamedIndividual, <http://purl.oclc.org/NET/ssnx/qu/dim#Density> ;
  rdfs:label "mass concentration of carbon monoxide in air" ;
  rdfs:isDefinedBy <http://purl.oclc.org/NET/ssnx/cf/cf-property> ;
  rdfs:comment " Mass concentration means mass per unit volume and is used in the construction mass_concentration_of_X_in_Y, where X is a material constituent of Y.  A chemical species denoted by X may be described by a single term such as 'nitrogen' or a phrase such as 'nox_expressed_as_nitrogen'. The chemical formula of carbon monoxide is CO." .

<http://purl.oclc.org/NET/ssnx/cf/cf-property#mass_concentration_of_carbon_tetrachloride_in_air>
  a owl:NamedIndividual, <http://purl.oclc.org/NET/ssnx/qu/dim#Density> ;
  rdfs:label "mass concentration of carbon tetrachloride in air" ;
  rdfs:isDefinedBy <http://purl.oclc.org/NET/ssnx/cf/cf-property> ;
  rdfs:comment " Mass concentration means mass per unit volume and is used in the construction mass_concentration_of_X_in_Y, where X is a material constituent of Y.  A chemical species denoted by X may be described by a single term such as 'nitrogen' or a phrase such as 'nox_expressed_as_nitrogen'. The chemical formula of carbon tetrachloride is CCl4." .

<http://purl.oclc.org/NET/ssnx/cf/cf-property#mass_concentration_of_cfc113_in_air>
  a owl:NamedIndividual, <http://purl.oclc.org/NET/ssnx/qu/dim#Density> ;
  rdfs:label "mass concentration of cfc113 in air" ;
  rdfs:isDefinedBy <http://purl.oclc.org/NET/ssnx/cf/cf-property> ;
  rdfs:comment " Mass concentration means mass per unit volume and is used in the construction mass_concentration_of_X_in_Y, where X is a material constituent of Y.  A chemical species denoted by X may be described by a single term such as 'nitrogen' or a phrase such as 'nox_expressed_as_nitrogen'. The chemical formula of CFC113 is CCl2FCClF2. The IUPAC name for CFC113 is 1,1,2-trichloro-1,2,2-trifluoro-ethane." .

<http://purl.oclc.org/NET/ssnx/cf/cf-property#mass_concentration_of_cfc113a_in_air>
  a owl:NamedIndividual, <http://purl.oclc.org/NET/ssnx/qu/dim#Density> ;
  rdfs:label "mass concentration of cfc113a in air" ;
  rdfs:isDefinedBy <http://purl.oclc.org/NET/ssnx/cf/cf-property> ;
  rdfs:comment " Mass concentration means mass per unit volume and is used in the construction mass_concentration_of_X_in_Y, where X is a material constituent of Y.  A chemical species denoted by X may be described by a single term such as 'nitrogen' or a phrase such as 'nox_expressed_as_nitrogen'. The chemical formula of CFC113a CCl3CF3.  The IUPAC name for CFC113a is 1,1,1-trichloro-2,2,2-trifluoro-ethane." .

<http://purl.oclc.org/NET/ssnx/cf/cf-property#mass_concentration_of_cfc114_in_air>
  a owl:NamedIndividual, <http://purl.oclc.org/NET/ssnx/qu/dim#Density> ;
  rdfs:label "mass concentration of cfc114 in air" ;
  rdfs:isDefinedBy <http://purl.oclc.org/NET/ssnx/cf/cf-property> ;
  rdfs:comment " Mass concentration means mass per unit volume and is used in the construction mass_concentration_of_X_in_Y, where X is a material constituent of Y.  A chemical species denoted by X may be described by a single term such as 'nitrogen' or a phrase such as 'nox_expressed_as_nitrogen'. The chemical formula of CFC114 is CClF2CClF2. The IUPAC name for CFC114 is 1,2-dichloro-1,1,2,2-tetrafluoro-ethane." .

<http://purl.oclc.org/NET/ssnx/cf/cf-property#mass_concentration_of_cfc115_in_air>
  a owl:NamedIndividual, <http://purl.oclc.org/NET/ssnx/qu/dim#Density> ;
  rdfs:label "mass concentration of cfc115 in air" ;
  rdfs:isDefinedBy <http://purl.oclc.org/NET/ssnx/cf/cf-property> ;
  rdfs:comment " Mass concentration means mass per unit volume and is used in the construction mass_concentration_of_X_in_Y, where X is a material constituent of Y.  A chemical species denoted by X may be described by a single term such as 'nitrogen' or a phrase such as 'nox_expressed_as_nitrogen'. The chemical formula of CFC115 is CClF2CF3. The IUPAC name for CFC115 is 1-chloro-1,1,2,2,2-pentafluoro-ethane." .

<http://purl.oclc.org/NET/ssnx/cf/cf-property#mass_concentration_of_cfc11_in_air>
  a owl:NamedIndividual, <http://purl.oclc.org/NET/ssnx/qu/dim#Density> ;
  rdfs:label "mass concentration of cfc11 in air" ;
  rdfs:isDefinedBy <http://purl.oclc.org/NET/ssnx/cf/cf-property> ;
  rdfs:comment " Mass concentration means mass per unit volume and is used in the construction mass_concentration_of_X_in_Y, where X is a material constituent of Y.  A chemical species denoted by X may be described by a single term such as 'nitrogen' or a phrase such as 'nox_expressed_as_nitrogen'. The chemical formula of CFC11 is CFCl3. The IUPAC name fof CFC11 is trichloro-fluoro-methane." .

<http://purl.oclc.org/NET/ssnx/cf/cf-property#mass_concentration_of_cfc12_in_air>
  a owl:NamedIndividual, <http://purl.oclc.org/NET/ssnx/qu/dim#Density> ;
  rdfs:label "mass concentration of cfc12 in air" ;
  rdfs:isDefinedBy <http://purl.oclc.org/NET/ssnx/cf/cf-property> ;
  rdfs:comment " Mass concentration means mass per unit volume and is used in the construction mass_concentration_of_X_in_Y, where X is a material constituent of Y.  A chemical species denoted by X may be described by a single term such as 'nitrogen' or a phrase such as 'nox_expressed_as_nitrogen'. The chemical formula for CFC12 is CF2Cl2.  The IUPAC name for CFC12 is dichloro-difluoro-methane." .

<http://purl.oclc.org/NET/ssnx/cf/cf-property#mass_concentration_of_chlorine_dioxide_in_air>
  a owl:NamedIndividual, <http://purl.oclc.org/NET/ssnx/qu/dim#Density> ;
  rdfs:label "mass concentration of chlorine dioxide in air" ;
  rdfs:isDefinedBy <http://purl.oclc.org/NET/ssnx/cf/cf-property> ;
  rdfs:comment " Mass concentration means mass per unit volume and is used in the construction mass_concentration_of_X_in_Y, where X is a material constituent of Y.  A chemical species denoted by X may be described by a single term such as 'nitrogen' or a phrase such as 'nox_expressed_as_nitrogen'. The chemical formula for chlorine dioxide is OClO." .

<http://purl.oclc.org/NET/ssnx/cf/cf-property#mass_concentration_of_chlorine_monoxide_in_air>
  a owl:NamedIndividual, <http://purl.oclc.org/NET/ssnx/qu/dim#Density> ;
  rdfs:label "mass concentration of chlorine monoxide in air" ;
  rdfs:isDefinedBy <http://purl.oclc.org/NET/ssnx/cf/cf-property> ;
  rdfs:comment " Mass concentration means mass per unit volume and is used in the construction mass_concentration_of_X_in_Y, where X is a material constituent of Y.  A chemical species denoted by X may be described by a single term such as 'nitrogen' or a phrase such as 'nox_expressed_as_nitrogen'. The chemical formula for chlorine monoxide is ClO." .

<http://purl.oclc.org/NET/ssnx/cf/cf-property#mass_concentration_of_chlorine_nitrate_in_air>
  a owl:NamedIndividual, <http://purl.oclc.org/NET/ssnx/qu/dim#Density> ;
  rdfs:label "mass concentration of chlorine nitrate in air" ;
  rdfs:isDefinedBy <http://purl.oclc.org/NET/ssnx/cf/cf-property> ;
  rdfs:comment " Mass concentration means mass per unit volume and is used in the construction mass_concentration_of_X_in_Y, where X is a material constituent of Y.  A chemical species denoted by X may be described by a single term such as 'nitrogen' or a phrase such as 'nox_expressed_as_nitrogen'. The chemical formula for chlorine nitrate is ClONO2. " .

<http://purl.oclc.org/NET/ssnx/cf/cf-property#mass_concentration_of_clox_expressed_as_chlorine_in_air>
  a owl:NamedIndividual, <http://purl.oclc.org/NET/ssnx/qu/dim#Density> ;
  rdfs:label "mass concentration of clox expressed as chlorine in air" ;
  rdfs:isDefinedBy <http://purl.oclc.org/NET/ssnx/cf/cf-property> ;
  rdfs:comment " Mass concentration means mass per unit volume and is used in the construction mass_concentration_of_X_in_Y, where X is a material constituent of Y.  A chemical species denoted by X may be described by a single term such as 'nitrogen' or a phrase such as 'nox_expressed_as_nitrogen'. Clox describes a family of chemical species consisting of inorganic chlorine compounds with the exception of  hydrogen chloride (HCl) and chlorine nitrate (ClONO2). Clox is the term used in standard names for all species belonging to the family that are represented within a given model. The list of individual species that are included in a quantity with a group chemical standard name can vary between models.  Where possible, the data variable should be accompanied by a complete description of the species represented, for example, by using a comment attribute. Inorganic chlorine, sometimes referred to as Cly, describes a family of chemical species which result from the degradation of source gases containing chlorine (CFCs, HCFCs, VSLS) and natural inorganic chlorine sources such as seasalt and other aerosols.   Standard names that use the term inorganic_chlorine are used for quantities that contain all inorganic chlorine species including HCl and ClONO2. The phrase 'expressed_as' is used in the construction A_expressed_as_B, where B is a chemical constituent of A. It means that the quantity indicated by the standard name is calculated solely with respect to the B contained in A, neglecting all other chemical constituents of A." .

<http://purl.oclc.org/NET/ssnx/cf/cf-property#mass_concentration_of_dichlorine_peroxide_in_air>
  a owl:NamedIndividual, <http://purl.oclc.org/NET/ssnx/qu/dim#Density> ;
  rdfs:label "mass concentration of dichlorine peroxide in air" ;
  rdfs:isDefinedBy <http://purl.oclc.org/NET/ssnx/cf/cf-property> ;
  rdfs:comment " Mass concentration means mass per unit volume and is used in the construction mass_concentration_of_X_in_Y, where X is a material constituent of Y.  A chemical species denoted by X may be described by a single term such as 'nitrogen' or a phrase such as 'nox_expressed_as_nitrogen'. The chemical formula for dichlorine peroxide is Cl2O2." .

<http://purl.oclc.org/NET/ssnx/cf/cf-property#mass_concentration_of_dimethyl_sulfide_in_air>
  a owl:NamedIndividual, <http://purl.oclc.org/NET/ssnx/qu/dim#Density> ;
  rdfs:label "mass concentration of dimethyl sulfide in air" ;
  rdfs:isDefinedBy <http://purl.oclc.org/NET/ssnx/cf/cf-property> ;
  rdfs:comment " Mass concentration means mass per unit volume and is used in the construction mass_concentration_of_X_in_Y, where X is a material constituent of Y.  A chemical species denoted by X may be described by a single term such as 'nitrogen' or a phrase such as 'nox_expressed_as_nitrogen'. The chemical formula for dimethyl sulfide is (CH3)2S.  Dimethyl sulfide is sometimes referred to as DMS." .

<http://purl.oclc.org/NET/ssnx/cf/cf-property#mass_concentration_of_dinitrogen_pentoxide_in_air>
  a owl:NamedIndividual, <http://purl.oclc.org/NET/ssnx/qu/dim#Density> ;
  rdfs:label "mass concentration of dinitrogen pentoxide in air" ;
  rdfs:isDefinedBy <http://purl.oclc.org/NET/ssnx/cf/cf-property> ;
  rdfs:comment " Mass concentration means mass per unit volume and is used in the construction mass_concentration_of_X_in_Y, where X is a material constituent of Y.  A chemical species denoted by X may be described by a single term such as 'nitrogen' or a phrase such as 'nox_expressed_as_nitrogen'. The chemical formula for dinitrogen pentoxide is N2O5." .

<http://purl.oclc.org/NET/ssnx/cf/cf-property#mass_concentration_of_dust_dry_aerosol_in_air>
  a owl:NamedIndividual, <http://purl.oclc.org/NET/ssnx/qu/dim#Density> ;
  rdfs:label "mass concentration of dust dry aerosol in air" ;
  rdfs:isDefinedBy <http://purl.oclc.org/NET/ssnx/cf/cf-property> ;
  rdfs:comment " Mass concentration means mass per unit volume and is used in the construction mass_concentration_of_X_in_Y, where X is a material constituent of Y.  A chemical species denoted by X may be described by a single term such as 'nitrogen' or a phrase such as 'nox_expressed_as_nitrogen'. Aerosol means the suspended liquid or solid particles in air (except cloud droplets).  Aerosol takes up ambient water (a process known as hygroscopic growth) depending on the relative humidity and the composition of the aerosol. Dry aerosol means aerosol without water." .

<http://purl.oclc.org/NET/ssnx/cf/cf-property#mass_concentration_of_ethane_in_air>
  a owl:NamedIndividual, <http://purl.oclc.org/NET/ssnx/qu/dim#Density> ;
  rdfs:label "mass concentration of ethane in air" ;
  rdfs:isDefinedBy <http://purl.oclc.org/NET/ssnx/cf/cf-property> ;
  rdfs:comment " Mass concentration means mass per unit volume and is used in the construction mass_concentration_of_X_in_Y, where X is a material constituent of Y.  A chemical species denoted by X may be described by a single term such as 'nitrogen' or a phrase such as 'nox_expressed_as_nitrogen'. The chemical formula for ethane is C2H6. Ethane is a member of the group of hydrocarbons known as alkanes.  There are standard names for the alkane group as well as for some of the individual species." .

<http://purl.oclc.org/NET/ssnx/cf/cf-property#mass_concentration_of_ethanol_in_air>
  a owl:NamedIndividual, <http://purl.oclc.org/NET/ssnx/qu/dim#Density> ;
  rdfs:label "mass concentration of ethanol in air" ;
  rdfs:isDefinedBy <http://purl.oclc.org/NET/ssnx/cf/cf-property> ;
  rdfs:comment " Mass concentration means mass per unit volume and is used in the construction mass_concentration_of_X_in_Y, where X is a material constituent of Y.  A chemical species denoted by X may be described by a single term such as 'nitrogen' or a phrase such as 'nox_expressed_as_nitrogen'. The chemical formula for ethanol is C2H5OH." .

<http://purl.oclc.org/NET/ssnx/cf/cf-property#mass_concentration_of_ethene_in_air>
  a owl:NamedIndividual, <http://purl.oclc.org/NET/ssnx/qu/dim#Density> ;
  rdfs:label "mass concentration of ethene in air" ;
  rdfs:isDefinedBy <http://purl.oclc.org/NET/ssnx/cf/cf-property> ;
  rdfs:comment " Mass concentration means mass per unit volume and is used in the construction mass_concentration_of_X_in_Y, where X is a material constituent of Y.  A chemical species denoted by X may be described by a single term such as 'nitrogen' or a phrase such as 'nox_expressed_as_nitrogen'. The chemical formula for ethene is C2H4. Ethene is a member of the group of hydrocarbons known as alkenes.  There are standard names for the alkene group as well as for some of the individual species." .

<http://purl.oclc.org/NET/ssnx/cf/cf-property#mass_concentration_of_ethyne_in_air>
  a owl:NamedIndividual, <http://purl.oclc.org/NET/ssnx/qu/dim#Density> ;
  rdfs:label "mass concentration of ethyne in air" ;
  rdfs:isDefinedBy <http://purl.oclc.org/NET/ssnx/cf/cf-property> ;
  rdfs:comment " Mass concentration means mass per unit volume and is used in the construction mass_concentration_of_X_in_Y, where X is a material constituent of Y.  A chemical species denoted by X may be described by a single term such as 'nitrogen' or a phrase such as 'nox_expressed_as_nitrogen'. The chemical formula for ethyne is HC2H.  Ethyne is the IUPAC name for this species, which is also commonly known as acetylene." .

<http://purl.oclc.org/NET/ssnx/cf/cf-property#mass_concentration_of_formaldehyde_in_air>
  a owl:NamedIndividual, <http://purl.oclc.org/NET/ssnx/qu/dim#Density> ;
  rdfs:label "mass concentration of formaldehyde in air" ;
  rdfs:isDefinedBy <http://purl.oclc.org/NET/ssnx/cf/cf-property> ;
  rdfs:comment " Mass concentration means mass per unit volume and is used in the construction mass_concentration_of_X_in_Y, where X is a material constituent of Y.  A chemical species denoted by X may be described by a single term such as 'nitrogen' or a phrase such as 'nox_expressed_as_nitrogen'. The chemical formula for formaldehyde is CH2O. The IUPAC name for formaldehyde is methanal." .

<http://purl.oclc.org/NET/ssnx/cf/cf-property#mass_concentration_of_formic_acid_in_air>
  a owl:NamedIndividual, <http://purl.oclc.org/NET/ssnx/qu/dim#Density> ;
  rdfs:label "mass concentration of formic acid in air" ;
  rdfs:isDefinedBy <http://purl.oclc.org/NET/ssnx/cf/cf-property> ;
  rdfs:comment " Mass concentration means mass per unit volume and is used in the construction mass_concentration_of_X_in_Y, where X is a material constituent of Y.  A chemical species denoted by X may be described by a single term such as 'nitrogen' or a phrase such as 'nox_expressed_as_nitrogen'. The chemical formula for formic acid is HCOOH.  The IUPAC name for formic acid is methanoic acid." .

<http://purl.oclc.org/NET/ssnx/cf/cf-property#mass_concentration_of_gaseous_divalent_mercury_in_air>
  a owl:NamedIndividual, <http://purl.oclc.org/NET/ssnx/qu/dim#Density> ;
  rdfs:label "mass concentration of gaseous divalent mercury in air" ;
  rdfs:isDefinedBy <http://purl.oclc.org/NET/ssnx/cf/cf-property> ;
  rdfs:comment " Mass concentration means mass per unit volume and is used in the construction mass_concentration_of_X_in_Y, where X is a material constituent of Y.  A chemical species denoted by X may be described by a single term such as 'nitrogen' or a phrase such as 'nox_expressed_as_nitrogen'. Divalent mercury means all compounds in which the mercury has two binding sites to other ion(s) in a salt or to other atom(s) in a molecule." .

<http://purl.oclc.org/NET/ssnx/cf/cf-property#mass_concentration_of_gaseous_elemental_mercury_in_air>
  a owl:NamedIndividual, <http://purl.oclc.org/NET/ssnx/qu/dim#Density> ;
  rdfs:label "mass concentration of gaseous elemental mercury in air" ;
  rdfs:isDefinedBy <http://purl.oclc.org/NET/ssnx/cf/cf-property> ;
  rdfs:comment " Mass concentration means mass per unit volume and is used in the construction mass_concentration_of_X_in_Y, where X is a material constituent of Y.  A chemical species denoted by X may be described by a single term such as 'nitrogen' or a phrase such as 'nox_expressed_as_nitrogen'. The chemical symbol for mercury is Hg." .

<http://purl.oclc.org/NET/ssnx/cf/cf-property#mass_concentration_of_halon1202_in_air>
  a owl:NamedIndividual, <http://purl.oclc.org/NET/ssnx/qu/dim#Density> ;
  rdfs:label "mass concentration of halon1202 in air" ;
  rdfs:isDefinedBy <http://purl.oclc.org/NET/ssnx/cf/cf-property> ;
  rdfs:comment " Mass concentration means mass per unit volume and is used in the construction mass_concentration_of_X_in_Y, where X is a material constituent of Y.  A chemical species denoted by X may be described by a single term such as 'nitrogen' or a phrase such as 'nox_expressed_as_nitrogen'. The chemical formula for halon1202 is CBr2F2. The IUPAC name for halon1202 is dibromo-difluoro-methane." .

<http://purl.oclc.org/NET/ssnx/cf/cf-property#mass_concentration_of_halon1211_in_air>
  a owl:NamedIndividual, <http://purl.oclc.org/NET/ssnx/qu/dim#Density> ;
  rdfs:label "mass concentration of halon1211 in air" ;
  rdfs:isDefinedBy <http://purl.oclc.org/NET/ssnx/cf/cf-property> ;
  rdfs:comment " Mass concentration means mass per unit volume and is used in the construction mass_concentration_of_X_in_Y, where X is a material constituent of Y.  A chemical species denoted by X may be described by a single term such as 'nitrogen' or a phrase such as 'nox_expressed_as_nitrogen'. The chemical formula for halon1211 is CBrClF2. The IUPAC name for halon1211 is bromo-chloro-difluoro-methane." .

<http://purl.oclc.org/NET/ssnx/cf/cf-property#mass_concentration_of_halon1301_in_air>
  a owl:NamedIndividual, <http://purl.oclc.org/NET/ssnx/qu/dim#Density> ;
  rdfs:label "mass concentration of halon1301 in air" ;
  rdfs:isDefinedBy <http://purl.oclc.org/NET/ssnx/cf/cf-property> ;
  rdfs:comment " Mass concentration means mass per unit volume and is used in the construction mass_concentration_of_X_in_Y, where X is a material constituent of Y.  A chemical species denoted by X may be described by a single term such as 'nitrogen' or a phrase such as 'nox_expressed_as_nitrogen'. The chemical formula for halon1301 is CBrF3. The IUPAC name for halon1301 is bromo-trifluoro-methane." .

<http://purl.oclc.org/NET/ssnx/cf/cf-property#mass_concentration_of_halon2402_in_air>
  a owl:NamedIndividual, <http://purl.oclc.org/NET/ssnx/qu/dim#Density> ;
  rdfs:label "mass concentration of halon2402 in air" ;
  rdfs:isDefinedBy <http://purl.oclc.org/NET/ssnx/cf/cf-property> ;
  rdfs:comment " Mass concentration means mass per unit volume and is used in the construction mass_concentration_of_X_in_Y, where X is a material constituent of Y.  A chemical species denoted by X may be described by a single term such as 'nitrogen' or a phrase such as 'nox_expressed_as_nitrogen'. The chemical formula for halo2402 is C2Br2F4. The IUPAC name for halon2402 is 1,2-dibromo-1,1,2,2-tetrafluoro-ethane." .

<http://purl.oclc.org/NET/ssnx/cf/cf-property#mass_concentration_of_hcc140a_in_air>
  a owl:NamedIndividual, <http://purl.oclc.org/NET/ssnx/qu/dim#Density> ;
  rdfs:label "mass concentration of hcc140a in air" ;
  rdfs:isDefinedBy <http://purl.oclc.org/NET/ssnx/cf/cf-property> ;
  rdfs:comment " Mass concentration means mass per unit volume and is used in the construction mass_concentration_of_X_in_Y, where X is a material constituent of Y.  A chemical species denoted by X may be described by a single term such as 'nitrogen' or a phrase such as 'nox_expressed_as_nitrogen'. The chemical formula for hcc140a is CH3CCl3. The IUPAC name for hcc140a is 1,1,1-trichloro-ethane." .

<http://purl.oclc.org/NET/ssnx/cf/cf-property#mass_concentration_of_hcfc141b_in_air>
  a owl:NamedIndividual, <http://purl.oclc.org/NET/ssnx/qu/dim#Density> ;
  rdfs:label "mass concentration of hcfc141b in air" ;
  rdfs:isDefinedBy <http://purl.oclc.org/NET/ssnx/cf/cf-property> ;
  rdfs:comment " Mass concentration means mass per unit volume and is used in the construction mass_concentration_of_X_in_Y, where X is a material constituent of Y.  A chemical species denoted by X may be described by a single term such as 'nitrogen' or a phrase such as 'nox_expressed_as_nitrogen'. The chemical formula for HCFC141b is CH3CCl2F. The IUPAC name for HCFC141b is 1,1-dichloro-1-fluoroethane." .

<http://purl.oclc.org/NET/ssnx/cf/cf-property#mass_concentration_of_hcfc142b_in_air>
  a owl:NamedIndividual, <http://purl.oclc.org/NET/ssnx/qu/dim#Density> ;
  rdfs:label "mass concentration of hcfc142b in air" ;
  rdfs:isDefinedBy <http://purl.oclc.org/NET/ssnx/cf/cf-property> ;
  rdfs:comment " Mass concentration means mass per unit volume and is used in the construction mass_concentration_of_X_in_Y, where X is a material constituent of Y.  A chemical species denoted by X may be described by a single term such as 'nitrogen' or a phrase such as 'nox_expressed_as_nitrogen'. The chemical formula for HCFC142b is CH3CClF2. The IUPAC name for HCFC142b is 1-chloro-1,1-difluoroethane." .

<http://purl.oclc.org/NET/ssnx/cf/cf-property#mass_concentration_of_hcfc22_in_air>
  a owl:NamedIndividual, <http://purl.oclc.org/NET/ssnx/qu/dim#Density> ;
  rdfs:label "mass concentration of hcfc22 in air" ;
  rdfs:isDefinedBy <http://purl.oclc.org/NET/ssnx/cf/cf-property> ;
  rdfs:comment " Mass concentration means mass per unit volume and is used in the construction mass_concentration_of_X_in_Y, where X is a material constituent of Y.  A chemical species denoted by X may be described by a single term such as 'nitrogen' or a phrase such as 'nox_expressed_as_nitrogen'. The chemical formula for HCFC22 is CHClF2.  The IUPAC name for HCFC22 is chloro-difluoro-methane." .

<http://purl.oclc.org/NET/ssnx/cf/cf-property#mass_concentration_of_hexachlorobiphenyl_in_air>
  a owl:NamedIndividual, <http://purl.oclc.org/NET/ssnx/qu/dim#Density> ;
  rdfs:label "mass concentration of hexachlorobiphenyl in air" ;
  rdfs:isDefinedBy <http://purl.oclc.org/NET/ssnx/cf/cf-property> ;
  rdfs:comment " Mass concentration means mass per unit volume and is used in the construction mass_concentration_of_X_in_Y, where X is a material constituent of Y.  A chemical species denoted by X may be described by a single term such as 'nitrogen' or a phrase such as 'nox_expressed_as_nitrogen'. The chemical formula for hexachlorobiphenyl is C12H4Cl6.  This structure of this species consists of two linked benzene rings, each of which is additionally bonded to three chlorine atoms." .

<http://purl.oclc.org/NET/ssnx/cf/cf-property#mass_concentration_of_hox_expressed_as_hydrogen_in_air>
  a owl:NamedIndividual, <http://purl.oclc.org/NET/ssnx/qu/dim#Density> ;
  rdfs:label "mass concentration of hox expressed as hydrogen in air" ;
  rdfs:isDefinedBy <http://purl.oclc.org/NET/ssnx/cf/cf-property> ;
  rdfs:comment " Mass concentration means mass per unit volume and is used in the construction mass_concentration_of_X_in_Y, where X is a material constituent of Y.  A chemical species denoted by X may be described by a single term such as 'nitrogen' or a phrase such as 'nox_expressed_as_nitrogen'. HOx means a combination of two radical species containing hydrogen and oxygen: OH and HO2. The phrase 'expressed_as' is used in the construction A_expressed_as_B, where B is a chemical constituent of A. It means that the quantity indicated by the standard name is calculated solely with respect to the B contained in A, neglecting all other chemical constituents of A." .

<http://purl.oclc.org/NET/ssnx/cf/cf-property#mass_concentration_of_hydrogen_bromide_in_air>
  a owl:NamedIndividual, <http://purl.oclc.org/NET/ssnx/qu/dim#Density> ;
  rdfs:label "mass concentration of hydrogen bromide in air" ;
  rdfs:isDefinedBy <http://purl.oclc.org/NET/ssnx/cf/cf-property> ;
  rdfs:comment " Mass concentration means mass per unit volume and is used in the construction mass_concentration_of_X_in_Y, where X is a material constituent of Y.  A chemical species denoted by X may be described by a single term such as 'nitrogen' or a phrase such as 'nox_expressed_as_nitrogen'. The chemical formula for hydrogen bromide is HBr." .

<http://purl.oclc.org/NET/ssnx/cf/cf-property#mass_concentration_of_hydrogen_chloride_in_air>
  a owl:NamedIndividual, <http://purl.oclc.org/NET/ssnx/qu/dim#Density> ;
  rdfs:label "mass concentration of hydrogen chloride in air" ;
  rdfs:isDefinedBy <http://purl.oclc.org/NET/ssnx/cf/cf-property> ;
  rdfs:comment " Mass concentration means mass per unit volume and is used in the construction mass_concentration_of_X_in_Y, where X is a material constituent of Y.  A chemical species denoted by X may be described by a single term such as 'nitrogen' or a phrase such as 'nox_expressed_as_nitrogen'. The chemical formula for hydrogen chloride is HCl." .

<http://purl.oclc.org/NET/ssnx/cf/cf-property#mass_concentration_of_hydrogen_cyanide_in_air>
  a owl:NamedIndividual, <http://purl.oclc.org/NET/ssnx/qu/dim#Density> ;
  rdfs:label "mass concentration of hydrogen cyanide in air" ;
  rdfs:isDefinedBy <http://purl.oclc.org/NET/ssnx/cf/cf-property> ;
  rdfs:comment " Mass concentration means mass per unit volume and is used in the construction mass_concentration_of_X_in_Y, where X is a material constituent of Y.  A chemical species denoted by X may be described by a single term such as 'nitrogen' or a phrase such as 'nox_expressed_as_nitrogen'. The chemical formula for hydrogen cyanide is HCN." .

<http://purl.oclc.org/NET/ssnx/cf/cf-property#mass_concentration_of_hydrogen_peroxide_in_air>
  a owl:NamedIndividual, <http://purl.oclc.org/NET/ssnx/qu/dim#Density> ;
  rdfs:label "mass concentration of hydrogen peroxide in air" ;
  rdfs:isDefinedBy <http://purl.oclc.org/NET/ssnx/cf/cf-property> ;
  rdfs:comment " Mass concentration means mass per unit volume and is used in the construction mass_concentration_of_X_in_Y, where X is a material constituent of Y.  A chemical species denoted by X may be described by a single term such as 'nitrogen' or a phrase such as 'nox_expressed_as_nitrogen'. The chemical formula for hydrogen peroxide is H2O2." .

<http://purl.oclc.org/NET/ssnx/cf/cf-property#mass_concentration_of_hydroperoxyl_radical_in_air>
  a owl:NamedIndividual, <http://purl.oclc.org/NET/ssnx/qu/dim#Density> ;
  rdfs:label "mass concentration of hydroperoxyl radical in air" ;
  rdfs:isDefinedBy <http://purl.oclc.org/NET/ssnx/cf/cf-property> ;
  rdfs:comment " Mass concentration means mass per unit volume and is used in the construction mass_concentration_of_X_in_Y, where X is a material constituent of Y.  A chemical species denoted by X may be described by a single term such as 'nitrogen' or a phrase such as 'nox_expressed_as_nitrogen'. The chemical formula for the hydroperoxyl radical is HO2. In chemistry, a 'radical' is a highly reactive, and therefore shortlived, species." .

<http://purl.oclc.org/NET/ssnx/cf/cf-property#mass_concentration_of_hydroxyl_radical_in_air>
  a owl:NamedIndividual, <http://purl.oclc.org/NET/ssnx/qu/dim#Density> ;
  rdfs:label "mass concentration of hydroxyl radical in air" ;
  rdfs:isDefinedBy <http://purl.oclc.org/NET/ssnx/cf/cf-property> ;
  rdfs:comment " Mass concentration means mass per unit volume and is used in the construction mass_concentration_of_X_in_Y, where X is a material constituent of Y.  A chemical species denoted by X may be described by a single term such as 'nitrogen' or a phrase such as 'nox_expressed_as_nitrogen'. The chemical formula for the hydroxyl radical is OH. In chemistry, a 'radical' is a highly reactive, and therefore shortlived, species." .

<http://purl.oclc.org/NET/ssnx/cf/cf-property#mass_concentration_of_hypobromous_acid_in_air>
  a owl:NamedIndividual, <http://purl.oclc.org/NET/ssnx/qu/dim#Density> ;
  rdfs:label "mass concentration of hypobromous acid in air" ;
  rdfs:isDefinedBy <http://purl.oclc.org/NET/ssnx/cf/cf-property> ;
  rdfs:comment " Mass concentration means mass per unit volume and is used in the construction mass_concentration_of_X_in_Y, where X is a material constituent of Y.  A chemical species denoted by X may be described by a single term such as 'nitrogen' or a phrase such as 'nox_expressed_as_nitrogen'. The chemical formula for hypobromous acid is HOBr." .

<http://purl.oclc.org/NET/ssnx/cf/cf-property#mass_concentration_of_hypochlorous_acid_in_air>
  a owl:NamedIndividual, <http://purl.oclc.org/NET/ssnx/qu/dim#Density> ;
  rdfs:label "mass concentration of hypochlorous acid in air" ;
  rdfs:isDefinedBy <http://purl.oclc.org/NET/ssnx/cf/cf-property> ;
  rdfs:comment " Mass concentration means mass per unit volume and is used in the construction mass_concentration_of_X_in_Y, where X is a material constituent of Y.  A chemical species denoted by X may be described by a single term such as 'nitrogen' or a phrase such as 'nox_expressed_as_nitrogen'. The chemical formula for hypochlorous acid is HOCl." .

<http://purl.oclc.org/NET/ssnx/cf/cf-property#mass_concentration_of_inorganic_bromine_in_air>
  a owl:NamedIndividual, <http://purl.oclc.org/NET/ssnx/qu/dim#Density> ;
  rdfs:label "mass concentration of inorganic bromine in air" ;
  rdfs:isDefinedBy <http://purl.oclc.org/NET/ssnx/cf/cf-property> ;
  rdfs:comment " Mass concentration means mass per unit volume and is used in the construction mass_concentration_of_X_in_Y, where X is a material constituent of Y.  A chemical species denoted by X may be described by a single term such as 'nitrogen' or a phrase such as 'nox_expressed_as_nitrogen'. Inorganic bromine, sometimes referred to as Bry, describes a family of chemical species which result from the degradation of source gases containing bromine (halons, methyl bromide, VSLS) and natural inorganic bromine sources such as volcanoes, seasalt and other aerosols. Inorganic bromine is the term used in standard names for all species belonging to the family that are represented within a given model. The list of individual species that are included in a quantity having a group chemical standard name can vary between models.  Where possible, the data variable should be accompanied by a complete description of the species represented, for example, by using a comment attribute. Standard names that use the term brox are used for quantities that contain all inorganic bromine species except HBr and BrONO2." .

<http://purl.oclc.org/NET/ssnx/cf/cf-property#mass_concentration_of_inorganic_chlorine_in_air>
  a owl:NamedIndividual, <http://purl.oclc.org/NET/ssnx/qu/dim#Density> ;
  rdfs:label "mass concentration of inorganic chlorine in air" ;
  rdfs:isDefinedBy <http://purl.oclc.org/NET/ssnx/cf/cf-property> ;
  rdfs:comment " Mass concentration means mass per unit volume and is used in the construction mass_concentration_of_X_in_Y, where X is a material constituent of Y.  A chemical species denoted by X may be described by a single term such as 'nitrogen' or a phrase such as 'nox_expressed_as_nitrogen'. Inorganic chlorine, sometimes referred to as Cly, describes a family of chemical species which result from the degradation of source gases containing chlorine (CFCs, HCFCs, VSLS) and natural inorganic chlorine sources such as seasalt and other aerosols. Inorganic chlorine is the term used in standard names for all species belonging to the family that are represented within a given model. The list of individual species that are included in a quantity having a group chemical standard name can vary between models.  Where possible, the data variable should be accompanied by a complete description of the species represented, for example, by using a comment attribute. Standard names that use the term clox are used for quantities that contain all inorganic chlorine species except HCl and ClONO2." .

<http://purl.oclc.org/NET/ssnx/cf/cf-property#mass_concentration_of_isoprene_in_air>
  a owl:NamedIndividual, <http://purl.oclc.org/NET/ssnx/qu/dim#Density> ;
  rdfs:label "mass concentration of isoprene in air" ;
  rdfs:isDefinedBy <http://purl.oclc.org/NET/ssnx/cf/cf-property> ;
  rdfs:comment " Mass concentration means mass per unit volume and is used in the construction mass_concentration_of_X_in_Y, where X is a material constituent of Y.  A chemical species denoted by X may be described by a single term such as 'nitrogen' or a phrase such as 'nox_expressed_as_nitrogen'. The chemical formula for isoprene is CH2=C(CH3)CH=CH2. The IUPAC name for isoprene is 2-methyl-buta-1,3-diene. Isoprene is a member of the group of hydrocarbons known as terpenes.  There are standard names for the terpene group as well as for some of the individual species." .

<http://purl.oclc.org/NET/ssnx/cf/cf-property#mass_concentration_of_limonene_in_air>
  a owl:NamedIndividual, <http://purl.oclc.org/NET/ssnx/qu/dim#Density> ;
  rdfs:label "mass concentration of limonene in air" ;
  rdfs:isDefinedBy <http://purl.oclc.org/NET/ssnx/cf/cf-property> ;
  rdfs:comment " Mass concentration means mass per unit volume and is used in the construction mass_concentration_of_X_in_Y, where X is a material constituent of Y.  A chemical species denoted by X may be described by a single term such as 'nitrogen' or a phrase such as 'nox_expressed_as_nitrogen'. The chemical formula for limonene is C10H16. The IUPAC name for limonene is 1-methyl-4-prop-1-en-2-yl-cyclohexene. Limonene is a member of the group of hydrocarbons known as terpenes.  There are standard names for the terpene group as well as for some of the individual species." .

<http://purl.oclc.org/NET/ssnx/cf/cf-property#mass_concentration_of_mercury_dry_aerosol_in_air>
  a owl:NamedIndividual, <http://purl.oclc.org/NET/ssnx/qu/dim#Density> ;
  rdfs:label "mass concentration of mercury dry aerosol in air" ;
  rdfs:isDefinedBy <http://purl.oclc.org/NET/ssnx/cf/cf-property> ;
  rdfs:comment " Mass concentration means mass per unit volume and is used in the construction mass_concentration_of_X_in_Y, where X is a material constituent of Y.  A chemical species denoted by X may be described by a single term such as 'nitrogen' or a phrase such as 'nox_expressed_as_nitrogen'. Aerosol means the suspended liquid or solid particles in air (except cloud droplets).  Aerosol takes up ambient water (a process known as hygroscopic growth) depending on the relative humidity and the composition of the aerosol. Dry aerosol means aerosol without water." .

<http://purl.oclc.org/NET/ssnx/cf/cf-property#mass_concentration_of_methane_in_air>
  a owl:NamedIndividual, <http://purl.oclc.org/NET/ssnx/qu/dim#Density> ;
  rdfs:label "mass concentration of methane in air" ;
  rdfs:isDefinedBy <http://purl.oclc.org/NET/ssnx/cf/cf-property> ;
  rdfs:comment " Mass concentration means mass per unit volume and is used in the construction mass_concentration_of_X_in_Y, where X is a material constituent of Y.  A chemical species denoted by X may be described by a single term such as 'nitrogen' or a phrase such as 'nox_expressed_as_nitrogen'. The chemical formula for methane is CH4. Methane is a member of the group of hydrocarbons known as alkanes.  There are standard names for the alkane group as well as for some of the individual species." .

<http://purl.oclc.org/NET/ssnx/cf/cf-property#mass_concentration_of_methanol_in_air>
  a owl:NamedIndividual, <http://purl.oclc.org/NET/ssnx/qu/dim#Density> ;
  rdfs:label "mass concentration of methanol in air" ;
  rdfs:isDefinedBy <http://purl.oclc.org/NET/ssnx/cf/cf-property> ;
  rdfs:comment " Mass concentration means mass per unit volume and is used in the construction mass_concentration_of_X_in_Y, where X is a material constituent of Y.  A chemical species denoted by X may be described by a single term such as 'nitrogen' or a phrase such as 'nox_expressed_as_nitrogen'. The chemical formula for methanol is CH3OH." .

<http://purl.oclc.org/NET/ssnx/cf/cf-property#mass_concentration_of_methyl_bromide_in_air>
  a owl:NamedIndividual, <http://purl.oclc.org/NET/ssnx/qu/dim#Density> ;
  rdfs:label "mass concentration of methyl bromide in air" ;
  rdfs:isDefinedBy <http://purl.oclc.org/NET/ssnx/cf/cf-property> ;
  rdfs:comment " Mass concentration means mass per unit volume and is used in the construction mass_concentration_of_X_in_Y, where X is a material constituent of Y.  A chemical species denoted by X may be described by a single term such as 'nitrogen' or a phrase such as 'nox_expressed_as_nitrogen'. The chemical formula for methyl bromide is CH3Br. The IUPAC name for methyl bromide is bromomethane." .

<http://purl.oclc.org/NET/ssnx/cf/cf-property#mass_concentration_of_methyl_chloride_in_air>
  a owl:NamedIndividual, <http://purl.oclc.org/NET/ssnx/qu/dim#Density> ;
  rdfs:label "mass concentration of methyl chloride in air" ;
  rdfs:isDefinedBy <http://purl.oclc.org/NET/ssnx/cf/cf-property> ;
  rdfs:comment " Mass concentration means mass per unit volume and is used in the construction mass_concentration_of_X_in_Y, where X is a material constituent of Y.  A chemical species denoted by X may be described by a single term such as 'nitrogen' or a phrase such as 'nox_expressed_as_nitrogen'. The chemical formula for methyl chloride is CH3Cl. The IUPAC name for methyl chloride is chloromethane." .

<http://purl.oclc.org/NET/ssnx/cf/cf-property#mass_concentration_of_methyl_hydroperoxide_in_air>
  a owl:NamedIndividual, <http://purl.oclc.org/NET/ssnx/qu/dim#Density> ;
  rdfs:label "mass concentration of methyl hydroperoxide in air" ;
  rdfs:isDefinedBy <http://purl.oclc.org/NET/ssnx/cf/cf-property> ;
  rdfs:comment " Mass concentration means mass per unit volume and is used in the construction mass_concentration_of_X_in_Y, where X is a material constituent of Y.  A chemical species denoted by X may be described by a single term such as 'nitrogen' or a phrase such as 'nox_expressed_as_nitrogen'. The chemical formula for methyl hydroperoxide is CH3OOH." .

<http://purl.oclc.org/NET/ssnx/cf/cf-property#mass_concentration_of_methyl_peroxy_radical_in_air>
  a owl:NamedIndividual, <http://purl.oclc.org/NET/ssnx/qu/dim#Density> ;
  rdfs:label "mass concentration of methyl peroxy radical in air" ;
  rdfs:isDefinedBy <http://purl.oclc.org/NET/ssnx/cf/cf-property> ;
  rdfs:comment " Mass concentration means mass per unit volume and is used in the construction mass_concentration_of_X_in_Y, where X is a material constituent of Y.  A chemical species denoted by X may be described by a single term such as 'nitrogen' or a phrase such as 'nox_expressed_as_nitrogen'. The chemical formula for methyl_peroxy_radical is CH3O2. In chemistry, a 'radical' is a highly reactive, and therefore shortlived, species." .

<http://purl.oclc.org/NET/ssnx/cf/cf-property#mass_concentration_of_molecular_hydrogen_in_air>
  a owl:NamedIndividual, <http://purl.oclc.org/NET/ssnx/qu/dim#Density> ;
  rdfs:label "mass concentration of molecular hydrogen in air" ;
  rdfs:isDefinedBy <http://purl.oclc.org/NET/ssnx/cf/cf-property> ;
  rdfs:comment " Mass concentration means mass per unit volume and is used in the construction mass_concentration_of_X_in_Y, where X is a material constituent of Y.  A chemical species denoted by X may be described by a single term such as 'nitrogen' or a phrase such as 'nox_expressed_as_nitrogen'. The chemical formula for molecular hydrogen is H2." .

<http://purl.oclc.org/NET/ssnx/cf/cf-property#mass_concentration_of_nitrate_dry_aerosol_in_air>
  a owl:NamedIndividual, <http://purl.oclc.org/NET/ssnx/qu/dim#Density> ;
  rdfs:label "mass concentration of nitrate dry aerosol in air" ;
  rdfs:isDefinedBy <http://purl.oclc.org/NET/ssnx/cf/cf-property> ;
  rdfs:comment " Mass concentration means mass per unit volume and is used in the construction mass_concentration_of_X_in_Y, where X is a material constituent of Y.  A chemical species denoted by X may be described by a single term such as 'nitrogen' or a phrase such as 'nox_expressed_as_nitrogen'. Aerosol means the suspended liquid or solid particles in air (except cloud droplets).  Aerosol takes up ambient water (a process known as hygroscopic growth) depending on the relative humidity and the composition of the aerosol. Dry aerosol means aerosol without water. The chemical formula for the nitrate anion is NO3-." .

<http://purl.oclc.org/NET/ssnx/cf/cf-property#mass_concentration_of_nitrate_radical_in_air>
  a owl:NamedIndividual, <http://purl.oclc.org/NET/ssnx/qu/dim#Density> ;
  rdfs:label "mass concentration of nitrate radical in air" ;
  rdfs:isDefinedBy <http://purl.oclc.org/NET/ssnx/cf/cf-property> ;
  rdfs:comment " Mass concentration means mass per unit volume and is used in the construction mass_concentration_of_X_in_Y, where X is a material constituent of Y.  A chemical species denoted by X may be described by a single term such as 'nitrogen' or a phrase such as 'nox_expressed_as_nitrogen'. In chemistry, a 'radical' is a highly reactive, and therefore shortlived, species." .

<http://purl.oclc.org/NET/ssnx/cf/cf-property#mass_concentration_of_nitric_acid_in_air>
  a owl:NamedIndividual, <http://purl.oclc.org/NET/ssnx/qu/dim#Density> ;
  rdfs:label "mass concentration of nitric acid in air" ;
  rdfs:isDefinedBy <http://purl.oclc.org/NET/ssnx/cf/cf-property> ;
  rdfs:comment " Mass concentration means mass per unit volume and is used in the construction mass_concentration_of_X_in_Y, where X is a material constituent of Y.  A chemical species denoted by X may be described by a single term such as 'nitrogen' or a phrase such as 'nox_expressed_as_nitrogen'. The chemical formula for nitric acid is HNO3." .

<http://purl.oclc.org/NET/ssnx/cf/cf-property#mass_concentration_of_nitric_acid_trihydrate_ambient_aerosol_in_air>
  a owl:NamedIndividual, <http://purl.oclc.org/NET/ssnx/qu/dim#Density> ;
  rdfs:label "mass concentration of nitric acid trihydrate ambient aerosol in air" ;
  rdfs:isDefinedBy <http://purl.oclc.org/NET/ssnx/cf/cf-property> ;
  rdfs:comment " Mass concentration means mass per unit volume and is used in the construction mass_concentration_of_X_in_Y, where X is a material constituent of Y.  A chemical species denoted by X may be described by a single term such as 'nitrogen' or a phrase such as 'nox_expressed_as_nitrogen'. Aerosol means the suspended liquid or solid particles in air (except cloud droplets).  Ambient aerosol is aerosol that has taken up ambient water through hygroscopic growth. The extent of hygroscopic growth depends on the relative humidity and the composition of the aerosol. The chemical formula for nitric acid is HNO3. Nitric acid trihydrate, sometimes referred to as NAT, is a stable crystalline substance consisting of three molecules of water to one molecule of nitric acid." .

<http://purl.oclc.org/NET/ssnx/cf/cf-property#mass_concentration_of_nitrogen_dioxide_in_air>
  a owl:NamedIndividual, <http://purl.oclc.org/NET/ssnx/qu/dim#Density> ;
  rdfs:label "mass concentration of nitrogen dioxide in air" ;
  rdfs:isDefinedBy <http://purl.oclc.org/NET/ssnx/cf/cf-property> ;
  rdfs:comment " Mass concentration means mass per unit volume and is used in the construction mass_concentration_of_X_in_Y, where X is a material constituent of Y.  A chemical species denoted by X may be described by a single term such as 'nitrogen' or a phrase such as 'nox_expressed_as_nitrogen'. The chemical formula for nitrogen dioxide is NO2." .

<http://purl.oclc.org/NET/ssnx/cf/cf-property#mass_concentration_of_nitrogen_monoxide_in_air>
  a owl:NamedIndividual, <http://purl.oclc.org/NET/ssnx/qu/dim#Density> ;
  rdfs:label "mass concentration of nitrogen monoxide in air" ;
  rdfs:isDefinedBy <http://purl.oclc.org/NET/ssnx/cf/cf-property> ;
  rdfs:comment " Mass concentration means mass per unit volume and is used in the construction mass_concentration_of_X_in_Y, where X is a material constituent of Y.  A chemical species denoted by X may be described by a single term such as 'nitrogen' or a phrase such as 'nox_expressed_as_nitrogen'. The chemical formula for nitrogen monoxide is NO." .

<http://purl.oclc.org/NET/ssnx/cf/cf-property#mass_concentration_of_nitrous_acid_in_air>
  a owl:NamedIndividual, <http://purl.oclc.org/NET/ssnx/qu/dim#Density> ;
  rdfs:label "mass concentration of nitrous acid in air" ;
  rdfs:isDefinedBy <http://purl.oclc.org/NET/ssnx/cf/cf-property> ;
  rdfs:comment " Mass concentration means mass per unit volume and is used in the construction mass_concentration_of_X_in_Y, where X is a material constituent of Y.  A chemical species denoted by X may be described by a single term such as 'nitrogen' or a phrase such as 'nox_expressed_as_nitrogen'. The chemical formula for nitrous acid is HNO2." .

<http://purl.oclc.org/NET/ssnx/cf/cf-property#mass_concentration_of_nitrous_oxide_in_air>
  a owl:NamedIndividual, <http://purl.oclc.org/NET/ssnx/qu/dim#Density> ;
  rdfs:label "mass concentration of nitrous oxide in air" ;
  rdfs:isDefinedBy <http://purl.oclc.org/NET/ssnx/cf/cf-property> ;
  rdfs:comment " Mass concentration means mass per unit volume and is used in the construction mass_concentration_of_X_in_Y, where X is a material constituent of Y.  A chemical species denoted by X may be described by a single term such as 'nitrogen' or a phrase such as 'nox_expressed_as_nitrogen'. The chemical formula for nitrous oxide is N2O." .

<http://purl.oclc.org/NET/ssnx/cf/cf-property#mass_concentration_of_nmvoc_expressed_as_carbon_in_air>
  a owl:NamedIndividual, <http://purl.oclc.org/NET/ssnx/qu/dim#Density> ;
  rdfs:label "mass concentration of nmvoc expressed as carbon in air" ;
  rdfs:isDefinedBy <http://purl.oclc.org/NET/ssnx/cf/cf-property> ;
  rdfs:comment " Mass concentration means mass per unit volume and is used in the construction mass_concentration_of_X_in_Y, where X is a material constituent of Y.  A chemical species denoted by X may be described by a single term such as 'nitrogen' or a phrase such as 'nox_expressed_as_nitrogen'. nmvoc means non methane volatile organic compounds. The phrase 'expressed_as' is used in the construction A_expressed_as_B, where B is a chemical constituent of A. It means that the quantity indicated by the standard name is calculated solely with respect to the B contained in A, neglecting all other chemical constituents of A." .

<http://purl.oclc.org/NET/ssnx/cf/cf-property#mass_concentration_of_nox_expressed_as_nitrogen_in_air>
  a owl:NamedIndividual, <http://purl.oclc.org/NET/ssnx/qu/dim#Density> ;
  rdfs:label "mass concentration of nox expressed as nitrogen in air" ;
  rdfs:isDefinedBy <http://purl.oclc.org/NET/ssnx/cf/cf-property> ;
  rdfs:comment " Mass concentration means mass per unit volume and is used in the construction mass_concentration_of_X_in_Y, where X is a material constituent of Y.  A chemical species denoted by X may be described by a single term such as 'nitrogen' or a phrase such as 'nox_expressed_as_nitrogen'. Nox means a combination of two radical species containing nitrogen and oxygen: NO+NO2. The phrase 'expressed_as' is used in the construction A_expressed_as_B, where B is a chemical constituent of A. It means that the quantity indicated by the standard name is calculated solely with respect to the B contained in A, neglecting all other chemical constituents of A." .

<http://purl.oclc.org/NET/ssnx/cf/cf-property#mass_concentration_of_noy_expressed_as_nitrogen_in_air>
  a owl:NamedIndividual, <http://purl.oclc.org/NET/ssnx/qu/dim#Density> ;
  rdfs:label "mass concentration of noy expressed as nitrogen in air" ;
  rdfs:isDefinedBy <http://purl.oclc.org/NET/ssnx/cf/cf-property> ;
  rdfs:comment " Mass concentration means mass per unit volume and is used in the construction mass_concentration_of_X_in_Y, where X is a material constituent of Y.  A chemical species denoted by X may be described by a single term such as 'nitrogen' or a phrase such as 'nox_expressed_as_nitrogen'. Noy describes a family of chemical species. The family usually includes atomic nitrogen (N), nitrogen monoxide (NO), nitrogen dioxide (NO2), dinitrogen pentoxide (N2O5), nitric acid (HNO3), peroxynitric acid (HNO4), bromine nitrate (BrONO2) , chlorine nitrate (ClONO2) and organic nitrates (most notably peroxyacetyl nitrate, sometimes referred to as PAN, (CH3COO2NO2)). The list of individual species that are included in a quantity having a group chemical standard name can vary between models.  Where possible, the data variable should be accompanied by a complete description of the species represented, for example, by using a comment attribute. The phrase 'expressed_as' is used in the construction A_expressed_as_B, where B is a chemical constituent of A. It means that the quantity indicated by the standard name is calculated solely with respect to the B contained in A, neglecting all other chemical constituents of A." .

<http://purl.oclc.org/NET/ssnx/cf/cf-property#mass_concentration_of_oxygenated_hydrocarbons_in_air>
  a owl:NamedIndividual, <http://purl.oclc.org/NET/ssnx/qu/dim#Density> ;
  rdfs:label "mass concentration of oxygenated hydrocarbons in air" ;
  rdfs:isDefinedBy <http://purl.oclc.org/NET/ssnx/cf/cf-property> ;
  rdfs:comment " Mass concentration means mass per unit volume and is used in the construction mass_concentration_of_X_in_Y, where X is a material constituent of Y.  A chemical species denoted by X may be described by a single term such as 'nitrogen' or a phrase such as 'nox_expressed_as_nitrogen'.  Oxygenated means containing oxygen. Hydrocarbon means a compound containing hydrogen and carbon." .

<http://purl.oclc.org/NET/ssnx/cf/cf-property#mass_concentration_of_ozone_in_air>
  a owl:NamedIndividual, <http://purl.oclc.org/NET/ssnx/qu/dim#Density> ;
  rdfs:label "mass concentration of ozone in air" ;
  rdfs:isDefinedBy <http://purl.oclc.org/NET/ssnx/cf/cf-property> ;
  rdfs:comment " Mass concentration means mass per unit volume and is used in the construction mass_concentration_of_X_in_Y, where X is a material constituent of Y.  A chemical species denoted by X may be described by a single term such as 'nitrogen' or a phrase such as 'nox_expressed_as_nitrogen'. The chemical formula for ozone is O3." .

<http://purl.oclc.org/NET/ssnx/cf/cf-property#mass_concentration_of_particulate_organic_matter_dry_aerosol_in_air>
  a owl:NamedIndividual, <http://purl.oclc.org/NET/ssnx/qu/dim#Density> ;
  rdfs:label "mass concentration of particulate organic matter dry aerosol in air" ;
  rdfs:isDefinedBy <http://purl.oclc.org/NET/ssnx/cf/cf-property> ;
  rdfs:comment " Mass concentration means mass per unit volume and is used in the construction mass_concentration_of_X_in_Y, where X is a material constituent of Y.  A chemical species denoted by X may be described by a single term such as 'nitrogen' or a phrase such as 'nox_expressed_as_nitrogen'. Aerosol means the suspended liquid or solid particles in air (except cloud droplets).  Aerosol takes up ambient water (a process known as hygroscopic growth) depending on the relative humidity and the composition of the aerosol. Dry aerosol means aerosol without water. The term particulate_organic_matter_dry_aerosol means all particulate organic matter dry aerosol except black carbon. It is the sum of primary_particulate_organic_matter_dry_aerosol and secondary_particulate_organic_matter_dry_aerosol." .

<http://purl.oclc.org/NET/ssnx/cf/cf-property#mass_concentration_of_peroxy_radicals_in_air>
  a owl:NamedIndividual, <http://purl.oclc.org/NET/ssnx/qu/dim#Density> ;
  rdfs:label "mass concentration of peroxy radicals in air" ;
  rdfs:isDefinedBy <http://purl.oclc.org/NET/ssnx/cf/cf-property> ;
  rdfs:comment " Mass concentration means mass per unit volume and is used in the construction mass_concentration_of_X_in_Y, where X is a material constituent of Y.  A chemical species denoted by X may be described by a single term such as 'nitrogen' or a phrase such as 'nox_expressed_as_nitrogen'. The term peroxy_radicals means all organic and inorganic peroxy radicals. This includes HO2 and all organic peroxy radicals, sometimes referred to as RO2. In chemistry, a 'radical' is a highly reactive, and therefore shortlived, species." .

<http://purl.oclc.org/NET/ssnx/cf/cf-property#mass_concentration_of_peroxyacetyl_nitrate_in_air>
  a owl:NamedIndividual, <http://purl.oclc.org/NET/ssnx/qu/dim#Density> ;
  rdfs:label "mass concentration of peroxyacetyl nitrate in air" ;
  rdfs:isDefinedBy <http://purl.oclc.org/NET/ssnx/cf/cf-property> ;
  rdfs:comment " Mass concentration means mass per unit volume and is used in the construction mass_concentration_of_X_in_Y, where X is a material constituent of Y.  A chemical species denoted by X may be described by a single term such as 'nitrogen' or a phrase such as 'nox_expressed_as_nitrogen'. The chemical formula for peroxyacetyl nitrate, sometimes referred to as PAN, is CH3COO2NO2.  The IUPAC name for peroxyacetyl_nitrate is nitroethaneperoxoate." .

<http://purl.oclc.org/NET/ssnx/cf/cf-property#mass_concentration_of_peroxynitric_acid_in_air>
  a owl:NamedIndividual, <http://purl.oclc.org/NET/ssnx/qu/dim#Density> ;
  rdfs:label "mass concentration of peroxynitric acid in air" ;
  rdfs:isDefinedBy <http://purl.oclc.org/NET/ssnx/cf/cf-property> ;
  rdfs:comment " Mass concentration means mass per unit volume and is used in the construction mass_concentration_of_X_in_Y, where X is a material constituent of Y.  A chemical species denoted by X may be described by a single term such as 'nitrogen' or a phrase such as 'nox_expressed_as_nitrogen'. The chemical formula for peroxynitric acid, sometimes referred to as PNA, is HO2NO2." .

<http://purl.oclc.org/NET/ssnx/cf/cf-property#mass_concentration_of_primary_particulate_organic_matter_dry_aerosol_in_air>
  a owl:NamedIndividual, <http://purl.oclc.org/NET/ssnx/qu/dim#Density> ;
  rdfs:label "mass concentration of primary particulate organic matter dry aerosol in air" ;
  rdfs:isDefinedBy <http://purl.oclc.org/NET/ssnx/cf/cf-property> ;
  rdfs:comment " Mass concentration means mass per unit volume and is used in the construction mass_concentration_of_X_in_Y, where X is a material constituent of Y.  A chemical species denoted by X may be described by a single term such as 'nitrogen' or a phrase such as 'nox_expressed_as_nitrogen'. Aerosol means the suspended liquid or solid particles in air (except cloud droplets).  Aerosol takes up ambient water (a process known as hygroscopic growth) depending on the relative humidity and the composition of the aerosol. Dry aerosol means aerosol without water. Primary particulate organic matter  means all organic matter emitted directly to the atmosphere as particles except black carbon. The sum of primary_particulate_organic_matter_dry_aerosol and secondary_particulate_organic_matter_dry_aerosol is particulate_organic_matter_dry_aerosol." .

<http://purl.oclc.org/NET/ssnx/cf/cf-property#mass_concentration_of_propane_in_air>
  a owl:NamedIndividual, <http://purl.oclc.org/NET/ssnx/qu/dim#Density> ;
  rdfs:label "mass concentration of propane in air" ;
  rdfs:isDefinedBy <http://purl.oclc.org/NET/ssnx/cf/cf-property> ;
  rdfs:comment " Mass concentration means mass per unit volume and is used in the construction mass_concentration_of_X_in_Y, where X is a material constituent of Y.  A chemical species denoted by X may be described by a single term such as 'nitrogen' or a phrase such as 'nox_expressed_as_nitrogen'. The chemical formula for propane is C3H8. Propane is a member of the group of hydrocarbons known as alkanes.  There are standard names for the alkane group as well as for some of the individual species." .

<http://purl.oclc.org/NET/ssnx/cf/cf-property#mass_concentration_of_propene_in_air>
  a owl:NamedIndividual, <http://purl.oclc.org/NET/ssnx/qu/dim#Density> ;
  rdfs:label "mass concentration of propene in air" ;
  rdfs:isDefinedBy <http://purl.oclc.org/NET/ssnx/cf/cf-property> ;
  rdfs:comment " Mass concentration means mass per unit volume and is used in the construction mass_concentration_of_X_in_Y, where X is a material constituent of Y.  A chemical species denoted by X may be described by a single term such as 'nitrogen' or a phrase such as 'nox_expressed_as_nitrogen'. The chemical formula for propene is C3H6. Propene is a member of the group of hydrocarbons known as alkenes.  There are standard names for the alkene group as well as for some of the individual species." .

<http://purl.oclc.org/NET/ssnx/cf/cf-property#mass_concentration_of_radon_in_air>
  a owl:NamedIndividual, <http://purl.oclc.org/NET/ssnx/qu/dim#Density> ;
  rdfs:label "mass concentration of radon in air" ;
  rdfs:isDefinedBy <http://purl.oclc.org/NET/ssnx/cf/cf-property> ;
  rdfs:comment " Mass concentration means mass per unit volume and is used in the construction mass_concentration_of_X_in_Y, where X is a material constituent of Y.  A chemical species denoted by X may be described by a single term such as 'nitrogen' or a phrase such as 'nox_expressed_as_nitrogen'. The chemical symbol for radon is Rn." .

<http://purl.oclc.org/NET/ssnx/cf/cf-property#mass_concentration_of_seasalt_dry_aerosol_in_air>
  a owl:NamedIndividual, <http://purl.oclc.org/NET/ssnx/qu/dim#Density> ;
  rdfs:label "mass concentration of seasalt dry aerosol in air" ;
  rdfs:isDefinedBy <http://purl.oclc.org/NET/ssnx/cf/cf-property> ;
  rdfs:comment " Mass concentration means mass per unit volume and is used in the construction mass_concentration_of_X_in_Y, where X is a material constituent of Y.  A chemical species denoted by X may be described by a single term such as 'nitrogen' or a phrase such as 'nox_expressed_as_nitrogen'. Aerosol means the suspended liquid or solid particles in air (except cloud droplets).  Aerosol takes up ambient water (a process known as hygroscopic growth) depending on the relative humidity and the composition of the aerosol. Dry aerosol means aerosol without water." .

<http://purl.oclc.org/NET/ssnx/cf/cf-property#mass_concentration_of_secondary_particulate_organic_matter_dry_aerosol_in_air>
  a owl:NamedIndividual, <http://purl.oclc.org/NET/ssnx/qu/dim#Density> ;
  rdfs:label "mass concentration of secondary particulate organic matter dry aerosol in air" ;
  rdfs:isDefinedBy <http://purl.oclc.org/NET/ssnx/cf/cf-property> ;
  rdfs:comment " Mass concentration means mass per unit volume and is used in the construction mass_concentration_of_X_in_Y, where X is a material constituent of Y.  A chemical species denoted by X may be described by a single term such as 'nitrogen' or a phrase such as 'nox_expressed_as_nitrogen'. Aerosol means the suspended liquid or solid particles in air (except cloud droplets).  Aerosol takes up ambient water (a process known as hygroscopic growth) depending on the relative humidity and the composition of the aerosol. Dry aerosol means aerosol without water. Secondary particulate organic matter  means particulate organic matter formed within the atmosphere from gaseous precursors. The sum of primary_particulate_organic_matter_dry_aerosol and secondary_particulate_organic_matter_dry_aerosol is particulate_organic_matter_dry_aerosol." .

<http://purl.oclc.org/NET/ssnx/cf/cf-property#mass_concentration_of_sulfate_ambient_aerosol_in_air>
  a owl:NamedIndividual, <http://purl.oclc.org/NET/ssnx/qu/dim#Density> ;
  rdfs:label "mass concentration of sulfate ambient aerosol in air" ;
  rdfs:isDefinedBy <http://purl.oclc.org/NET/ssnx/cf/cf-property> ;
  rdfs:comment "Mass concentration means mass per unit volume and is used in the construction mass_concentration_of_X_in_Y, where X is a material constituent of Y. A chemical species denoted by X may be described by a single term such as 'nitrogen' or a phrase such as 'nox_expressed_as_nitrogen'. Aerosol means the suspended liquid or solid particles in air (except cloud droplets).  Ambient aerosol is aerosol that has taken up ambient water through hygroscopic growth. The extent of hygroscopic growth depends on the relative humidity and the composition of the aerosol." .

<http://purl.oclc.org/NET/ssnx/cf/cf-property#mass_concentration_of_sulfate_dry_aerosol_in_air>
  a owl:NamedIndividual, <http://purl.oclc.org/NET/ssnx/qu/dim#Density> ;
  rdfs:label "mass concentration of sulfate dry aerosol in air" ;
  rdfs:isDefinedBy <http://purl.oclc.org/NET/ssnx/cf/cf-property> ;
  rdfs:comment " Mass concentration means mass per unit volume and is used in the construction mass_concentration_of_X_in_Y, where X is a material constituent of Y.  A chemical species denoted by X may be described by a single term such as 'nitrogen' or a phrase such as 'nox_expressed_as_nitrogen'. Aerosol means the suspended liquid or solid particles in air (except cloud droplets).  Aerosol takes up ambient water (a process known as hygroscopic growth) depending on the relative humidity and the composition of the aerosol. Dry aerosol means aerosol without water. The chemical formula for the sulfate anion is SO4(2-)." .

<http://purl.oclc.org/NET/ssnx/cf/cf-property#mass_concentration_of_sulfur_dioxide_in_air>
  a owl:NamedIndividual, <http://purl.oclc.org/NET/ssnx/qu/dim#Density> ;
  rdfs:label "mass concentration of sulfur dioxide in air" ;
  rdfs:isDefinedBy <http://purl.oclc.org/NET/ssnx/cf/cf-property> ;
  rdfs:comment " Mass concentration means mass per unit volume and is used in the construction mass_concentration_of_X_in_Y, where X is a material constituent of Y.  A chemical species denoted by X may be described by a single term such as 'nitrogen' or a phrase such as 'nox_expressed_as_nitrogen'. The chemical formula for sulfur dioxide is SO2." .

<http://purl.oclc.org/NET/ssnx/cf/cf-property#mass_concentration_of_terpenes_in_air>
  a owl:NamedIndividual, <http://purl.oclc.org/NET/ssnx/qu/dim#Density> ;
  rdfs:label "mass concentration of terpenes in air" ;
  rdfs:isDefinedBy <http://purl.oclc.org/NET/ssnx/cf/cf-property> ;
  rdfs:comment " Mass concentration means mass per unit volume and is used in the construction mass_concentration_of_X_in_Y, where X is a material constituent of Y.  A chemical species denoted by X may be described by a single term such as 'nitrogen' or a phrase such as 'nox_expressed_as_nitrogen'. Terpenes are hydrocarbons, that is, they contain only hydrogen and carbon combined in the general proportions (C5H8)n where n is an integer greater than on equal to one. The term terpenes is used in standard names to describe the group of chemical species having this common structure that are represented within a given model. The list of individual species that are included in a quantity having a group chemical standard name can vary between models.  Where possible, the data variable should be accompanied by a complete description of the species represented, for example, by using a comment attribute.  Standard names exist for some individual terpene species, e.g., isoprene and limonene." .

<http://purl.oclc.org/NET/ssnx/cf/cf-property#mass_concentration_of_toluene_in_air>
  a owl:NamedIndividual, <http://purl.oclc.org/NET/ssnx/qu/dim#Density> ;
  rdfs:label "mass concentration of toluene in air" ;
  rdfs:isDefinedBy <http://purl.oclc.org/NET/ssnx/cf/cf-property> ;
  rdfs:comment " Mass concentration means mass per unit volume and is used in the construction mass_concentration_of_X_in_Y, where X is a material constituent of Y.  A chemical species denoted by X may be described by a single term such as 'nitrogen' or a phrase such as 'nox_expressed_as_nitrogen'. The chemical formula for toluene is C6H5CH3.  Toluene has the same structure as benzene, except that one of the hydrogen atoms is replaced by a methyl group.  The systematic name for toluene is methylbenzene." .

<http://purl.oclc.org/NET/ssnx/cf/cf-property#mass_concentration_of_water_in_ambient_aerosol_in_air>
  a owl:NamedIndividual, <http://purl.oclc.org/NET/ssnx/qu/dim#Density> ;
  rdfs:label "mass concentration of water in ambient aerosol in air" ;
  rdfs:isDefinedBy <http://purl.oclc.org/NET/ssnx/cf/cf-property> ;
  rdfs:comment " Water means water in all phases.  Mass concentration means mass per unit volume and is used in the construction mass_concentration_of_X_in_Y, where X is a material constituent of Y.  A chemical species denoted by X may be described by a single term such as 'nitrogen' or a phrase such as 'nox_expressed_as_nitrogen'. Aerosol means the suspended liquid or solid particles in air (except cloud droplets).  Ambient aerosol is aerosol that has taken up ambient water through hygroscopic growth. The extent of hygroscopic growth depends on the relative humidity and the composition of the aerosol." .

<http://purl.oclc.org/NET/ssnx/cf/cf-property#mass_concentration_of_water_vapor_in_air>
  a owl:NamedIndividual, <http://purl.oclc.org/NET/ssnx/qu/dim#Density> ;
  rdfs:label "mass concentration of water vapor in air" ;
  rdfs:isDefinedBy <http://purl.oclc.org/NET/ssnx/cf/cf-property> ;
  rdfs:comment " Mass concentration means mass per unit volume and is used in the construction mass_concentration_of_X_in_Y, where X is a material constituent of Y.  A chemical species denoted by X may be described by a single term such as 'nitrogen' or a phrase such as 'nox_expressed_as_nitrogen'." .

<http://purl.oclc.org/NET/ssnx/cf/cf-property#mass_concentration_of_xylene_in_air>
  a owl:NamedIndividual, <http://purl.oclc.org/NET/ssnx/qu/dim#Density> ;
  rdfs:label "mass concentration of xylene in air" ;
  rdfs:isDefinedBy <http://purl.oclc.org/NET/ssnx/cf/cf-property> ;
  rdfs:comment " Mass concentration means mass per unit volume and is used in the construction mass_concentration_of_X_in_Y, where X is a material constituent of Y.  A chemical species denoted by X may be described by a single term such as 'nitrogen' or a phrase such as 'nox_expressed_as_nitrogen'. The chemical formula for xylene is C6H4C2H6. In chemistry, xylene is a generic term for a group of three isomers of dimethylbenzene. The IUPAC names for the isomers are 1,2-dimethylbenzene, 1,3-dimethylbenzene and 1,4-dimethylbenzene. Xylene is an aromatic hydrocarbon. There are standard names that refer to aromatic_compounds as a group, as well as those for individual species." .

<http://purl.oclc.org/NET/ssnx/cf/cf-property#mass_fraction_of_acetic_acid_in_air>
  a owl:NamedIndividual, <http://purl.oclc.org/NET/ssnx/qu/dim#Dimensionless> ;
  rdfs:label "mass fraction of acetic acid in air" ;
  rdfs:isDefinedBy <http://purl.oclc.org/NET/ssnx/cf/cf-property> ;
  rdfs:comment " Mass fraction is used in the construction mass_fraction_of_X_in_Y, where X is a material constituent of Y. It means the ratio of the mass of X to the mass of Y (including X).  A chemical species denoted by X may be described by a single term such as 'nitrogen' or a phrase such as 'nox_expressed_as_nitrogen'. The chemical formula for acetic_acid is CH3COOH. The IUPAC name for acetic acid is ethanoic acid." .

<http://purl.oclc.org/NET/ssnx/cf/cf-property#mass_fraction_of_aceto_nitrile_in_air>
  a owl:NamedIndividual, <http://purl.oclc.org/NET/ssnx/qu/dim#Dimensionless> ;
  rdfs:label "mass fraction of aceto nitrile in air" ;
  rdfs:isDefinedBy <http://purl.oclc.org/NET/ssnx/cf/cf-property> ;
  rdfs:comment " Mass fraction is used in the construction mass_fraction_of_X_in_Y, where X is a material constituent of Y. It means the ratio of the mass of X to the mass of Y (including X).  A chemical species denoted by X may be described by a single term such as 'nitrogen' or a phrase such as 'nox_expressed_as_nitrogen'. The chemical formula for aceto-nitrile is CH3CN. The IUPAC name for aceto-nitrile is ethanenitrile." .

<http://purl.oclc.org/NET/ssnx/cf/cf-property#mass_fraction_of_alkanes_in_air>
  a owl:NamedIndividual, <http://purl.oclc.org/NET/ssnx/qu/dim#Dimensionless> ;
  rdfs:label "mass fraction of alkanes in air" ;
  rdfs:isDefinedBy <http://purl.oclc.org/NET/ssnx/cf/cf-property> ;
  rdfs:comment " Mass fraction is used in the construction mass_fraction_of_X_in_Y, where X is a material constituent of Y. It means the ratio of the mass of X to the mass of Y (including X).  A chemical species denoted by X may be described by a single term such as 'nitrogen' or a phrase such as 'nox_expressed_as_nitrogen'. Alkanes are saturated hydrocarbons, i.e. they do not contain any chemical double bonds.  Alkanes contain only hydrogen and carbon combined in the general proportions C(n)H(2n+2); alkanes is the term used in standard names to describe the group of chemical species having this common structure that are represented within a given model. The list of individual species that are included in a quantity having a group chemical standard name can vary between models.  Where possible, the data variable should be accompanied by a complete description of the species represented, for example, by using a comment attribute. Standard names exist for some individual alkane species, e.g., methane and ethane." .

<http://purl.oclc.org/NET/ssnx/cf/cf-property#mass_fraction_of_alkenes_in_air>
  a owl:NamedIndividual, <http://purl.oclc.org/NET/ssnx/qu/dim#Dimensionless> ;
  rdfs:label "mass fraction of alkenes in air" ;
  rdfs:isDefinedBy <http://purl.oclc.org/NET/ssnx/cf/cf-property> ;
  rdfs:comment " Mass fraction is used in the construction mass_fraction_of_X_in_Y, where X is a material constituent of Y. It means the ratio of the mass of X to the mass of Y (including X).  A chemical species denoted by X may be described by a single term such as 'nitrogen' or a phrase such as 'nox_expressed_as_nitrogen'. Alkenes are unsaturated hydrocarbons as they contain chemical double bonds between adjacent carbon atoms.  Alkenes contain only hydrogen and carbon combined in the general proportions C(n)H(2n); alkenes is the term used in standard names to describe the group of chemical species having this common structure that are represented within a given model. The list of individual species that are included in a quantity having a group chemical standard name can vary between models.  Where possible, the data variable should be accompanied by a complete description of the species represented, for example, by using a comment attribute. Standard names exist for some individual alkene species, e.g., ethene and propene." .

<http://purl.oclc.org/NET/ssnx/cf/cf-property#mass_fraction_of_alpha_hexachlorocyclohexane_in_air>
  a owl:NamedIndividual, <http://purl.oclc.org/NET/ssnx/qu/dim#Dimensionless> ;
  rdfs:label "mass fraction of alpha hexachlorocyclohexane in air" ;
  rdfs:isDefinedBy <http://purl.oclc.org/NET/ssnx/cf/cf-property> ;
  rdfs:comment " Mass fraction is used in the construction mass_fraction_of_X_in_Y, where X is a material constituent of Y. It means the ratio of the mass of X to the mass of Y (including X).  A chemical species denoted by X may be described by a single term such as 'nitrogen' or a phrase such as 'nox_expressed_as_nitrogen'. The chemical formula for alpha_hexachlorocyclohexane is C6H6Cl6." .

<http://purl.oclc.org/NET/ssnx/cf/cf-property#mass_fraction_of_alpha_pinene_in_air>
  a owl:NamedIndividual, <http://purl.oclc.org/NET/ssnx/qu/dim#Dimensionless> ;
  rdfs:label "mass fraction of alpha pinene in air" ;
  rdfs:isDefinedBy <http://purl.oclc.org/NET/ssnx/cf/cf-property> ;
  rdfs:comment " Mass fraction is used in the construction mass_fraction_of_X_in_Y, where X is a material constituent of Y. It means the ratio of the mass of X to the mass of Y (including X).  A chemical species denoted by X may be described by a single term such as 'nitrogen' or a phrase such as 'nox_expressed_as_nitrogen'. The chemical formula for alpha_pinene is C10H16. The IUPAC name for alpha-pinene is (1S,5S)-2,6,6-trimethylbicyclo[3.1.1]hept-2-ene." .

<http://purl.oclc.org/NET/ssnx/cf/cf-property#mass_fraction_of_ammonia_in_air>
  a owl:NamedIndividual, <http://purl.oclc.org/NET/ssnx/qu/dim#Dimensionless> ;
  rdfs:label "mass fraction of ammonia in air" ;
  rdfs:isDefinedBy <http://purl.oclc.org/NET/ssnx/cf/cf-property> ;
  rdfs:comment " Mass fraction is used in the construction mass_fraction_of_X_in_Y, where X is a material constituent of Y. It means the ratio of the mass of X to the mass of Y (including X).  A chemical species denoted by X may be described by a single term such as 'nitrogen' or a phrase such as 'nox_expressed_as_nitrogen'. The chemical formula for ammonia is NH3." .

<http://purl.oclc.org/NET/ssnx/cf/cf-property#mass_fraction_of_ammonium_dry_aerosol_in_air>
  a owl:NamedIndividual, <http://purl.oclc.org/NET/ssnx/qu/dim#Dimensionless> ;
  rdfs:label "mass fraction of ammonium dry aerosol in air" ;
  rdfs:isDefinedBy <http://purl.oclc.org/NET/ssnx/cf/cf-property> ;
  rdfs:comment "Mass fraction is used in the construction mass_fraction_of_X_in_Y, where X is a material constituent of Y. It means the ratio of the mass of X to the mass of Y (including X).  Mass_fraction_of_ammonium means that the mass is expressed as mass of NH4.  Aerosol means the suspended liquid or solid particles in air (except cloud droplets).  Aerosol takes up ambient water (a process known as hygroscopic growth) depending on the relative humidity and the composition of the aerosol. Dry aerosol means aerosol without water." .

<http://purl.oclc.org/NET/ssnx/cf/cf-property#mass_fraction_of_anthropogenic_nmvoc_expressed_as_carbon_in_air>
  a owl:NamedIndividual, <http://purl.oclc.org/NET/ssnx/qu/dim#Dimensionless> ;
  rdfs:label "mass fraction of anthropogenic nmvoc expressed as carbon in air" ;
  rdfs:isDefinedBy <http://purl.oclc.org/NET/ssnx/cf/cf-property> ;
  rdfs:comment " Mass fraction is used in the construction mass_fraction_of_X_in_Y, where X is a material constituent of Y. It means the ratio of the mass of X to the mass of Y (including X).  A chemical species denoted by X may be described by a single term such as 'nitrogen' or a phrase such as 'nox_expressed_as_nitrogen'. nmvoc means non methane volatile organic compounds. Anthropogenic means influenced, caused, or created by human activity.  The phrase 'expressed_as' is used in the construction A_expressed_as_B, where B is a chemical constituent of A. It means that the quantity indicated by the standard name is calculated solely with respect to the B contained in A, neglecting all other chemical constituents of A." .

<http://purl.oclc.org/NET/ssnx/cf/cf-property#mass_fraction_of_aromatic_compounds_in_air>
  a owl:NamedIndividual, <http://purl.oclc.org/NET/ssnx/qu/dim#Dimensionless> ;
  rdfs:label "mass fraction of aromatic compounds in air" ;
  rdfs:isDefinedBy <http://purl.oclc.org/NET/ssnx/cf/cf-property> ;
  rdfs:comment " Mass fraction is used in the construction mass_fraction_of_X_in_Y, where X is a material constituent of Y. It means the ratio of the mass of X to the mass of Y (including X).  A chemical species denoted by X may be described by a single term such as 'nitrogen' or a phrase such as 'nox_expressed_as_nitrogen'. Aromatic compounds in organic chemistry are compounds that contain at least one benzene ring of six carbon atoms joined by alternating single and double covalent bonds.  The simplest aromatic compound is benzene itself.  In standard names aromatic_compounds is the term used to describe the group of aromatic chemical species that  are represented within a given model.  The list of individual species that are included in a quantity having a group chemical standard name can vary between models.  Where possible, the data variable should be accompanied by a complete description of the species represented, for example, by using a comment attribute.  Standard names exist for some individual aromatic species, e.g. benzene and xylene." .

<http://purl.oclc.org/NET/ssnx/cf/cf-property#mass_fraction_of_atomic_bromine_in_air>
  a owl:NamedIndividual, <http://purl.oclc.org/NET/ssnx/qu/dim#Dimensionless> ;
  rdfs:label "mass fraction of atomic bromine in air" ;
  rdfs:isDefinedBy <http://purl.oclc.org/NET/ssnx/cf/cf-property> ;
  rdfs:comment " Mass fraction is used in the construction mass_fraction_of_X_in_Y, where X is a material constituent of Y. It means the ratio of the mass of X to the mass of Y (including X).  A chemical species denoted by X may be described by a single term such as 'nitrogen' or a phrase such as 'nox_expressed_as_nitrogen'. The chemical symbol for atomic bromine is Br." .

<http://purl.oclc.org/NET/ssnx/cf/cf-property#mass_fraction_of_atomic_chlorine_in_air>
  a owl:NamedIndividual, <http://purl.oclc.org/NET/ssnx/qu/dim#Dimensionless> ;
  rdfs:label "mass fraction of atomic chlorine in air" ;
  rdfs:isDefinedBy <http://purl.oclc.org/NET/ssnx/cf/cf-property> ;
  rdfs:comment " Mass fraction is used in the construction mass_fraction_of_X_in_Y, where X is a material constituent of Y. It means the ratio of the mass of X to the mass of Y (including X).  A chemical species denoted by X may be described by a single term such as 'nitrogen' or a phrase such as 'nox_expressed_as_nitrogen'. The chemical symbol for atomic chlorine is Cl." .

<http://purl.oclc.org/NET/ssnx/cf/cf-property#mass_fraction_of_atomic_nitrogen_in_air>
  a owl:NamedIndividual, <http://purl.oclc.org/NET/ssnx/qu/dim#Dimensionless> ;
  rdfs:label "mass fraction of atomic nitrogen in air" ;
  rdfs:isDefinedBy <http://purl.oclc.org/NET/ssnx/cf/cf-property> ;
  rdfs:comment " Mass fraction is used in the construction mass_fraction_of_X_in_Y, where X is a material constituent of Y. It means the ratio of the mass of X to the mass of Y (including X).  A chemical species denoted by X may be described by a single term such as 'nitrogen' or a phrase such as 'nox_expressed_as_nitrogen'. The chemical symbol for atomic nitrogen is N." .

<http://purl.oclc.org/NET/ssnx/cf/cf-property#mass_fraction_of_benzene_in_air>
  a owl:NamedIndividual, <http://purl.oclc.org/NET/ssnx/qu/dim#Dimensionless> ;
  rdfs:label "mass fraction of benzene in air" ;
  rdfs:isDefinedBy <http://purl.oclc.org/NET/ssnx/cf/cf-property> ;
  rdfs:comment " Mass fraction is used in the construction mass_fraction_of_X_in_Y, where X is a material constituent of Y. It means the ratio of the mass of X to the mass of Y (including X).  A chemical species denoted by X may be described by a single term such as 'nitrogen' or a phrase such as 'nox_expressed_as_nitrogen'. The chemical formula for benzene is C6H6.  Benzene is the simplest aromatic hydrocarbon and has a ring structure consisting of six carbon atoms joined by alternating single and double chemical bonds. Each carbon atom is additionally bonded to one hydrogen atom. There are standard names that refer to aromatic_compounds as a group, as well as those for individual species." .

<http://purl.oclc.org/NET/ssnx/cf/cf-property#mass_fraction_of_beta_pinene_in_air>
  a owl:NamedIndividual, <http://purl.oclc.org/NET/ssnx/qu/dim#Dimensionless> ;
  rdfs:label "mass fraction of beta pinene in air" ;
  rdfs:isDefinedBy <http://purl.oclc.org/NET/ssnx/cf/cf-property> ;
  rdfs:comment " Mass fraction is used in the construction mass_fraction_of_X_in_Y, where X is a material constituent of Y. It means the ratio of the mass of X to the mass of Y (including X).  A chemical species denoted by X may be described by a single term such as 'nitrogen' or a phrase such as 'nox_expressed_as_nitrogen'. The chemical formula for beta_pinene is C10H16.  The IUPAC name for beta-pinene is (1S,5S)-6,6-dimethyl-2-methylenebicyclo[3.1.1]heptane." .

<http://purl.oclc.org/NET/ssnx/cf/cf-property#mass_fraction_of_biogenic_nmvoc_expressed_as_carbon_in_air>
  a owl:NamedIndividual, <http://purl.oclc.org/NET/ssnx/qu/dim#Dimensionless> ;
  rdfs:label "mass fraction of biogenic nmvoc expressed as carbon in air" ;
  rdfs:isDefinedBy <http://purl.oclc.org/NET/ssnx/cf/cf-property> ;
  rdfs:comment " Mass fraction is used in the construction mass_fraction_of_X_in_Y, where X is a material constituent of Y. It means the ratio of the mass of X to the mass of Y (including X).  A chemical species denoted by X may be described by a single term such as 'nitrogen' or a phrase such as 'nox_expressed_as_nitrogen'. nmvoc means non methane volatile organic compounds. Biogenic means influenced, caused, or created by natural processes. The phrase 'expressed_as' is used in the construction A_expressed_as_B, where B is a chemical constituent of A. It means that the quantity indicated by the standard name is calculated solely with respect to the B contained in A, neglecting all other chemical constituents of A." .

<http://purl.oclc.org/NET/ssnx/cf/cf-property#mass_fraction_of_black_carbon_dry_aerosol_in_air>
  a owl:NamedIndividual, <http://purl.oclc.org/NET/ssnx/qu/dim#Dimensionless> ;
  rdfs:label "mass fraction of black carbon dry aerosol in air" ;
  rdfs:isDefinedBy <http://purl.oclc.org/NET/ssnx/cf/cf-property> ;
  rdfs:comment "Mass fraction is used in the construction mass_fraction_of_X_in_Y, where X is a material constituent of Y. It means the ratio of the mass of X to the mass of Y (including X).  Aerosol means the suspended liquid or solid particles in air (except cloud droplets).  Aerosol takes up ambient water (a process known as hygroscopic growth) depending on the relative humidity and the composition of the aerosol. Dry aerosol means aerosol without water.  Black carbon aerosol is composed of elemental carbon.  It is strongly light absorbing." .

<http://purl.oclc.org/NET/ssnx/cf/cf-property#mass_fraction_of_bromine_chloride_in_air>
  a owl:NamedIndividual, <http://purl.oclc.org/NET/ssnx/qu/dim#Dimensionless> ;
  rdfs:label "mass fraction of bromine chloride in air" ;
  rdfs:isDefinedBy <http://purl.oclc.org/NET/ssnx/cf/cf-property> ;
  rdfs:comment " Mass fraction is used in the construction mass_fraction_of_X_in_Y, whereX is a material constituent of Y. It means the ratio of the mass of X to the mass of Y (including X).  A chemical species denoted by X may be described by a single term such as 'nitrogen' or a phrase such as 'nox_expressed_as_nitrogen'. The chemical formula for bromine chloride is BrCl." .

<http://purl.oclc.org/NET/ssnx/cf/cf-property#mass_fraction_of_bromine_monoxide_in_air>
  a owl:NamedIndividual, <http://purl.oclc.org/NET/ssnx/qu/dim#Dimensionless> ;
  rdfs:label "mass fraction of bromine monoxide in air" ;
  rdfs:isDefinedBy <http://purl.oclc.org/NET/ssnx/cf/cf-property> ;
  rdfs:comment " Mass fraction is used in the construction mass_fraction_of_X_in_Y, whereX is a material constituent of Y. It means the ratio of the mass of X to the mass of Y (including X).  A chemical species denoted by X may be described by a single term such as 'nitrogen' or a phrase such as 'nox_expressed_as_nitrogen'. The chemical formula for bromine monoxide is BrO." .

<http://purl.oclc.org/NET/ssnx/cf/cf-property#mass_fraction_of_bromine_nitrate_in_air>
  a owl:NamedIndividual, <http://purl.oclc.org/NET/ssnx/qu/dim#Dimensionless> ;
  rdfs:label "mass fraction of bromine nitrate in air" ;
  rdfs:isDefinedBy <http://purl.oclc.org/NET/ssnx/cf/cf-property> ;
  rdfs:comment " Mass fraction is used in the construction mass_fraction_of_X_in_Y, whereX is a material constituent of Y. It means the ratio of the mass of X to the mass of Y (including X).  A chemical species denoted by X may be described by a single term such as 'nitrogen' or a phrase such as 'nox_expressed_as_nitrogen'. The chemical formula for bromine nitrate is BrONO2." .

<http://purl.oclc.org/NET/ssnx/cf/cf-property#mass_fraction_of_brox_expressed_as_bromine_in_air>
  a owl:NamedIndividual, <http://purl.oclc.org/NET/ssnx/qu/dim#Dimensionless> ;
  rdfs:label "mass fraction of brox expressed as bromine in air" ;
  rdfs:isDefinedBy <http://purl.oclc.org/NET/ssnx/cf/cf-property> ;
  rdfs:comment " Mass fraction is used in the construction mass_fraction_of_X_in_Y, whereX is a material constituent of Y. It means the ratio of the mass of X to the mass of Y (including X).  A chemical species denoted by X may be described by a single term such as 'nitrogen' or a phrase such as 'nox_expressed_as_nitrogen'. Brox  describes a family of chemical species consisting of inorganic bromine compounds with the exception of  hydrogen bromide (HBr) and bromine nitrate (BrONO2). Brox is the term used in standard names for all species belonging to the family that are represented within a given model. The list of individual species that are included in a quantity with a group chemical standard name can vary between models.  Where possible, the data variable should be accompaniedby a complete description of the species represented, for example, by using a comment attribute. Inorganic bromine, sometimes referred to as Bry, describes a family of chemical species which result from the degradation of source gases containing bromine (halons, methyl bromide, VSLS) and natural inorganic bromine sources such as volcanoes, seasalt and other aerosols.  Standard names that use the term inorganic_bromine are usedfor quantities that contain all inorganic bromine species including HCl and ClONO2. The phrase 'expressed_as' is used in the construction A_expressed_as_B, where B is a chemical constituent of A. It means that the quantity indicated by the standard name is calculated solely with respect to the B contained in A, neglecting all other chemical constituents of A." .

<http://purl.oclc.org/NET/ssnx/cf/cf-property#mass_fraction_of_butane_in_air>
  a owl:NamedIndividual, <http://purl.oclc.org/NET/ssnx/qu/dim#Dimensionless> ;
  rdfs:label "mass fraction of butane in air" ;
  rdfs:isDefinedBy <http://purl.oclc.org/NET/ssnx/cf/cf-property> ;
  rdfs:comment " Mass fraction is used in the construction mass_fraction_of_X_in_Y, whereX is a material constituent of Y. It means the ratio of the mass of X to the mass of Y (including X).  A chemical species denoted by X may be described by a single term such as 'nitrogen' or a phrase such as 'nox_expressed_as_nitrogen'. The chemical formula for butane is C4H10. Butane is a member of the group of hydrocarbons known as alkanes.  There are standard names for the alkane group as well as for some of the individual species." .

<http://purl.oclc.org/NET/ssnx/cf/cf-property#mass_fraction_of_carbon_dioxide_in_air>
  a owl:NamedIndividual, <http://purl.oclc.org/NET/ssnx/qu/dim#Dimensionless> ;
  rdfs:label "mass fraction of carbon dioxide in air" ;
  rdfs:isDefinedBy <http://purl.oclc.org/NET/ssnx/cf/cf-property> ;
  rdfs:comment " Mass fraction is used in the construction mass_fraction_of_X_in_Y, whereX is a material constituent of Y. It means the ratio of the mass of X to the mass of Y (including X).  A chemical species denoted by X may be described by a single term such as 'nitrogen' or a phrase such as 'nox_expressed_as_nitrogen'. The chemical formula for carbon dioxide is CO2." .

<http://purl.oclc.org/NET/ssnx/cf/cf-property#mass_fraction_of_carbon_monoxide_in_air>
  a owl:NamedIndividual, <http://purl.oclc.org/NET/ssnx/qu/dim#Dimensionless> ;
  rdfs:label "mass fraction of carbon monoxide in air" ;
  rdfs:isDefinedBy <http://purl.oclc.org/NET/ssnx/cf/cf-property> ;
  rdfs:comment " Mass fraction is used in the construction mass_fraction_of_X_in_Y, whereX is a material constituent of Y. It means the ratio of the mass of X to the mass of Y (including X).  A chemical species denoted by X may be described by a single term such as 'nitrogen' or a phrase such as 'nox_expressed_as_nitrogen'. The chemical formula of carbon monoxide is CO." .

<http://purl.oclc.org/NET/ssnx/cf/cf-property#mass_fraction_of_carbon_tetrachloride_in_air>
  a owl:NamedIndividual, <http://purl.oclc.org/NET/ssnx/qu/dim#Dimensionless> ;
  rdfs:label "mass fraction of carbon tetrachloride in air" ;
  rdfs:isDefinedBy <http://purl.oclc.org/NET/ssnx/cf/cf-property> ;
  rdfs:comment " Mass fraction is used in the construction mass_fraction_of_X_in_Y, whereX is a material constituent of Y. It means the ratio of the mass of X to the mass of Y (including X).  A chemical species denoted by X may be described by a single term such as 'nitrogen' or a phrase such as 'nox_expressed_as_nitrogen'. The chemical formula of carbon tetrachloride is CCl4." .

<http://purl.oclc.org/NET/ssnx/cf/cf-property#mass_fraction_of_cfc113_in_air>
  a owl:NamedIndividual, <http://purl.oclc.org/NET/ssnx/qu/dim#Dimensionless> ;
  rdfs:label "mass fraction of cfc113 in air" ;
  rdfs:isDefinedBy <http://purl.oclc.org/NET/ssnx/cf/cf-property> ;
  rdfs:comment " Mass fraction is used in the construction mass_fraction_of_X_in_Y, where X is a material constituent of Y. It means the ratio of the mass of X to the mass of Y (including X).  A chemical species denoted by X may be described by a single term such as 'nitrogen' or a phrase such as 'nox_expressed_as_nitrogen'. The chemical formula of CFC113 is CCl2FCClF2. The IUPAC name for CFC113 is 1,1,2-trichloro-1,2,2-trifluoro-ethane." .

<http://purl.oclc.org/NET/ssnx/cf/cf-property#mass_fraction_of_cfc113a_in_air>
  a owl:NamedIndividual, <http://purl.oclc.org/NET/ssnx/qu/dim#Dimensionless> ;
  rdfs:label "mass fraction of cfc113a in air" ;
  rdfs:isDefinedBy <http://purl.oclc.org/NET/ssnx/cf/cf-property> ;
  rdfs:comment " Mass fraction is used in the construction mass_fraction_of_X_in_Y, whereX is a material constituent of Y. It means the ratio of the mass of X to the mass of Y (including X).  A chemical species denoted by X may be described by a single term such as 'nitrogen' or a phrase such as 'nox_expressed_as_nitrogen'. The chemical formula of CFC113a CCl3CF3.  The IUPAC name for CFC113a is 1,1,1-trichloro-2,2,2-trifluoro-ethane." .

<http://purl.oclc.org/NET/ssnx/cf/cf-property#mass_fraction_of_cfc114_in_air>
  a owl:NamedIndividual, <http://purl.oclc.org/NET/ssnx/qu/dim#Dimensionless> ;
  rdfs:label "mass fraction of cfc114 in air" ;
  rdfs:isDefinedBy <http://purl.oclc.org/NET/ssnx/cf/cf-property> ;
  rdfs:comment " Mass fraction is used in the construction mass_fraction_of_X_in_Y, whereX is a material constituent of Y. It means the ratio of the mass of X to the mass of Y (including X).  A chemical species denoted by X may be described by a single term such as 'nitrogen' or a phrase such as 'nox_expressed_as_nitrogen'. The chemical formula of CFC114 is CClF2CClF2. The IUPAC name for CFC114 is 1,2-dichloro-1,1,2,2-tetrafluoro-ethane." .

<http://purl.oclc.org/NET/ssnx/cf/cf-property#mass_fraction_of_cfc115_in_air>
  a owl:NamedIndividual, <http://purl.oclc.org/NET/ssnx/qu/dim#Dimensionless> ;
  rdfs:label "mass fraction of cfc115 in air" ;
  rdfs:isDefinedBy <http://purl.oclc.org/NET/ssnx/cf/cf-property> ;
  rdfs:comment " Mass fraction is used in the construction mass_fraction_of_X_in_Y, whereX is a material constituent of Y. It means the ratio of the mass of X to the mass of Y (including X).  A chemical species denoted by X may be described by a single term such as 'nitrogen' or a phrase such as 'nox_expressed_as_nitrogen'. The chemical formula of CFC115 is CClF2CF3. The IUPAC name for CFC115 is 1-chloro-1,1,2,2,2-pentafluoro-ethane." .

<http://purl.oclc.org/NET/ssnx/cf/cf-property#mass_fraction_of_cfc11_in_air>
  a owl:NamedIndividual, <http://purl.oclc.org/NET/ssnx/qu/dim#Dimensionless> ;
  rdfs:label "mass fraction of cfc11 in air" ;
  rdfs:isDefinedBy <http://purl.oclc.org/NET/ssnx/cf/cf-property> ;
  rdfs:comment " Mass fraction is used in the construction mass_fraction_of_X_in_Y, whereX is a material constituent of Y. It means the ratio of the mass of X to the mass of Y (including X).  A chemical species denoted by X may be described by a single term such as 'nitrogen' or a phrase such as 'nox_expressed_as_nitrogen'. The chemical formula of CFC11 is CFCl3. The IUPAC name fof CFC11 is trichloro-fluoro-methane." .

<http://purl.oclc.org/NET/ssnx/cf/cf-property#mass_fraction_of_cfc12_in_air>
  a owl:NamedIndividual, <http://purl.oclc.org/NET/ssnx/qu/dim#Dimensionless> ;
  rdfs:label "mass fraction of cfc12 in air" ;
  rdfs:isDefinedBy <http://purl.oclc.org/NET/ssnx/cf/cf-property> ;
  rdfs:comment " Mass fraction is used in the construction mass_fraction_of_X_in_Y, whereX is a material constituent of Y. It means the ratio of the mass of X to the mass of Y (including X).  A chemical species denoted by X may be described by a single term such as 'nitrogen' or a phrase such as 'nox_expressed_as_nitrogen'. The chemical formula for CFC12 is CF2Cl2.  The IUPAC name for CFC12 is dichloro-difluoro-methane." .

<http://purl.oclc.org/NET/ssnx/cf/cf-property#mass_fraction_of_chlorine_dioxide_in_air>
  a owl:NamedIndividual, <http://purl.oclc.org/NET/ssnx/qu/dim#Dimensionless> ;
  rdfs:label "mass fraction of chlorine dioxide in air" ;
  rdfs:isDefinedBy <http://purl.oclc.org/NET/ssnx/cf/cf-property> ;
  rdfs:comment " Mass fraction is used in the construction mass_fraction_of_X_in_Y, whereX is a material constituent of Y. It means the ratio of the mass of X to the mass of Y (including X).  A chemical species denoted by X may be described by a single term such as 'nitrogen' or a phrase such as 'nox_expressed_as_nitrogen'. The chemical formula for chlorine dioxide is OClO." .

<http://purl.oclc.org/NET/ssnx/cf/cf-property#mass_fraction_of_chlorine_monoxide_in_air>
  a owl:NamedIndividual, <http://purl.oclc.org/NET/ssnx/qu/dim#Dimensionless> ;
  rdfs:label "mass fraction of chlorine monoxide in air" ;
  rdfs:isDefinedBy <http://purl.oclc.org/NET/ssnx/cf/cf-property> ;
  rdfs:comment " Mass fraction is used in the construction mass_fraction_of_X_in_Y, whereX is a material constituent of Y. It means the ratio of the mass of X to the mass of Y (including X).  A chemical species denoted by X may be described by a single term such as 'nitrogen' or a phrase such as 'nox_expressed_as_nitrogen'. The chemical formula for chlorine monoxide is ClO." .

<http://purl.oclc.org/NET/ssnx/cf/cf-property#mass_fraction_of_chlorine_nitrate_in_air>
  a owl:NamedIndividual, <http://purl.oclc.org/NET/ssnx/qu/dim#Dimensionless> ;
  rdfs:label "mass fraction of chlorine nitrate in air" ;
  rdfs:isDefinedBy <http://purl.oclc.org/NET/ssnx/cf/cf-property> ;
  rdfs:comment " Mass fraction is used in the construction mass_fraction_of_X_in_Y, whereX is a material constituent of Y. It means the ratio of the mass of X to the mass of Y (including X).  A chemical species denoted by X may be described by a single term such as 'nitrogen' or a phrase such as 'nox_expressed_as_nitrogen'. The chemical formula for chlorine nitrate is ClONO2." .

<http://purl.oclc.org/NET/ssnx/cf/cf-property#mass_fraction_of_cloud_condensed_water_in_air>
  a owl:NamedIndividual, <http://purl.oclc.org/NET/ssnx/qu/dim#Dimensionless> ;
  rdfs:label "mass fraction of cloud condensed water in air" ;
  rdfs:isDefinedBy <http://purl.oclc.org/NET/ssnx/cf/cf-property> ;
  rdfs:comment "condensed_water means liquid and ice. Mass fraction is used in the construction mass_fraction_of_X_in_Y, where X is a material constituent of Y. It means the ratio of the mass of X to the mass of Y (including X)." .

<http://purl.oclc.org/NET/ssnx/cf/cf-property#mass_fraction_of_cloud_ice_in_air>
  a owl:NamedIndividual, <http://purl.oclc.org/NET/ssnx/qu/dim#Dimensionless> ;
  rdfs:label "mass fraction of cloud ice in air" ;
  rdfs:isDefinedBy <http://purl.oclc.org/NET/ssnx/cf/cf-property> ;
  rdfs:comment "Mass fraction is used in the construction mass_fraction_of_X_in_Y, where X is a material constituent of Y. It means the ratio of the mass of X to the mass of Y (including X)." .

<http://purl.oclc.org/NET/ssnx/cf/cf-property#mass_fraction_of_cloud_liquid_water_in_air>
  a owl:NamedIndividual, <http://purl.oclc.org/NET/ssnx/qu/dim#Dimensionless> ;
  rdfs:label "mass fraction of cloud liquid water in air" ;
  rdfs:isDefinedBy <http://purl.oclc.org/NET/ssnx/cf/cf-property> ;
  rdfs:comment "Mass fraction is used in the construction mass_fraction_of_X_in_Y, where X is a material constituent of Y. It means the ratio of the mass of X to the mass of Y (including X)." .

<http://purl.oclc.org/NET/ssnx/cf/cf-property#mass_fraction_of_clox_expressed_as_chlorine_in_air>
  a owl:NamedIndividual, <http://purl.oclc.org/NET/ssnx/qu/dim#Dimensionless> ;
  rdfs:label "mass fraction of clox expressed as chlorine in air" ;
  rdfs:isDefinedBy <http://purl.oclc.org/NET/ssnx/cf/cf-property> ;
  rdfs:comment " Mass fraction is used in the construction mass_fraction_of_X_in_Y, whereX is a material constituent of Y. It means the ratio of the mass of X to the mass of Y (including X).  A chemical species denoted by X may be described by a single term such as 'nitrogen' or a phrase such as 'nox_expressed_as_nitrogen'. Clox describes a familyof chemical species consisting of inorganic chlorine compounds with the exception of  hydrogen chloride (HCl) and chlorine nitrate (ClONO2). Clox is the term used in standard names for all species belonging to the family that are represented within a given model. The list of individual species that are included in a quantity with a group chemical standard name can vary between models.  Where possible, the data variable should be accompanied by a complete description of the species represented, for example, by using a comment attribute. Inorganic chlorine, sometimes referred to as Cly, describes a family of chemical species which result from the degradation of source gases containing chlorine (CFCs, HCFCs, VSLS) and natural inorganic chlorine sources such as seasalt and other aerosols.   Standard names that use the term inorganic_chlorine are used for quantitiesthat contain all inorganic chlorine species including HCl and ClONO2. The phrase 'expressed_as' is used in the construction A_expressed_as_B, where B is a chemical constituent of A.It means that the quantity indicated by the standard name is calculated solely with respect to the B contained in A, neglecting all other chemical constituents of A." .

<http://purl.oclc.org/NET/ssnx/cf/cf-property#mass_fraction_of_convective_cloud_condensed_water_in_air>
  a owl:NamedIndividual, <http://purl.oclc.org/NET/ssnx/qu/dim#Dimensionless> ;
  rdfs:label "mass fraction of convective cloud condensed water in air" ;
  rdfs:isDefinedBy <http://purl.oclc.org/NET/ssnx/cf/cf-property> ;
  rdfs:comment "condensed_water means liquid and ice. Mass fraction is used in the construction mass_fraction_of_X_in_Y, where X is a material constituent of Y. It means the ratio of the mass of X to the mass of Y (including X)." .

<http://purl.oclc.org/NET/ssnx/cf/cf-property#mass_fraction_of_convective_cloud_ice_in_air>
  a owl:NamedIndividual, <http://purl.oclc.org/NET/ssnx/qu/dim#Dimensionless> ;
  rdfs:label "mass fraction of convective cloud ice in air" ;
  rdfs:isDefinedBy <http://purl.oclc.org/NET/ssnx/cf/cf-property> ;
  rdfs:comment "Mass fraction is used in the construction mass_fraction_of_X_in_Y, where X is a material constituent of Y. It means the ratio of the mass of X to the mass of Y (including X). Convective cloud is that produced by the convection schemes in an atmosphere model." .

<http://purl.oclc.org/NET/ssnx/cf/cf-property#mass_fraction_of_convective_cloud_liquid_water_in_air>
  a owl:NamedIndividual, <http://purl.oclc.org/NET/ssnx/qu/dim#Dimensionless> ;
  rdfs:label "mass fraction of convective cloud liquid water in air" ;
  rdfs:isDefinedBy <http://purl.oclc.org/NET/ssnx/cf/cf-property> ;
  rdfs:comment "Mass fraction is used in the construction mass_fraction_of_X_in_Y, where X is a material constituent of Y. It means the ratio of the mass of X to the mass of Y (including X). Convective cloud is that produced by the convection schemes in an atmosphere model." .

<http://purl.oclc.org/NET/ssnx/cf/cf-property#mass_fraction_of_dichlorine_peroxide_in_air>
  a owl:NamedIndividual, <http://purl.oclc.org/NET/ssnx/qu/dim#Dimensionless> ;
  rdfs:label "mass fraction of dichlorine peroxide in air" ;
  rdfs:isDefinedBy <http://purl.oclc.org/NET/ssnx/cf/cf-property> ;
  rdfs:comment " Mass fraction is used in the construction mass_fraction_of_X_in_Y, whereX is a material constituent of Y. It means the ratio of the mass of X to the mass of Y (including X).  A chemical species denoted by X may be described by a single term such as 'nitrogen' or a phrase such as 'nox_expressed_as_nitrogen'. The chemical formula for dichlorineperoxide is Cl2O2." .

<http://purl.oclc.org/NET/ssnx/cf/cf-property#mass_fraction_of_dimethyl_sulfide_in_air>
  a owl:NamedIndividual, <http://purl.oclc.org/NET/ssnx/qu/dim#Dimensionless> ;
  rdfs:label "mass fraction of dimethyl sulfide in air" ;
  rdfs:isDefinedBy <http://purl.oclc.org/NET/ssnx/cf/cf-property> ;
  rdfs:comment "Mass fraction is used in the construction mass_fraction_of_X_in_Y, where X is a material constituent of Y. It means the ratio of the mass of X to the mass of Y (including X)." .

<http://purl.oclc.org/NET/ssnx/cf/cf-property#mass_fraction_of_dinitrogen_pentoxide_in_air>
  a owl:NamedIndividual, <http://purl.oclc.org/NET/ssnx/qu/dim#Dimensionless> ;
  rdfs:label "mass fraction of dinitrogen pentoxide in air" ;
  rdfs:isDefinedBy <http://purl.oclc.org/NET/ssnx/cf/cf-property> ;
  rdfs:comment " Mass fraction is used in the construction mass_fraction_of_X_in_Y, whereX is a material constituent of Y. It means the ratio of the mass of X to the mass of Y (including X).  A chemical species denoted by X may be described by a single term such as 'nitrogen' or a phrase such as 'nox_expressed_as_nitrogen'. The chemical formula for dinitrogenpentoxide is N2O5." .

<http://purl.oclc.org/NET/ssnx/cf/cf-property#mass_fraction_of_dust_dry_aerosol_in_air>
  a owl:NamedIndividual, <http://purl.oclc.org/NET/ssnx/qu/dim#Dimensionless> ;
  rdfs:label "mass fraction of dust dry aerosol in air" ;
  rdfs:isDefinedBy <http://purl.oclc.org/NET/ssnx/cf/cf-property> ;
  rdfs:comment "Mass fraction is used in the construction mass_fraction_of_X_in_Y, where X is a material constituent of Y. It means the ratio of the mass of X to the mass of Y (including X).  Aerosol means the suspended liquid or solid particles in air (except cloud droplets).  Aerosol takes up ambient water (a process known as hygroscopic growth) depending on the relative humidity and the composition of the aerosol. Dry aerosol means aerosol without water." .

<http://purl.oclc.org/NET/ssnx/cf/cf-property#mass_fraction_of_ethane_in_air>
  a owl:NamedIndividual, <http://purl.oclc.org/NET/ssnx/qu/dim#Dimensionless> ;
  rdfs:label "mass fraction of ethane in air" ;
  rdfs:isDefinedBy <http://purl.oclc.org/NET/ssnx/cf/cf-property> ;
  rdfs:comment " Mass fraction is used in the construction mass_fraction_of_X_in_Y, whereX is a material constituent of Y. It means the ratio of the mass of X to the mass of Y (including X).  A chemical species denoted by X may be described by a single term such as 'nitrogen' or a phrase such as 'nox_expressed_as_nitrogen'. The chemical formula for ethane is C2H6. Ethane is a member of the group of hydrocarbons known as alkanes.  There are standardnames for the alkane group as well as for some of the individual species." .

<http://purl.oclc.org/NET/ssnx/cf/cf-property#mass_fraction_of_ethanol_in_air>
  a owl:NamedIndividual, <http://purl.oclc.org/NET/ssnx/qu/dim#Dimensionless> ;
  rdfs:label "mass fraction of ethanol in air" ;
  rdfs:isDefinedBy <http://purl.oclc.org/NET/ssnx/cf/cf-property> ;
  rdfs:comment " Mass fraction is used in the construction mass_fraction_of_X_in_Y, whereX is a material constituent of Y. It means the ratio of the mass of X to the mass of Y (including X).  A chemical species denoted by X may be described by a single term such as 'nitrogen' or a phrase such as 'nox_expressed_as_nitrogen'. The chemical formula for ethanol isC2H5OH." .

<http://purl.oclc.org/NET/ssnx/cf/cf-property#mass_fraction_of_ethene_in_air>
  a owl:NamedIndividual, <http://purl.oclc.org/NET/ssnx/qu/dim#Dimensionless> ;
  rdfs:label "mass fraction of ethene in air" ;
  rdfs:isDefinedBy <http://purl.oclc.org/NET/ssnx/cf/cf-property> ;
  rdfs:comment " Mass fraction is used in the construction mass_fraction_of_X_in_Y, whereX is a material constituent of Y. It means the ratio of the mass of X to the mass of Y (including X).  A chemical species denoted by X may be described by a single term such as 'nitrogen' or a phrase such as 'nox_expressed_as_nitrogen'. The chemical formula for ethene is C2H4. Ethene is a member of the group of hydrocarbons known as alkenes.  There are standardnames for the alkene group as well as for some of the individual species." .

<http://purl.oclc.org/NET/ssnx/cf/cf-property#mass_fraction_of_ethyne_in_air>
  a owl:NamedIndividual, <http://purl.oclc.org/NET/ssnx/qu/dim#Dimensionless> ;
  rdfs:label "mass fraction of ethyne in air" ;
  rdfs:isDefinedBy <http://purl.oclc.org/NET/ssnx/cf/cf-property> ;
  rdfs:comment " Mass fraction is used in the construction mass_fraction_of_X_in_Y, whereX is a material constituent of Y. It means the ratio of the mass of X to the mass of Y (including X).  A chemical species denoted by X may be described by a single term such as 'nitrogen' or a phrase such as 'nox_expressed_as_nitrogen'. The chemical formula for ethyne is HC2H.  Ethyne is the IUPAC name for this species, which is also commonly known as acetylene." .

<http://purl.oclc.org/NET/ssnx/cf/cf-property#mass_fraction_of_formaldehyde_in_air>
  a owl:NamedIndividual, <http://purl.oclc.org/NET/ssnx/qu/dim#Dimensionless> ;
  rdfs:label "mass fraction of formaldehyde in air" ;
  rdfs:isDefinedBy <http://purl.oclc.org/NET/ssnx/cf/cf-property> ;
  rdfs:comment " Mass fraction is used in the construction mass_fraction_of_X_in_Y, whereX is a material constituent of Y. It means the ratio of the mass of X to the mass of Y (including X).  A chemical species denoted by X may be described by a single term such as 'nitrogen' or a phrase such as 'nox_expressed_as_nitrogen'. The chemical formula for formaldehyde is CH2O. The IUPAC name for formaldehyde is methanal." .

<http://purl.oclc.org/NET/ssnx/cf/cf-property#mass_fraction_of_formic_acid_in_air>
  a owl:NamedIndividual, <http://purl.oclc.org/NET/ssnx/qu/dim#Dimensionless> ;
  rdfs:label "mass fraction of formic acid in air" ;
  rdfs:isDefinedBy <http://purl.oclc.org/NET/ssnx/cf/cf-property> ;
  rdfs:comment " Mass fraction is used in the construction mass_fraction_of_X_in_Y, whereX is a material constituent of Y. It means the ratio of the mass of X to the mass of Y (including X).  A chemical species denoted by X may be described by a single term such as 'nitrogen' or a phrase such as 'nox_expressed_as_nitrogen'. The chemical formula for formic acid is HCOOH.  The IUPAC name for formic acid is methanoic acid." .

<http://purl.oclc.org/NET/ssnx/cf/cf-property#mass_fraction_of_gaseous_divalent_mercury_in_air>
  a owl:NamedIndividual, <http://purl.oclc.org/NET/ssnx/qu/dim#Dimensionless> ;
  rdfs:label "mass fraction of gaseous divalent mercury in air" ;
  rdfs:isDefinedBy <http://purl.oclc.org/NET/ssnx/cf/cf-property> ;
  rdfs:comment " Mass fraction is used in the construction mass_fraction_of_X_in_Y, whereX is a material constituent of Y. It means the ratio of the mass of X to the mass of Y (including X).  A chemical species denoted by X may be described by a single term such as 'nitrogen' or a phrase such as 'nox_expressed_as_nitrogen'. Divalent mercury means all compounds in which the mercury has two binding sites to other ion(s) in a salt or to other atom(s) in a molecule." .

<http://purl.oclc.org/NET/ssnx/cf/cf-property#mass_fraction_of_gaseous_elemental_mercury_in_air>
  a owl:NamedIndividual, <http://purl.oclc.org/NET/ssnx/qu/dim#Dimensionless> ;
  rdfs:label "mass fraction of gaseous elemental mercury in air" ;
  rdfs:isDefinedBy <http://purl.oclc.org/NET/ssnx/cf/cf-property> ;
  rdfs:comment " Mass fraction is used in the construction mass_fraction_of_X_in_Y, whereX is a material constituent of Y. It means the ratio of the mass of X to the mass of Y (including X).  A chemical species denoted by X may be described by a single term such as 'nitrogen' or a phrase such as 'nox_expressed_as_nitrogen'. The chemical symbol for mercury is Hg." .

<http://purl.oclc.org/NET/ssnx/cf/cf-property#mass_fraction_of_graupel_in_air>
  a owl:NamedIndividual, <http://purl.oclc.org/NET/ssnx/qu/dim#Dimensionless> ;
  rdfs:label "mass fraction of graupel in air" ;
  rdfs:isDefinedBy <http://purl.oclc.org/NET/ssnx/cf/cf-property> ;
  rdfs:comment "Mass fraction is used in the construction mass_fraction_of_X_in_Y, where X is a material constituent of Y. It means the ratio of the mass of X to the mass of Y (including X)." .

<http://purl.oclc.org/NET/ssnx/cf/cf-property#mass_fraction_of_halon1202_in_air>
  a owl:NamedIndividual, <http://purl.oclc.org/NET/ssnx/qu/dim#Dimensionless> ;
  rdfs:label "mass fraction of halon1202 in air" ;
  rdfs:isDefinedBy <http://purl.oclc.org/NET/ssnx/cf/cf-property> ;
  rdfs:comment " Mass fraction is used in the construction mass_fraction_of_X_in_Y, whereX is a material constituent of Y. It means the ratio of the mass of X to the mass of Y (including X).  A chemical species denoted by X may be described by a single term such as 'nitrogen' or a phrase such as 'nox_expressed_as_nitrogen'. The chemical formula for halon1202 is CBr2F2. The IUPAC name for halon1202 is dibromo-difluoro-methane." .

<http://purl.oclc.org/NET/ssnx/cf/cf-property#mass_fraction_of_halon1211_in_air>
  a owl:NamedIndividual, <http://purl.oclc.org/NET/ssnx/qu/dim#Dimensionless> ;
  rdfs:label "mass fraction of halon1211 in air" ;
  rdfs:isDefinedBy <http://purl.oclc.org/NET/ssnx/cf/cf-property> ;
  rdfs:comment " Mass fraction is used in the construction mass_fraction_of_X_in_Y, whereX is a material constituent of Y. It means the ratio of the mass of X to the mass of Y (including X).  A chemical species denoted by X may be described by a single term such as 'nitrogen' or a phrase such as 'nox_expressed_as_nitrogen'. The chemical formula for halon1211 is CBrClF2. The IUPAC name for halon1211 is bromo-chloro-difluoro-methane." .

<http://purl.oclc.org/NET/ssnx/cf/cf-property#mass_fraction_of_halon1301_in_air>
  a owl:NamedIndividual, <http://purl.oclc.org/NET/ssnx/qu/dim#Dimensionless> ;
  rdfs:label "mass fraction of halon1301 in air" ;
  rdfs:isDefinedBy <http://purl.oclc.org/NET/ssnx/cf/cf-property> ;
  rdfs:comment " Mass fraction is used in the construction mass_fraction_of_X_in_Y, whereX is a material constituent of Y. It means the ratio of the mass of X to the mass of Y (including X).  A chemical species denoted by X may be described by a single term such as 'nitrogen' or a phrase such as 'nox_expressed_as_nitrogen'. The chemical formula for halon1301 is CBrF3. The IUPAC name for halon1301 is bromo-trifluoro-methane." .

<http://purl.oclc.org/NET/ssnx/cf/cf-property#mass_fraction_of_halon2402_in_air>
  a owl:NamedIndividual, <http://purl.oclc.org/NET/ssnx/qu/dim#Dimensionless> ;
  rdfs:label "mass fraction of halon2402 in air" ;
  rdfs:isDefinedBy <http://purl.oclc.org/NET/ssnx/cf/cf-property> ;
  rdfs:comment " Mass fraction is used in the construction mass_fraction_of_X_in_Y, whereX is a material constituent of Y. It means the ratio of the mass of X to the mass of Y (including X).  A chemical species denoted by X may be described by a single term such as 'nitrogen' or a phrase such as 'nox_expressed_as_nitrogen'. The chemical formula for halo2402 is C2Br2F4. The IUPAC name for halon2402 is 1,2-dibromo-1,1,2,2-tetrafluoro-ethane." .

<http://purl.oclc.org/NET/ssnx/cf/cf-property#mass_fraction_of_hcc140a_in_air>
  a owl:NamedIndividual, <http://purl.oclc.org/NET/ssnx/qu/dim#Dimensionless> ;
  rdfs:label "mass fraction of hcc140a in air" ;
  rdfs:isDefinedBy <http://purl.oclc.org/NET/ssnx/cf/cf-property> ;
  rdfs:comment " Mass fraction is used in the construction mass_fraction_of_X_in_Y, whereX is a material constituent of Y. It means the ratio of the mass of X to the mass of Y (including X).  A chemical species denoted by X may be described by a single term such as 'nitrogen' or a phrase such as 'nox_expressed_as_nitrogen'. The chemical formula for hcc140a isCH3CCl3. The IUPAC name for hcc140a is 1,1,1-trichloro-ethane." .

<http://purl.oclc.org/NET/ssnx/cf/cf-property#mass_fraction_of_hcfc141b_in_air>
  a owl:NamedIndividual, <http://purl.oclc.org/NET/ssnx/qu/dim#Dimensionless> ;
  rdfs:label "mass fraction of hcfc141b in air" ;
  rdfs:isDefinedBy <http://purl.oclc.org/NET/ssnx/cf/cf-property> ;
  rdfs:comment " Mass fraction is used in the construction mass_fraction_of_X_in_Y, whereX is a material constituent of Y. It means the ratio of the mass of X to the mass of Y (including X).  A chemical species denoted by X may be described by a single term such as 'nitrogen' or a phrase such as 'nox_expressed_as_nitrogen'. The chemical formula for HCFC141b is CH3CCl2F. The IUPAC name for HCFC141b is 1,1-dichloro-1-fluoroethane." .

<http://purl.oclc.org/NET/ssnx/cf/cf-property#mass_fraction_of_hcfc142b_in_air>
  a owl:NamedIndividual, <http://purl.oclc.org/NET/ssnx/qu/dim#Dimensionless> ;
  rdfs:label "mass fraction of hcfc142b in air" ;
  rdfs:isDefinedBy <http://purl.oclc.org/NET/ssnx/cf/cf-property> ;
  rdfs:comment " Mass fraction is used in the construction mass_fraction_of_X_in_Y, whereX is a material constituent of Y. It means the ratio of the mass of X to the mass of Y (including X).  A chemical species denoted by X may be described by a single term such as 'nitrogen' or a phrase such as 'nox_expressed_as_nitrogen'. The chemical formula for HCFC142b is CH3CClF2. The IUPAC name for HCFC142b is 1-chloro-1,1-difluoroethane." .

<http://purl.oclc.org/NET/ssnx/cf/cf-property#mass_fraction_of_hcfc22_in_air>
  a owl:NamedIndividual, <http://purl.oclc.org/NET/ssnx/qu/dim#Dimensionless> ;
  rdfs:label "mass fraction of hcfc22 in air" ;
  rdfs:isDefinedBy <http://purl.oclc.org/NET/ssnx/cf/cf-property> ;
  rdfs:comment " Mass fraction is used in the construction mass_fraction_of_X_in_Y, whereX is a material constituent of Y. It means the ratio of the mass of X to the mass of Y (including X).  A chemical species denoted by X may be described by a single term such as 'nitrogen' or a phrase such as 'nox_expressed_as_nitrogen'. The chemical formula for HCFC22 is CHClF2.  The IUPAC name for HCFC22 is chloro-difluoro-methane." .

<http://purl.oclc.org/NET/ssnx/cf/cf-property#mass_fraction_of_hexachlorobiphenyl_in_air>
  a owl:NamedIndividual, <http://purl.oclc.org/NET/ssnx/qu/dim#Dimensionless> ;
  rdfs:label "mass fraction of hexachlorobiphenyl in air" ;
  rdfs:isDefinedBy <http://purl.oclc.org/NET/ssnx/cf/cf-property> ;
  rdfs:comment " Mass fraction is used in the construction mass_fraction_of_X_in_Y, whereX is a material constituent of Y. It means the ratio of the mass of X to the mass of Y (including X).  A chemical species denoted by X may be described by a single term such as 'nitrogen' or a phrase such as 'nox_expressed_as_nitrogen'. The chemical formula for hexachlorobiphenyl is C12H4Cl6.  This structure of this species consists of two linked benzene rings,each of which is additionally bonded to three chlorine atoms." .

<http://purl.oclc.org/NET/ssnx/cf/cf-property#mass_fraction_of_hox_expressed_as_hydrogen_in_air>
  a owl:NamedIndividual, <http://purl.oclc.org/NET/ssnx/qu/dim#Dimensionless> ;
  rdfs:label "mass fraction of hox expressed as hydrogen in air" ;
  rdfs:isDefinedBy <http://purl.oclc.org/NET/ssnx/cf/cf-property> ;
  rdfs:comment " Mass fraction is used in the construction mass_fraction_of_X_in_Y, whereX is a material constituent of Y. It means the ratio of the mass of X to the mass of Y (including X).  A chemical species denoted by X may be described by a single term such as 'nitrogen' or a phrase such as 'nox_expressed_as_nitrogen'. HOx means a combinationof two radical species containing hydrogen and oxygen: OH and HO2. The phrase 'expressed_as' is used in the construction A_expressed_as_B, where B is a chemical constituent of A. Itmeans that the quantity indicated by the standard name is calculated solely with respect to the B contained in A, neglecting all other chemical constituents of A." .

<http://purl.oclc.org/NET/ssnx/cf/cf-property#mass_fraction_of_hydrogen_bromide_in_air>
  a owl:NamedIndividual, <http://purl.oclc.org/NET/ssnx/qu/dim#Dimensionless> ;
  rdfs:label "mass fraction of hydrogen bromide in air" ;
  rdfs:isDefinedBy <http://purl.oclc.org/NET/ssnx/cf/cf-property> ;
  rdfs:comment " Mass fraction is used in the construction mass_fraction_of_X_in_Y, whereX is a material constituent of Y. It means the ratio of the mass of X to the mass of Y (including X).  A chemical species denoted by X may be described by a single term such as 'nitrogen' or a phrase such as 'nox_expressed_as_nitrogen'. The chemical formula for hydrogen bromide is HBr." .

<http://purl.oclc.org/NET/ssnx/cf/cf-property#mass_fraction_of_hydrogen_chloride_in_air>
  a owl:NamedIndividual, <http://purl.oclc.org/NET/ssnx/qu/dim#Dimensionless> ;
  rdfs:label "mass fraction of hydrogen chloride in air" ;
  rdfs:isDefinedBy <http://purl.oclc.org/NET/ssnx/cf/cf-property> ;
  rdfs:comment " Mass fraction is used in the construction mass_fraction_of_X_in_Y, whereX is a material constituent of Y. It means the ratio of the mass of X to the mass of Y (including X).  A chemical species denoted by X may be described by a single term such as 'nitrogen' or a phrase such as 'nox_expressed_as_nitrogen'. The chemical formula for hydrogen chloride is HCl." .

<http://purl.oclc.org/NET/ssnx/cf/cf-property#mass_fraction_of_hydrogen_cyanide_in_air>
  a owl:NamedIndividual, <http://purl.oclc.org/NET/ssnx/qu/dim#Dimensionless> ;
  rdfs:label "mass fraction of hydrogen cyanide in air" ;
  rdfs:isDefinedBy <http://purl.oclc.org/NET/ssnx/cf/cf-property> ;
  rdfs:comment " Mass fraction is used in the construction mass_fraction_of_X_in_Y, whereX is a material constituent of Y. It means the ratio of the mass of X to the mass of Y (including X).  A chemical species denoted by X may be described by a single term such as 'nitrogen' or a phrase such as 'nox_expressed_as_nitrogen'. The chemical formula for hydrogen cyanide is HCN." .

<http://purl.oclc.org/NET/ssnx/cf/cf-property#mass_fraction_of_hydrogen_peroxide_in_air>
  a owl:NamedIndividual, <http://purl.oclc.org/NET/ssnx/qu/dim#Dimensionless> ;
  rdfs:label "mass fraction of hydrogen peroxide in air" ;
  rdfs:isDefinedBy <http://purl.oclc.org/NET/ssnx/cf/cf-property> ;
  rdfs:comment " Mass fraction is used in the construction mass_fraction_of_X_in_Y, whereX is a material constituent of Y. It means the ratio of the mass of X to the mass of Y (including X).  A chemical species denoted by X may be described by a single term such as 'nitrogen' or a phrase such as 'nox_expressed_as_nitrogen'. The chemical formula for hydrogen peroxide is H2O2." .

<http://purl.oclc.org/NET/ssnx/cf/cf-property#mass_fraction_of_hydroperoxyl_radical_in_air>
  a owl:NamedIndividual, <http://purl.oclc.org/NET/ssnx/qu/dim#Dimensionless> ;
  rdfs:label "mass fraction of hydroperoxyl radical in air" ;
  rdfs:isDefinedBy <http://purl.oclc.org/NET/ssnx/cf/cf-property> ;
  rdfs:comment " Mass fraction is used in the construction mass_fraction_of_X_in_Y, whereX is a material constituent of Y. It means the ratio of the mass of X to the mass of Y (including X).  A chemical species denoted by X may be described by a single term such as 'nitrogen' or a phrase such as 'nox_expressed_as_nitrogen'. The chemical formula for the hydroperoxyl radical is HO2. In chemistry, a 'radical' is a highly reactive, and therefore shortlived, species." .

<http://purl.oclc.org/NET/ssnx/cf/cf-property#mass_fraction_of_hydroxyl_radical_in_air>
  a owl:NamedIndividual, <http://purl.oclc.org/NET/ssnx/qu/dim#Dimensionless> ;
  rdfs:label "mass fraction of hydroxyl radical in air" ;
  rdfs:isDefinedBy <http://purl.oclc.org/NET/ssnx/cf/cf-property> ;
  rdfs:comment " Mass fraction is used in the construction mass_fraction_of_X_in_Y, whereX is a material constituent of Y. It means the ratio of the mass of X to the mass of Y (including X).  A chemical species denoted by X may be described by a single term such as 'nitrogen' or a phrase such as 'nox_expressed_as_nitrogen'. The chemical formula for the hydroxyl radical is OH. In chemistry, a 'radical' is a highly reactive, and therefore shortlived,species." .

<http://purl.oclc.org/NET/ssnx/cf/cf-property#mass_fraction_of_hypobromous_acid_in_air>
  a owl:NamedIndividual, <http://purl.oclc.org/NET/ssnx/qu/dim#Dimensionless> ;
  rdfs:label "mass fraction of hypobromous acid in air" ;
  rdfs:isDefinedBy <http://purl.oclc.org/NET/ssnx/cf/cf-property> ;
  rdfs:comment " Mass fraction is used in the construction mass_fraction_of_X_in_Y, whereX is a material constituent of Y. It means the ratio of the mass of X to the mass of Y (including X).  A chemical species denoted by X may be described by a single term such as 'nitrogen' or a phrase such as 'nox_expressed_as_nitrogen'. The chemical formula for hypobromous acid is HOBr." .

<http://purl.oclc.org/NET/ssnx/cf/cf-property#mass_fraction_of_hypochlorous_acid_in_air>
  a owl:NamedIndividual, <http://purl.oclc.org/NET/ssnx/qu/dim#Dimensionless> ;
  rdfs:label "mass fraction of hypochlorous acid in air" ;
  rdfs:isDefinedBy <http://purl.oclc.org/NET/ssnx/cf/cf-property> ;
  rdfs:comment " Mass fraction is used in the construction mass_fraction_of_X_in_Y, whereX is a material constituent of Y. It means the ratio of the mass of X to the mass of Y (including X).  A chemical species denoted by X may be described by a single term such as 'nitrogen' or a phrase such as 'nox_expressed_as_nitrogen'. The chemical formula for hypochlorous acid is HOCl." .

<http://purl.oclc.org/NET/ssnx/cf/cf-property#mass_fraction_of_inorganic_bromine_in_air>
  a owl:NamedIndividual, <http://purl.oclc.org/NET/ssnx/qu/dim#Dimensionless> ;
  rdfs:label "mass fraction of inorganic bromine in air" ;
  rdfs:isDefinedBy <http://purl.oclc.org/NET/ssnx/cf/cf-property> ;
  rdfs:comment " Mass fraction is used in the construction mass_fraction_of_X_in_Y, whereX is a material constituent of Y. It means the ratio of the mass of X to the mass of Y (including X).  A chemical species denoted by X may be described by a single term such as 'nitrogen' or a phrase such as 'nox_expressed_as_nitrogen'. Inorganic bromine, sometimes referred to as Bry, describes a family of chemical species which result from the degradation of source gases containing bromine (halons, methyl bromide, VSLS) and natural inorganic bromine sources such as volcanoes, seasalt and other aerosols. Inorganic bromine is the term used in standard names for all species belonging to the family that are represented within a given model. The list of individual species that are included in a quantity having a group chemical standard name can vary between models.  Where possible, the data variable should be accompanied by a complete description of the species represented, for example, by using a comment attribute. Standard names that use the term brox are used for quantities that contain all inorganic bromine species except HBr and BrONO2." .

<http://purl.oclc.org/NET/ssnx/cf/cf-property#mass_fraction_of_inorganic_chlorine_in_air>
  a owl:NamedIndividual, <http://purl.oclc.org/NET/ssnx/qu/dim#Dimensionless> ;
  rdfs:label "mass fraction of inorganic chlorine in air" ;
  rdfs:isDefinedBy <http://purl.oclc.org/NET/ssnx/cf/cf-property> ;
  rdfs:comment " Mass fraction is used in the construction mass_fraction_of_X_in_Y, whereX is a material constituent of Y. It means the ratio of the mass of X to the mass of Y (including X).  A chemical species denoted by X may be described by a single term such as 'nitrogen' or a phrase such as 'nox_expressed_as_nitrogen'. Inorganic chlorine, sometimes referred to as Cly, describes a family of chemical species which result from the degradation of source gases containing chlorine (CFCs, HCFCs, VSLS) and natural inorganic chlorine sources such as seasalt and other aerosols. Inorganic chlorine is the termused in standard names for all species belonging to the family that are represented withina given model. The list of individual species that are included in a quantity having a group chemical standard name can vary between models.  Where possible, the data variable should be accompanied by a complete description of the species represented, for example, by using a comment attribute. Standard names that use the term clox are used for quantities that contain all inorganic chlorine species except HCl and ClONO2." .

<http://purl.oclc.org/NET/ssnx/cf/cf-property#mass_fraction_of_isoprene_in_air>
  a owl:NamedIndividual, <http://purl.oclc.org/NET/ssnx/qu/dim#Dimensionless> ;
  rdfs:label "mass fraction of isoprene in air" ;
  rdfs:isDefinedBy <http://purl.oclc.org/NET/ssnx/cf/cf-property> ;
  rdfs:comment " Mass fraction is used in the construction mass_fraction_of_X_in_Y, whereX is a material constituent of Y. It means the ratio of the mass of X to the mass of Y (including X).  A chemical species denoted by X may be described by a single term such as 'nitrogen' or a phrase such as 'nox_expressed_as_nitrogen'. The chemical formula for isoprene is CH2=C(CH3)CH=CH2. The IUPAC name for isoprene is 2-methyl-buta-1,3-diene. Isoprene is a member of the group of hydrocarbons known as terpenes.  There are standard names for the terpene group as well as for some of the individual species." .

<http://purl.oclc.org/NET/ssnx/cf/cf-property#mass_fraction_of_limonene_in_air>
  a owl:NamedIndividual, <http://purl.oclc.org/NET/ssnx/qu/dim#Dimensionless> ;
  rdfs:label "mass fraction of limonene in air" ;
  rdfs:isDefinedBy <http://purl.oclc.org/NET/ssnx/cf/cf-property> ;
  rdfs:comment " Mass fraction is used in the construction mass_fraction_of_X_in_Y, whereX is a material constituent of Y. It means the ratio of the mass of X to the mass of Y (including X).  A chemical species denoted by X may be described by a single term such as 'nitrogen' or a phrase such as 'nox_expressed_as_nitrogen'. The chemical formula for limonene is C10H16. The IUPAC name for limonene is 1-methyl-4-prop-1-en-2-yl-cyclohexene. Limonene is a  member of the group of hydrocarbons known as terpenes.  There are standard names for theterpene group as well as for some of the individual species." .

<http://purl.oclc.org/NET/ssnx/cf/cf-property#mass_fraction_of_mercury_dry_aerosol_in_air>
  a owl:NamedIndividual, <http://purl.oclc.org/NET/ssnx/qu/dim#Dimensionless> ;
  rdfs:label "mass fraction of mercury dry aerosol in air" ;
  rdfs:isDefinedBy <http://purl.oclc.org/NET/ssnx/cf/cf-property> ;
  rdfs:comment "Mass fraction is used in the construction mass_fraction_of_X_in_Y, where X is a material constituent of Y. It means the ratio of the mass of X to the mass of Y (including X).  Aerosol means the suspended liquid or solid particles in air (except cloud droplets).  Aerosol takes up ambient water (a process known as hygroscopic growth) depending on the relative humidity and the composition of the aerosol. Dry aerosol means aerosol without water." .

<http://purl.oclc.org/NET/ssnx/cf/cf-property#mass_fraction_of_methane_in_air>
  a owl:NamedIndividual, <http://purl.oclc.org/NET/ssnx/qu/dim#Dimensionless> ;
  rdfs:label "mass fraction of methane in air" ;
  rdfs:isDefinedBy <http://purl.oclc.org/NET/ssnx/cf/cf-property> ;
  rdfs:comment " Mass fraction is used in the construction mass_fraction_of_X_in_Y, whereX is a material constituent of Y. It means the ratio of the mass of X to the mass of Y (including X).  A chemical species denoted by X may be described by a single term such as 'nitrogen' or a phrase such as 'nox_expressed_as_nitrogen'. The chemical formula for methane isCH4. Methane is a member of the group of hydrocarbons known as alkanes.  There are standard names for the alkane group as well as for some of the individual species." .

<http://purl.oclc.org/NET/ssnx/cf/cf-property#mass_fraction_of_methanol_in_air>
  a owl:NamedIndividual, <http://purl.oclc.org/NET/ssnx/qu/dim#Dimensionless> ;
  rdfs:label "mass fraction of methanol in air" ;
  rdfs:isDefinedBy <http://purl.oclc.org/NET/ssnx/cf/cf-property> ;
  rdfs:comment " Mass fraction is used in the construction mass_fraction_of_X_in_Y, whereX is a material constituent of Y. It means the ratio of the mass of X to the mass of Y (including X).  A chemical species denoted by X may be described by a single term such as 'nitrogen' or a phrase such as 'nox_expressed_as_nitrogen'. The chemical formula for ethanol isC2H5OH. The chemical formula for methanol is CH3OH." .

<http://purl.oclc.org/NET/ssnx/cf/cf-property#mass_fraction_of_methyl_bromide_in_air>
  a owl:NamedIndividual, <http://purl.oclc.org/NET/ssnx/qu/dim#Dimensionless> ;
  rdfs:label "mass fraction of methyl bromide in air" ;
  rdfs:isDefinedBy <http://purl.oclc.org/NET/ssnx/cf/cf-property> ;
  rdfs:comment " Mass fraction is used in the construction mass_fraction_of_X_in_Y, whereX is a material constituent of Y. It means the ratio of the mass of X to the mass of Y (including X).  A chemical species denoted by X may be described by a single term such as 'nitrogen' or a phrase such as 'nox_expressed_as_nitrogen'. The chemical formula for methyl bromide is CH3Br. The IUPAC name for methyl bromide is bromomethane." .

<http://purl.oclc.org/NET/ssnx/cf/cf-property#mass_fraction_of_methyl_chloride_in_air>
  a owl:NamedIndividual, <http://purl.oclc.org/NET/ssnx/qu/dim#Dimensionless> ;
  rdfs:label "mass fraction of methyl chloride in air" ;
  rdfs:isDefinedBy <http://purl.oclc.org/NET/ssnx/cf/cf-property> ;
  rdfs:comment " Mass fraction is used in the construction mass_fraction_of_X_in_Y, whereX is a material constituent of Y. It means the ratio of the mass of X to the mass of Y (including X).  A chemical species denoted by X may be described by a single term such as 'nitrogen' or a phrase such as 'nox_expressed_as_nitrogen'. The chemical formula for methyl chloride is CH3Cl. The IUPAC name for methyl chloride is chloromethane." .

<http://purl.oclc.org/NET/ssnx/cf/cf-property#mass_fraction_of_methyl_hydroperoxide_in_air>
  a owl:NamedIndividual, <http://purl.oclc.org/NET/ssnx/qu/dim#Dimensionless> ;
  rdfs:label "mass fraction of methyl hydroperoxide in air" ;
  rdfs:isDefinedBy <http://purl.oclc.org/NET/ssnx/cf/cf-property> ;
  rdfs:comment " Mass fraction is used in the construction mass_fraction_of_X_in_Y, whereX is a material constituent of Y. It means the ratio of the mass of X to the mass of Y (including X).  A chemical species denoted by X may be described by a single term such as 'nitrogen' or a phrase such as 'nox_expressed_as_nitrogen'. The chemical formula for methyl hydroperoxide is CH3OOH." .

<http://purl.oclc.org/NET/ssnx/cf/cf-property#mass_fraction_of_methyl_peroxy_radical_in_air>
  a owl:NamedIndividual, <http://purl.oclc.org/NET/ssnx/qu/dim#Dimensionless> ;
  rdfs:label "mass fraction of methyl peroxy radical in air" ;
  rdfs:isDefinedBy <http://purl.oclc.org/NET/ssnx/cf/cf-property> ;
  rdfs:comment " Mass fraction is used in the construction mass_fraction_of_X_in_Y, whereX is a material constituent of Y. It means the ratio of the mass of X to the mass of Y (including X).  A chemical species denoted by X may be described by a single term such as 'nitrogen' or a phrase such as 'nox_expressed_as_nitrogen'. The chemical formula for methyl_peroxy_radical is CH3O2. In chemistry, a 'radical' is a highly reactive, and therefore shortlived, species." .

<http://purl.oclc.org/NET/ssnx/cf/cf-property#mass_fraction_of_molecular_hydrogen_in_air>
  a owl:NamedIndividual, <http://purl.oclc.org/NET/ssnx/qu/dim#Dimensionless> ;
  rdfs:label "mass fraction of molecular hydrogen in air" ;
  rdfs:isDefinedBy <http://purl.oclc.org/NET/ssnx/cf/cf-property> ;
  rdfs:comment " Mass fraction is used in the construction mass_fraction_of_X_in_Y, whereX is a material constituent of Y. It means the ratio of the mass of X to the mass of Y (including X).  A chemical species denoted by X may be described by a single term such as 'nitrogen' or a phrase such as 'nox_expressed_as_nitrogen'. The chemical formula for molecular hydrogen is H2." .

<http://purl.oclc.org/NET/ssnx/cf/cf-property#mass_fraction_of_nitrate_dry_aerosol_in_air>
  a owl:NamedIndividual, <http://purl.oclc.org/NET/ssnx/qu/dim#Dimensionless> ;
  rdfs:label "mass fraction of nitrate dry aerosol in air" ;
  rdfs:isDefinedBy <http://purl.oclc.org/NET/ssnx/cf/cf-property> ;
  rdfs:comment "Mass fraction is used in the construction mass_fraction_of_X_in_Y, where X is a material constituent of Y. It means the ratio of the mass of X to the mass of Y (including X). Mass_fraction_of_nitrate means that the mass is expressed as mass of NO3.  Aerosol means the suspended liquid or solid particles in air (except cloud droplets).  Aerosol takes up ambient water (a process known as hygroscopic growth) depending on the relative humidity and the composition of the aerosol. Dry aerosol means aerosol without water." .

<http://purl.oclc.org/NET/ssnx/cf/cf-property#mass_fraction_of_nitrate_radical_in_air>
  a owl:NamedIndividual, <http://purl.oclc.org/NET/ssnx/qu/dim#Dimensionless> ;
  rdfs:label "mass fraction of nitrate radical in air" ;
  rdfs:isDefinedBy <http://purl.oclc.org/NET/ssnx/cf/cf-property> ;
  rdfs:comment " Mass fraction is used in the construction mass_fraction_of_X_in_Y, whereX is a material constituent of Y. It means the ratio of the mass of X to the mass of Y (including X).  A chemical species denoted by X may be described by a single term such as 'nitrogen' or a phrase such as 'nox_expressed_as_nitrogen'. In chemistry, a 'radical' is a highly reactive, and therefore shortlived, species." .

<http://purl.oclc.org/NET/ssnx/cf/cf-property#mass_fraction_of_nitric_acid_in_air>
  a owl:NamedIndividual, <http://purl.oclc.org/NET/ssnx/qu/dim#Dimensionless> ;
  rdfs:label "mass fraction of nitric acid in air" ;
  rdfs:isDefinedBy <http://purl.oclc.org/NET/ssnx/cf/cf-property> ;
  rdfs:comment " Mass fraction is used in the construction mass_fraction_of_X_in_Y, whereX is a material constituent of Y. It means the ratio of the mass of X to the mass of Y (including X).  A chemical species denoted by X may be described by a single term such as 'nitrogen' or a phrase such as 'nox_expressed_as_nitrogen'. The chemical formula for nitric acid is HNO3." .

<http://purl.oclc.org/NET/ssnx/cf/cf-property#mass_fraction_of_nitric_acid_trihydrate_ambient_aerosol_in_air>
  a owl:NamedIndividual, <http://purl.oclc.org/NET/ssnx/qu/dim#Dimensionless> ;
  rdfs:label "mass fraction of nitric acid trihydrate ambient aerosol in air" ;
  rdfs:isDefinedBy <http://purl.oclc.org/NET/ssnx/cf/cf-property> ;
  rdfs:comment " Mass fraction is used in the construction mass_fraction_of_X_in_Y, whereX is a material constituent of Y. It means the ratio of the mass of X to the mass of Y (including X).  A chemical species denoted by X may be described by a single term such as 'nitrogen' or a phrase such as 'nox_expressed_as_nitrogen'. Aerosol means the suspended liquid or solid particles in air (except cloud droplets).  Ambient aerosolis aerosol that has taken up ambient water through hygroscopic growth. The extent of hygroscopic growth depends on the relative humidity and the composition of the aerosol. The chemical formula for nitric acid is HNO3. Nitric acid trihydrate, sometimes referred to as NAT,is a stable crystalline substance consisting of three molecules of water to one molecule of nitric acid." .

<http://purl.oclc.org/NET/ssnx/cf/cf-property#mass_fraction_of_nitrogen_dioxide_in_air>
  a owl:NamedIndividual, <http://purl.oclc.org/NET/ssnx/qu/dim#Dimensionless> ;
  rdfs:label "mass fraction of nitrogen dioxide in air" ;
  rdfs:isDefinedBy <http://purl.oclc.org/NET/ssnx/cf/cf-property> ;
  rdfs:comment " Mass fraction is used in the construction mass_fraction_of_X_in_Y, whereX is a material constituent of Y. It means the ratio of the mass of X to the mass of Y (including X).  A chemical species denoted by X may be described by a single term such as 'nitrogen' or a phrase such as 'nox_expressed_as_nitrogen'. The chemical formula for nitrogen dioxide is NO2." .

<http://purl.oclc.org/NET/ssnx/cf/cf-property#mass_fraction_of_nitrogen_monoxide_in_air>
  a owl:NamedIndividual, <http://purl.oclc.org/NET/ssnx/qu/dim#Dimensionless> ;
  rdfs:label "mass fraction of nitrogen monoxide in air" ;
  rdfs:isDefinedBy <http://purl.oclc.org/NET/ssnx/cf/cf-property> ;
  rdfs:comment " Mass fraction is used in the construction mass_fraction_of_X_in_Y, whereX is a material constituent of Y. It means the ratio of the mass of X to the mass of Y (including X).  A chemical species denoted by X may be described by a single term such as 'nitrogen' or a phrase such as 'nox_expressed_as_nitrogen'. The chemical formula for nitrogen monoxide is NO." .

<http://purl.oclc.org/NET/ssnx/cf/cf-property#mass_fraction_of_nitrous_acid_in_air>
  a owl:NamedIndividual, <http://purl.oclc.org/NET/ssnx/qu/dim#Dimensionless> ;
  rdfs:label "mass fraction of nitrous acid in air" ;
  rdfs:isDefinedBy <http://purl.oclc.org/NET/ssnx/cf/cf-property> ;
  rdfs:comment " Mass fraction is used in the construction mass_fraction_of_X_in_Y, whereX is a material constituent of Y. It means the ratio of the mass of X to the mass of Y (including X).  A chemical species denoted by X may be described by a single term such as 'nitrogen' or a phrase such as 'nox_expressed_as_nitrogen'. The chemical formula for nitrous acid is HNO2." .

<http://purl.oclc.org/NET/ssnx/cf/cf-property#mass_fraction_of_nitrous_oxide_in_air>
  a owl:NamedIndividual, <http://purl.oclc.org/NET/ssnx/qu/dim#Dimensionless> ;
  rdfs:label "mass fraction of nitrous oxide in air" ;
  rdfs:isDefinedBy <http://purl.oclc.org/NET/ssnx/cf/cf-property> ;
  rdfs:comment " Mass fraction is used in the construction mass_fraction_of_X_in_Y, whereX is a material constituent of Y. It means the ratio of the mass of X to the mass of Y (including X).  A chemical species denoted by X may be described by a single term such as 'nitrogen' or a phrase such as 'nox_expressed_as_nitrogen'. The chemical formula for nitrous oxide is N2O." .

<http://purl.oclc.org/NET/ssnx/cf/cf-property#mass_fraction_of_nmvoc_expressed_as_carbon_in_air>
  a owl:NamedIndividual, <http://purl.oclc.org/NET/ssnx/qu/dim#Dimensionless> ;
  rdfs:label "mass fraction of nmvoc expressed as carbon in air" ;
  rdfs:isDefinedBy <http://purl.oclc.org/NET/ssnx/cf/cf-property> ;
  rdfs:comment " Mass fraction is used in the construction mass_fraction_of_X_in_Y, whereX is a material constituent of Y. It means the ratio of the mass of X to the mass of Y (including X).  A chemical species denoted by X may be described by a single term such as 'nitrogen' or a phrase such as 'nox_expressed_as_nitrogen'. nmvoc means non methanevolatile organic compounds. The phrase 'expressed_as' is used in the construction A_expressed_as_B, where B is a chemical constituent of A. It means that the quantity indicated by the standard name is calculated solely with respect to the B contained in A, neglecting all other chemical constituents of A." .

<http://purl.oclc.org/NET/ssnx/cf/cf-property#mass_fraction_of_nox_expressed_as_nitrogen_in_air>
  a owl:NamedIndividual, <http://purl.oclc.org/NET/ssnx/qu/dim#Dimensionless> ;
  rdfs:label "mass fraction of nox expressed as nitrogen in air" ;
  rdfs:isDefinedBy <http://purl.oclc.org/NET/ssnx/cf/cf-property> ;
  rdfs:comment " Mass fraction is used in the construction mass_fraction_of_X_in_Y, whereX is a material constituent of Y. It means the ratio of the mass of X to the mass of Y (including X).  A chemical species denoted by X may be described by a single term such as 'nitrogen' or a phrase such as 'nox_expressed_as_nitrogen'. Nox means a combinationof two radical species containing nitrogen and oxygen: NO+NO2. The phrase 'expressed_as' is used in the construction A_expressed_as_B, where B is a chemical constituent of A. It means that the quantity indicated by the standard name is calculated solely with respect to the B contained in A, neglecting all other chemical constituents of A." .

<http://purl.oclc.org/NET/ssnx/cf/cf-property#mass_fraction_of_noy_expressed_as_nitrogen_in_air>
  a owl:NamedIndividual, <http://purl.oclc.org/NET/ssnx/qu/dim#Dimensionless> ;
  rdfs:label "mass fraction of noy expressed as nitrogen in air" ;
  rdfs:isDefinedBy <http://purl.oclc.org/NET/ssnx/cf/cf-property> ;
  rdfs:comment " Mass fraction is used in the construction mass_fraction_of_X_in_Y, whereX is a material constituent of Y. It means the ratio of the mass of X to the mass of Y (including X).  A chemical species denoted by X may be described by a single term such as 'nitrogen' or a phrase such as 'nox_expressed_as_nitrogen'. Noy describes a family of chemical species. The family usually includes atomic nitrogen (N), nitrogen monoxide (NO), nitrogen dioxide (NO2), dinitrogen pentoxide (N2O5), nitric acid (HNO3), peroxynitric acid (HNO4), bromine nitrate (BrONO2) , chlorine nitrate (ClONO2) and organic nitrates (most notably peroxyacetyl nitrate, sometimes referred to as PAN, (CH3COO2NO2)). The list of individual species that are included in a quantity having a group chemical standard name can vary between models.  Where possible, the data variable should be accompanied by a complete description of the species represented, for example, by using a comment attribute. The phrase 'expressed_as' is used in the construction A_expressed_as_B, where B is a chemical constituent of A. It means that the quantity indicated by the standard name is calculated solely with respect to the B contained in A, neglecting all other chemical constituents of A." .

<http://purl.oclc.org/NET/ssnx/cf/cf-property#mass_fraction_of_oxygenated_hydrocarbons_in_air>
  a owl:NamedIndividual, <http://purl.oclc.org/NET/ssnx/qu/dim#Dimensionless> ;
  rdfs:label "mass fraction of oxygenated hydrocarbons in air" ;
  rdfs:isDefinedBy <http://purl.oclc.org/NET/ssnx/cf/cf-property> ;
  rdfs:comment " Mass fraction is used in the construction mass_fraction_of_X_in_Y, whereX is a material constituent of Y. It means the ratio of the mass of X to the mass of Y (including X).  A chemical species denoted by X may be described by a single term such as 'nitrogen' or a phrase such as 'nox_expressed_as_nitrogen'.  Oxygenated means containing oxygen. Hydrocarbon means a compound containing hydrogen and carbon." .

<http://purl.oclc.org/NET/ssnx/cf/cf-property#mass_fraction_of_ozone_in_air>
  a owl:NamedIndividual, <http://purl.oclc.org/NET/ssnx/qu/dim#Dimensionless> ;
  rdfs:label "mass fraction of ozone in air" ;
  rdfs:isDefinedBy <http://purl.oclc.org/NET/ssnx/cf/cf-property> ;
  rdfs:comment "Mass fraction is used in the construction mass_fraction_of_X_in_Y, where X is a material constituent of Y. It means the ratio of the mass of X to the mass of Y (including X)." .

<http://purl.oclc.org/NET/ssnx/cf/cf-property#mass_fraction_of_particulate_organic_matter_dry_aerosol_in_air>
  a owl:NamedIndividual, <http://purl.oclc.org/NET/ssnx/qu/dim#Dimensionless> ;
  rdfs:label "mass fraction of particulate organic matter dry aerosol in air" ;
  rdfs:isDefinedBy <http://purl.oclc.org/NET/ssnx/cf/cf-property> ;
  rdfs:comment "Mass fraction is used in the construction mass_fraction_of_X_in_Y, where X is a material constituent of Y. It means the ratio of the mass of X to the mass of Y (including X).  Aerosol means the suspended liquid or solid particles in air (except cloud droplets).  Aerosol takes up ambient water (a process known as hygroscopic growth) depending on the relative humidity and the composition of the aerosol. Dry aerosol means aerosol without water.  particulate_organic_matter_dry_aerosol means all particulate organic matter dry aerosol except black carbon.  It is the sum of primary_particulate_organic_matter_dry_aerosol and secondary_particulate_organic_matter_dry_aerosol." .

<http://purl.oclc.org/NET/ssnx/cf/cf-property#mass_fraction_of_peroxy_radicals_in_air>
  a owl:NamedIndividual, <http://purl.oclc.org/NET/ssnx/qu/dim#Dimensionless> ;
  rdfs:label "mass fraction of peroxy radicals in air" ;
  rdfs:isDefinedBy <http://purl.oclc.org/NET/ssnx/cf/cf-property> ;
  rdfs:comment " Mass fraction is used in the construction mass_fraction_of_X_in_Y, whereX is a material constituent of Y. It means the ratio of the mass of X to the mass of Y (including X).  A chemical species denoted by X may be described by a single term such as 'nitrogen' or a phrase such as 'nox_expressed_as_nitrogen'. The term peroxy_radicals means all organic and inorganic peroxy radicals. This includes HO2 and all organic peroxyradicals, sometimes referred to as RO2. In chemistry, a 'radical' is a highly reactive, and therefore shortlived, species." .

<http://purl.oclc.org/NET/ssnx/cf/cf-property#mass_fraction_of_peroxyacetyl_nitrate_in_air>
  a owl:NamedIndividual, <http://purl.oclc.org/NET/ssnx/qu/dim#Dimensionless> ;
  rdfs:label "mass fraction of peroxyacetyl nitrate in air" ;
  rdfs:isDefinedBy <http://purl.oclc.org/NET/ssnx/cf/cf-property> ;
  rdfs:comment " Mass fraction is used in the construction mass_fraction_of_X_in_Y, whereX is a material constituent of Y. It means the ratio of the mass of X to the mass of Y (including X).  A chemical species denoted by X may be described by a single term such as 'nitrogen' or a phrase such as 'nox_expressed_as_nitrogen'. The chemical formula for peroxyacetyl nitrate, sometimes referred to as PAN, is CH3COO2NO2.  The IUPAC name for peroxyacetyl_nitrate is nitroethaneperoxoate." .

<http://purl.oclc.org/NET/ssnx/cf/cf-property#mass_fraction_of_peroxynitric_acid_in_air>
  a owl:NamedIndividual, <http://purl.oclc.org/NET/ssnx/qu/dim#Dimensionless> ;
  rdfs:label "mass fraction of peroxynitric acid in air" ;
  rdfs:isDefinedBy <http://purl.oclc.org/NET/ssnx/cf/cf-property> ;
  rdfs:comment " Mass fraction is used in the construction mass_fraction_of_X_in_Y, whereX is a material constituent of Y. It means the ratio of the mass of X to the mass of Y (including X).  A chemical species denoted by X may be described by a single term such as 'nitrogen' or a phrase such as 'nox_expressed_as_nitrogen'. The chemical formula for peroxynitric acid, sometimes referred to as PNA, is HO2NO2." .

<http://purl.oclc.org/NET/ssnx/cf/cf-property#mass_fraction_of_pm10_ambient_aerosol_in_air>
  a owl:NamedIndividual, <http://purl.oclc.org/NET/ssnx/qu/dim#Dimensionless> ;
  rdfs:label "mass fraction of pm10 ambient aerosol in air" ;
  rdfs:isDefinedBy <http://purl.oclc.org/NET/ssnx/cf/cf-property> ;
  rdfs:comment "Mass fraction is used in the construction mass_fraction_of_X_in_Y, where X is a material constituent of Y. It means the ratio of the mass of X to the mass of Y (including X).  A chemical species denoted by X may be described by a single term such as 'nitrogen' or a phrase such as 'nox_expressed_as_nitrogen'. Aerosol means the suspended liquid or solid particles in air (except cloud droplets).  Ambient aerosol is aerosol that has taken up ambient water through hygroscopic growth. The extent of hygroscopic growth depends on the relative humidity and the composition of the aerosol. Pm10 aerosol is an air pollutant with an aerodynamic diameter of less than or equal to 10 micrometers. To specify the relative humidity and temperature at which the particle size applies, provide scalar coordinate variables with the standard names of, respectively, relative_humidity and air_temperature." .

<http://purl.oclc.org/NET/ssnx/cf/cf-property#mass_fraction_of_pm1_ambient_aerosol_in_air>
  a owl:NamedIndividual, <http://purl.oclc.org/NET/ssnx/qu/dim#Dimensionless> ;
  rdfs:label "mass fraction of pm1 ambient aerosol in air" ;
  rdfs:isDefinedBy <http://purl.oclc.org/NET/ssnx/cf/cf-property> ;
  rdfs:comment "Mass fraction is used in the construction mass_fraction_of_X_in_Y, where X is a material constituent of Y. It means the ratio of the mass of X to the mass of Y (including X).  A chemical species denoted by X may be described by a single term such as 'nitrogen' or a phrase such as 'nox_expressed_as_nitrogen'. Aerosol means the suspended liquidor solid particles in air (except cloud droplets).  Ambient aerosol is aerosol that has taken up ambient water through hygroscopic growth. The extent of hygroscopic growth dependson the relative humidity and the composition of the aerosol. Pm1 aerosol is an air pollutant with an aerodynamic diameter of less than or equal to 1 micrometer. To specify the relative humidity and temperature at which the particle size applies, provide scalar coordinate variables with the standard names of, respectively, relative_humidity and air_temperature." .

<http://purl.oclc.org/NET/ssnx/cf/cf-property#mass_fraction_of_pm2p5_ambient_aerosol_in_air>
  a owl:NamedIndividual, <http://purl.oclc.org/NET/ssnx/qu/dim#Dimensionless> ;
  rdfs:label "mass fraction of pm2p5 ambient aerosol in air" ;
  rdfs:isDefinedBy <http://purl.oclc.org/NET/ssnx/cf/cf-property> ;
  rdfs:comment "Mass fraction is used in the construction mass_fraction_of_X_in_Y, where X is a material constituent of Y. It means the ratio of the mass of X to the mass of Y (including X).  A chemical species denoted by X may be described by a single term such as 'nitrogen' or a phrase such as 'nox_expressed_as_nitrogen'. Aerosol means the suspended liquid or solid particles in air (except cloud droplets).  Ambient aerosol is aerosol that has taken up ambient water through hygroscopic growth. The extent of hygroscopic growth depends on the relative humidity and the composition of the aerosol. Pm2p5 aerosol is an air pollutant with an aerodynamic diameter of less than or equal to 2.5 micrometers. To specify the relative humidity and temperature at which the particle size applies, provide scalar coordinate variables with the standard names of, respectively, relative_humidity and air_temperature." .

<http://purl.oclc.org/NET/ssnx/cf/cf-property#mass_fraction_of_precipitation_in_air>
  a owl:NamedIndividual, <http://purl.oclc.org/NET/ssnx/qu/dim#Dimensionless> ;
  rdfs:label "mass fraction of precipitation in air" ;
  rdfs:isDefinedBy <http://purl.oclc.org/NET/ssnx/cf/cf-property> ;
  rdfs:comment "Mass fraction is used in the construction mass_fraction_of_X_in_Y, where X is a material constituent of Y. It means the ratio of the mass of X to the mass of Y (including X)." .

<http://purl.oclc.org/NET/ssnx/cf/cf-property#mass_fraction_of_primary_particulate_organic_matter_dry_aerosol_in_air>
  a owl:NamedIndividual, <http://purl.oclc.org/NET/ssnx/qu/dim#Dimensionless> ;
  rdfs:label "mass fraction of primary particulate organic matter dry aerosol in air" ;
  rdfs:isDefinedBy <http://purl.oclc.org/NET/ssnx/cf/cf-property> ;
  rdfs:comment "Mass fraction is used in the construction mass_fraction_of_X_in_Y, where X is a material constituent of Y. It means the ratio of the mass of X to the mass of Y (including X).  Aerosol means the suspended liquid or solid particles in air (except cloud droplets).  Aerosol takes up ambient water (a process known as hygroscopic growth) depending on the relative humidity and the composition of the aerosol. Dry aerosol means aerosol without water.  Primary particulate organic matter  means all organic matter emitted directly to the atmosphere as particles except black carbon.  The sum of primary_particulate_organic_matter_dry_aerosol and secondary_particulate_organic_matter_dry_aerosol is particulate_organic_matter_dry_aerosol." .

<http://purl.oclc.org/NET/ssnx/cf/cf-property#mass_fraction_of_propane_in_air>
  a owl:NamedIndividual, <http://purl.oclc.org/NET/ssnx/qu/dim#Dimensionless> ;
  rdfs:label "mass fraction of propane in air" ;
  rdfs:isDefinedBy <http://purl.oclc.org/NET/ssnx/cf/cf-property> ;
  rdfs:comment " Mass fraction is used in the construction mass_fraction_of_X_in_Y, whereX is a material constituent of Y. It means the ratio of the mass of X to the mass of Y (including X).  A chemical species denoted by X may be described by a single term such as 'nitrogen' or a phrase such as 'nox_expressed_as_nitrogen'. The chemical formula for propane isC3H8. Propane is a member of the group of hydrocarbons known as alkanes.  There are standard names for the alkane group as well as for some of the individual species." .

<http://purl.oclc.org/NET/ssnx/cf/cf-property#mass_fraction_of_propene_in_air>
  a owl:NamedIndividual, <http://purl.oclc.org/NET/ssnx/qu/dim#Dimensionless> ;
  rdfs:label "mass fraction of propene in air" ;
  rdfs:isDefinedBy <http://purl.oclc.org/NET/ssnx/cf/cf-property> ;
  rdfs:comment " Mass fraction is used in the construction mass_fraction_of_X_in_Y, whereX is a material constituent of Y. It means the ratio of the mass of X to the mass of Y (including X).  A chemical species denoted by X may be described by a single term such as 'nitrogen' or a phrase such as 'nox_expressed_as_nitrogen'. The chemical formula for propene isC3H6. Propene is a member of the group of hydrocarbons known as alkenes.  There are standard names for the alkene group as well as for some of the individual species." .

<http://purl.oclc.org/NET/ssnx/cf/cf-property#mass_fraction_of_radon_in_air>
  a owl:NamedIndividual, <http://purl.oclc.org/NET/ssnx/qu/dim#Dimensionless> ;
  rdfs:label "mass fraction of radon in air" ;
  rdfs:isDefinedBy <http://purl.oclc.org/NET/ssnx/cf/cf-property> ;
  rdfs:comment " Mass fraction is used in the construction mass_fraction_of_X_in_Y, whereX is a material constituent of Y. It means the ratio of the mass of X to the mass of Y (including X).  A chemical species denoted by X may be described by a single term such as 'nitrogen' or a phrase such as 'nox_expressed_as_nitrogen'. The chemical symbol for radon is Rn." .

<http://purl.oclc.org/NET/ssnx/cf/cf-property#mass_fraction_of_rain_in_air>
  a owl:NamedIndividual, <http://purl.oclc.org/NET/ssnx/qu/dim#Dimensionless> ;
  rdfs:label "mass fraction of rain in air" ;
  rdfs:isDefinedBy <http://purl.oclc.org/NET/ssnx/cf/cf-property> ;
  rdfs:comment "Mass fraction is used in the construction mass_fraction_of_X_in_Y, where X is a material constituent of Y. It means the ratio of the mass of X to the mass of Y (including X)." .

<http://purl.oclc.org/NET/ssnx/cf/cf-property#mass_fraction_of_seasalt_dry_aerosol_in_air>
  a owl:NamedIndividual, <http://purl.oclc.org/NET/ssnx/qu/dim#Dimensionless> ;
  rdfs:label "mass fraction of seasalt dry aerosol in air" ;
  rdfs:isDefinedBy <http://purl.oclc.org/NET/ssnx/cf/cf-property> ;
  rdfs:comment "Mass fraction is used in the construction mass_fraction_of_X_in_Y, where X is a material constituent of Y. It means the ratio of the mass of X to the mass of Y (including X).  Aerosol means the suspended liquid or solid particles in air (except cloud droplets).  Aerosol takes up ambient water (a process known as hygroscopic growth) depending on the relative humidity and the composition of the aerosol. Dry aerosol means aerosol without water." .

<http://purl.oclc.org/NET/ssnx/cf/cf-property#mass_fraction_of_secondary_particulate_organic_matter_dry_aerosol_in_air>
  a owl:NamedIndividual, <http://purl.oclc.org/NET/ssnx/qu/dim#Dimensionless> ;
  rdfs:label "mass fraction of secondary particulate organic matter dry aerosol in air" ;
  rdfs:isDefinedBy <http://purl.oclc.org/NET/ssnx/cf/cf-property> ;
  rdfs:comment "Mass fraction is used in the construction mass_fraction_of_X_in_Y, where X is a material constituent of Y. It means the ratio of the mass of X to the mass of Y (including X).  Aerosol means the suspended liquid or solid particles in air (except cloud droplets).  Aerosol takes up ambient water (a process known as hygroscopic growth) depending on the relative humidity and the composition of the aerosol. Dry aerosol means aerosol without water.  Secondary particulate organic matter  means particulate organic matter formed within the atmosphere from gaseous precursors.  The sum of primary_particulate_organic_matter_dry_aerosol and secondary_particulate_organic_matter_dry_aerosol is particulate_organic_matter_dry_aerosol." .

<http://purl.oclc.org/NET/ssnx/cf/cf-property#mass_fraction_of_snow_in_air>
  a owl:NamedIndividual, <http://purl.oclc.org/NET/ssnx/qu/dim#Dimensionless> ;
  rdfs:label "mass fraction of snow in air" ;
  rdfs:isDefinedBy <http://purl.oclc.org/NET/ssnx/cf/cf-property> ;
  rdfs:comment "Mass fraction is used in the construction mass_fraction_of_X_in_Y, where X is a material constituent of Y. It means the ratio of the mass of X to the mass of Y (including X)." .

<http://purl.oclc.org/NET/ssnx/cf/cf-property#mass_fraction_of_stratiform_cloud_ice_in_air>
  a owl:NamedIndividual, <http://purl.oclc.org/NET/ssnx/qu/dim#Dimensionless> ;
  rdfs:label "mass fraction of stratiform cloud ice in air" ;
  rdfs:isDefinedBy <http://purl.oclc.org/NET/ssnx/cf/cf-property> ;
  rdfs:comment "Mass fraction is used in the construction mass_fraction_of_X_in_Y, where X is a material constituent of Y. It means the ratio of the mass of X to the mass of Y (including X). In an atmosphere model, stratiform cloud is that produced by large-scale convergence (not the convection schemes)." .

<http://purl.oclc.org/NET/ssnx/cf/cf-property#mass_fraction_of_stratiform_cloud_liquid_water_in_air>
  a owl:NamedIndividual, <http://purl.oclc.org/NET/ssnx/qu/dim#Dimensionless> ;
  rdfs:label "mass fraction of stratiform cloud liquid water in air" ;
  rdfs:isDefinedBy <http://purl.oclc.org/NET/ssnx/cf/cf-property> ;
  rdfs:comment "Mass fraction is used in the construction mass_fraction_of_X_in_Y, where X is a material constituent of Y. It means the ratio of the mass of X to the mass of Y (including X). In an atmosphere model, stratiform cloud is that produced by large-scale convergence (not the convection schemes)." .

<http://purl.oclc.org/NET/ssnx/cf/cf-property#mass_fraction_of_sulfate_dry_aerosol_in_air>
  a owl:NamedIndividual, <http://purl.oclc.org/NET/ssnx/qu/dim#Dimensionless> ;
  rdfs:label "mass fraction of sulfate dry aerosol in air" ;
  rdfs:isDefinedBy <http://purl.oclc.org/NET/ssnx/cf/cf-property> ;
  rdfs:comment "Mass fraction is used in the construction mass_fraction_of_X_in_Y, where X is a material constituent of Y. It means the ratio of the mass of X to the mass of Y (including X).  Mass_fraction_of_sulfate means that the mass is expressed as mass of SO4.  Aerosol means the suspended liquid or solid particles in air (except cloud droplets).  Aerosol takes up ambient water (a process known as hygroscopic growth) depending on the relative humidity and the composition of the aerosol. Dry aerosol means aerosol without water." .

<http://purl.oclc.org/NET/ssnx/cf/cf-property#mass_fraction_of_sulfur_dioxide_in_air>
  a owl:NamedIndividual, <http://purl.oclc.org/NET/ssnx/qu/dim#Dimensionless> ;
  rdfs:label "mass fraction of sulfur dioxide in air" ;
  rdfs:isDefinedBy <http://purl.oclc.org/NET/ssnx/cf/cf-property> ;
  rdfs:comment "Mass fraction is used in the construction mass_fraction_of_X_in_Y, where X is a material constituent of Y. It means the ratio of the mass of X to the mass of Y (including X)." .

<http://purl.oclc.org/NET/ssnx/cf/cf-property#mass_fraction_of_sulfuric_acid_in_air>
  a owl:NamedIndividual, <http://purl.oclc.org/NET/ssnx/qu/dim#Dimensionless> ;
  rdfs:label "mass fraction of sulfuric acid in air" ;
  rdfs:isDefinedBy <http://purl.oclc.org/NET/ssnx/cf/cf-property> ;
  rdfs:comment " Mass fraction is used in the construction mass_fraction_of_X_in_Y, whereX is a material constituent of Y. It means the ratio of the mass of X to the mass of Y (including X).  A chemical species denoted by X may be described by a single term such as 'nitrogen' or a phrase such as 'nox_expressed_as_nitrogen'." .

<http://purl.oclc.org/NET/ssnx/cf/cf-property#mass_fraction_of_terpenes_in_air>
  a owl:NamedIndividual, <http://purl.oclc.org/NET/ssnx/qu/dim#Dimensionless> ;
  rdfs:label "mass fraction of terpenes in air" ;
  rdfs:isDefinedBy <http://purl.oclc.org/NET/ssnx/cf/cf-property> ;
  rdfs:comment " Mass fraction is used in the construction mass_fraction_of_X_in_Y, whereX is a material constituent of Y. It means the ratio of the mass of X to the mass of Y (including X).  A chemical species denoted by X may be described by a single term such as 'nitrogen' or a phrase such as 'nox_expressed_as_nitrogen'. Terpenes are hydrocarbons, that is,they contain only hydrogen and carbon combined in the general proportions (C5H8)n where n is an integer greater than on equal to one. The term terpenes is used in standard names to describe the group of chemical species having this common structure that are represented within a given model. The list of individual species that are included in a quantity having a group chemical standard name can vary between models.  Where possible, the data variable should be accompanied by a complete description of the species represented, for example, by using a comment attribute.  Standard names exist for some individual terpene species, e.g., isoprene and limonene." .

<http://purl.oclc.org/NET/ssnx/cf/cf-property#mass_fraction_of_toluene_in_air>
  a owl:NamedIndividual, <http://purl.oclc.org/NET/ssnx/qu/dim#Dimensionless> ;
  rdfs:label "mass fraction of toluene in air" ;
  rdfs:isDefinedBy <http://purl.oclc.org/NET/ssnx/cf/cf-property> ;
  rdfs:comment " Mass fraction is used in the construction mass_fraction_of_X_in_Y, whereX is a material constituent of Y. It means the ratio of the mass of X to the mass of Y (including X).  A chemical species denoted by X may be described by a single term such as 'nitrogen' or a phrase such as 'nox_expressed_as_nitrogen'. The chemical formula for toluene isC6H5CH3.  Toluene has the same structure as benzene, except that one of the hydrogen atomsis replaced by a methyl group.  The systematic name for toluene is methylbenzene." .

<http://purl.oclc.org/NET/ssnx/cf/cf-property#mass_fraction_of_water_in_air>
  a owl:NamedIndividual, <http://purl.oclc.org/NET/ssnx/qu/dim#Dimensionless> ;
  rdfs:label "mass fraction of water in air" ;
  rdfs:isDefinedBy <http://purl.oclc.org/NET/ssnx/cf/cf-property> ;
  rdfs:comment "Water means water in all phases. Mass fraction is used in the construction mass_fraction_of_X_in_Y, where X is a material constituent of Y. It means the ratio of the mass of X to the mass of Y (including X)." .

<http://purl.oclc.org/NET/ssnx/cf/cf-property#mass_fraction_of_water_in_ambient_aerosol_in_air>
  a owl:NamedIndividual, <http://purl.oclc.org/NET/ssnx/qu/dim#Dimensionless> ;
  rdfs:label "mass fraction of water in ambient aerosol in air" ;
  rdfs:isDefinedBy <http://purl.oclc.org/NET/ssnx/cf/cf-property> ;
  rdfs:comment "Mass fraction is used in the construction mass_fraction_of_X_in_Y, where X is a material constituent of Y. It means the ratio of the mass of X to the mass of Y (including X).  Aerosol means the suspended liquid or solid particles in air (except cloud droplets).  Aerosol takes up ambient water (a process known as hygroscopic growth) depending on the relative humidity and the composition of the aerosol." .

<http://purl.oclc.org/NET/ssnx/cf/cf-property#mass_fraction_of_xylene_in_air>
  a owl:NamedIndividual, <http://purl.oclc.org/NET/ssnx/qu/dim#Dimensionless> ;
  rdfs:label "mass fraction of xylene in air" ;
  rdfs:isDefinedBy <http://purl.oclc.org/NET/ssnx/cf/cf-property> ;
  rdfs:comment " Mass fraction is used in the construction mass_fraction_of_X_in_Y, whereX is a material constituent of Y. It means the ratio of the mass of X to the mass of Y (including X).  A chemical species denoted by X may be described by a single term such as 'nitrogen' or a phrase such as 'nox_expressed_as_nitrogen'. The chemical formula for xylene is C6H4C2H6. In chemistry, xylene is a generic term for a group of three isomers of dimethylbenzene. The IUPAC names for the isomers are 1,2-dimethylbenzene, 1,3-dimethylbenzene and 1,4-dimethylbenzene. Xylene is an aromatic hydrocarbon. There are standard names that refer toaromatic_compounds as a group, as well as those for individual species." .

<http://purl.oclc.org/NET/ssnx/cf/cf-property#mole_concentration_of_acetic_acid_in_air>
  a owl:NamedIndividual, <http://purl.oclc.org/NET/ssnx/qu/dim#Concentration> ;
  rdfs:label "mole concentration of acetic acid in air" ;
  rdfs:isDefinedBy <http://purl.oclc.org/NET/ssnx/cf/cf-property> ;
  rdfs:comment " Mole concentration means number of moles per unit volume, also called molarity, and is used in the construction mole_concentration_of_X_in_Y, where X is a material constituent of Y.  A chemical species denoted by X may be described by a single term such as 'nitrogen' or a phrase such as 'nox_expressed_as_nitrogen'. The chemical formula for acetic_acid is CH3COOH. The IUPAC name for acetic acid is ethanoic acid." .

<http://purl.oclc.org/NET/ssnx/cf/cf-property#mole_concentration_of_aceto_nitrile_in_air>
  a owl:NamedIndividual, <http://purl.oclc.org/NET/ssnx/qu/dim#Concentration> ;
  rdfs:label "mole concentration of aceto nitrile in air" ;
  rdfs:isDefinedBy <http://purl.oclc.org/NET/ssnx/cf/cf-property> ;
  rdfs:comment " Mole concentration means number of moles per unit volume, also called molarity, and is used in the construction mole_concentration_of_X_in_Y, where X is a material constituent of Y.  A chemical species denoted by X may be described by a single term such as 'nitrogen' or a phrase such as 'nox_expressed_as_nitrogen'. The chemical formula for aceto-nitrile is CH3CN. The IUPAC name for aceto-nitrile is ethanenitrile." .

<http://purl.oclc.org/NET/ssnx/cf/cf-property#mole_concentration_of_alpha_hexachlorocyclohexane_in_air>
  a owl:NamedIndividual, <http://purl.oclc.org/NET/ssnx/qu/dim#Concentration> ;
  rdfs:label "mole concentration of alpha hexachlorocyclohexane in air" ;
  rdfs:isDefinedBy <http://purl.oclc.org/NET/ssnx/cf/cf-property> ;
  rdfs:comment " Mole concentration means number of moles per unit volume, also called molarity, and is used in the construction mole_concentration_of_X_in_Y, where X is a material constituent of Y.  A chemical species denoted by X may be described by a single term such as 'nitrogen' or a phrase such as 'nox_expressed_as_nitrogen'. The chemical formula for alpha_hexachlorocyclohexane is C6H6Cl6." .

<http://purl.oclc.org/NET/ssnx/cf/cf-property#mole_concentration_of_alpha_pinene_in_air>
  a owl:NamedIndividual, <http://purl.oclc.org/NET/ssnx/qu/dim#Concentration> ;
  rdfs:label "mole concentration of alpha pinene in air" ;
  rdfs:isDefinedBy <http://purl.oclc.org/NET/ssnx/cf/cf-property> ;
  rdfs:comment " Mole concentration means number of moles per unit volume, also called molarity, and is used in the construction mole_concentration_of_X_in_Y, where X is a material constituent of Y.  A chemical species denoted by X may be described by a single term such as 'nitrogen' or a phrase such as 'nox_expressed_as_nitrogen'. The chemical formula for alpha_pinene is C10H16. The IUPAC name for alpha-pinene is (1S,5S)-2,6,6-trimethylbicyclo[3.1.1]hept-2-ene." .

<http://purl.oclc.org/NET/ssnx/cf/cf-property#mole_concentration_of_ammonia_in_air>
  a owl:NamedIndividual, <http://purl.oclc.org/NET/ssnx/qu/dim#Concentration> ;
  rdfs:label "mole concentration of ammonia in air" ;
  rdfs:isDefinedBy <http://purl.oclc.org/NET/ssnx/cf/cf-property> ;
  rdfs:comment " Mole concentration means number of moles per unit volume, also called molarity, and is used in the construction mole_concentration_of_X_in_Y, where X is a material constituent of Y.  A chemical species denoted by X may be described by a single term such as 'nitrogen' or a phrase such as 'nox_expressed_as_nitrogen'. The chemical formula for ammonia is NH3." .

<http://purl.oclc.org/NET/ssnx/cf/cf-property#mole_concentration_of_anthropogenic_nmvoc_expressed_as_carbon_in_air>
  a owl:NamedIndividual, <http://purl.oclc.org/NET/ssnx/qu/dim#Concentration> ;
  rdfs:label "mole concentration of anthropogenic nmvoc expressed as carbon in air" ;
  rdfs:isDefinedBy <http://purl.oclc.org/NET/ssnx/cf/cf-property> ;
  rdfs:comment " Mole concentration means number of moles per unit volume, also called molarity, and is used in the construction mole_concentration_of_X_in_Y, where X is a material constituent of Y.  A chemical species denoted by X may be described by a single term such as 'nitrogen' or a phrase such as 'nox_expressed_as_nitrogen'. nmvoc means non methane volatile organic compounds. Anthropogenic means influenced,caused, or created by human activity.  The phrase 'expressed_as' is used in the construction A_expressed_as_B, where B is a chemical constituent of A. It means that the quantity indicated by the standard name is calculated solely with respect to the B contained in A, neglecting all other chemical constituentsof A." .

<http://purl.oclc.org/NET/ssnx/cf/cf-property#mole_concentration_of_atomic_bromine_in_air>
  a owl:NamedIndividual, <http://purl.oclc.org/NET/ssnx/qu/dim#Concentration> ;
  rdfs:label "mole concentration of atomic bromine in air" ;
  rdfs:isDefinedBy <http://purl.oclc.org/NET/ssnx/cf/cf-property> ;
  rdfs:comment " Mole concentration means number of moles per unit volume, also called molarity, and is used in the construction mole_concentration_of_X_in_Y, where X is a material constituent of Y.  A chemical species denoted by X may be described by a single term such as 'nitrogen' or a phrase such as 'nox_expressed_as_nitrogen'. The chemical symbol for atomic bromine is Br." .

<http://purl.oclc.org/NET/ssnx/cf/cf-property#mole_concentration_of_atomic_chlorine_in_air>
  a owl:NamedIndividual, <http://purl.oclc.org/NET/ssnx/qu/dim#Concentration> ;
  rdfs:label "mole concentration of atomic chlorine in air" ;
  rdfs:isDefinedBy <http://purl.oclc.org/NET/ssnx/cf/cf-property> ;
  rdfs:comment " Mole concentration means number of moles per unit volume, also called molarity, and is used in the construction mole_concentration_of_X_in_Y, where X is a material constituent of Y.  A chemical species denoted by X may be described by a single term such as 'nitrogen' or a phrase such as 'nox_expressed_as_nitrogen'. The chemical symbol for atomic chlorine is Cl." .

<http://purl.oclc.org/NET/ssnx/cf/cf-property#mole_concentration_of_atomic_nitrogen_in_air>
  a owl:NamedIndividual, <http://purl.oclc.org/NET/ssnx/qu/dim#Concentration> ;
  rdfs:label "mole concentration of atomic nitrogen in air" ;
  rdfs:isDefinedBy <http://purl.oclc.org/NET/ssnx/cf/cf-property> ;
  rdfs:comment " Mole concentration means number of moles per unit volume, also called molarity, and is used in the construction mole_concentration_of_X_in_Y, where X is a material constituent of Y.  A chemical species denoted by X may be described by a single term such as 'nitrogen' or a phrase such as 'nox_expressed_as_nitrogen'. The chemical symbol for atomic nitrogen is N." .

<http://purl.oclc.org/NET/ssnx/cf/cf-property#mole_concentration_of_benzene_in_air>
  a owl:NamedIndividual, <http://purl.oclc.org/NET/ssnx/qu/dim#Concentration> ;
  rdfs:label "mole concentration of benzene in air" ;
  rdfs:isDefinedBy <http://purl.oclc.org/NET/ssnx/cf/cf-property> ;
  rdfs:comment " Mole concentration means number of moles per unit volume, also called molarity, and is used in the construction mole_concentration_of_X_in_Y, where X is a material constituent of Y.  A chemical species denoted by X may be described by a single term such as 'nitrogen' or a phrase such as 'nox_expressed_as_nitrogen'. The chemical formula for benzene is C6H6.  Benzene is the simplest aromatic hydrocarbon and has a ring structure consisting of six carbon atoms joined by alternating single and double chemical bonds. Each carbon atom is additionally bonded to one hydrogen atom. There are standard names that refer to aromatic_compounds as a group, as well as those for individual species." .

<http://purl.oclc.org/NET/ssnx/cf/cf-property#mole_concentration_of_beta_pinene_in_air>
  a owl:NamedIndividual, <http://purl.oclc.org/NET/ssnx/qu/dim#Concentration> ;
  rdfs:label "mole concentration of beta pinene in air" ;
  rdfs:isDefinedBy <http://purl.oclc.org/NET/ssnx/cf/cf-property> ;
  rdfs:comment " Mole concentration means number of moles per unit volume, also called molarity, and is used in the construction mole_concentration_of_X_in_Y, where X is a material constituent of Y.  A chemical species denoted by X may be described by a single term such as 'nitrogen' or a phrase such as 'nox_expressed_as_nitrogen'. The chemical formula for beta_pinene is C10H16.  The IUPAC name for beta-pinene is (1S,5S)-6,6-dimethyl-2-methylenebicyclo[3.1.1]heptane." .

<http://purl.oclc.org/NET/ssnx/cf/cf-property#mole_concentration_of_biogenic_nmvoc_expressed_as_carbon_in_air>
  a owl:NamedIndividual, <http://purl.oclc.org/NET/ssnx/qu/dim#Concentration> ;
  rdfs:label "mole concentration of biogenic nmvoc expressed as carbon in air" ;
  rdfs:isDefinedBy <http://purl.oclc.org/NET/ssnx/cf/cf-property> ;
  rdfs:comment " Mole concentration means number of moles per unit volume, also called molarity, and is used in the construction mole_concentration_of_X_in_Y, where X is a material constituent of Y.  A chemical species denoted by X may be described by a single term such as 'nitrogen' or a phrase such as 'nox_expressed_as_nitrogen'. nmvoc means non methane volatile organic compounds. Biogenic means influenced, caused, or created by natural processes.  The phrase 'expressed_as' is used in the construction A_expressed_as_B, where B is a chemical constituent of A. It means that the quantity indicated by the standard name is calculated solely with respect to the B contained in A, neglecting all other chemical constituentsof A." .

<http://purl.oclc.org/NET/ssnx/cf/cf-property#mole_concentration_of_bromine_chloride_in_air>
  a owl:NamedIndividual, <http://purl.oclc.org/NET/ssnx/qu/dim#Concentration> ;
  rdfs:label "mole concentration of bromine chloride in air" ;
  rdfs:isDefinedBy <http://purl.oclc.org/NET/ssnx/cf/cf-property> ;
  rdfs:comment " Mole concentration means number of moles per unit volume, also called molarity, and is used in the construction mole_concentration_of_X_in_Y, where X is a material constituent of Y.  A chemical species denoted by X may be described by a single term such as 'nitrogen' or a phrase such as 'nox_expressed_as_nitrogen'. The chemical formula for bromine chloride is BrCl." .

<http://purl.oclc.org/NET/ssnx/cf/cf-property#mole_concentration_of_bromine_monoxide_in_air>
  a owl:NamedIndividual, <http://purl.oclc.org/NET/ssnx/qu/dim#Concentration> ;
  rdfs:label "mole concentration of bromine monoxide in air" ;
  rdfs:isDefinedBy <http://purl.oclc.org/NET/ssnx/cf/cf-property> ;
  rdfs:comment " Mole concentration means number of moles per unit volume, also called molarity, and is used in the construction mole_concentration_of_X_in_Y, where X is a material constituent of Y.  A chemical species denoted by X may be described by a single term such as 'nitrogen' or a phrase such as 'nox_expressed_as_nitrogen'. The chemical formula for bromine monoxide is BrO." .

<http://purl.oclc.org/NET/ssnx/cf/cf-property#mole_concentration_of_bromine_nitrate_in_air>
  a owl:NamedIndividual, <http://purl.oclc.org/NET/ssnx/qu/dim#Concentration> ;
  rdfs:label "mole concentration of bromine nitrate in air" ;
  rdfs:isDefinedBy <http://purl.oclc.org/NET/ssnx/cf/cf-property> ;
  rdfs:comment " Mole concentration means number of moles per unit volume, also called molarity, and is used in the construction mole_concentration_of_X_in_Y, where X is a material constituent of Y.  A chemical species denoted by X may be described by a single term such as 'nitrogen' or a phrase such as 'nox_expressed_as_nitrogen'. The chemical formula for bromine nitrate is BrONO2." .

<http://purl.oclc.org/NET/ssnx/cf/cf-property#mole_concentration_of_brox_expressed_as_bromine_in_air>
  a owl:NamedIndividual, <http://purl.oclc.org/NET/ssnx/qu/dim#Concentration> ;
  rdfs:label "mole concentration of brox expressed as bromine in air" ;
  rdfs:isDefinedBy <http://purl.oclc.org/NET/ssnx/cf/cf-property> ;
  rdfs:comment " Mole concentration means number of moles per unit volume, also called molarity, and is used in the construction mole_concentration_of_X_in_Y, where X is a material constituent of Y.  A chemical species denoted by X may be described by a single term such as 'nitrogen' or a phrase such as 'nox_expressed_as_nitrogen'. Brox describes a family of chemical species consisting of inorganic bromine compounds with theexception of  hydrogen bromide (HBr) and bromine nitrate (BrONO2). Brox is theterm used in standard names for all species belonging to the family that are represented within a given model. The list of individual species that are included in a quantity with a group chemical standard name can vary between models.  Where possible, the data variable should be accompanied by a complete description of the species represented, for example, by using a comment attribute. Inorganic bromine, sometimes referred to as Bry, describes a family of chemical species which result from the degradation of source gases containing bromine (halons, methyl bromide, VSLS) and natural inorganic bromine sources such as volcanoes, seasalt and other aerosols.  Standard names that use the term inorganic_bromine are used for quantities that contain all inorganic bromine species including HCland ClONO2. The phrase 'expressed_as' is used in the construction A_expressed_as_B, where B is a chemical constituent of A. It means that the quantity indicated by the standard nameis calculated solely with respect to the B contained in A, neglecting all other chemical constituents of A." .

<http://purl.oclc.org/NET/ssnx/cf/cf-property#mole_concentration_of_butane_in_air>
  a owl:NamedIndividual, <http://purl.oclc.org/NET/ssnx/qu/dim#Concentration> ;
  rdfs:label "mole concentration of butane in air" ;
  rdfs:isDefinedBy <http://purl.oclc.org/NET/ssnx/cf/cf-property> ;
  rdfs:comment " Mole concentration means number of moles per unit volume, also called molarity, and is used in the construction mole_concentration_of_X_in_Y, where X is a material constituent of Y.  A chemical species denoted by X may be described by a single term such as 'nitrogen' or a phrase such as 'nox_expressed_as_nitrogen'. The chemical formula for butane is C4H10. Butane is a member of the group of hydrocarbons known as alkanes. There are standard names for the alkane group as well as for some of the individual species." .

<http://purl.oclc.org/NET/ssnx/cf/cf-property#mole_concentration_of_carbon_dioxide_in_air>
  a owl:NamedIndividual, <http://purl.oclc.org/NET/ssnx/qu/dim#Concentration> ;
  rdfs:label "mole concentration of carbon dioxide in air" ;
  rdfs:isDefinedBy <http://purl.oclc.org/NET/ssnx/cf/cf-property> ;
  rdfs:comment " Mole concentration means number of moles per unit volume, also called molarity, and is used in the construction mole_concentration_of_X_in_Y, where X is a material constituent of Y.  A chemical species denoted by X may be described by a single term such as 'nitrogen' or a phrase such as 'nox_expressed_as_nitrogen'. The chemical formula for carbon dioxide is CO2." .

<http://purl.oclc.org/NET/ssnx/cf/cf-property#mole_concentration_of_carbon_monoxide_in_air>
  a owl:NamedIndividual, <http://purl.oclc.org/NET/ssnx/qu/dim#Concentration> ;
  rdfs:label "mole concentration of carbon monoxide in air" ;
  rdfs:isDefinedBy <http://purl.oclc.org/NET/ssnx/cf/cf-property> ;
  rdfs:comment " Mole concentration means number of moles per unit volume, also called molarity, and is used in the construction mole_concentration_of_X_in_Y, where X is a material constituent of Y.  A chemical species denoted by X may be described by a single term such as 'nitrogen' or a phrase such as 'nox_expressed_as_nitrogen'. The chemical formula of carbon monoxide is CO." .

<http://purl.oclc.org/NET/ssnx/cf/cf-property#mole_concentration_of_carbon_tetrachloride_in_air>
  a owl:NamedIndividual, <http://purl.oclc.org/NET/ssnx/qu/dim#Concentration> ;
  rdfs:label "mole concentration of carbon tetrachloride in air" ;
  rdfs:isDefinedBy <http://purl.oclc.org/NET/ssnx/cf/cf-property> ;
  rdfs:comment " Mole concentration means number of moles per unit volume, also called molarity, and is used in the construction mole_concentration_of_X_in_Y, where X is a material constituent of Y.  A chemical species denoted by X may be described by a single term such as 'nitrogen' or a phrase such as 'nox_expressed_as_nitrogen'. The chemical formula of carbon tetrachloride is CCl4." .

<http://purl.oclc.org/NET/ssnx/cf/cf-property#mole_concentration_of_cfc113_in_air>
  a owl:NamedIndividual, <http://purl.oclc.org/NET/ssnx/qu/dim#Concentration> ;
  rdfs:label "mole concentration of cfc113 in air" ;
  rdfs:isDefinedBy <http://purl.oclc.org/NET/ssnx/cf/cf-property> ;
  rdfs:comment " Mole concentration means number of moles per unit volume, also called molarity, and is used in the construction mole_concentration_of_X_in_Y, where X is a material constituent of Y.  A chemical species denoted by X may be described by a single term such as 'nitrogen' or a phrase such as 'nox_expressed_as_nitrogen'. The chemical formula of CFC113 is CCl2FCClF2. The IUPAC name for CFC113 is 1,1,2-trichloro-1,2,2-trifluoro-ethane." .

<http://purl.oclc.org/NET/ssnx/cf/cf-property#mole_concentration_of_cfc113a_in_air>
  a owl:NamedIndividual, <http://purl.oclc.org/NET/ssnx/qu/dim#Concentration> ;
  rdfs:label "mole concentration of cfc113a in air" ;
  rdfs:isDefinedBy <http://purl.oclc.org/NET/ssnx/cf/cf-property> ;
  rdfs:comment " Mole concentration means number of moles per unit volume, also called molarity, and is used in the construction mole_concentration_of_X_in_Y, where X is a material constituent of Y.  A chemical species denoted by X may be described by a single term such as 'nitrogen' or a phrase such as 'nox_expressed_as_nitrogen'. The chemical formula of CFC113a CCl3CF3.  The IUPAC name for CFC113a is 1,1,1-trichloro-2,2,2-trifluoro-ethane." .

<http://purl.oclc.org/NET/ssnx/cf/cf-property#mole_concentration_of_cfc114_in_air>
  a owl:NamedIndividual, <http://purl.oclc.org/NET/ssnx/qu/dim#Concentration> ;
  rdfs:label "mole concentration of cfc114 in air" ;
  rdfs:isDefinedBy <http://purl.oclc.org/NET/ssnx/cf/cf-property> ;
  rdfs:comment " Mole concentration means number of moles per unit volume, also called molarity, and is used in the construction mole_concentration_of_X_in_Y, where X is a material constituent of Y.  A chemical species denoted by X may be described by a single term such as 'nitrogen' or a phrase such as 'nox_expressed_as_nitrogen'. The chemical formula of CFC114 is CClF2CClF2. The IUPAC name for CFC114 is 1,2-dichloro-1,1,2,2-tetrafluoro-ethane." .

<http://purl.oclc.org/NET/ssnx/cf/cf-property#mole_concentration_of_cfc115_in_air>
  a owl:NamedIndividual, <http://purl.oclc.org/NET/ssnx/qu/dim#Concentration> ;
  rdfs:label "mole concentration of cfc115 in air" ;
  rdfs:isDefinedBy <http://purl.oclc.org/NET/ssnx/cf/cf-property> ;
  rdfs:comment " Mole concentration means number of moles per unit volume, also called molarity, and is used in the construction mole_concentration_of_X_in_Y, where X is a material constituent of Y.  A chemical species denoted by X may be described by a single term such as 'nitrogen' or a phrase such as 'nox_expressed_as_nitrogen'. The chemical formula of CFC115 is CClF2CF3. The IUPAC name for CFC115 is 1-chloro-1,1,2,2,2-pentafluoro-ethane." .

<http://purl.oclc.org/NET/ssnx/cf/cf-property#mole_concentration_of_cfc11_in_air>
  a owl:NamedIndividual, <http://purl.oclc.org/NET/ssnx/qu/dim#Concentration> ;
  rdfs:label "mole concentration of cfc11 in air" ;
  rdfs:isDefinedBy <http://purl.oclc.org/NET/ssnx/cf/cf-property> ;
  rdfs:comment " Mole concentration means number of moles per unit volume, also called molarity, and is used in the construction mole_concentration_of_X_in_Y, where X is a material constituent of Y.  A chemical species denoted by X may be described by a single term such as 'nitrogen' or a phrase such as 'nox_expressed_as_nitrogen'. The chemical formula of CFC11 is CFCl3. The IUPAC name fof CFC11 is trichloro-fluoro-methane." .

<http://purl.oclc.org/NET/ssnx/cf/cf-property#mole_concentration_of_cfc12_in_air>
  a owl:NamedIndividual, <http://purl.oclc.org/NET/ssnx/qu/dim#Concentration> ;
  rdfs:label "mole concentration of cfc12 in air" ;
  rdfs:isDefinedBy <http://purl.oclc.org/NET/ssnx/cf/cf-property> ;
  rdfs:comment " Mole concentration means number of moles per unit volume, also called molarity, and is used in the construction mole_concentration_of_X_in_Y, where X is a material constituent of Y.  A chemical species denoted by X may be described by a single term such as 'nitrogen' or a phrase such as 'nox_expressed_as_nitrogen'. The chemical formula for CFC12 is CF2Cl2.  The IUPAC name for CFC12 is dichloro-difluoro-methane." .

<http://purl.oclc.org/NET/ssnx/cf/cf-property#mole_concentration_of_chlorine_dioxide_in_air>
  a owl:NamedIndividual, <http://purl.oclc.org/NET/ssnx/qu/dim#Concentration> ;
  rdfs:label "mole concentration of chlorine dioxide in air" ;
  rdfs:isDefinedBy <http://purl.oclc.org/NET/ssnx/cf/cf-property> ;
  rdfs:comment " Mole concentration means number of moles per unit volume, also called molarity, and is used in the construction mole_concentration_of_X_in_Y, where X is a material constituent of Y.  A chemical species denoted by X may be described by a single term such as 'nitrogen' or a phrase such as 'nox_expressed_as_nitrogen'. The chemical formula for chlorine dioxide is OClO." .

<http://purl.oclc.org/NET/ssnx/cf/cf-property#mole_concentration_of_chlorine_monoxide_in_air>
  a owl:NamedIndividual, <http://purl.oclc.org/NET/ssnx/qu/dim#Concentration> ;
  rdfs:label "mole concentration of chlorine monoxide in air" ;
  rdfs:isDefinedBy <http://purl.oclc.org/NET/ssnx/cf/cf-property> ;
  rdfs:comment " Mole concentration means number of moles per unit volume, also called molarity, and is used in the construction mole_concentration_of_X_in_Y, where X is a material constituent of Y.  A chemical species denoted by X may be described by a single term such as 'nitrogen' or a phrase such as 'nox_expressed_as_nitrogen'. The chemical formula for chlorine monoxide is ClO." .

<http://purl.oclc.org/NET/ssnx/cf/cf-property#mole_concentration_of_chlorine_nitrate_in_air>
  a owl:NamedIndividual, <http://purl.oclc.org/NET/ssnx/qu/dim#Concentration> ;
  rdfs:label "mole concentration of chlorine nitrate in air" ;
  rdfs:isDefinedBy <http://purl.oclc.org/NET/ssnx/cf/cf-property> ;
  rdfs:comment " Mole concentration means number of moles per unit volume, also called molarity, and is used in the construction mole_concentration_of_X_in_Y, where X is a material constituent of Y.  A chemical species denoted by X may be described by a single term such as 'nitrogen' or a phrase such as 'nox_expressed_as_nitrogen'. The chemical formula for chlorine nitrate is ClONO2." .

<http://purl.oclc.org/NET/ssnx/cf/cf-property#mole_concentration_of_clox_expressed_as_chlorine_in_air>
  a owl:NamedIndividual, <http://purl.oclc.org/NET/ssnx/qu/dim#Concentration> ;
  rdfs:label "mole concentration of clox expressed as chlorine in air" ;
  rdfs:isDefinedBy <http://purl.oclc.org/NET/ssnx/cf/cf-property> ;
  rdfs:comment " Mole concentration means number of moles per unit volume, also called molarity, and is used in the construction mole_concentration_of_X_in_Y, where X is a material constituent of Y.  A chemical species denoted by X may be described by a single term such as 'nitrogen' or a phrase such as 'nox_expressed_as_nitrogen'. Cloxdescribes a family of chemical species consisting of inorganic chlorine compounds with theexception of  hydrogen chloride (HCl) and chlorine nitrate (ClONO2). Clox is the term used in standard names for all species belonging to the family that are representedwithin a given model. The list of individual species that are included in a quantity with a group chemical standard name can vary between models.  Where possible, the data variable should be accompanied by a complete description of the species represented, for example, byusing a comment attribute. Inorganic chlorine, sometimes referred to as Cly, describes a family of chemical species which result from the degradation of source gases containing chlorine (CFCs, HCFCs, VSLS) and natural inorganic chlorine sources such as seasaltand other aerosols.   Standard names that use the term inorganic_chlorine are used for quantities that contain all inorganic chlorine species including HCl and ClONO2. The phrase 'expressed_as' is used in the construction A_expressed_as_B, where B is a chemical constituent of A. It means that the quantity indicated by the standard name is calculatedsolely with respect to the B contained in A, neglecting all other chemical constituents ofA." .

<http://purl.oclc.org/NET/ssnx/cf/cf-property#mole_concentration_of_dichlorine_peroxide_in_air>
  a owl:NamedIndividual, <http://purl.oclc.org/NET/ssnx/qu/dim#Concentration> ;
  rdfs:label "mole concentration of dichlorine peroxide in air" ;
  rdfs:isDefinedBy <http://purl.oclc.org/NET/ssnx/cf/cf-property> ;
  rdfs:comment " Mole concentration means number of moles per unit volume, also called molarity, and is used in the construction mole_concentration_of_X_in_Y, where X is a material constituent of Y.  A chemical species denoted by X may be described by a single term such as 'nitrogen' or a phrase such as 'nox_expressed_as_nitrogen'. The chemical formula for dichlorine peroxide is Cl2O2." .

<http://purl.oclc.org/NET/ssnx/cf/cf-property#mole_concentration_of_dimethyl_sulfide_in_air>
  a owl:NamedIndividual, <http://purl.oclc.org/NET/ssnx/qu/dim#Concentration> ;
  rdfs:label "mole concentration of dimethyl sulfide in air" ;
  rdfs:isDefinedBy <http://purl.oclc.org/NET/ssnx/cf/cf-property> ;
  rdfs:comment " Mole concentration means number of moles per unit volume, also called molarity, and is used in the construction mole_concentration_of_X_in_Y, where X is a material constituent of Y.  A chemical species denoted by X may be described by a single term such as 'nitrogen' or a phrase such as 'nox_expressed_as_nitrogen'. The chemical formula for dimethyl sulfide is (CH3)2S.  Dimethyl sulfide is sometimes referred to as DMS." .

<http://purl.oclc.org/NET/ssnx/cf/cf-property#mole_concentration_of_dinitrogen_pentoxide_in_air>
  a owl:NamedIndividual, <http://purl.oclc.org/NET/ssnx/qu/dim#Concentration> ;
  rdfs:label "mole concentration of dinitrogen pentoxide in air" ;
  rdfs:isDefinedBy <http://purl.oclc.org/NET/ssnx/cf/cf-property> ;
  rdfs:comment " Mole concentration means number of moles per unit volume, also called molarity, and is used in the construction mole_concentration_of_X_in_Y, where X is a material constituent of Y.  A chemical species denoted by X may be described by a single term such as 'nitrogen' or a phrase such as 'nox_expressed_as_nitrogen'. The chemical formula for dinitrogen pentoxide is N2O5." .

<http://purl.oclc.org/NET/ssnx/cf/cf-property#mole_concentration_of_ethane_in_air>
  a owl:NamedIndividual, <http://purl.oclc.org/NET/ssnx/qu/dim#Concentration> ;
  rdfs:label "mole concentration of ethane in air" ;
  rdfs:isDefinedBy <http://purl.oclc.org/NET/ssnx/cf/cf-property> ;
  rdfs:comment " Mole concentration means number of moles per unit volume, also called molarity, and is used in the construction mole_concentration_of_X_in_Y, where X is a material constituent of Y.  A chemical species denoted by X may be described by a single term such as 'nitrogen' or a phrase such as 'nox_expressed_as_nitrogen'. The chemical formula for ethane is C2H6. Ethane is a member of the group of hydrocarbons known as alkanes.There are standard names for the alkane group as well as for some of the individual species." .

<http://purl.oclc.org/NET/ssnx/cf/cf-property#mole_concentration_of_ethanol_in_air>
  a owl:NamedIndividual, <http://purl.oclc.org/NET/ssnx/qu/dim#Concentration> ;
  rdfs:label "mole concentration of ethanol in air" ;
  rdfs:isDefinedBy <http://purl.oclc.org/NET/ssnx/cf/cf-property> ;
  rdfs:comment " Mole concentration means number of moles per unit volume, also called molarity, and is used in the construction mole_concentration_of_X_in_Y, where X is a material constituent of Y.  A chemical species denoted by X may be described by a single term such as 'nitrogen' or a phrase such as 'nox_expressed_as_nitrogen'. The chemical formula for ethanol is C2H5OH." .

<http://purl.oclc.org/NET/ssnx/cf/cf-property#mole_concentration_of_ethene_in_air>
  a owl:NamedIndividual, <http://purl.oclc.org/NET/ssnx/qu/dim#Concentration> ;
  rdfs:label "mole concentration of ethene in air" ;
  rdfs:isDefinedBy <http://purl.oclc.org/NET/ssnx/cf/cf-property> ;
  rdfs:comment " Mole concentration means number of moles per unit volume, also called molarity, and is used in the construction mole_concentration_of_X_in_Y, where X is a material constituent of Y.  A chemical species denoted by X may be described by a single term such as 'nitrogen' or a phrase such as 'nox_expressed_as_nitrogen'. The chemical formula for ethene is C2H4. Ethene is a member of the group of hydrocarbons known as alkenes.There are standard names for the alkene group as well as for some of the individual species." .

<http://purl.oclc.org/NET/ssnx/cf/cf-property#mole_concentration_of_ethyne_in_air>
  a owl:NamedIndividual, <http://purl.oclc.org/NET/ssnx/qu/dim#Concentration> ;
  rdfs:label "mole concentration of ethyne in air" ;
  rdfs:isDefinedBy <http://purl.oclc.org/NET/ssnx/cf/cf-property> ;
  rdfs:comment " Mole concentration means number of moles per unit volume, also called molarity, and is used in the construction mole_concentration_of_X_in_Y, where X is a material constituent of Y.  A chemical species denoted by X may be described by a single term such as 'nitrogen' or a phrase such as 'nox_expressed_as_nitrogen'. The chemical formula for ethyne is HC2H.  Ethyne is the IUPAC name for this species, which is also commonlyknown as acetylene." .

<http://purl.oclc.org/NET/ssnx/cf/cf-property#mole_concentration_of_formaldehyde_in_air>
  a owl:NamedIndividual, <http://purl.oclc.org/NET/ssnx/qu/dim#Concentration> ;
  rdfs:label "mole concentration of formaldehyde in air" ;
  rdfs:isDefinedBy <http://purl.oclc.org/NET/ssnx/cf/cf-property> ;
  rdfs:comment " Mole concentration means number of moles per unit volume, also called molarity, and is used in the construction mole_concentration_of_X_in_Y, where X is a material constituent of Y.  A chemical species denoted by X may be described by a single term such as 'nitrogen' or a phrase such as 'nox_expressed_as_nitrogen'. The chemical formula for formaldehyde is CH2O. The IUPAC name for formaldehyde is methanal." .

<http://purl.oclc.org/NET/ssnx/cf/cf-property#mole_concentration_of_formic_acid_in_air>
  a owl:NamedIndividual, <http://purl.oclc.org/NET/ssnx/qu/dim#Concentration> ;
  rdfs:label "mole concentration of formic acid in air" ;
  rdfs:isDefinedBy <http://purl.oclc.org/NET/ssnx/cf/cf-property> ;
  rdfs:comment " Mole concentration means number of moles per unit volume, also called molarity, and is used in the construction mole_concentration_of_X_in_Y, where X is a material constituent of Y.  A chemical species denoted by X may be described by a single term such as 'nitrogen' or a phrase such as 'nox_expressed_as_nitrogen'. The chemical formula for formic acid is HCOOH.  The IUPAC name for formic acid is methanoic acid." .

<http://purl.oclc.org/NET/ssnx/cf/cf-property#mole_concentration_of_gaseous_divalent_mercury_in_air>
  a owl:NamedIndividual, <http://purl.oclc.org/NET/ssnx/qu/dim#Concentration> ;
  rdfs:label "mole concentration of gaseous divalent mercury in air" ;
  rdfs:isDefinedBy <http://purl.oclc.org/NET/ssnx/cf/cf-property> ;
  rdfs:comment " Mole concentration means number of moles per unit volume, also called molarity, and is used in the construction mole_concentration_of_X_in_Y, where X is a material constituent of Y.  A chemical species denoted by X may be described by a single term such as 'nitrogen' or a phrase such as 'nox_expressed_as_nitrogen'. Divalent mercury means all compounds in which the mercury has two binding sites to other ion(s)in a salt or to other atom(s) in a molecule." .

<http://purl.oclc.org/NET/ssnx/cf/cf-property#mole_concentration_of_gaseous_elemental_mercury_in_air>
  a owl:NamedIndividual, <http://purl.oclc.org/NET/ssnx/qu/dim#Concentration> ;
  rdfs:label "mole concentration of gaseous elemental mercury in air" ;
  rdfs:isDefinedBy <http://purl.oclc.org/NET/ssnx/cf/cf-property> ;
  rdfs:comment " Mole concentration means number of moles per unit volume, also called molarity, and is used in the construction mole_concentration_of_X_in_Y, where X is a material constituent of Y.  A chemical species denoted by X may be described by a single term such as 'nitrogen' or a phrase such as 'nox_expressed_as_nitrogen'. The chemical symbol for mercury is Hg." .

<http://purl.oclc.org/NET/ssnx/cf/cf-property#mole_concentration_of_halon1202_in_air>
  a owl:NamedIndividual, <http://purl.oclc.org/NET/ssnx/qu/dim#Concentration> ;
  rdfs:label "mole concentration of halon1202 in air" ;
  rdfs:isDefinedBy <http://purl.oclc.org/NET/ssnx/cf/cf-property> ;
  rdfs:comment " Mole concentration means number of moles per unit volume, also called molarity, and is used in the construction mole_concentration_of_X_in_Y, where X is a material constituent of Y.  A chemical species denoted by X may be described by a single term such as 'nitrogen' or a phrase such as 'nox_expressed_as_nitrogen'. The chemical formula for halon1202 is CBr2F2. The IUPAC name for halon1202 is dibromo-difluoro-methane." .

<http://purl.oclc.org/NET/ssnx/cf/cf-property#mole_concentration_of_halon1211_in_air>
  a owl:NamedIndividual, <http://purl.oclc.org/NET/ssnx/qu/dim#Concentration> ;
  rdfs:label "mole concentration of halon1211 in air" ;
  rdfs:isDefinedBy <http://purl.oclc.org/NET/ssnx/cf/cf-property> ;
  rdfs:comment " Mole concentration means number of moles per unit volume, also called molarity, and is used in the construction mole_concentration_of_X_in_Y, where X is a material constituent of Y.  A chemical species denoted by X may be described by a single term such as 'nitrogen' or a phrase such as 'nox_expressed_as_nitrogen'. The chemical formula for halon1211 is CBrClF2. The IUPAC name for halon1211 is bromo-chloro-difluoro-methane." .

<http://purl.oclc.org/NET/ssnx/cf/cf-property#mole_concentration_of_halon1301_in_air>
  a owl:NamedIndividual, <http://purl.oclc.org/NET/ssnx/qu/dim#Concentration> ;
  rdfs:label "mole concentration of halon1301 in air" ;
  rdfs:isDefinedBy <http://purl.oclc.org/NET/ssnx/cf/cf-property> ;
  rdfs:comment " Mole concentration means number of moles per unit volume, also called molarity, and is used in the construction mole_concentration_of_X_in_Y, where X is a material constituent of Y.  A chemical species denoted by X may be described by a single term such as 'nitrogen' or a phrase such as 'nox_expressed_as_nitrogen'. The chemical formula for halon1301 is CBrF3. The IUPAC name for halon1301 is bromo-trifluoro-methane." .

<http://purl.oclc.org/NET/ssnx/cf/cf-property#mole_concentration_of_halon2402_in_air>
  a owl:NamedIndividual, <http://purl.oclc.org/NET/ssnx/qu/dim#Concentration> ;
  rdfs:label "mole concentration of halon2402 in air" ;
  rdfs:isDefinedBy <http://purl.oclc.org/NET/ssnx/cf/cf-property> ;
  rdfs:comment " Mole concentration means number of moles per unit volume, also called molarity, and is used in the construction mole_concentration_of_X_in_Y, where X is a material constituent of Y.  A chemical species denoted by X may be described by a single term such as 'nitrogen' or a phrase such as 'nox_expressed_as_nitrogen'. The chemical formula for halo2402 is C2Br2F4. The IUPAC name for halon2402 is 1,2-dibromo-1,1,2,2-tetrafluoro-ethane." .

<http://purl.oclc.org/NET/ssnx/cf/cf-property#mole_concentration_of_hcc140a_in_air>
  a owl:NamedIndividual, <http://purl.oclc.org/NET/ssnx/qu/dim#Concentration> ;
  rdfs:label "mole concentration of hcc140a in air" ;
  rdfs:isDefinedBy <http://purl.oclc.org/NET/ssnx/cf/cf-property> ;
  rdfs:comment " Mole concentration means number of moles per unit volume, also called molarity, and is used in the construction mole_concentration_of_X_in_Y, where X is a material constituent of Y.  A chemical species denoted by X may be described by a single term such as 'nitrogen' or a phrase such as 'nox_expressed_as_nitrogen'. The chemical formula for hcc140a is CH3CCl3. The IUPAC name for hcc140a is 1,1,1-trichloro-ethane." .

<http://purl.oclc.org/NET/ssnx/cf/cf-property#mole_concentration_of_hcfc141b_in_air>
  a owl:NamedIndividual, <http://purl.oclc.org/NET/ssnx/qu/dim#Concentration> ;
  rdfs:label "mole concentration of hcfc141b in air" ;
  rdfs:isDefinedBy <http://purl.oclc.org/NET/ssnx/cf/cf-property> ;
  rdfs:comment " Mole concentration means number of moles per unit volume, also called molarity, and is used in the construction mole_concentration_of_X_in_Y, where X is a material constituent of Y.  A chemical species denoted by X may be described by a single term such as 'nitrogen' or a phrase such as 'nox_expressed_as_nitrogen'. The chemical formula for HCFC141b is CH3CCl2F. The IUPAC name for HCFC141b is 1,1-dichloro-1-fluoroethane." .

<http://purl.oclc.org/NET/ssnx/cf/cf-property#mole_concentration_of_hcfc142b_in_air>
  a owl:NamedIndividual, <http://purl.oclc.org/NET/ssnx/qu/dim#Concentration> ;
  rdfs:label "mole concentration of hcfc142b in air" ;
  rdfs:isDefinedBy <http://purl.oclc.org/NET/ssnx/cf/cf-property> ;
  rdfs:comment " Mole concentration means number of moles per unit volume, also called molarity, and is used in the construction mole_concentration_of_X_in_Y, where X is a material constituent of Y.  A chemical species denoted by X may be described by a single term such as 'nitrogen' or a phrase such as 'nox_expressed_as_nitrogen'. The chemical formula for HCFC142b is CH3CClF2. The IUPAC name for HCFC142b is 1-chloro-1,1-difluoroethane." .

<http://purl.oclc.org/NET/ssnx/cf/cf-property#mole_concentration_of_hcfc22_in_air>
  a owl:NamedIndividual, <http://purl.oclc.org/NET/ssnx/qu/dim#Concentration> ;
  rdfs:label "mole concentration of hcfc22 in air" ;
  rdfs:isDefinedBy <http://purl.oclc.org/NET/ssnx/cf/cf-property> ;
  rdfs:comment " Mole concentration means number of moles per unit volume, also called molarity, and is used in the construction mole_concentration_of_X_in_Y, where X is a material constituent of Y.  A chemical species denoted by X may be described by a single term such as 'nitrogen' or a phrase such as 'nox_expressed_as_nitrogen'. The chemical formula for HCFC22 is CHClF2.  The IUPAC name for HCFC22 is chloro-difluoro-methane." .

<http://purl.oclc.org/NET/ssnx/cf/cf-property#mole_concentration_of_hexachlorobiphenyl_in_air>
  a owl:NamedIndividual, <http://purl.oclc.org/NET/ssnx/qu/dim#Concentration> ;
  rdfs:label "mole concentration of hexachlorobiphenyl in air" ;
  rdfs:isDefinedBy <http://purl.oclc.org/NET/ssnx/cf/cf-property> ;
  rdfs:comment " Mole concentration means number of moles per unit volume, also called molarity, and is used in the construction mole_concentration_of_X_in_Y, where X is a material constituent of Y.  A chemical species denoted by X may be described by a single term such as 'nitrogen' or a phrase such as 'nox_expressed_as_nitrogen'. The chemical formula for hexachlorobiphenyl is C12H4Cl6.  This structure of this species consists of two linked benzene rings, each of which is additionally bonded to three chlorine atoms." .

<http://purl.oclc.org/NET/ssnx/cf/cf-property#mole_concentration_of_hox_expressed_as_hydrogen_in_air>
  a owl:NamedIndividual, <http://purl.oclc.org/NET/ssnx/qu/dim#Concentration> ;
  rdfs:label "mole concentration of hox expressed as hydrogen in air" ;
  rdfs:isDefinedBy <http://purl.oclc.org/NET/ssnx/cf/cf-property> ;
  rdfs:comment " Mole concentration means number of moles per unit volume, also called molarity, and is used in the construction mole_concentration_of_X_in_Y, where X is a material constituent of Y.  A chemical species denoted by X may be described by a single term such as 'nitrogen' or a phrase such as 'nox_expressed_as_nitrogen'. HOx means a combination of two radical species containing hydrogen and oxygen: OH and HO2. The phrase 'expressed_as' is used in the construction A_expressed_as_B, where B is a chemical constituent of A. It means that the quantity indicated by the standard name is calculated solely with respect to the B contained in A, neglecting all other chemical constituents of A." .

<http://purl.oclc.org/NET/ssnx/cf/cf-property#mole_concentration_of_hydrogen_bromide_in_air>
  a owl:NamedIndividual, <http://purl.oclc.org/NET/ssnx/qu/dim#Concentration> ;
  rdfs:label "mole concentration of hydrogen bromide in air" ;
  rdfs:isDefinedBy <http://purl.oclc.org/NET/ssnx/cf/cf-property> ;
  rdfs:comment " Mole concentration means number of moles per unit volume, also called molarity, and is used in the construction mole_concentration_of_X_in_Y, where X is a material constituent of Y.  A chemical species denoted by X may be described by a single term such as 'nitrogen' or a phrase such as 'nox_expressed_as_nitrogen'. The chemical formula for hydrogen bromide is HBr." .

<http://purl.oclc.org/NET/ssnx/cf/cf-property#mole_concentration_of_hydrogen_chloride_in_air>
  a owl:NamedIndividual, <http://purl.oclc.org/NET/ssnx/qu/dim#Concentration> ;
  rdfs:label "mole concentration of hydrogen chloride in air" ;
  rdfs:isDefinedBy <http://purl.oclc.org/NET/ssnx/cf/cf-property> ;
  rdfs:comment " Mole concentration means number of moles per unit volume, also called molarity, and is used in the construction mole_concentration_of_X_in_Y, where X is a material constituent of Y.  A chemical species denoted by X may be described by a single term such as 'nitrogen' or a phrase such as 'nox_expressed_as_nitrogen'. The chemical formula for hydrogen chloride is HCl." .

<http://purl.oclc.org/NET/ssnx/cf/cf-property#mole_concentration_of_hydrogen_cyanide_in_air>
  a owl:NamedIndividual, <http://purl.oclc.org/NET/ssnx/qu/dim#Concentration> ;
  rdfs:label "mole concentration of hydrogen cyanide in air" ;
  rdfs:isDefinedBy <http://purl.oclc.org/NET/ssnx/cf/cf-property> ;
  rdfs:comment " Mole concentration means number of moles per unit volume, also called molarity, and is used in the construction mole_concentration_of_X_in_Y, where X is a material constituent of Y.  A chemical species denoted by X may be described by a single term such as 'nitrogen' or a phrase such as 'nox_expressed_as_nitrogen'. The chemical formula for hydrogen cyanide is HCN." .

<http://purl.oclc.org/NET/ssnx/cf/cf-property#mole_concentration_of_hydrogen_peroxide_in_air>
  a owl:NamedIndividual, <http://purl.oclc.org/NET/ssnx/qu/dim#Concentration> ;
  rdfs:label "mole concentration of hydrogen peroxide in air" ;
  rdfs:isDefinedBy <http://purl.oclc.org/NET/ssnx/cf/cf-property> ;
  rdfs:comment " Mole concentration means number of moles per unit volume, also called molarity, and is used in the construction mole_concentration_of_X_in_Y, where X is a material constituent of Y.  A chemical species denoted by X may be described by a single term such as 'nitrogen' or a phrase such as 'nox_expressed_as_nitrogen'. The chemical formula for hydrogen peroxide is H2O2." .

<http://purl.oclc.org/NET/ssnx/cf/cf-property#mole_concentration_of_hydroperoxyl_radical_in_air>
  a owl:NamedIndividual, <http://purl.oclc.org/NET/ssnx/qu/dim#Concentration> ;
  rdfs:label "mole concentration of hydroperoxyl radical in air" ;
  rdfs:isDefinedBy <http://purl.oclc.org/NET/ssnx/cf/cf-property> ;
  rdfs:comment " Mole concentration means number of moles per unit volume, also called molarity, and is used in the construction mole_concentration_of_X_in_Y, where X is a material constituent of Y.  A chemical species denoted by X may be described by a single term such as 'nitrogen' or a phrase such as 'nox_expressed_as_nitrogen'. The chemical formula for the hydroperoxyl radical is HO2. In chemistry, a 'radical' is a highly reactive, and therefore shortlived, species." .

<http://purl.oclc.org/NET/ssnx/cf/cf-property#mole_concentration_of_hydroxyl_radical_in_air>
  a owl:NamedIndividual, <http://purl.oclc.org/NET/ssnx/qu/dim#Concentration> ;
  rdfs:label "mole concentration of hydroxyl radical in air" ;
  rdfs:isDefinedBy <http://purl.oclc.org/NET/ssnx/cf/cf-property> ;
  rdfs:comment " Mole concentration means number of moles per unit volume, also called molarity, and is used in the construction mole_concentration_of_X_in_Y, where X is a material constituent of Y.  A chemical species denoted by X may be described by a single term such as 'nitrogen' or a phrase such as 'nox_expressed_as_nitrogen'. The chemical formula for the hydroxyl radical is OH. In chemistry, a 'radical' is a highly reactive, and therefore shortlived, species." .

<http://purl.oclc.org/NET/ssnx/cf/cf-property#mole_concentration_of_hypobromous_acid_in_air>
  a owl:NamedIndividual, <http://purl.oclc.org/NET/ssnx/qu/dim#Concentration> ;
  rdfs:label "mole concentration of hypobromous acid in air" ;
  rdfs:isDefinedBy <http://purl.oclc.org/NET/ssnx/cf/cf-property> ;
  rdfs:comment " Mole concentration means number of moles per unit volume, also called molarity, and is used in the construction mole_concentration_of_X_in_Y, where X is a material constituent of Y.  A chemical species denoted by X may be described by a single term such as 'nitrogen' or a phrase such as 'nox_expressed_as_nitrogen'. The chemical formula for hypobromous acid is HOBr." .

<http://purl.oclc.org/NET/ssnx/cf/cf-property#mole_concentration_of_hypochlorous_acid_in_air>
  a owl:NamedIndividual, <http://purl.oclc.org/NET/ssnx/qu/dim#Concentration> ;
  rdfs:label "mole concentration of hypochlorous acid in air" ;
  rdfs:isDefinedBy <http://purl.oclc.org/NET/ssnx/cf/cf-property> ;
  rdfs:comment " Mole concentration means number of moles per unit volume, also called molarity, and is used in the construction mole_concentration_of_X_in_Y, where X is a material constituent of Y.  A chemical species denoted by X may be described by a single term such as 'nitrogen' or a phrase such as 'nox_expressed_as_nitrogen'. The chemical formula for hypochlorous acid is HOCl." .

<http://purl.oclc.org/NET/ssnx/cf/cf-property#mole_concentration_of_inorganic_bromine_in_air>
  a owl:NamedIndividual, <http://purl.oclc.org/NET/ssnx/qu/dim#Concentration> ;
  rdfs:label "mole concentration of inorganic bromine in air" ;
  rdfs:isDefinedBy <http://purl.oclc.org/NET/ssnx/cf/cf-property> ;
  rdfs:comment " Mole concentration means number of moles per unit volume, also called molarity, and is used in the construction mole_concentration_of_X_in_Y, where X is a material constituent of Y.  A chemical species denoted by X may be described by a single term such as 'nitrogen' or a phrase such as 'nox_expressed_as_nitrogen'. Inorganic bromine, sometimes referred to as Bry, describes a family of chemical species which result from the degradation of source gases containing bromine (halons, methyl bromide, VSLS) and natural inorganic bromine sources such as volcanoes, seasalt and other aerosols. Inorganic bromine is the term used in standard names for all species belonging to the family that are represented within a given model. The list of individual species that are included in a quantity having a group chemical standard name can vary between models.  Where possible, the data variable should be accompanied by a complete description of the species represented, for example, by using a comment attribute. Standard names that use the term brox are used for quantities that contain all inorganic bromine species except HBr and BrONO2." .

<http://purl.oclc.org/NET/ssnx/cf/cf-property#mole_concentration_of_inorganic_chlorine_in_air>
  a owl:NamedIndividual, <http://purl.oclc.org/NET/ssnx/qu/dim#Concentration> ;
  rdfs:label "mole concentration of inorganic chlorine in air" ;
  rdfs:isDefinedBy <http://purl.oclc.org/NET/ssnx/cf/cf-property> ;
  rdfs:comment " Mole concentration means number of moles per unit volume, also called molarity, and is used in the construction mole_concentration_of_X_in_Y, where X is a material constituent of Y.  A chemical species denoted by X may be described by a single term such as 'nitrogen' or a phrase such as 'nox_expressed_as_nitrogen'. Inorganic chlorine, sometimes referred to as Cly, describes a family of chemical species which result from the degradation of source gases containing chlorine (CFCs, HCFCs, VSLS) and natural inorganic chlorine sources such as seasalt and other aerosols. Inorganic chlorine is the term used in standard names for all species belonging to the family that arerepresented within a given model. The list of individual species that are included in a quantity having a group chemical standard name can vary between models.  Where possible, the data variable should be accompanied by a complete description of the species represented, for example, by using a comment attribute. Standard names that use the term cloxare used for quantities that contain all inorganic chlorine species except HCl and ClONO2." .

<http://purl.oclc.org/NET/ssnx/cf/cf-property#mole_concentration_of_isoprene_in_air>
  a owl:NamedIndividual, <http://purl.oclc.org/NET/ssnx/qu/dim#Concentration> ;
  rdfs:label "mole concentration of isoprene in air" ;
  rdfs:isDefinedBy <http://purl.oclc.org/NET/ssnx/cf/cf-property> ;
  rdfs:comment " Mole concentration means number of moles per unit volume, also called molarity, and is used in the construction mole_concentration_of_X_in_Y, where X is a material constituent of Y.  A chemical species denoted by X may be described by a single term such as 'nitrogen' or a phrase such as 'nox_expressed_as_nitrogen'. The chemical formula for isoprene is CH2=C(CH3)CH=CH2. The IUPAC name for isoprene is 2-methyl-buta-1,3-diene. Isoprene is a member of the group of hydrocarbons known as terpenes.  There are standard names for the terpene group as well as for some of the individual species." .

<http://purl.oclc.org/NET/ssnx/cf/cf-property#mole_concentration_of_limonene_in_air>
  a owl:NamedIndividual, <http://purl.oclc.org/NET/ssnx/qu/dim#Concentration> ;
  rdfs:label "mole concentration of limonene in air" ;
  rdfs:isDefinedBy <http://purl.oclc.org/NET/ssnx/cf/cf-property> ;
  rdfs:comment " Mole concentration means number of moles per unit volume, also called molarity, and is used in the construction mole_concentration_of_X_in_Y, where X is a material constituent of Y.  A chemical species denoted by X may be described by a single term such as 'nitrogen' or a phrase such as 'nox_expressed_as_nitrogen'. The chemical formula for methyl hydroperoxide is CH3OOH." .

<http://purl.oclc.org/NET/ssnx/cf/cf-property#mole_concentration_of_methane_in_air>
  a owl:NamedIndividual, <http://purl.oclc.org/NET/ssnx/qu/dim#Concentration> ;
  rdfs:label "mole concentration of methane in air" ;
  rdfs:isDefinedBy <http://purl.oclc.org/NET/ssnx/cf/cf-property> ;
  rdfs:comment " Mole concentration means number of moles per unit volume, also called molarity, and is used in the construction mole_concentration_of_X_in_Y, where X is a material constituent of Y.  A chemical species denoted by X may be described by a single term such as 'nitrogen' or a phrase such as 'nox_expressed_as_nitrogen'. The chemical formula for methane is CH4. Methane is a member of the group of hydrocarbons known as alkanes. There are standard names for the alkane group as well as for some of the individual species." .

<http://purl.oclc.org/NET/ssnx/cf/cf-property#mole_concentration_of_methanol_in_air>
  a owl:NamedIndividual, <http://purl.oclc.org/NET/ssnx/qu/dim#Concentration> ;
  rdfs:label "mole concentration of methanol in air" ;
  rdfs:isDefinedBy <http://purl.oclc.org/NET/ssnx/cf/cf-property> ;
  rdfs:comment " Mole concentration means number of moles per unit volume, also called molarity, and is used in the construction mole_concentration_of_X_in_Y, where X is a material constituent of Y.  A chemical species denoted by X may be described by a single term such as 'nitrogen' or a phrase such as 'nox_expressed_as_nitrogen'. The chemical formula for methanol is CH3OH." .

<http://purl.oclc.org/NET/ssnx/cf/cf-property#mole_concentration_of_methyl_bromide_in_air>
  a owl:NamedIndividual, <http://purl.oclc.org/NET/ssnx/qu/dim#Concentration> ;
  rdfs:label "mole concentration of methyl bromide in air" ;
  rdfs:isDefinedBy <http://purl.oclc.org/NET/ssnx/cf/cf-property> ;
  rdfs:comment " Mole concentration means number of moles per unit volume, also called molarity, and is used in the construction mole_concentration_of_X_in_Y, where X is a material constituent of Y.  A chemical species denoted by X may be described by a single term such as 'nitrogen' or a phrase such as 'nox_expressed_as_nitrogen'. The chemical formula for methyl bromide is CH3Br. The IUPAC name for methyl bromide is bromomethane." .

<http://purl.oclc.org/NET/ssnx/cf/cf-property#mole_concentration_of_methyl_chloride_in_air>
  a owl:NamedIndividual, <http://purl.oclc.org/NET/ssnx/qu/dim#Concentration> ;
  rdfs:label "mole concentration of methyl chloride in air" ;
  rdfs:isDefinedBy <http://purl.oclc.org/NET/ssnx/cf/cf-property> ;
  rdfs:comment " Mole concentration means number of moles per unit volume, also called molarity, and is used in the construction mole_concentration_of_X_in_Y, where X is a material constituent of Y.  A chemical species denoted by X may be described by a single term such as 'nitrogen' or a phrase such as 'nox_expressed_as_nitrogen'. The chemical formula for methyl chloride is CH3Cl. The IUPAC name for methyl chloride is chloromethane." .

<http://purl.oclc.org/NET/ssnx/cf/cf-property#mole_concentration_of_methyl_hydroperoxide_in_air>
  a owl:NamedIndividual, <http://purl.oclc.org/NET/ssnx/qu/dim#Concentration> ;
  rdfs:label "mole concentration of methyl hydroperoxide in air" ;
  rdfs:isDefinedBy <http://purl.oclc.org/NET/ssnx/cf/cf-property> ;
  rdfs:comment " Mole concentration means number of moles per unit volume, also called molarity, and is used in the construction mole_concentration_of_X_in_Y, where X is a material constituent of Y.  A chemical species denoted by X may be described by a single term such as 'nitrogen' or a phrase such as 'nox_expressed_as_nitrogen'. The chemical formula for methyl hydroperoxide is CH3OOH." .

<http://purl.oclc.org/NET/ssnx/cf/cf-property#mole_concentration_of_methyl_peroxy_radical_in_air>
  a owl:NamedIndividual, <http://purl.oclc.org/NET/ssnx/qu/dim#Concentration> ;
  rdfs:label "mole concentration of methyl peroxy radical in air" ;
  rdfs:isDefinedBy <http://purl.oclc.org/NET/ssnx/cf/cf-property> ;
  rdfs:comment " Mole concentration means number of moles per unit volume, also called molarity, and is used in the construction mole_concentration_of_X_in_Y, where X is a material constituent of Y.  A chemical species denoted by X may be described by a single term such as 'nitrogen' or a phrase such as 'nox_expressed_as_nitrogen'. The chemical formula for methyl_peroxy_radical is CH3O2. In chemistry, a 'radical' is a highly reactive, and therefore shortlived, species." .

<http://purl.oclc.org/NET/ssnx/cf/cf-property#mole_concentration_of_molecular_hydrogen_in_air>
  a owl:NamedIndividual, <http://purl.oclc.org/NET/ssnx/qu/dim#Concentration> ;
  rdfs:label "mole concentration of molecular hydrogen in air" ;
  rdfs:isDefinedBy <http://purl.oclc.org/NET/ssnx/cf/cf-property> ;
  rdfs:comment " Mole concentration means number of moles per unit volume, also called molarity, and is used in the construction mole_concentration_of_X_in_Y, where X is a material constituent of Y.  A chemical species denoted by X may be described by a single term such as 'nitrogen' or a phrase such as 'nox_expressed_as_nitrogen'. The chemical formula for molecular hydrogen is H2." .

<http://purl.oclc.org/NET/ssnx/cf/cf-property#mole_concentration_of_nitrate_radical_in_air>
  a owl:NamedIndividual, <http://purl.oclc.org/NET/ssnx/qu/dim#Concentration> ;
  rdfs:label "mole concentration of nitrate radical in air" ;
  rdfs:isDefinedBy <http://purl.oclc.org/NET/ssnx/cf/cf-property> ;
  rdfs:comment " Mole concentration means number of moles per unit volume, also called molarity, and is used in the construction mole_concentration_of_X_in_Y, where X is a material constituent of Y.  A chemical species denoted by X may be described by a single term such as 'nitrogen' or a phrase such as 'nox_expressed_as_nitrogen'. In chemistry, a 'radical' is a highly reactive, and therefore shortlived, species." .

<http://purl.oclc.org/NET/ssnx/cf/cf-property#mole_concentration_of_nitric_acid_in_air>
  a owl:NamedIndividual, <http://purl.oclc.org/NET/ssnx/qu/dim#Concentration> ;
  rdfs:label "mole concentration of nitric acid in air" ;
  rdfs:isDefinedBy <http://purl.oclc.org/NET/ssnx/cf/cf-property> ;
  rdfs:comment " Mole concentration means number of moles per unit volume, also called molarity, and is used in the construction mole_concentration_of_X_in_Y, where X is a material constituent of Y.  A chemical species denoted by X may be described by a single term such as 'nitrogen' or a phrase such as 'nox_expressed_as_nitrogen'. The chemical formula for nitric acid is HNO3." .

<http://purl.oclc.org/NET/ssnx/cf/cf-property#mole_concentration_of_nitric_acid_trihydrate_ambient_aerosol_in_air>
  a owl:NamedIndividual, <http://purl.oclc.org/NET/ssnx/qu/dim#Concentration> ;
  rdfs:label "mole concentration of nitric acid trihydrate ambient aerosol in air" ;
  rdfs:isDefinedBy <http://purl.oclc.org/NET/ssnx/cf/cf-property> ;
  rdfs:comment " Mole concentration means number of moles per unit volume, also called molarity, and is used in the construction mole_concentration_of_X_in_Y, where X is a material constituent of Y.  A chemical species denoted by X may be described by a single term such as 'nitrogen' or a phrase such as 'nox_expressed_as_nitrogen'. Aerosol means the suspended liquid or solid particles in air (except cloud droplets).  Ambient aerosol is aerosol that has taken up ambient water through hygroscopic growth. The extent of hygroscopic growth depends on the relative humidity and the composition of the aerosol. The chemical formula for nitric acid is HNO3. Nitric acid trihydrate, sometimes referred to as NAT, is a stable crystalline substance consisting of three molecules of water to one molecule of nitric acid." .

<http://purl.oclc.org/NET/ssnx/cf/cf-property#mole_concentration_of_nitrogen_dioxide_in_air>
  a owl:NamedIndividual, <http://purl.oclc.org/NET/ssnx/qu/dim#Concentration> ;
  rdfs:label "mole concentration of nitrogen dioxide in air" ;
  rdfs:isDefinedBy <http://purl.oclc.org/NET/ssnx/cf/cf-property> ;
  rdfs:comment " Mole concentration means number of moles per unit volume, also called molarity, and is used in the construction mole_concentration_of_X_in_Y, where X is a material constituent of Y.  A chemical species denoted by X may be described by a single term such as 'nitrogen' or a phrase such as 'nox_expressed_as_nitrogen'. The chemical formula for nitrogen dioxide is NO2." .

<http://purl.oclc.org/NET/ssnx/cf/cf-property#mole_concentration_of_nitrogen_monoxide_in_air>
  a owl:NamedIndividual, <http://purl.oclc.org/NET/ssnx/qu/dim#Concentration> ;
  rdfs:label "mole concentration of nitrogen monoxide in air" ;
  rdfs:isDefinedBy <http://purl.oclc.org/NET/ssnx/cf/cf-property> ;
  rdfs:comment " Mole concentration means number of moles per unit volume, also called molarity, and is used in the construction mole_concentration_of_X_in_Y, where X is a material constituent of Y.  A chemical species denoted by X may be described by a single term such as 'nitrogen' or a phrase such as 'nox_expressed_as_nitrogen'. The chemical formula for nitrogen monoxide is NO." .

<http://purl.oclc.org/NET/ssnx/cf/cf-property#mole_concentration_of_nitrous_acid_in_air>
  a owl:NamedIndividual, <http://purl.oclc.org/NET/ssnx/qu/dim#Concentration> ;
  rdfs:label "mole concentration of nitrous acid in air" ;
  rdfs:isDefinedBy <http://purl.oclc.org/NET/ssnx/cf/cf-property> ;
  rdfs:comment " Mole concentration means number of moles per unit volume, also called molarity, and is used in the construction mole_concentration_of_X_in_Y, where X is a material constituent of Y.  A chemical species denoted by X may be described by a single term such as 'nitrogen' or a phrase such as 'nox_expressed_as_nitrogen'. The chemical formula for nitrous acid is HNO2." .

<http://purl.oclc.org/NET/ssnx/cf/cf-property#mole_concentration_of_nitrous_oxide_in_air>
  a owl:NamedIndividual, <http://purl.oclc.org/NET/ssnx/qu/dim#Concentration> ;
  rdfs:label "mole concentration of nitrous oxide in air" ;
  rdfs:isDefinedBy <http://purl.oclc.org/NET/ssnx/cf/cf-property> ;
  rdfs:comment " Mole concentration means number of moles per unit volume, also called molarity, and is used in the construction mole_concentration_of_X_in_Y, where X is a material constituent of Y.  A chemical species denoted by X may be described by a single term such as 'nitrogen' or a phrase such as 'nox_expressed_as_nitrogen'. The chemical formula for nitrous oxide is N2O." .

<http://purl.oclc.org/NET/ssnx/cf/cf-property#mole_concentration_of_nmvoc_expressed_as_carbon_in_air>
  a owl:NamedIndividual, <http://purl.oclc.org/NET/ssnx/qu/dim#Concentration> ;
  rdfs:label "mole concentration of nmvoc expressed as carbon in air" ;
  rdfs:isDefinedBy <http://purl.oclc.org/NET/ssnx/cf/cf-property> ;
  rdfs:comment " Mole concentration means number of moles per unit volume, also called molarity, and is used in the construction mole_concentration_of_X_in_Y, where X is a material constituent of Y.  A chemical species denoted by X may be described by a single term such as 'nitrogen' or a phrase such as 'nox_expressed_as_nitrogen'. nmvoc means non methane volatile organic compounds. The phrase 'expressed_as' is used in the construction A_expressed_as_B, where B is a chemical constituent of A. It means that the quantity indicated by the standard name is calculated solely with respect to the B contained inA, neglecting all other chemical constituents of A." .

<http://purl.oclc.org/NET/ssnx/cf/cf-property#mole_concentration_of_nox_expressed_as_nitrogen_in_air>
  a owl:NamedIndividual, <http://purl.oclc.org/NET/ssnx/qu/dim#Concentration> ;
  rdfs:label "mole concentration of nox expressed as nitrogen in air" ;
  rdfs:isDefinedBy <http://purl.oclc.org/NET/ssnx/cf/cf-property> ;
  rdfs:comment " Mole concentration means number of moles per unit volume, also called molarity, and is used in the construction mole_concentration_of_X_in_Y, where X is a material constituent of Y.  A chemical species denoted by X may be described by a single term such as 'nitrogen' or a phrase such as 'nox_expressed_as_nitrogen'. Nox means a combination of two radical species containing nitrogen and oxygen: NO+NO2. The phrase 'expressed_as' is used in the construction A_expressed_as_B, where B is a chemical constituent of A. It means that the quantity indicated by the standard name is calculated solelywith respect to the B contained in A, neglecting all other chemical constituents of A." .

<http://purl.oclc.org/NET/ssnx/cf/cf-property#mole_concentration_of_noy_expressed_as_nitrogen_in_air>
  a owl:NamedIndividual, <http://purl.oclc.org/NET/ssnx/qu/dim#Concentration> ;
  rdfs:label "mole concentration of noy expressed as nitrogen in air" ;
  rdfs:isDefinedBy <http://purl.oclc.org/NET/ssnx/cf/cf-property> ;
  rdfs:comment " Mole concentration means number of moles per unit volume, also called molarity, and is used in the construction mole_concentration_of_X_in_Y, where X is a material constituent of Y.  A chemical species denoted by X may be described by a single term such as 'nitrogen' or a phrase such as 'nox_expressed_as_nitrogen'. Noy describes a family of chemical species. The family usually includes atomic nitrogen (N), nitrogen monoxide (NO), nitrogen dioxide (NO2), dinitrogen pentoxide (N2O5), nitric acid (HNO3), peroxynitric acid (HNO4), bromine nitrate (BrONO2) , chlorine nitrate (ClONO2) and organic nitrates (most notably peroxyacetyl nitrate, sometimes referred to as PAN, (CH3COO2NO2)). The list of individual species that are included in a quantity having a group chemical standard name can vary between models.  Where possible, the data variable should be accompanied by a complete description of the species represented, for example, by using a comment attribute. The phrase 'expressed_as' is used in the construction A_expressed_as_B, where B is a chemical constituent of A. It means that the quantity indicated by the standard name iscalculated solely with respect to the B contained in A, neglecting all other chemical constituents of A." .

<http://purl.oclc.org/NET/ssnx/cf/cf-property#mole_concentration_of_ozone_in_air>
  a owl:NamedIndividual, <http://purl.oclc.org/NET/ssnx/qu/dim#Concentration> ;
  rdfs:label "mole concentration of ozone in air" ;
  rdfs:isDefinedBy <http://purl.oclc.org/NET/ssnx/cf/cf-property> ;
  rdfs:comment " Mole concentration means number of moles per unit volume, also called molarity, and is used in the construction mole_concentration_of_X_in_Y, where X is a material constituent of Y.  A chemical species denoted by X may be described by a single term such as 'nitrogen' or a phrase such as 'nox_expressed_as_nitrogen'. The chemical formula for ozone is O3." .

<http://purl.oclc.org/NET/ssnx/cf/cf-property#mole_concentration_of_peroxyacetyl_nitrate_in_air>
  a owl:NamedIndividual, <http://purl.oclc.org/NET/ssnx/qu/dim#Concentration> ;
  rdfs:label "mole concentration of peroxyacetyl nitrate in air" ;
  rdfs:isDefinedBy <http://purl.oclc.org/NET/ssnx/cf/cf-property> ;
  rdfs:comment " Mole concentration means number of moles per unit volume, also called molarity, and is used in the construction mole_concentration_of_X_in_Y, where X is a material constituent of Y.  A chemical species denoted by X may be described by a single term such as 'nitrogen' or a phrase such as 'nox_expressed_as_nitrogen'. The chemical formula for peroxyacetyl nitrate, sometimes referred to as PAN, is CH3COO2NO2.  The IUPAC namefor peroxyacetyl_nitrate is nitroethaneperoxoate." .

<http://purl.oclc.org/NET/ssnx/cf/cf-property#mole_concentration_of_peroxynitric_acid_in_air>
  a owl:NamedIndividual, <http://purl.oclc.org/NET/ssnx/qu/dim#Concentration> ;
  rdfs:label "mole concentration of peroxynitric acid in air" ;
  rdfs:isDefinedBy <http://purl.oclc.org/NET/ssnx/cf/cf-property> ;
  rdfs:comment " Mole concentration means number of moles per unit volume, also called molarity, and is used in the construction mole_concentration_of_X_in_Y, where X is a material constituent of Y.  A chemical species denoted by X may be described by a single term such as 'nitrogen' or a phrase such as 'nox_expressed_as_nitrogen'. The chemical formula for peroxynitric acid, sometimes referred to as PNA, is HO2NO2." .

<http://purl.oclc.org/NET/ssnx/cf/cf-property#mole_concentration_of_propane_in_air>
  a owl:NamedIndividual, <http://purl.oclc.org/NET/ssnx/qu/dim#Concentration> ;
  rdfs:label "mole concentration of propane in air" ;
  rdfs:isDefinedBy <http://purl.oclc.org/NET/ssnx/cf/cf-property> ;
  rdfs:comment " Mole concentration means number of moles per unit volume, also called molarity, and is used in the construction mole_concentration_of_X_in_Y, where X is a material constituent of Y.  A chemical species denoted by X may be described by a single term such as 'nitrogen' or a phrase such as 'nox_expressed_as_nitrogen'. The chemical formula for propane is C3H8. Propane is a member of the group of hydrocarbons known as alkanes.  There are standard names for the alkane group as well as for some of the individual species." .

<http://purl.oclc.org/NET/ssnx/cf/cf-property#mole_concentration_of_propene_in_air>
  a owl:NamedIndividual, <http://purl.oclc.org/NET/ssnx/qu/dim#Concentration> ;
  rdfs:label "mole concentration of propene in air" ;
  rdfs:isDefinedBy <http://purl.oclc.org/NET/ssnx/cf/cf-property> ;
  rdfs:comment " Mole concentration means number of moles per unit volume, also called molarity, and is used in the construction mole_concentration_of_X_in_Y, where X is a material constituent of Y.  A chemical species denoted by X may be described by a single term such as 'nitrogen' or a phrase such as 'nox_expressed_as_nitrogen'. The chemical formula for propene is C3H6. Propene is a member of the group of hydrocarbons known as alkenes.  There are standard names for the alkene group as well as for some of the individual species." .

<http://purl.oclc.org/NET/ssnx/cf/cf-property#mole_concentration_of_radon_in_air>
  a owl:NamedIndividual, <http://purl.oclc.org/NET/ssnx/qu/dim#Concentration> ;
  rdfs:label "mole concentration of radon in air" ;
  rdfs:isDefinedBy <http://purl.oclc.org/NET/ssnx/cf/cf-property> ;
  rdfs:comment " Mole concentration means number of moles per unit volume, also called molarity, and is used in the construction mole_concentration_of_X_in_Y, where X is a material constituent of Y.  A chemical species denoted by X may be described by a single term such as 'nitrogen' or a phrase such as 'nox_expressed_as_nitrogen'. The chemical symbol for radon is Rn." .

<http://purl.oclc.org/NET/ssnx/cf/cf-property#mole_concentration_of_sulfur_dioxide_in_air>
  a owl:NamedIndividual, <http://purl.oclc.org/NET/ssnx/qu/dim#Concentration> ;
  rdfs:label "mole concentration of sulfur dioxide in air" ;
  rdfs:isDefinedBy <http://purl.oclc.org/NET/ssnx/cf/cf-property> ;
  rdfs:comment " Mole concentration means number of moles per unit volume, also called molarity, and is used in the construction mole_concentration_of_X_in_Y, where X is a material constituent of Y.  A chemical species denoted by X may be described by a single term such as 'nitrogen' or a phrase such as 'nox_expressed_as_nitrogen'. The chemical formula for sulfur dioxide is SO2." .

<http://purl.oclc.org/NET/ssnx/cf/cf-property#mole_concentration_of_toluene_in_air>
  a owl:NamedIndividual, <http://purl.oclc.org/NET/ssnx/qu/dim#Concentration> ;
  rdfs:label "mole concentration of toluene in air" ;
  rdfs:isDefinedBy <http://purl.oclc.org/NET/ssnx/cf/cf-property> ;
  rdfs:comment " Mole concentration means number of moles per unit volume, also called molarity, and is used in the construction mole_concentration_of_X_in_Y, where X is a material constituent of Y.  A chemical species denoted by X may be described by a single term such as 'nitrogen' or a phrase such as 'nox_expressed_as_nitrogen'. The chemical formula for toluene is C6H5CH3.  Toluene has the same structure as benzene, except that one ofthe hydrogen atoms is replaced by a methyl group.  The systematic name for toluene is methylbenzene." .

<http://purl.oclc.org/NET/ssnx/cf/cf-property#mole_concentration_of_water_vapor_in_air>
  a owl:NamedIndividual, <http://purl.oclc.org/NET/ssnx/qu/dim#Concentration> ;
  rdfs:label "mole concentration of water vapor in air" ;
  rdfs:isDefinedBy <http://purl.oclc.org/NET/ssnx/cf/cf-property> ;
  rdfs:comment " Mole concentration means number of moles per unit volume, also called molarity, and is used in the construction mole_concentration_of_X_in_Y, where X is a material constituent of Y.  A chemical species denoted by X may be described by a single term such as 'nitrogen' or a phrase such as 'nox_expressed_as_nitrogen'." .

<http://purl.oclc.org/NET/ssnx/cf/cf-property#mole_concentration_of_xylene_in_air>
  a owl:NamedIndividual, <http://purl.oclc.org/NET/ssnx/qu/dim#Concentration> ;
  rdfs:label "mole concentration of xylene in air" ;
  rdfs:isDefinedBy <http://purl.oclc.org/NET/ssnx/cf/cf-property> ;
  rdfs:comment " Mole concentration means number of moles per unit volume, also called molarity, and is used in the construction mole_concentration_of_X_in_Y, where X is a material constituent of Y.  A chemical species denoted by X may be described by a single term such as 'nitrogen' or a phrase such as 'nox_expressed_as_nitrogen'. The chemical formula for xylene is C6H4C2H6. In chemistry, xylene is a generic term for a group of three isomers of dimethylbenzene. The IUPAC names for the isomers are 1,2-dimethylbenzene, 1,3-dimethylbenzene and 1,4-dimethylbenzene. Xylene is an aromatic hydrocarbon. There are standard names that refer to aromatic_compounds as a group, as well as those for individual species." .

<http://purl.oclc.org/NET/ssnx/cf/cf-property#mole_fraction_of_acetic_acid_in_air>
  a owl:NamedIndividual, <http://purl.oclc.org/NET/ssnx/qu/dim#Dimensionless> ;
  rdfs:label "mole fraction of acetic acid in air" ;
  rdfs:isDefinedBy <http://purl.oclc.org/NET/ssnx/cf/cf-property> ;
  rdfs:comment " Mole fraction is used in the construction mole_fraction_of_X_in_Y, whereX is a material constituent of Y.  A chemical species denoted by X may be described by a single term such as 'nitrogen' or a phrase such as 'nox_expressed_as_nitrogen'. The chemicalformula for acetic_acid is CH3COOH. The IUPAC name for acetic acid is ethanoic acid." .

<http://purl.oclc.org/NET/ssnx/cf/cf-property#mole_fraction_of_aceto_nitrile_in_air>
  a owl:NamedIndividual, <http://purl.oclc.org/NET/ssnx/qu/dim#Dimensionless> ;
  rdfs:label "mole fraction of aceto nitrile in air" ;
  rdfs:isDefinedBy <http://purl.oclc.org/NET/ssnx/cf/cf-property> ;
  rdfs:comment " Mole fraction is used in the construction mole_fraction_of_X_in_Y, whereX is a material constituent of Y.  A chemical species denoted by X may be described by a single term such as 'nitrogen' or a phrase such as 'nox_expressed_as_nitrogen'. The chemicalformula for aceto-nitrile is CH3CN. The IUPAC name for aceto-nitrile is ethanenitrile." .

<http://purl.oclc.org/NET/ssnx/cf/cf-property#mole_fraction_of_alpha_hexachlorocyclohexane_in_air>
  a owl:NamedIndividual, <http://purl.oclc.org/NET/ssnx/qu/dim#Dimensionless> ;
  rdfs:label "mole fraction of alpha hexachlorocyclohexane in air" ;
  rdfs:isDefinedBy <http://purl.oclc.org/NET/ssnx/cf/cf-property> ;
  rdfs:comment "Mole fraction is used in the construction mole_fraction_of_X_in_Y, where X is a material constituent of Y." .

<http://purl.oclc.org/NET/ssnx/cf/cf-property#mole_fraction_of_alpha_pinene_in_air>
  a owl:NamedIndividual, <http://purl.oclc.org/NET/ssnx/qu/dim#Dimensionless> ;
  rdfs:label "mole fraction of alpha pinene in air" ;
  rdfs:isDefinedBy <http://purl.oclc.org/NET/ssnx/cf/cf-property> ;
  rdfs:comment " Mole fraction is used in the construction mole_fraction_of_X_in_Y, whereX is a material constituent of Y.  A chemical species denoted by X may be described by a single term such as 'nitrogen' or a phrase such as 'nox_expressed_as_nitrogen'. The chemicalformula for alpha_pinene is C10H16. The IUPAC name for alpha-pinene is (1S,5S)-2,6,6-trimethylbicyclo[3.1.1]hept-2-ene." .

<http://purl.oclc.org/NET/ssnx/cf/cf-property#mole_fraction_of_ammonia_in_air>
  a owl:NamedIndividual, <http://purl.oclc.org/NET/ssnx/qu/dim#Dimensionless> ;
  rdfs:label "mole fraction of ammonia in air" ;
  rdfs:isDefinedBy <http://purl.oclc.org/NET/ssnx/cf/cf-property> ;
  rdfs:comment " Mole fraction is used in the construction mole_fraction_of_X_in_Y, whereX is a material constituent of Y.  A chemical species denoted by X may be described by a single term such as 'nitrogen' or a phrase such as 'nox_expressed_as_nitrogen'. The chemicalformula for ammonia is NH3." .

<http://purl.oclc.org/NET/ssnx/cf/cf-property#mole_fraction_of_anthropogenic_nmvoc_expressed_as_carbon_in_air>
  a owl:NamedIndividual, <http://purl.oclc.org/NET/ssnx/qu/dim#Dimensionless> ;
  rdfs:label "mole fraction of anthropogenic nmvoc expressed as carbon in air" ;
  rdfs:isDefinedBy <http://purl.oclc.org/NET/ssnx/cf/cf-property> ;
  rdfs:comment " Mole fraction is used in the construction mole_fraction_of_X_in_Y, whereX is a material constituent of Y.  A chemical species denoted by X may be described by a single term such as 'nitrogen' or a phrase such as 'nox_expressed_as_nitrogen'. nmvoc means non methane volatile organic compounds. Anthropogenic means influenced, caused, or created by human activity. The phrase 'expressed_as' is used in the construction A_expressed_as_B, where B is a chemical constituent of A. It means that the quantity indicated by the standard name is calculated solely with respect to the B contained in A, neglecting all other chemical constituents of A." .

<http://purl.oclc.org/NET/ssnx/cf/cf-property#mole_fraction_of_atomic_bromine_in_air>
  a owl:NamedIndividual, <http://purl.oclc.org/NET/ssnx/qu/dim#Dimensionless> ;
  rdfs:label "mole fraction of atomic bromine in air" ;
  rdfs:isDefinedBy <http://purl.oclc.org/NET/ssnx/cf/cf-property> ;
  rdfs:comment "Mole fraction is used in the construction mole_fraction_of_X_in_Y, where X is a material constituent of Y.  The chemical symbol of atomic bromine is Br." .

<http://purl.oclc.org/NET/ssnx/cf/cf-property#mole_fraction_of_atomic_chlorine_in_air>
  a owl:NamedIndividual, <http://purl.oclc.org/NET/ssnx/qu/dim#Dimensionless> ;
  rdfs:label "mole fraction of atomic chlorine in air" ;
  rdfs:isDefinedBy <http://purl.oclc.org/NET/ssnx/cf/cf-property> ;
  rdfs:comment "Mole fraction is used in the construction mole_fraction_of_X_in_Y, where X is a material constituent of Y.  The chemical symbol of atomic chlorine is Cl." .

<http://purl.oclc.org/NET/ssnx/cf/cf-property#mole_fraction_of_atomic_nitrogen_in_air>
  a owl:NamedIndividual, <http://purl.oclc.org/NET/ssnx/qu/dim#Dimensionless> ;
  rdfs:label "mole fraction of atomic nitrogen in air" ;
  rdfs:isDefinedBy <http://purl.oclc.org/NET/ssnx/cf/cf-property> ;
  rdfs:comment "Mole fraction is used in the construction mole_fraction_of_X_in_Y, where X is a material constituent of Y.  The chemical symbol of atomic nitrogen is N." .

<http://purl.oclc.org/NET/ssnx/cf/cf-property#mole_fraction_of_benzene_in_air>
  a owl:NamedIndividual, <http://purl.oclc.org/NET/ssnx/qu/dim#Dimensionless> ;
  rdfs:label "mole fraction of benzene in air" ;
  rdfs:isDefinedBy <http://purl.oclc.org/NET/ssnx/cf/cf-property> ;
  rdfs:comment "Mole fraction is used in the construction mole_fraction_of_X_in_Y, where X is a material constituent of Y." .

<http://purl.oclc.org/NET/ssnx/cf/cf-property#mole_fraction_of_beta_pinene_in_air>
  a owl:NamedIndividual, <http://purl.oclc.org/NET/ssnx/qu/dim#Dimensionless> ;
  rdfs:label "mole fraction of beta pinene in air" ;
  rdfs:isDefinedBy <http://purl.oclc.org/NET/ssnx/cf/cf-property> ;
  rdfs:comment " Mole fraction is used in the construction mole_fraction_of_X_in_Y, whereX is a material constituent of Y.  A chemical species denoted by X may be described by a single term such as 'nitrogen' or a phrase such as 'nox_expressed_as_nitrogen'. The chemicalformula for beta_pinene is C10H16.  The IUPAC name for beta-pinene is (1S,5S)-6,6-dimethyl-2-methylenebicyclo[3.1.1]heptane." .

<http://purl.oclc.org/NET/ssnx/cf/cf-property#mole_fraction_of_biogenic_nmvoc_expressed_as_carbon_in_air>
  a owl:NamedIndividual, <http://purl.oclc.org/NET/ssnx/qu/dim#Dimensionless> ;
  rdfs:label "mole fraction of biogenic nmvoc expressed as carbon in air" ;
  rdfs:isDefinedBy <http://purl.oclc.org/NET/ssnx/cf/cf-property> ;
  rdfs:comment " Mole fraction is used in the construction mole_fraction_of_X_in_Y, whereX is a material constituent of Y.  A chemical species denoted by X may be described by a single term such as 'nitrogen' or a phrase such as 'nox_expressed_as_nitrogen'. nmvoc means non methane volatile organic compounds. Biogenic means influenced, caused, or created by natural processes. The phrase 'expressed_as' is used in the construction A_expressed_as_B, where B is a chemical constituent of A. It means that the quantity indicated by the standard name is calculated solely with respect to the B contained in A, neglecting all other chemical constituents of A." .

<http://purl.oclc.org/NET/ssnx/cf/cf-property#mole_fraction_of_bromine_chloride_in_air>
  a owl:NamedIndividual, <http://purl.oclc.org/NET/ssnx/qu/dim#Dimensionless> ;
  rdfs:label "mole fraction of bromine chloride in air" ;
  rdfs:isDefinedBy <http://purl.oclc.org/NET/ssnx/cf/cf-property> ;
  rdfs:comment "Mole fraction is used in the construction mole_fraction_of_X_in_Y, where X is a material constituent of Y.  The chemical formula of bromine chloride is BrCl." .

<http://purl.oclc.org/NET/ssnx/cf/cf-property#mole_fraction_of_bromine_monoxide_in_air>
  a owl:NamedIndividual, <http://purl.oclc.org/NET/ssnx/qu/dim#Dimensionless> ;
  rdfs:label "mole fraction of bromine monoxide in air" ;
  rdfs:isDefinedBy <http://purl.oclc.org/NET/ssnx/cf/cf-property> ;
  rdfs:comment "Mole fraction is used in the construction mole_fraction_of_X_in_Y, where X is a material constituent of Y.  The chemical formula of bromine monoxide is BrO." .

<http://purl.oclc.org/NET/ssnx/cf/cf-property#mole_fraction_of_bromine_nitrate_in_air>
  a owl:NamedIndividual, <http://purl.oclc.org/NET/ssnx/qu/dim#Dimensionless> ;
  rdfs:label "mole fraction of bromine nitrate in air" ;
  rdfs:isDefinedBy <http://purl.oclc.org/NET/ssnx/cf/cf-property> ;
  rdfs:comment "Mole fraction is used in the construction mole_fraction_of_X_in_Y, where X is a material constituent of Y. The chemical formula of bromine nitrate is BrONO2." .

<http://purl.oclc.org/NET/ssnx/cf/cf-property#mole_fraction_of_brox_expressed_as_bromine_in_air>
  a owl:NamedIndividual, <http://purl.oclc.org/NET/ssnx/qu/dim#Dimensionless> ;
  rdfs:label "mole fraction of brox expressed as bromine in air" ;
  rdfs:isDefinedBy <http://purl.oclc.org/NET/ssnx/cf/cf-property> ;
  rdfs:comment " Mole fraction is used in the construction mole_fraction_of_X_in_Y, whereX is a material constituent of Y.  A chemical species denoted by X may be described by a single term such as 'nitrogen' or a phrase such as 'nox_expressed_as_nitrogen'. Brox  describes a family of chemical species consisting of inorganic bromine compounds withthe exception of  hydrogen bromide (HBr) and bromine nitrate (BrONO2). Brox isthe term used in standard names for all species belonging to the family that are represented within a given model. The list of individual species that are included in a quantity with a group chemical standard name can vary between models.  Where possible, the data variable should be accompanied by a complete description of the species represented, for example, by using a comment attribute. Inorganic bromine, sometimes referred to as Bry, describes a family of chemical species which result from the degradation of source gases containing bromine (halons, methyl bromide, VSLS) and natural inorganic bromine sources such as volcanoes, seasalt and other aerosols.  Standard names that use the term inorganic_bromine are used for quantities that contain all inorganic bromine species includingHCl and ClONO2. The phrase 'expressed_as' is used in the construction A_expressed_as_B, where B is a chemical constituent of A. It means that the quantity indicated by the standard name is calculated solely with respect to the B contained in A, neglecting all other chemical constituents of A." .

<http://purl.oclc.org/NET/ssnx/cf/cf-property#mole_fraction_of_butane_in_air>
  a owl:NamedIndividual, <http://purl.oclc.org/NET/ssnx/qu/dim#Dimensionless> ;
  rdfs:label "mole fraction of butane in air" ;
  rdfs:isDefinedBy <http://purl.oclc.org/NET/ssnx/cf/cf-property> ;
  rdfs:comment " Mole fraction is used in the construction mole_fraction_of_X_in_Y, whereX is a material constituent of Y.  A chemical species denoted by X may be described by a single term such as 'nitrogen' or a phrase such as 'nox_expressed_as_nitrogen'. The chemicalformula for butane is C4H10. Butane is a member of the group of hydrocarbons known as alkanes.  There are standard names for the alkane group as well as for some of the individual species." .

<http://purl.oclc.org/NET/ssnx/cf/cf-property#mole_fraction_of_carbon_dioxide_in_air>
  a owl:NamedIndividual, <http://purl.oclc.org/NET/ssnx/qu/dim#Dimensionless> ;
  rdfs:label "mole fraction of carbon dioxide in air" ;
  rdfs:isDefinedBy <http://purl.oclc.org/NET/ssnx/cf/cf-property> ;
  rdfs:comment "Mole fraction is used in the construction mole_fraction_of_X_in_Y, where X is a material constituent of Y." .

<http://purl.oclc.org/NET/ssnx/cf/cf-property#mole_fraction_of_carbon_monoxide_in_air>
  a owl:NamedIndividual, <http://purl.oclc.org/NET/ssnx/qu/dim#Dimensionless> ;
  rdfs:label "mole fraction of carbon monoxide in air" ;
  rdfs:isDefinedBy <http://purl.oclc.org/NET/ssnx/cf/cf-property> ;
  rdfs:comment "Mole fraction is used in the construction mole_fraction_of_X_in_Y, where X is a material constituent of Y." .

<http://purl.oclc.org/NET/ssnx/cf/cf-property#mole_fraction_of_carbon_tetrachloride_in_air>
  a owl:NamedIndividual, <http://purl.oclc.org/NET/ssnx/qu/dim#Dimensionless> ;
  rdfs:label "mole fraction of carbon tetrachloride in air" ;
  rdfs:isDefinedBy <http://purl.oclc.org/NET/ssnx/cf/cf-property> ;
  rdfs:comment "Mole fraction is used in the construction mole_fraction_of_X_in_Y, where X is a material constituent of Y.  The chemical formula of carbon tetrachloride is CCl4." .

<http://purl.oclc.org/NET/ssnx/cf/cf-property#mole_fraction_of_cfc113_in_air>
  a owl:NamedIndividual, <http://purl.oclc.org/NET/ssnx/qu/dim#Dimensionless> ;
  rdfs:label "mole fraction of cfc113 in air" ;
  rdfs:isDefinedBy <http://purl.oclc.org/NET/ssnx/cf/cf-property> ;
  rdfs:comment "Mole fraction is used in the construction mole_fraction_of_X_in_Y, where X is a material constituent of Y.  The chemical formula of CFC113 is CCl2FCClF2.  The IUPAC name for CFC113 is 1,1,2-trichloro-1,2,2-trifluoro-ethane." .

<http://purl.oclc.org/NET/ssnx/cf/cf-property#mole_fraction_of_cfc113a_in_air>
  a owl:NamedIndividual, <http://purl.oclc.org/NET/ssnx/qu/dim#Dimensionless> ;
  rdfs:label "mole fraction of cfc113a in air" ;
  rdfs:isDefinedBy <http://purl.oclc.org/NET/ssnx/cf/cf-property> ;
  rdfs:comment "Mole fraction is used in the construction mole_fraction_of_X_in_Y, where X is a material constituent of Y.  The chemical formula of CFC113a CCl3CF3.  The IUPAC name for CFC113a is 1,1,1-trichloro-2,2,2-trifluoro-ethane." .

<http://purl.oclc.org/NET/ssnx/cf/cf-property#mole_fraction_of_cfc114_in_air>
  a owl:NamedIndividual, <http://purl.oclc.org/NET/ssnx/qu/dim#Dimensionless> ;
  rdfs:label "mole fraction of cfc114 in air" ;
  rdfs:isDefinedBy <http://purl.oclc.org/NET/ssnx/cf/cf-property> ;
  rdfs:comment "Mole fraction is used in the construction mole_fraction_of_X_in_Y, where X is a material constituent of Y.  The chemical formula of CFC114 is CClF2CClF2.  The IUPAC name for CFC114 is 1,2-dichloro-1,1,2,2-tetrafluoro-ethane." .

<http://purl.oclc.org/NET/ssnx/cf/cf-property#mole_fraction_of_cfc115_in_air>
  a owl:NamedIndividual, <http://purl.oclc.org/NET/ssnx/qu/dim#Dimensionless> ;
  rdfs:label "mole fraction of cfc115 in air" ;
  rdfs:isDefinedBy <http://purl.oclc.org/NET/ssnx/cf/cf-property> ;
  rdfs:comment "Mole fraction is used in the construction mole_fraction_of_X_in_Y, where X is a material constituent of Y.  The chemical formula of CFC115 is CClF2CF3.  The IUPAC name for CFC115 is 1-chloro-1,1,2,2,2-pentafluoro-ethane." .

<http://purl.oclc.org/NET/ssnx/cf/cf-property#mole_fraction_of_cfc11_in_air>
  a owl:NamedIndividual, <http://purl.oclc.org/NET/ssnx/qu/dim#Dimensionless> ;
  rdfs:label "mole fraction of cfc11 in air" ;
  rdfs:isDefinedBy <http://purl.oclc.org/NET/ssnx/cf/cf-property> ;
  rdfs:comment "Mole fraction is used in the construction mole_fraction_of_X_in_Y, where X is a material constituent of Y.  The chemical formula of CFC11 is CFCl3.  The IUPAC name for CFC11 is trichloro-fluoro-methane." .

<http://purl.oclc.org/NET/ssnx/cf/cf-property#mole_fraction_of_cfc12_in_air>
  a owl:NamedIndividual, <http://purl.oclc.org/NET/ssnx/qu/dim#Dimensionless> ;
  rdfs:label "mole fraction of cfc12 in air" ;
  rdfs:isDefinedBy <http://purl.oclc.org/NET/ssnx/cf/cf-property> ;
  rdfs:comment "Mole fraction is used in the construction mole_fraction_of_X_in_Y, where X is a material constituent of Y.  The chemical formula of CFC12 is CF2Cl2.  The IUPAC name for CFC12 is dichloro-difluoro-methane." .

<http://purl.oclc.org/NET/ssnx/cf/cf-property#mole_fraction_of_chlorine_dioxide_in_air>
  a owl:NamedIndividual, <http://purl.oclc.org/NET/ssnx/qu/dim#Dimensionless> ;
  rdfs:label "mole fraction of chlorine dioxide in air" ;
  rdfs:isDefinedBy <http://purl.oclc.org/NET/ssnx/cf/cf-property> ;
  rdfs:comment "Mole fraction is used in the construction mole_fraction_of_X_in_Y, where X is a material constituent of Y.  The chemical formula of chlorine dioxide is OClO." .

<http://purl.oclc.org/NET/ssnx/cf/cf-property#mole_fraction_of_chlorine_monoxide_in_air>
  a owl:NamedIndividual, <http://purl.oclc.org/NET/ssnx/qu/dim#Dimensionless> ;
  rdfs:label "mole fraction of chlorine monoxide in air" ;
  rdfs:isDefinedBy <http://purl.oclc.org/NET/ssnx/cf/cf-property> ;
  rdfs:comment "Mole fraction is used in the construction mole_fraction_of_X_in_Y, where X is a material constituent of Y.  The chemical formula of chlorine monoxide is ClO." .

<http://purl.oclc.org/NET/ssnx/cf/cf-property#mole_fraction_of_chlorine_nitrate_in_air>
  a owl:NamedIndividual, <http://purl.oclc.org/NET/ssnx/qu/dim#Dimensionless> ;
  rdfs:label "mole fraction of chlorine nitrate in air" ;
  rdfs:isDefinedBy <http://purl.oclc.org/NET/ssnx/cf/cf-property> ;
  rdfs:comment "Mole fraction is used in the construction mole_fraction_of_X_in_Y, where X is a material constituent of Y.  The chemical formula of chlorine nitrate is ClONO2." .

<http://purl.oclc.org/NET/ssnx/cf/cf-property#mole_fraction_of_clox_expressed_as_chlorine_in_air>
  a owl:NamedIndividual, <http://purl.oclc.org/NET/ssnx/qu/dim#Dimensionless> ;
  rdfs:label "mole fraction of clox expressed as chlorine in air" ;
  rdfs:isDefinedBy <http://purl.oclc.org/NET/ssnx/cf/cf-property> ;
  rdfs:comment " Mole fraction is used in the construction mole_fraction_of_X_in_Y, whereX is a material constituent of Y.  A chemical species denoted by X may be described by a single term such as 'nitrogen' or a phrase such as 'nox_expressed_as_nitrogen'. Clox describes a family of chemical species consisting of inorganic chlorine compounds withthe exception of  hydrogen chloride (HCl) and chlorine nitrate (ClONO2). Clox is the term used in standard names for all species belonging to the family that are represented within a given model. The list of individual species that are included in a quantity with a group chemical standard name can vary between models.  Where possible, the data variable should be accompanied by a complete description of the species represented, for example, by using a comment attribute. Inorganic chlorine, sometimes referred to as Cly, describes a family of chemical species which result from the degradation of source gasescontaining chlorine (CFCs, HCFCs, VSLS) and natural inorganic chlorine sources such as seasalt and other aerosols.   Standard names that use the term inorganic_chlorine are used for quantities that contain all inorganic chlorine species including HCl and ClONO2. The phrase 'expressed_as' is used in the construction A_expressed_as_B, where B is a chemical constituent of A. It means that the quantity indicated by the standard name is calculated solely with respect to the B contained in A, neglecting all other chemical constituents of A." .

<http://purl.oclc.org/NET/ssnx/cf/cf-property#mole_fraction_of_dichlorine_peroxide_in_air>
  a owl:NamedIndividual, <http://purl.oclc.org/NET/ssnx/qu/dim#Dimensionless> ;
  rdfs:label "mole fraction of dichlorine peroxide in air" ;
  rdfs:isDefinedBy <http://purl.oclc.org/NET/ssnx/cf/cf-property> ;
  rdfs:comment "Mole fraction is used in the construction mole_fraction_of_X_in_Y, where X is a material constituent of Y.   The chemical formula of dichlorine peroxide is Cl2O2." .

<http://purl.oclc.org/NET/ssnx/cf/cf-property#mole_fraction_of_dimethyl_sulfide_in_air>
  a owl:NamedIndividual, <http://purl.oclc.org/NET/ssnx/qu/dim#Dimensionless> ;
  rdfs:label "mole fraction of dimethyl sulfide in air" ;
  rdfs:isDefinedBy <http://purl.oclc.org/NET/ssnx/cf/cf-property> ;
  rdfs:comment "Mole fraction is used in the construction mole_fraction_of_X_in_Y, where X is a material constituent of Y." .

<http://purl.oclc.org/NET/ssnx/cf/cf-property#mole_fraction_of_dinitrogen_pentoxide_in_air>
  a owl:NamedIndividual, <http://purl.oclc.org/NET/ssnx/qu/dim#Dimensionless> ;
  rdfs:label "mole fraction of dinitrogen pentoxide in air" ;
  rdfs:isDefinedBy <http://purl.oclc.org/NET/ssnx/cf/cf-property> ;
  rdfs:comment "Mole fraction is used in the construction mole_fraction_of_X_in_Y, where X is a material constituent of Y.  The chemical formula of dinitrogen pentoxide is N2O5." .

<http://purl.oclc.org/NET/ssnx/cf/cf-property#mole_fraction_of_ethane_in_air>
  a owl:NamedIndividual, <http://purl.oclc.org/NET/ssnx/qu/dim#Dimensionless> ;
  rdfs:label "mole fraction of ethane in air" ;
  rdfs:isDefinedBy <http://purl.oclc.org/NET/ssnx/cf/cf-property> ;
  rdfs:comment "Mole fraction is used in the construction mole_fraction_of_X_in_Y, where X is a material constituent of Y." .

<http://purl.oclc.org/NET/ssnx/cf/cf-property#mole_fraction_of_ethanol_in_air>
  a owl:NamedIndividual, <http://purl.oclc.org/NET/ssnx/qu/dim#Dimensionless> ;
  rdfs:label "mole fraction of ethanol in air" ;
  rdfs:isDefinedBy <http://purl.oclc.org/NET/ssnx/cf/cf-property> ;
  rdfs:comment " Mole fraction is used in the construction mole_fraction_of_X_in_Y, whereX is a material constituent of Y.  A chemical species denoted by X may be described by a single term such as 'nitrogen' or a phrase such as 'nox_expressed_as_nitrogen'. The chemicalformula for ethanol is C2H5OH." .

<http://purl.oclc.org/NET/ssnx/cf/cf-property#mole_fraction_of_ethene_in_air>
  a owl:NamedIndividual, <http://purl.oclc.org/NET/ssnx/qu/dim#Dimensionless> ;
  rdfs:label "mole fraction of ethene in air" ;
  rdfs:isDefinedBy <http://purl.oclc.org/NET/ssnx/cf/cf-property> ;
  rdfs:comment "Mole fraction is used in the construction mole_fraction_of_X_in_Y, where X is a material constituent of Y." .

<http://purl.oclc.org/NET/ssnx/cf/cf-property#mole_fraction_of_ethyne_in_air>
  a owl:NamedIndividual, <http://purl.oclc.org/NET/ssnx/qu/dim#Dimensionless> ;
  rdfs:label "mole fraction of ethyne in air" ;
  rdfs:isDefinedBy <http://purl.oclc.org/NET/ssnx/cf/cf-property> ;
  rdfs:comment "Mole fraction is used in the construction mole_fraction_of_X_in_Y, where X is a material constituent of Y." .

<http://purl.oclc.org/NET/ssnx/cf/cf-property#mole_fraction_of_formaldehyde_in_air>
  a owl:NamedIndividual, <http://purl.oclc.org/NET/ssnx/qu/dim#Dimensionless> ;
  rdfs:label "mole fraction of formaldehyde in air" ;
  rdfs:isDefinedBy <http://purl.oclc.org/NET/ssnx/cf/cf-property> ;
  rdfs:comment "Mole fraction is used in the construction mole_fraction_of_X_in_Y, where X is a material constituent of Y." .

<http://purl.oclc.org/NET/ssnx/cf/cf-property#mole_fraction_of_formic_acid_in_air>
  a owl:NamedIndividual, <http://purl.oclc.org/NET/ssnx/qu/dim#Dimensionless> ;
  rdfs:label "mole fraction of formic acid in air" ;
  rdfs:isDefinedBy <http://purl.oclc.org/NET/ssnx/cf/cf-property> ;
  rdfs:comment " Mole fraction is used in the construction mole_fraction_of_X_in_Y, whereX is a material constituent of Y.  A chemical species denoted by X may be described by a single term such as 'nitrogen' or a phrase such as 'nox_expressed_as_nitrogen'. The chemicalformula for formic acid is HCOOH.  The IUPAC name for formic acid is methanoic acid." .

<http://purl.oclc.org/NET/ssnx/cf/cf-property#mole_fraction_of_gaseous_divalent_mercury_in_air>
  a owl:NamedIndividual, <http://purl.oclc.org/NET/ssnx/qu/dim#Dimensionless> ;
  rdfs:label "mole fraction of gaseous divalent mercury in air" ;
  rdfs:isDefinedBy <http://purl.oclc.org/NET/ssnx/cf/cf-property> ;
  rdfs:comment "Mole fraction is used in the construction mole_fraction_of_X_in_Y, where X is a material constituent of Y.  Divalent mercury means all compounds in which the mercury has two binding sites to other ion(s) in a salt or to other atom(s) in a molecule. " .

<http://purl.oclc.org/NET/ssnx/cf/cf-property#mole_fraction_of_gaseous_elemental_mercury_in_air>
  a owl:NamedIndividual, <http://purl.oclc.org/NET/ssnx/qu/dim#Dimensionless> ;
  rdfs:label "mole fraction of gaseous elemental mercury in air" ;
  rdfs:isDefinedBy <http://purl.oclc.org/NET/ssnx/cf/cf-property> ;
  rdfs:comment "Mole fraction is used in the construction mole_fraction_of_X_in_Y, where X is a material constituent of Y." .

<http://purl.oclc.org/NET/ssnx/cf/cf-property#mole_fraction_of_halon1202_in_air>
  a owl:NamedIndividual, <http://purl.oclc.org/NET/ssnx/qu/dim#Dimensionless> ;
  rdfs:label "mole fraction of halon1202 in air" ;
  rdfs:isDefinedBy <http://purl.oclc.org/NET/ssnx/cf/cf-property> ;
  rdfs:comment "Mole fraction is used in the construction mole_fraction_of_X_in_Y, where X is a material constituent of Y.  The chemical formula of  halon1202  is CBr2F2.  The IUPAC name for halon 1202 is dibromo-difluoro-methane." .

<http://purl.oclc.org/NET/ssnx/cf/cf-property#mole_fraction_of_halon1211_in_air>
  a owl:NamedIndividual, <http://purl.oclc.org/NET/ssnx/qu/dim#Dimensionless> ;
  rdfs:label "mole fraction of halon1211 in air" ;
  rdfs:isDefinedBy <http://purl.oclc.org/NET/ssnx/cf/cf-property> ;
  rdfs:comment "Mole fraction is used in the construction mole_fraction_of_X_in_Y, where X is a material constituent of Y.  The chemical formula of halon1211 is CBrClF2.  The IUPAC name for halon 1211 is bromo-chloro-difluoro-methane." .

<http://purl.oclc.org/NET/ssnx/cf/cf-property#mole_fraction_of_halon1301_in_air>
  a owl:NamedIndividual, <http://purl.oclc.org/NET/ssnx/qu/dim#Dimensionless> ;
  rdfs:label "mole fraction of halon1301 in air" ;
  rdfs:isDefinedBy <http://purl.oclc.org/NET/ssnx/cf/cf-property> ;
  rdfs:comment "Mole fraction is used in the construction mole_fraction_of_X_in_Y, where X is a material constituent of Y.  The chemical formula of halon1301 is CBrF3.  The IUPAC name for halon 1301 is bromo-trifluoro-methane." .

<http://purl.oclc.org/NET/ssnx/cf/cf-property#mole_fraction_of_halon2402_in_air>
  a owl:NamedIndividual, <http://purl.oclc.org/NET/ssnx/qu/dim#Dimensionless> ;
  rdfs:label "mole fraction of halon2402 in air" ;
  rdfs:isDefinedBy <http://purl.oclc.org/NET/ssnx/cf/cf-property> ;
  rdfs:comment "Mole fraction is used in the construction mole_fraction_of_X_in_Y, where X is a material constituent of Y.  The chemical formula of halon2402 is C2Br2F4.  The IUPAC name for halon 2402 is 1,2-dibromo-1,1,2,2-tetrafluoro-ethane." .

<http://purl.oclc.org/NET/ssnx/cf/cf-property#mole_fraction_of_hcc140a_in_air>
  a owl:NamedIndividual, <http://purl.oclc.org/NET/ssnx/qu/dim#Dimensionless> ;
  rdfs:label "mole fraction of hcc140a in air" ;
  rdfs:isDefinedBy <http://purl.oclc.org/NET/ssnx/cf/cf-property> ;
  rdfs:comment " Mole fraction is used in the construction mole_fraction_of_X_in_Y, whereX is a material constituent of Y.  A chemical species denoted by X may be described by a single term such as 'nitrogen' or a phrase such as 'nox_expressed_as_nitrogen'. The chemicalformula for hcc140a is CH3CCl3. The IUPAC name for hcc140a is 1,1,1-trichloro-ethane." .

<http://purl.oclc.org/NET/ssnx/cf/cf-property#mole_fraction_of_hcfc141b_in_air>
  a owl:NamedIndividual, <http://purl.oclc.org/NET/ssnx/qu/dim#Dimensionless> ;
  rdfs:label "mole fraction of hcfc141b in air" ;
  rdfs:isDefinedBy <http://purl.oclc.org/NET/ssnx/cf/cf-property> ;
  rdfs:comment " Mole fraction is used in the construction mole_fraction_of_X_in_Y, whereX is a material constituent of Y.  A chemical species denoted by X may be described by a single term such as 'nitrogen' or a phrase such as 'nox_expressed_as_nitrogen'. The chemicalformula for HCFC141b is CH3CCl2F. The IUPAC name for HCFC141b is 1,1-dichloro-1-fluoroethane." .

<http://purl.oclc.org/NET/ssnx/cf/cf-property#mole_fraction_of_hcfc142b_in_air>
  a owl:NamedIndividual, <http://purl.oclc.org/NET/ssnx/qu/dim#Dimensionless> ;
  rdfs:label "mole fraction of hcfc142b in air" ;
  rdfs:isDefinedBy <http://purl.oclc.org/NET/ssnx/cf/cf-property> ;
  rdfs:comment " Mole fraction is used in the construction mole_fraction_of_X_in_Y, whereX is a material constituent of Y.  A chemical species denoted by X may be described by a single term such as 'nitrogen' or a phrase such as 'nox_expressed_as_nitrogen'. The chemicalformula for HCFC142b is CH3CClF2. The IUPAC name for HCFC142b is 1-chloro-1,1-difluoroethane." .

<http://purl.oclc.org/NET/ssnx/cf/cf-property#mole_fraction_of_hcfc22_in_air>
  a owl:NamedIndividual, <http://purl.oclc.org/NET/ssnx/qu/dim#Dimensionless> ;
  rdfs:label "mole fraction of hcfc22 in air" ;
  rdfs:isDefinedBy <http://purl.oclc.org/NET/ssnx/cf/cf-property> ;
  rdfs:comment " Mole fraction is used in the construction mole_fraction_of_X_in_Y, whereX is a material constituent of Y.  A chemical species denoted by X may be described by a single term such as 'nitrogen' or a phrase such as 'nox_expressed_as_nitrogen'. The chemicalformula for HCFC22 is CHClF2.  The IUPAC name for HCFC22 is chloro-difluoro-methane." .

<http://purl.oclc.org/NET/ssnx/cf/cf-property#mole_fraction_of_hexachlorobiphenyl_in_air>
  a owl:NamedIndividual, <http://purl.oclc.org/NET/ssnx/qu/dim#Dimensionless> ;
  rdfs:label "mole fraction of hexachlorobiphenyl in air" ;
  rdfs:isDefinedBy <http://purl.oclc.org/NET/ssnx/cf/cf-property> ;
  rdfs:comment "Mole fraction is used in the construction mole_fraction_of_X_in_Y, where X is a material constituent of Y." .

<http://purl.oclc.org/NET/ssnx/cf/cf-property#mole_fraction_of_hox_expressed_as_hydrogen_in_air>
  a owl:NamedIndividual, <http://purl.oclc.org/NET/ssnx/qu/dim#Dimensionless> ;
  rdfs:label "mole fraction of hox expressed as hydrogen in air" ;
  rdfs:isDefinedBy <http://purl.oclc.org/NET/ssnx/cf/cf-property> ;
  rdfs:comment " Mole fraction is used in the construction mole_fraction_of_X_in_Y, whereX is a material constituent of Y.  A chemical species denoted by X may be described by a single term such as 'nitrogen' or a phrase such as 'nox_expressed_as_nitrogen'. HOx means a combination of two radical species containing hydrogen and oxygen: OH and HO2. The phrase 'expressed_as' is used in the construction A_expressed_as_B, where B is a chemical constituent of A. It means that the quantity indicated by the standard name is calculated solely with respect to the B contained in A, neglecting all other chemical constituents of A." .

<http://purl.oclc.org/NET/ssnx/cf/cf-property#mole_fraction_of_hydrogen_bromide_in_air>
  a owl:NamedIndividual, <http://purl.oclc.org/NET/ssnx/qu/dim#Dimensionless> ;
  rdfs:label "mole fraction of hydrogen bromide in air" ;
  rdfs:isDefinedBy <http://purl.oclc.org/NET/ssnx/cf/cf-property> ;
  rdfs:comment "Mole fraction is used in the construction mole_fraction_of_X_in_Y, where X is a material constituent of Y.  The chemical formula of hydrogen bromide is HBr." .

<http://purl.oclc.org/NET/ssnx/cf/cf-property#mole_fraction_of_hydrogen_chloride_in_air>
  a owl:NamedIndividual, <http://purl.oclc.org/NET/ssnx/qu/dim#Dimensionless> ;
  rdfs:label "mole fraction of hydrogen chloride in air" ;
  rdfs:isDefinedBy <http://purl.oclc.org/NET/ssnx/cf/cf-property> ;
  rdfs:comment "Mole fraction is used in the construction mole_fraction_of_X_in_Y, where X is a material constituent of Y.  The chemical formula of hydrogen chloride is HCl." .

<http://purl.oclc.org/NET/ssnx/cf/cf-property#mole_fraction_of_hydrogen_cyanide_in_air>
  a owl:NamedIndividual, <http://purl.oclc.org/NET/ssnx/qu/dim#Dimensionless> ;
  rdfs:label "mole fraction of hydrogen cyanide in air" ;
  rdfs:isDefinedBy <http://purl.oclc.org/NET/ssnx/cf/cf-property> ;
  rdfs:comment "Mole fraction is used in the construction mole_fraction_of_X_in_Y, where X is a material constituent of Y.  The chemical formula of hydrogen cyanide is HCN." .

<http://purl.oclc.org/NET/ssnx/cf/cf-property#mole_fraction_of_hydrogen_peroxide_in_air>
  a owl:NamedIndividual, <http://purl.oclc.org/NET/ssnx/qu/dim#Dimensionless> ;
  rdfs:label "mole fraction of hydrogen peroxide in air" ;
  rdfs:isDefinedBy <http://purl.oclc.org/NET/ssnx/cf/cf-property> ;
  rdfs:comment "Mole fraction is used in the construction mole_fraction_of_X_in_Y, where X is a material constituent of Y.  The chemical formula of hydrogen peroxide is H202." .

<http://purl.oclc.org/NET/ssnx/cf/cf-property#mole_fraction_of_hydroperoxyl_radical_in_air>
  a owl:NamedIndividual, <http://purl.oclc.org/NET/ssnx/qu/dim#Dimensionless> ;
  rdfs:label "mole fraction of hydroperoxyl radical in air" ;
  rdfs:isDefinedBy <http://purl.oclc.org/NET/ssnx/cf/cf-property> ;
  rdfs:comment "Mole fraction is used in the construction mole_fraction_of_X_in_Y, where X is a material constituent of Y.  The chemical formula of hydroperoxyl radical is HO2." .

<http://purl.oclc.org/NET/ssnx/cf/cf-property#mole_fraction_of_hydroxyl_radical_in_air>
  a owl:NamedIndividual, <http://purl.oclc.org/NET/ssnx/qu/dim#Dimensionless> ;
  rdfs:label "mole fraction of hydroxyl radical in air" ;
  rdfs:isDefinedBy <http://purl.oclc.org/NET/ssnx/cf/cf-property> ;
  rdfs:comment "Mole fraction is used in the construction mole_fraction_of_X_in_Y, where X is a material constituent of Y." .

<http://purl.oclc.org/NET/ssnx/cf/cf-property#mole_fraction_of_hypobromous_acid_in_air>
  a owl:NamedIndividual, <http://purl.oclc.org/NET/ssnx/qu/dim#Dimensionless> ;
  rdfs:label "mole fraction of hypobromous acid in air" ;
  rdfs:isDefinedBy <http://purl.oclc.org/NET/ssnx/cf/cf-property> ;
  rdfs:comment "Mole fraction is used in the construction mole_fraction_of_X_in_Y, where X is a material constituent of Y.  The chemical formula of hypobromous acid is HOBr." .

<http://purl.oclc.org/NET/ssnx/cf/cf-property#mole_fraction_of_hypochlorous_acid_in_air>
  a owl:NamedIndividual, <http://purl.oclc.org/NET/ssnx/qu/dim#Dimensionless> ;
  rdfs:label "mole fraction of hypochlorous acid in air" ;
  rdfs:isDefinedBy <http://purl.oclc.org/NET/ssnx/cf/cf-property> ;
  rdfs:comment "Mole fraction is used in the construction mole_fraction_of_X_in_Y, where X is a material constituent of Y.  The chemical formula of hypochlorous acid is HOCl." .

<http://purl.oclc.org/NET/ssnx/cf/cf-property#mole_fraction_of_inorganic_bromine_in_air>
  a owl:NamedIndividual, <http://purl.oclc.org/NET/ssnx/qu/dim#Dimensionless> ;
  rdfs:label "mole fraction of inorganic bromine in air" ;
  rdfs:isDefinedBy <http://purl.oclc.org/NET/ssnx/cf/cf-property> ;
  rdfs:comment " Mole fraction is used in the construction mole_fraction_of_X_in_Y, where X is a material constituent of Y.  A chemical species denoted by X may be described by a single term such as 'nitrogen' or a phrase such as 'nox_expressed_as_nitrogen'. Inorganic bromine, sometimes referred to as Bry, describes a family of chemical species which result from the degradation of bromine containing source gases (halons, methyl bromide, VSLS) and natural inorganic bromine sources such as volcanoes, seasalt and other aerosols. Inorganic bromine is the term used in standard names for all species belonging to the family that are represented within a given model. The list of individual species that are included in a quantity having a group chemical standard name can vary between models.  Where possible, the data variable should be accompanied by a complete description of the species represented, for example, by using a comment attribute. Standard names that use the term brox are used for quantities that contain all inorganic bromine species except HBr and BrONO2." .

<http://purl.oclc.org/NET/ssnx/cf/cf-property#mole_fraction_of_inorganic_chlorine_in_air>
  a owl:NamedIndividual, <http://purl.oclc.org/NET/ssnx/qu/dim#Dimensionless> ;
  rdfs:label "mole fraction of inorganic chlorine in air" ;
  rdfs:isDefinedBy <http://purl.oclc.org/NET/ssnx/cf/cf-property> ;
  rdfs:comment "Mole fraction is used in the construction mole_fraction_of_X_in_Y, where X is a material constituent of Y.  Inorganic chlorine,sometimes referred to as Cly, describes a family of chemical species which result from the degradation of chlorine-containing source gases (CFCs, HCFCs, VSLS) and natural inorganic chlorine sources such as sea-salt and other aerosols.  mole_fraction_of_inorganic_chlorine is the sum of all species belonging to the family that are represented within a given model." .

<http://purl.oclc.org/NET/ssnx/cf/cf-property#mole_fraction_of_isoprene_in_air>
  a owl:NamedIndividual, <http://purl.oclc.org/NET/ssnx/qu/dim#Dimensionless> ;
  rdfs:label "mole fraction of isoprene in air" ;
  rdfs:isDefinedBy <http://purl.oclc.org/NET/ssnx/cf/cf-property> ;
  rdfs:comment "Mole fraction is used in the construction mole_fraction_of_X_in_Y, where X is a material constituent of Y." .

<http://purl.oclc.org/NET/ssnx/cf/cf-property#mole_fraction_of_limonene_in_air>
  a owl:NamedIndividual, <http://purl.oclc.org/NET/ssnx/qu/dim#Dimensionless> ;
  rdfs:label "mole fraction of limonene in air" ;
  rdfs:isDefinedBy <http://purl.oclc.org/NET/ssnx/cf/cf-property> ;
  rdfs:comment " Mole fraction is used in the construction mole_fraction_of_X_in_Y, whereX is a material constituent of Y.  A chemical species denoted by X may be described by a single term such as 'nitrogen' or a phrase such as 'nox_expressed_as_nitrogen'. The chemicalformula for limonene is C10H16. The IUPAC name for limonene is 1-methyl-4-prop-1-en-2-yl-cyclohexene. Limonene is a member of the group of hydrocarbons known as terpenes.  There arestandard names for the terpene group as well as for some of the individual species." .

<http://purl.oclc.org/NET/ssnx/cf/cf-property#mole_fraction_of_methane_in_air>
  a owl:NamedIndividual, <http://purl.oclc.org/NET/ssnx/qu/dim#Dimensionless> ;
  rdfs:label "mole fraction of methane in air" ;
  rdfs:isDefinedBy <http://purl.oclc.org/NET/ssnx/cf/cf-property> ;
  rdfs:comment "Mole fraction is used in the construction mole_fraction_of_X_in_Y, where X is a material constituent of Y." .

<http://purl.oclc.org/NET/ssnx/cf/cf-property#mole_fraction_of_methanol_in_air>
  a owl:NamedIndividual, <http://purl.oclc.org/NET/ssnx/qu/dim#Dimensionless> ;
  rdfs:label "mole fraction of methanol in air" ;
  rdfs:isDefinedBy <http://purl.oclc.org/NET/ssnx/cf/cf-property> ;
  rdfs:comment " Mole fraction is used in the construction mole_fraction_of_X_in_Y, whereX is a material constituent of Y.  A chemical species denoted by X may be described by a single term such as 'nitrogen' or a phrase such as 'nox_expressed_as_nitrogen'. The chemicalformula for methanol is CH3OH." .

<http://purl.oclc.org/NET/ssnx/cf/cf-property#mole_fraction_of_methyl_bromide_in_air>
  a owl:NamedIndividual, <http://purl.oclc.org/NET/ssnx/qu/dim#Dimensionless> ;
  rdfs:label "mole fraction of methyl bromide in air" ;
  rdfs:isDefinedBy <http://purl.oclc.org/NET/ssnx/cf/cf-property> ;
  rdfs:comment "Mole fraction is used in the construction mole_fraction_of_X_in_Y, where X is a material constituent of Y.  The chemical formula of methyl bromide is CH3Br." .

<http://purl.oclc.org/NET/ssnx/cf/cf-property#mole_fraction_of_methyl_chloride_in_air>
  a owl:NamedIndividual, <http://purl.oclc.org/NET/ssnx/qu/dim#Dimensionless> ;
  rdfs:label "mole fraction of methyl chloride in air" ;
  rdfs:isDefinedBy <http://purl.oclc.org/NET/ssnx/cf/cf-property> ;
  rdfs:comment "Mole fraction is used in the construction mole_fraction_of_X_in_Y, where X is a material constituent of Y.  The chemical formula of methyl chloride is CH3Cl." .

<http://purl.oclc.org/NET/ssnx/cf/cf-property#mole_fraction_of_methyl_hydroperoxide_in_air>
  a owl:NamedIndividual, <http://purl.oclc.org/NET/ssnx/qu/dim#Dimensionless> ;
  rdfs:label "mole fraction of methyl hydroperoxide in air" ;
  rdfs:isDefinedBy <http://purl.oclc.org/NET/ssnx/cf/cf-property> ;
  rdfs:comment "Mole fraction is used in the construction mole_fraction_of_X_in_Y, where X is a material constituent of Y.  The chemical formula of methyl hydroperoxide is CH3OOH." .

<http://purl.oclc.org/NET/ssnx/cf/cf-property#mole_fraction_of_methyl_peroxy_radical_in_air>
  a owl:NamedIndividual, <http://purl.oclc.org/NET/ssnx/qu/dim#Dimensionless> ;
  rdfs:label "mole fraction of methyl peroxy radical in air" ;
  rdfs:isDefinedBy <http://purl.oclc.org/NET/ssnx/cf/cf-property> ;
  rdfs:comment " Mole fraction is used in the construction mole_fraction_of_X_in_Y, whereX is a material constituent of Y.  A chemical species denoted by X may be described by a single term such as 'nitrogen' or a phrase such as 'nox_expressed_as_nitrogen'. The chemicalformula for methyl_peroxy_radical is CH3O2. In chemistry, a 'radical' is a highly reactive, and therefore shortlived, species." .

<http://purl.oclc.org/NET/ssnx/cf/cf-property#mole_fraction_of_molecular_hydrogen_in_air>
  a owl:NamedIndividual, <http://purl.oclc.org/NET/ssnx/qu/dim#Dimensionless> ;
  rdfs:label "mole fraction of molecular hydrogen in air" ;
  rdfs:isDefinedBy <http://purl.oclc.org/NET/ssnx/cf/cf-property> ;
  rdfs:comment "Mole fraction is used in the construction mole_fraction_of_X_in_Y, where X is a material constituent of Y.  The chemical formula of molecular hydrogen is H2." .

<http://purl.oclc.org/NET/ssnx/cf/cf-property#mole_fraction_of_nitrate_radical_in_air>
  a owl:NamedIndividual, <http://purl.oclc.org/NET/ssnx/qu/dim#Dimensionless> ;
  rdfs:label "mole fraction of nitrate radical in air" ;
  rdfs:isDefinedBy <http://purl.oclc.org/NET/ssnx/cf/cf-property> ;
  rdfs:comment " Mole fraction is used in the construction mole_fraction_of_X_in_Y, whereX is a material constituent of Y.  A chemical species denoted by X may be described by a single term such as 'nitrogen' or a phrase such as 'nox_expressed_as_nitrogen'. In chemistry, a 'radical' is a highly reactive, and therefore shortlived, species." .

<http://purl.oclc.org/NET/ssnx/cf/cf-property#mole_fraction_of_nitric_acid_in_air>
  a owl:NamedIndividual, <http://purl.oclc.org/NET/ssnx/qu/dim#Dimensionless> ;
  rdfs:label "mole fraction of nitric acid in air" ;
  rdfs:isDefinedBy <http://purl.oclc.org/NET/ssnx/cf/cf-property> ;
  rdfs:comment "Mole fraction is used in the construction mole_fraction_of_X_in_Y, where X is a material constituent of Y." .

<http://purl.oclc.org/NET/ssnx/cf/cf-property#mole_fraction_of_nitric_acid_trihydrate_ambient_aerosol_in_air>
  a owl:NamedIndividual, <http://purl.oclc.org/NET/ssnx/qu/dim#Dimensionless> ;
  rdfs:label "mole fraction of nitric acid trihydrate ambient aerosol in air" ;
  rdfs:isDefinedBy <http://purl.oclc.org/NET/ssnx/cf/cf-property> ;
  rdfs:comment " Mole fraction is used in the construction mole_fraction_of_X_in_Y, whereX is a material constituent of Y.  A chemical species denoted by X may be described by a single term such as 'nitrogen' or a phrase such as 'nox_expressed_as_nitrogen'. Aerosol means the suspended liquid or solid particles in air (except cloud droplets).  Ambient aerosol is aerosol that has taken up ambient water through hygroscopic growth. The extent of hygroscopic growth depends on the relative humidity and the composition of the aerosol. The chemical formula for nitric acid is HNO3. Nitric acid trihydrate, sometimes referred to as NAT, is a stable crystalline substance consisting of three molecules of water to one molecule of nitric acid." .

<http://purl.oclc.org/NET/ssnx/cf/cf-property#mole_fraction_of_nitrogen_dioxide_in_air>
  a owl:NamedIndividual, <http://purl.oclc.org/NET/ssnx/qu/dim#Dimensionless> ;
  rdfs:label "mole fraction of nitrogen dioxide in air" ;
  rdfs:isDefinedBy <http://purl.oclc.org/NET/ssnx/cf/cf-property> ;
  rdfs:comment "Mole fraction is used in the construction mole_fraction_of_X_in_Y, where X is a material constituent of Y." .

<http://purl.oclc.org/NET/ssnx/cf/cf-property#mole_fraction_of_nitrogen_monoxide_in_air>
  a owl:NamedIndividual, <http://purl.oclc.org/NET/ssnx/qu/dim#Dimensionless> ;
  rdfs:label "mole fraction of nitrogen monoxide in air" ;
  rdfs:isDefinedBy <http://purl.oclc.org/NET/ssnx/cf/cf-property> ;
  rdfs:comment "Mole fraction is used in the construction mole_fraction_of_X_in_Y, where X is a material constituent of Y." .

<http://purl.oclc.org/NET/ssnx/cf/cf-property#mole_fraction_of_nitrous_acid_in_air>
  a owl:NamedIndividual, <http://purl.oclc.org/NET/ssnx/qu/dim#Dimensionless> ;
  rdfs:label "mole fraction of nitrous acid in air" ;
  rdfs:isDefinedBy <http://purl.oclc.org/NET/ssnx/cf/cf-property> ;
  rdfs:comment " Mole fraction is used in the construction mole_fraction_of_X_in_Y, whereX is a material constituent of Y.  A chemical species denoted by X may be described by a single term such as 'nitrogen' or a phrase such as 'nox_expressed_as_nitrogen'. The chemicalformula for nitrous acid is HNO2." .

<http://purl.oclc.org/NET/ssnx/cf/cf-property#mole_fraction_of_nitrous_oxide_in_air>
  a owl:NamedIndividual, <http://purl.oclc.org/NET/ssnx/qu/dim#Dimensionless> ;
  rdfs:label "mole fraction of nitrous oxide in air" ;
  rdfs:isDefinedBy <http://purl.oclc.org/NET/ssnx/cf/cf-property> ;
  rdfs:comment "Mole fraction is used in the construction mole_fraction_of_X_in_Y, where X is a material constituent of Y.   The chemical formula of  nitrous oxide is N2O." .

<http://purl.oclc.org/NET/ssnx/cf/cf-property#mole_fraction_of_nmvoc_expressed_as_carbon_in_air>
  a owl:NamedIndividual, <http://purl.oclc.org/NET/ssnx/qu/dim#Dimensionless> ;
  rdfs:label "mole fraction of nmvoc expressed as carbon in air" ;
  rdfs:isDefinedBy <http://purl.oclc.org/NET/ssnx/cf/cf-property> ;
  rdfs:comment " Mole fraction is used in the construction mole_fraction_of_X_in_Y, whereX is a material constituent of Y.  A chemical species denoted by X may be described by a single term such as 'nitrogen' or a phrase such as 'nox_expressed_as_nitrogen'. nmvoc means non methane volatile organic compounds. The phrase 'expressed_as' is used in the construction A_expressed_as_B, where B is a chemical constituent of A. It means that the quantity indicated by the standard name is calculated solely with respect to the B contained in A, neglecting all other chemical constituents of A." .

<http://purl.oclc.org/NET/ssnx/cf/cf-property#mole_fraction_of_nox_expressed_as_nitrogen_in_air>
  a owl:NamedIndividual, <http://purl.oclc.org/NET/ssnx/qu/dim#Dimensionless> ;
  rdfs:label "mole fraction of nox expressed as nitrogen in air" ;
  rdfs:isDefinedBy <http://purl.oclc.org/NET/ssnx/cf/cf-property> ;
  rdfs:comment " Mole fraction is used in the construction mole_fraction_of_X_in_Y, whereX is a material constituent of Y.  A chemical species denoted by X may be described by a single term such as 'nitrogen' or a phrase such as 'nox_expressed_as_nitrogen'. Nox means a combination of two radical species containing nitrogen and oxygen: NO+NO2. The phrase 'expressed_as' is used in the construction A_expressed_as_B, where B is a chemical constituent of A. It means that the quantity indicated by the standard name is calculated solely with respect to the B contained in A, neglecting all other chemical constituents of A." .

<http://purl.oclc.org/NET/ssnx/cf/cf-property#mole_fraction_of_noy_expressed_as_nitrogen_in_air>
  a owl:NamedIndividual, <http://purl.oclc.org/NET/ssnx/qu/dim#Dimensionless> ;
  rdfs:label "mole fraction of noy expressed as nitrogen in air" ;
  rdfs:isDefinedBy <http://purl.oclc.org/NET/ssnx/cf/cf-property> ;
  rdfs:comment " Mole fraction is used in the construction mole_fraction_of_X_in_Y, whereX is a material constituent of Y.  A chemical species denoted by X may be described by a single term such as 'nitrogen' or a phrase such as 'nox_expressed_as_nitrogen'. Noy describes a family of chemical species. The family usually includes atomic nitrogen (N), nitrogen monoxide (NO), nitrogen dioxide (NO2), dinitrogen pentoxide (N2O5), nitric acid (HNO3), peroxynitric acid (HNO4), bromine nitrate (BrONO2) , chlorine nitrate (ClONO2) and organic nitrates (most notably peroxyacetyl nitrate, sometimes referred to as PAN, (CH3COO2NO2)). The list of individual species that are included in a quantity having a group chemical standard name can vary between models.  Where possible, the data variable should be accompanied by a complete description of the species represented, for example, by using a comment attribute. The phrase 'expressed_as' is used in the construction A_expressed_as_B, whereB is a chemical constituent of A. It means that the quantity indicated by the standard name is calculated solely with respect to the B contained in A, neglecting all other chemical constituents of A." .

<http://purl.oclc.org/NET/ssnx/cf/cf-property#mole_fraction_of_ozone_in_air>
  a owl:NamedIndividual, <http://purl.oclc.org/NET/ssnx/qu/dim#Dimensionless> ;
  rdfs:label "mole fraction of ozone in air" ;
  rdfs:isDefinedBy <http://purl.oclc.org/NET/ssnx/cf/cf-property> ;
  rdfs:comment "Mole fraction is used in the construction mole_fraction_of_X_in_Y, where X is a material constituent of Y." .

<http://purl.oclc.org/NET/ssnx/cf/cf-property#mole_fraction_of_peroxyacetyl_nitrate_in_air>
  a owl:NamedIndividual, <http://purl.oclc.org/NET/ssnx/qu/dim#Dimensionless> ;
  rdfs:label "mole fraction of peroxyacetyl nitrate in air" ;
  rdfs:isDefinedBy <http://purl.oclc.org/NET/ssnx/cf/cf-property> ;
  rdfs:comment "Mole fraction is used in the construction mole_fraction_of_X_in_Y, where X is a material constituent of Y." .

<http://purl.oclc.org/NET/ssnx/cf/cf-property#mole_fraction_of_peroxynitric_acid_in_air>
  a owl:NamedIndividual, <http://purl.oclc.org/NET/ssnx/qu/dim#Dimensionless> ;
  rdfs:label "mole fraction of peroxynitric acid in air" ;
  rdfs:isDefinedBy <http://purl.oclc.org/NET/ssnx/cf/cf-property> ;
  rdfs:comment "Mole fraction is used in the construction mole_fraction_of_X_in_Y, where X is a material constituent of Y.  The chemical formula of peroxynitric acid is HNO4." .

<http://purl.oclc.org/NET/ssnx/cf/cf-property#mole_fraction_of_propane_in_air>
  a owl:NamedIndividual, <http://purl.oclc.org/NET/ssnx/qu/dim#Dimensionless> ;
  rdfs:label "mole fraction of propane in air" ;
  rdfs:isDefinedBy <http://purl.oclc.org/NET/ssnx/cf/cf-property> ;
  rdfs:comment "Mole fraction is used in the construction mole_fraction_of_X_in_Y, where X is a material constituent of Y." .

<http://purl.oclc.org/NET/ssnx/cf/cf-property#mole_fraction_of_propene_in_air>
  a owl:NamedIndividual, <http://purl.oclc.org/NET/ssnx/qu/dim#Dimensionless> ;
  rdfs:label "mole fraction of propene in air" ;
  rdfs:isDefinedBy <http://purl.oclc.org/NET/ssnx/cf/cf-property> ;
  rdfs:comment "Mole fraction is used in the construction mole_fraction_of_X_in_Y, where X is a material constituent of Y." .

<http://purl.oclc.org/NET/ssnx/cf/cf-property#mole_fraction_of_radon_in_air>
  a owl:NamedIndividual, <http://purl.oclc.org/NET/ssnx/qu/dim#Dimensionless> ;
  rdfs:label "mole fraction of radon in air" ;
  rdfs:isDefinedBy <http://purl.oclc.org/NET/ssnx/cf/cf-property> ;
  rdfs:comment " Mole fraction is used in the construction mole_fraction_of_X_in_Y, whereX is a material constituent of Y.  A chemical species denoted by X may be described by a single term such as 'nitrogen' or a phrase such as 'nox_expressed_as_nitrogen'. The chemicalsymbol for radon is Rn." .

<http://purl.oclc.org/NET/ssnx/cf/cf-property#mole_fraction_of_sulfur_dioxide_in_air>
  a owl:NamedIndividual, <http://purl.oclc.org/NET/ssnx/qu/dim#Dimensionless> ;
  rdfs:label "mole fraction of sulfur dioxide in air" ;
  rdfs:isDefinedBy <http://purl.oclc.org/NET/ssnx/cf/cf-property> ;
  rdfs:comment "Mole fraction is used in the construction mole_fraction_of_X_in_Y, where X is a material constituent of Y." .

<http://purl.oclc.org/NET/ssnx/cf/cf-property#mole_fraction_of_toluene_in_air>
  a owl:NamedIndividual, <http://purl.oclc.org/NET/ssnx/qu/dim#Dimensionless> ;
  rdfs:label "mole fraction of toluene in air" ;
  rdfs:isDefinedBy <http://purl.oclc.org/NET/ssnx/cf/cf-property> ;
  rdfs:comment "Mole fraction is used in the construction mole_fraction_of_X_in_Y, where X is a material constituent of Y." .

<http://purl.oclc.org/NET/ssnx/cf/cf-property#mole_fraction_of_water_vapor_in_air>
  a owl:NamedIndividual, <http://purl.oclc.org/NET/ssnx/qu/dim#Dimensionless> ;
  rdfs:label "mole fraction of water vapor in air" ;
  rdfs:isDefinedBy <http://purl.oclc.org/NET/ssnx/cf/cf-property> ;
  rdfs:comment "Mole fraction is used in the construction mole_fraction_of_X_in_Y, where X is a material constituent of Y.  The chemical formula of water vapor is H2O." .

<http://purl.oclc.org/NET/ssnx/cf/cf-property#mole_fraction_of_xylene_in_air>
  a owl:NamedIndividual, <http://purl.oclc.org/NET/ssnx/qu/dim#Dimensionless> ;
  rdfs:label "mole fraction of xylene in air" ;
  rdfs:isDefinedBy <http://purl.oclc.org/NET/ssnx/cf/cf-property> ;
  rdfs:comment "Mole fraction is used in the construction mole_fraction_of_X_in_Y, where X is a material constituent of Y." .

<http://purl.oclc.org/NET/ssnx/cf/cf-property#net_downward_longwave_flux_in_air>
  a owl:NamedIndividual, <http://purl.oclc.org/NET/ssnx/qu/dim#EnergyFlux> ;
  rdfs:label "net downward longwave flux in air" ;
  rdfs:isDefinedBy <http://purl.oclc.org/NET/ssnx/cf/cf-property> ;
  rdfs:comment "longwave means longwave radiation. Downward indicates a vector component which is positive when directed downward (negative upward). Net downward radiation is the difference between radiation from above (downwelling) and radiation from below (upwelling). In accordance with common usage in geophysical disciplines, flux implies per unit area, called flux density in physics." .

<http://purl.oclc.org/NET/ssnx/cf/cf-property#net_downward_longwave_flux_in_air_assuming_clear_sky>
  a owl:NamedIndividual, <http://purl.oclc.org/NET/ssnx/qu/dim#EnergyFlux> ;
  rdfs:label "net downward longwave flux in air assuming clear sky" ;
  rdfs:isDefinedBy <http://purl.oclc.org/NET/ssnx/cf/cf-property> ;
  rdfs:comment "A phrase assuming_condition indicates that the named quantity is the value which would obtain if all aspects of the system were unaltered except for the assumption of the circumstances specified by the condition. longwave means longwave radiation. Downward indicates a vector component which is positive when directed downward (negative upward). Net downward radiation is the difference between radiation from above (downwelling) and radiation from below (upwelling). In accordance with common usage in geophysical disciplines, flux implies per unit area, called flux density in physics." .

<http://purl.oclc.org/NET/ssnx/cf/cf-property#net_downward_shortwave_flux_in_air>
  a owl:NamedIndividual, <http://purl.oclc.org/NET/ssnx/qu/dim#EnergyFlux> ;
  rdfs:label "net downward shortwave flux in air" ;
  rdfs:isDefinedBy <http://purl.oclc.org/NET/ssnx/cf/cf-property> ;
  rdfs:comment "shortwave means shortwave radiation. Downward indicates a vector component which is positive when directed downward (negative upward). Net downward radiation is the difference between radiation from above (downwelling) and radiation from below (upwelling). In accordance with common usage in geophysical disciplines, flux implies per unit area, called flux density in physics." .

<http://purl.oclc.org/NET/ssnx/cf/cf-property#net_downward_shortwave_flux_in_air_assuming_clear_sky>
  a owl:NamedIndividual, <http://purl.oclc.org/NET/ssnx/qu/dim#EnergyFlux> ;
  rdfs:label "net downward shortwave flux in air assuming clear sky" ;
  rdfs:isDefinedBy <http://purl.oclc.org/NET/ssnx/cf/cf-property> ;
  rdfs:comment "A phrase assuming_condition indicates that the named quantity is the value which would obtain if all aspects of the system were unaltered except for the assumption of the circumstances specified by the condition. shortwave means shortwave radiation. Downward indicates a vector component which is positive when directed downward (negative upward). Net downward radiation is the difference between radiation from above (downwelling) and radiation from below (upwelling). In accordance with common usage in geophysical disciplines, flux implies per unit area, called flux density in physics." .

<http://purl.oclc.org/NET/ssnx/cf/cf-property#net_upward_longwave_flux_in_air>
  a owl:NamedIndividual, <http://purl.oclc.org/NET/ssnx/qu/dim#EnergyFlux> ;
  rdfs:label "net upward longwave flux in air" ;
  rdfs:isDefinedBy <http://purl.oclc.org/NET/ssnx/cf/cf-property> ;
  rdfs:comment "longwave means longwave radiation. Upward indicates a vector component which is positive when directed upward (negative downward). Net upward radiation is the difference between radiation from below (upwelling) and radiation from above (downwelling). In accordance with common usage in geophysical disciplines, flux implies per unit area, called flux density in physics." .

<http://purl.oclc.org/NET/ssnx/cf/cf-property#net_upward_longwave_flux_in_air_assuming_clear_sky>
  a owl:NamedIndividual, <http://purl.oclc.org/NET/ssnx/qu/dim#EnergyFlux> ;
  rdfs:label "net upward longwave flux in air assuming clear sky" ;
  rdfs:isDefinedBy <http://purl.oclc.org/NET/ssnx/cf/cf-property> ;
  rdfs:comment "A phrase assuming_condition indicates that the named quantity is the value which would obtain if all aspects of the system were unaltered except for the assumption of the circumstances specified by the condition. longwave means longwave radiation. Upward indicates a vector component which is positive when directed upward (negative downward). Net upward radiation is the difference between radiation from below (upwelling) and radiation from above (downwelling). In accordance with common usage in geophysical disciplines, flux implies per unit area, called flux density in physics." .

<http://purl.oclc.org/NET/ssnx/cf/cf-property#net_upward_shortwave_flux_in_air>
  a owl:NamedIndividual, <http://purl.oclc.org/NET/ssnx/qu/dim#EnergyFlux> ;
  rdfs:label "net upward shortwave flux in air" ;
  rdfs:isDefinedBy <http://purl.oclc.org/NET/ssnx/cf/cf-property> ;
  rdfs:comment "shortwave means shortwave radiation. Upward indicates a vector component which is positive when directed upward (negative downward). Net upward radiation is the difference between radiation from below (upwelling) and radiation from above (downwelling). In accordance with common usage in geophysical disciplines, flux implies per unit area, called flux density in physics." .

<http://purl.oclc.org/NET/ssnx/cf/cf-property#net_upward_shortwave_flux_in_air_assuming_clear_sky>
  a owl:NamedIndividual, <http://purl.oclc.org/NET/ssnx/qu/dim#EnergyFlux> ;
  rdfs:label "net upward shortwave flux in air assuming clear sky" ;
  rdfs:isDefinedBy <http://purl.oclc.org/NET/ssnx/cf/cf-property> ;
  rdfs:comment "A phrase assuming_condition indicates that the named quantity is the value which would obtain if all aspects of the system were unaltered except for the assumption of the circumstances specified by the condition. shortwave means shortwave radiation. Upward indicates a vector component which is positive when directed upward (negative downward). Net upward radiation is the difference between radiation from below (upwelling) and radiation from above (downwelling). In accordance with common usage in geophysical disciplines, flux implies per unit area, called flux density in physics." .

<http://purl.oclc.org/NET/ssnx/cf/cf-property#northward_heat_flux_in_air_due_to_eddy_advection>
  a owl:NamedIndividual, <http://purl.oclc.org/NET/ssnx/qu/dim#EnergyFlux> ;
  rdfs:label "northward heat flux in air due to eddy advection" ;
  rdfs:isDefinedBy <http://purl.oclc.org/NET/ssnx/cf/cf-property> ;
  rdfs:comment "The specification of a physical process by the phrase due_to_process means that the quantity named is a single term in a sum of terms which together compose the general quantity named by omitting the phrase. Northward indicates a vector component which is positive when directed northward (negative southward).  In accordance with common usage in geophysical disciplines, flux implies per unit area, called flux density in physics." .

<http://purl.oclc.org/NET/ssnx/cf/cf-property#northward_mass_flux_of_air>
  a owl:NamedIndividual, <http://purl.oclc.org/NET/ssnx/qu/dim#MassPerTimePerArea> ;
  rdfs:label "northward mass flux of air" ;
  rdfs:isDefinedBy <http://purl.oclc.org/NET/ssnx/cf/cf-property> ;
  rdfs:comment "Northward indicates a vector component which is positive when directed northward (negative southward). In accordance with common usage in geophysical disciplines, flux implies per unit area, called flux density in physics." .

<http://purl.oclc.org/NET/ssnx/cf/cf-property#number_of_days_with_air_temperature_above_threshold>
  a owl:NamedIndividual, <http://purl.oclc.org/NET/ssnx/qu/dim#Dimensionless> ;
  rdfs:label "number of days with air temperature above threshold" ;
  rdfs:isDefinedBy <http://purl.oclc.org/NET/ssnx/cf/cf-property> ;
  rdfs:comment "Air temperature is the bulk temperature of the air, not the surface (skin) temperature.  A variable whose standard name has the form number_of_days_with_X_below|above_threshold is a count of the number of days on which the condition X_below|above_threshold is satisfied.  It must have a coordinate variable or scalar coordinate variable with the a standard name of X to supply the threshold(s). It must have a climatological time variable, and a cell_methods entry for within days which describes the processing of quantity X before the threshold is applied. A number_of_days is an extensive quantity in time, and the cell_methods entry for over days should be sum." .

<http://purl.oclc.org/NET/ssnx/cf/cf-property#number_of_days_with_air_temperature_below_threshold>
  a owl:NamedIndividual, <http://purl.oclc.org/NET/ssnx/qu/dim#Dimensionless> ;
  rdfs:label "number of days with air temperature below threshold" ;
  rdfs:isDefinedBy <http://purl.oclc.org/NET/ssnx/cf/cf-property> ;
  rdfs:comment "Air temperature is the bulk temperature of the air, not the surface (skin) temperature.  A variable whose standard name has the form number_of_days_with_X_below|above_threshold is a count of the number of days on which the condition X_below|above_threshold is satisfied.  It must have a coordinate variable or scalar coordinate variable with the a standard name of X to supply the threshold(s). It must have a climatological time variable, and a cell_methods entry for within days which describes the processing of quantity X before the threshold is applied. A number_of_days is an extensive quantity in time, and the cell_methods entry for over days should be sum." .

<http://purl.oclc.org/NET/ssnx/cf/cf-property#platform_speed_wrt_air>
  a owl:NamedIndividual, <http://purl.oclc.org/NET/ssnx/qu/dim#VelocityOrSpeed> ;
  rdfs:label "platform speed wrt air" ;
  rdfs:isDefinedBy <http://purl.oclc.org/NET/ssnx/cf/cf-property> ;
  rdfs:comment "wrt means with respect to. Speed is the magnitude of velocity. Standard names for platform describe the motion and orientation of the vehicle from which observations are made e.g. aeroplane or ship. The platform speed with respect to air is often called the air speed of the platform." .

<http://purl.oclc.org/NET/ssnx/cf/cf-property#product_of_air_temperature_and_specific_humidity>
  a owl:NamedIndividual, <http://purl.oclc.org/NET/ssnx/qu/dim#Temperature> ;
  rdfs:label "product of air temperature and specific humidity" ;
  rdfs:isDefinedBy <http://purl.oclc.org/NET/ssnx/cf/cf-property> ;
  rdfs:comment "product_of_X_and_Y means X*Y. specific means per unit mass. Air temperature is the bulk temperature of the air, not the surface (skin) temperature. Specific humidity is the mass fraction of water vapor in (moist) air." .

<http://purl.oclc.org/NET/ssnx/cf/cf-property#product_of_upward_air_velocity_and_specific_humidity>
  a owl:NamedIndividual, <http://purl.oclc.org/NET/ssnx/qu/dim#VelocityOrSpeed> ;
  rdfs:label "product of upward air velocity and specific humidity" ;
  rdfs:isDefinedBy <http://purl.oclc.org/NET/ssnx/cf/cf-property> ;
  rdfs:comment "product_of_X_and_Y means X*Y. specific means per unit mass. A velocity is a vector quantity. Upward indicates a vector component which is positive when directed upward (negative downward). Specific humidity is the mass fraction of water vapor in (moist) air. Upward air velocity is the vertical component of the 3D air velocity vector." .

<http://purl.oclc.org/NET/ssnx/cf/cf-property#sound_intensity_in_air>
  a owl:NamedIndividual, <http://purl.oclc.org/NET/ssnx/qu/dim#EnergyFlux> ;
  rdfs:label "sound intensity in air" ;
  rdfs:isDefinedBy <http://purl.oclc.org/NET/ssnx/cf/cf-property> ;
  rdfs:comment "Sound intensity is the sound energy per unit time per unit area." .

<http://purl.oclc.org/NET/ssnx/cf/cf-property#sound_pressure_in_air>
  a owl:NamedIndividual, <http://purl.oclc.org/NET/ssnx/qu/dim#StressOrPressure> ;
  rdfs:label "sound pressure in air" ;
  rdfs:isDefinedBy <http://purl.oclc.org/NET/ssnx/cf/cf-property> ;
  rdfs:comment "Sound pressure is the difference from the local ambient pressure caused by a sound wave at a particular location and time." .

<http://purl.oclc.org/NET/ssnx/cf/cf-property#speed_of_sound_in_air>
  a owl:NamedIndividual, <http://purl.oclc.org/NET/ssnx/qu/dim#VelocityOrSpeed> ;
  rdfs:label "speed of sound in air" ;
  rdfs:isDefinedBy <http://purl.oclc.org/NET/ssnx/cf/cf-property> ;
  rdfs:comment "Speed is the magnitude of velocity." .

<http://purl.oclc.org/NET/ssnx/cf/cf-property#surface_drag_coefficient_for_heat_in_air>
  a owl:NamedIndividual, <http://purl.oclc.org/NET/ssnx/qu/dim#Dimensionless> ;
  rdfs:label "surface drag coefficient for heat in air" ;
  rdfs:isDefinedBy <http://purl.oclc.org/NET/ssnx/cf/cf-property> ;
  rdfs:comment "The surface called surface means the lower boundary of the atmosphere." .

<http://purl.oclc.org/NET/ssnx/cf/cf-property#surface_drag_coefficient_for_momentum_in_air>
  a owl:NamedIndividual, <http://purl.oclc.org/NET/ssnx/qu/dim#Dimensionless> ;
  rdfs:label "surface drag coefficient for momentum in air" ;
  rdfs:isDefinedBy <http://purl.oclc.org/NET/ssnx/cf/cf-property> ;
  rdfs:comment "The surface called surface means the lower boundary of the atmosphere." .

<http://purl.oclc.org/NET/ssnx/cf/cf-property#surface_drag_coefficient_in_air>
  a owl:NamedIndividual, <http://purl.oclc.org/NET/ssnx/qu/dim#Dimensionless> ;
  rdfs:label "surface drag coefficient in air" ;
  rdfs:isDefinedBy <http://purl.oclc.org/NET/ssnx/cf/cf-property> ;
  rdfs:comment "The surface called surface means the lower boundary of the atmosphere." .

<http://purl.oclc.org/NET/ssnx/cf/cf-property#surface_partial_pressure_of_carbon_dioxide_in_air>
  a owl:NamedIndividual, <http://purl.oclc.org/NET/ssnx/qu/dim#StressOrPressure> ;
  rdfs:label "surface partial pressure of carbon dioxide in air" ;
  rdfs:isDefinedBy <http://purl.oclc.org/NET/ssnx/cf/cf-property> ;
  rdfs:comment "The surface called surface means the lower boundary of the atmosphere. The partial pressure of a gaseous constituent of air is the pressure which it alone would exert with unchanged temperature and number of moles per unit volume." .

<http://purl.oclc.org/NET/ssnx/cf/cf-property#surface_roughness_length_for_heat_in_air>
  a owl:NamedIndividual, <http://purl.oclc.org/NET/ssnx/qu/dim#Distance> ;
  rdfs:label "surface roughness length for heat in air" ;
  rdfs:isDefinedBy <http://purl.oclc.org/NET/ssnx/cf/cf-property> ;
  rdfs:comment "The surface called surface means the lower boundary of the atmosphere." .

<http://purl.oclc.org/NET/ssnx/cf/cf-property#surface_roughness_length_for_momentum_in_air>
  a owl:NamedIndividual, <http://purl.oclc.org/NET/ssnx/qu/dim#Distance> ;
  rdfs:label "surface roughness length for momentum in air" ;
  rdfs:isDefinedBy <http://purl.oclc.org/NET/ssnx/cf/cf-property> ;
  rdfs:comment "The surface called surface means the lower boundary of the atmosphere." .

<http://purl.oclc.org/NET/ssnx/cf/cf-property#tendency_of_air_temperature>
  a owl:NamedIndividual, <http://purl.oclc.org/NET/ssnx/qu/dim#TemperatureDrift> ;
  rdfs:label "tendency of air temperature" ;
  rdfs:isDefinedBy <http://purl.oclc.org/NET/ssnx/cf/cf-property> ;
  rdfs:comment "tendency_of_X means derivative of X with respect to time. Air temperature is the bulk temperature of the air, not the surface (skin) temperature." .

<http://purl.oclc.org/NET/ssnx/cf/cf-property#tendency_of_air_temperature_due_to_advection>
  a owl:NamedIndividual, <http://purl.oclc.org/NET/ssnx/qu/dim#TemperatureDrift> ;
  rdfs:label "tendency of air temperature due to advection" ;
  rdfs:isDefinedBy <http://purl.oclc.org/NET/ssnx/cf/cf-property> ;
  rdfs:comment "The specification of a physical process by the phrase due_to_process means that the quantity named is a single term in a sum of terms which together compose the general quantity named by omitting the phrase. tendency_of_X means derivative of X with respect to time. Air temperature is the bulk temperature of the air, not the surface (skin) temperature." .

<http://purl.oclc.org/NET/ssnx/cf/cf-property#tendency_of_air_temperature_due_to_convection>
  a owl:NamedIndividual, <http://purl.oclc.org/NET/ssnx/qu/dim#TemperatureDrift> ;
  rdfs:label "tendency of air temperature due to convection" ;
  rdfs:isDefinedBy <http://purl.oclc.org/NET/ssnx/cf/cf-property> ;
  rdfs:comment "Air temperature is the bulk temperature of the air, not the surface (skin) temperature.  The specification of a physical process by the phrase due_to_process means that the quantity named is a  single term in a sum of terms which together compose the general quantity  named by omitting the phrase.  tendency_of_X means derivative of X with respect to time. " .

<http://purl.oclc.org/NET/ssnx/cf/cf-property#tendency_of_air_temperature_due_to_diabatic_processes>
  a owl:NamedIndividual, <http://purl.oclc.org/NET/ssnx/qu/dim#TemperatureDrift> ;
  rdfs:label "tendency of air temperature due to diabatic processes" ;
  rdfs:isDefinedBy <http://purl.oclc.org/NET/ssnx/cf/cf-property> ;
  rdfs:comment "The specification of a physical process by the phrase due_to_process means that the quantity named is a single term in a sum of terms which together compose the general quantity named by omitting the phrase. tendency_of_X means derivative of X with respect to time. Air temperature is the bulk temperature of the air, not the surface (skin) temperature." .

<http://purl.oclc.org/NET/ssnx/cf/cf-property#tendency_of_air_temperature_due_to_diffusion>
  a owl:NamedIndividual, <http://purl.oclc.org/NET/ssnx/qu/dim#TemperatureDrift> ;
  rdfs:label "tendency of air temperature due to diffusion" ;
  rdfs:isDefinedBy <http://purl.oclc.org/NET/ssnx/cf/cf-property> ;
  rdfs:comment "The specification of a physical process by the phrase due_to_process means that the quantity named is a single term in a sum of terms which together compose the general quantity named by omitting the phrase. tendency_of_X means derivative of X with respect to time. Air temperature is the bulk temperature of the air, not the surface (skin) temperature." .

<http://purl.oclc.org/NET/ssnx/cf/cf-property#tendency_of_air_temperature_due_to_dry_convection>
  a owl:NamedIndividual, <http://purl.oclc.org/NET/ssnx/qu/dim#TemperatureDrift> ;
  rdfs:label "tendency of air temperature due to dry convection" ;
  rdfs:isDefinedBy <http://purl.oclc.org/NET/ssnx/cf/cf-property> ;
  rdfs:comment "The specification of a physical process by the phrase due_to_process means that the quantity named is a single term in a sum of terms which together compose the general quantity named by omitting the phrase. tendency_of_X means derivative of X with respect to time. Air temperature is the bulk temperature of the air, not the surface (skin) temperature." .

<http://purl.oclc.org/NET/ssnx/cf/cf-property#tendency_of_air_temperature_due_to_longwave_heating>
  a owl:NamedIndividual, <http://purl.oclc.org/NET/ssnx/qu/dim#TemperatureDrift> ;
  rdfs:label "tendency of air temperature due to longwave heating" ;
  rdfs:isDefinedBy <http://purl.oclc.org/NET/ssnx/cf/cf-property> ;
  rdfs:comment "The specification of a physical process by the phrase due_to_process means that the quantity named is a single term in a sum of terms which together compose the general quantity named by omitting the phrase. tendency_of_X means derivative of X with respect to time. longwave means longwave radiation. Air temperature is the bulk temperature of the air, not the surface (skin) temperature." .

<http://purl.oclc.org/NET/ssnx/cf/cf-property#tendency_of_air_temperature_due_to_longwave_heating_assuming_clear_sky>
  a owl:NamedIndividual, <http://purl.oclc.org/NET/ssnx/qu/dim#TemperatureDrift> ;
  rdfs:label "tendency of air temperature due to longwave heating assuming clear sky" ;
  rdfs:isDefinedBy <http://purl.oclc.org/NET/ssnx/cf/cf-property> ;
  rdfs:comment "The specification of a physical process by the phrase due_to_process means that the quantity named is a single term in a sum of terms which together compose the general quantity named by omitting the phrase. A phrase assuming_condition indicates that the named quantity is the value which would obtain if all aspects of the system were unaltered except for the assumption of the circumstances specified by the condition. tendency_of_X means derivative of X with respect to time. longwave means longwave radiation. Air temperature is the bulk temperature of the air, not the surface (skin) temperature." .

<http://purl.oclc.org/NET/ssnx/cf/cf-property#tendency_of_air_temperature_due_to_model_physics>
  a owl:NamedIndividual, <http://purl.oclc.org/NET/ssnx/qu/dim#TemperatureDrift> ;
  rdfs:label "tendency of air temperature due to model physics" ;
  rdfs:isDefinedBy <http://purl.oclc.org/NET/ssnx/cf/cf-property> ;
  rdfs:comment "Air temperature is the bulk temperature of the air, not the surface (skin) temperature.  The specification of a physical process by the phrase due_to_process means that the quantity named is a  single term in a sum of terms which together compose the general quantity  named by omitting the phrase.  tendency_of_X means derivative of X with respect to time. " .

<http://purl.oclc.org/NET/ssnx/cf/cf-property#tendency_of_air_temperature_due_to_moist_convection>
  a owl:NamedIndividual, <http://purl.oclc.org/NET/ssnx/qu/dim#TemperatureDrift> ;
  rdfs:label "tendency of air temperature due to moist convection" ;
  rdfs:isDefinedBy <http://purl.oclc.org/NET/ssnx/cf/cf-property> ;
  rdfs:comment "The specification of a physical process by the phrase due_to_process means that the quantity named is a single term in a sum of terms which together compose the general quantity named by omitting the phrase. tendency_of_X means derivative of X with respect to time. Air temperature is the bulk temperature of the air, not the surface (skin) temperature." .

<http://purl.oclc.org/NET/ssnx/cf/cf-property#tendency_of_air_temperature_due_to_radiative_heating>
  a owl:NamedIndividual, <http://purl.oclc.org/NET/ssnx/qu/dim#TemperatureDrift> ;
  rdfs:label "tendency of air temperature due to radiative heating" ;
  rdfs:isDefinedBy <http://purl.oclc.org/NET/ssnx/cf/cf-property> ;
  rdfs:comment "The specification of a physical process by the phrase due_to_process means that the quantity named is a single term in a sum of terms which together compose the general quantity named by omitting the phrase. tendency_of_X means derivative of X with respect to time. Air temperature is the bulk temperature of the air, not the surface (skin) temperature." .

<http://purl.oclc.org/NET/ssnx/cf/cf-property#tendency_of_air_temperature_due_to_shortwave_heating>
  a owl:NamedIndividual, <http://purl.oclc.org/NET/ssnx/qu/dim#TemperatureDrift> ;
  rdfs:label "tendency of air temperature due to shortwave heating" ;
  rdfs:isDefinedBy <http://purl.oclc.org/NET/ssnx/cf/cf-property> ;
  rdfs:comment "The specification of a physical process by the phrase due_to_process means that the quantity named is a single term in a sum of terms which together compose the general quantity named by omitting the phrase. tendency_of_X means derivative of X with respect to time. shortwave means shortwave radiation. Air temperature is the bulk temperature of the air, not the surface (skin) temperature." .

<http://purl.oclc.org/NET/ssnx/cf/cf-property#tendency_of_air_temperature_due_to_shortwave_heating_assuming_clear_sky>
  a owl:NamedIndividual, <http://purl.oclc.org/NET/ssnx/qu/dim#TemperatureDrift> ;
  rdfs:label "tendency of air temperature due to shortwave heating assuming clear sky" ;
  rdfs:isDefinedBy <http://purl.oclc.org/NET/ssnx/cf/cf-property> ;
  rdfs:comment "The specification of a physical process by the phrase due_to_process means that the quantity named is a single term in a sum of terms which together compose the general quantity named by omitting the phrase. A phrase assuming_condition indicates that the named quantity is the value which would obtain if all aspects of the system were unaltered except for the assumption of the circumstances specified by the condition. tendency_of_X means derivative of X with respect to time. shortwave means shortwave radiation. Air temperature is the bulk temperature of the air, not the surface (skin) temperature." .

<http://purl.oclc.org/NET/ssnx/cf/cf-property#tendency_of_air_temperature_due_to_stratiform_cloud_and_precipitation_and_boundary_layer_mixing>
  a owl:NamedIndividual, <http://purl.oclc.org/NET/ssnx/qu/dim#TemperatureDrift> ;
  rdfs:label "tendency of air temperature due to stratiform cloud and precipitation and boundary layer mixing" ;
  rdfs:isDefinedBy <http://purl.oclc.org/NET/ssnx/cf/cf-property> ;
  rdfs:comment "Air temperature is the bulk temperature of the air, not the surface (skin) temperature.  In an atmosphere model, stratiform cloud is that produced by large-scale convergence (not the convection schemes).  The specification of a physical process by the phrase due_to_process means that the quantity named is a  single term in a sum of terms which together compose the general quantity  named by omitting the phrase.  tendency_of_X means derivative of X with respect to time. " .

<http://purl.oclc.org/NET/ssnx/cf/cf-property#tendency_of_air_temperature_due_to_stratiform_precipitation>
  a owl:NamedIndividual, <http://purl.oclc.org/NET/ssnx/qu/dim#TemperatureDrift> ;
  rdfs:label "tendency of air temperature due to stratiform precipitation" ;
  rdfs:isDefinedBy <http://purl.oclc.org/NET/ssnx/cf/cf-property> ;
  rdfs:comment "Air temperature is the bulk temperature of the air, not the surface (skin) temperature. In an atmosphere model, stratiform cloud is that produced by large-scale convergence (not the convection schemes). The specification of a physical process by the phrase due_to_process means that the quantity named is a single term in a sum of terms which together compose the general quantity named by omitting the phrase. tendency_of_X means derivative of X with respect to time." .

<http://purl.oclc.org/NET/ssnx/cf/cf-property#tendency_of_air_temperature_due_to_turbulence>
  a owl:NamedIndividual, <http://purl.oclc.org/NET/ssnx/qu/dim#TemperatureDrift> ;
  rdfs:label "tendency of air temperature due to turbulence" ;
  rdfs:isDefinedBy <http://purl.oclc.org/NET/ssnx/cf/cf-property> ;
  rdfs:comment "The specification of a physical process by the phrase due_to_process means that the quantity named is a single term in a sum of terms which together compose the general quantity named by omitting the phrase. tendency_of_X means derivative of X with respect to time. Air temperature is the bulk temperature of the air, not the surface (skin) temperature." .

<http://purl.oclc.org/NET/ssnx/cf/cf-property#tendency_of_upward_air_velocity>
  a owl:NamedIndividual, <http://purl.oclc.org/NET/ssnx/qu/dim#Acceleration> ;
  rdfs:label "tendency of upward air velocity" ;
  rdfs:isDefinedBy <http://purl.oclc.org/NET/ssnx/cf/cf-property> ;
  rdfs:comment "tendency_of_X means derivative of X with respect to time. A velocity is a vector quantity. Upward indicates a vector component which is positive when directed upward (negative downward). Upward air velocity is the vertical component of the 3D air velocity vector." .

<http://purl.oclc.org/NET/ssnx/cf/cf-property#tendency_of_upward_air_velocity_due_to_advection>
  a owl:NamedIndividual, <http://purl.oclc.org/NET/ssnx/qu/dim#Acceleration> ;
  rdfs:label "tendency of upward air velocity due to advection" ;
  rdfs:isDefinedBy <http://purl.oclc.org/NET/ssnx/cf/cf-property> ;
  rdfs:comment "The specification of a physical process by the phrase due_to_process means that the quantity named is a single term in a sum of terms which together compose the general quantity named by omitting the phrase. tendency_of_X means derivative of X with respect to time. A velocity is a vector quantity. Upward indicates a vector component which is positive when directed upward (negative downward). Upward air velocity is the vertical component of the 3D air velocity vector." .

<http://purl.oclc.org/NET/ssnx/cf/cf-property#upward_air_velocity>
  a owl:NamedIndividual, <http://purl.oclc.org/NET/ssnx/qu/dim#VelocityOrSpeed> ;
  rdfs:label "upward air velocity" ;
  rdfs:isDefinedBy <http://purl.oclc.org/NET/ssnx/cf/cf-property> ;
  rdfs:comment "A velocity is a vector quantity. Upward indicates a vector component which is positive when directed upward (negative downward). Upward air velocity is the vertical component of the 3D air velocity vector." .

<http://purl.oclc.org/NET/ssnx/cf/cf-property#upward_eastward_momentum_flux_in_air_due_to_nonorographic_eastward_gravity_waves>
  a owl:NamedIndividual, <http://purl.oclc.org/NET/ssnx/qu/dim#StressOrPressure> ;
  rdfs:label "upward eastward momentum flux in air due to nonorographic eastward gravity waves" ;
  rdfs:isDefinedBy <http://purl.oclc.org/NET/ssnx/cf/cf-property> ;
  rdfs:comment "The specification of a physical process by the phrase due_to_process means that the quantity named is a single term in a sum of terms which together compose the general quantity named by omitting the phrase. Upward indicates a vector component which is positive when directed upward (negative downward). Eastward indicates a vector component which is positive when directed eastward (negative westward). Upward eastward indicates the ZX component of a tensor. An upward eastward momentum flux is an upward flux of eastward momentum, which accelerates the upper medium eastward and the lower medium westward.  Momentum flux is dimensionally equivalent to stress and pressure.  In accordance with common usage in geophysical disciplines, flux implies per unit area, called flux density in physics. The total upward eastward momentum flux due to gravity waves is the sum of the fluxes due to orographic gravity waves and nonorographic waves. The upward eastward momentum flux due to orographic gravity waves has the standard name upward_eastward_momentum_flux_in_air_due_to_orographic_gravity_waves. The total upward eastward momentum flux due to nonorographic gravity waves is the sum of the fluxes due to eastward and westward propagating waves. The latter has the standard name upward_eastward_momentum_flux_in_air_due_to_nonorographic_westward_gravity_waves." .

<http://purl.oclc.org/NET/ssnx/cf/cf-property#upward_eastward_momentum_flux_in_air_due_to_nonorographic_westward_gravity_waves>
  a owl:NamedIndividual, <http://purl.oclc.org/NET/ssnx/qu/dim#StressOrPressure> ;
  rdfs:label "upward eastward momentum flux in air due to nonorographic westward gravity waves" ;
  rdfs:isDefinedBy <http://purl.oclc.org/NET/ssnx/cf/cf-property> ;
  rdfs:comment "The specification of a physical process by the phrase due_to_process means that the quantity named is a single term in a sum of terms which together compose the general quantity named by omitting the phrase. Upward indicates a vector component which is positive when directed upward (negative downward).  Eastward indicates a vector component which is positive when directed eastward (negative westward).  Upward eastward indicates the ZX component of a tensor. An upward eastward momentum flux is an upward flux of eastward momentum, which accelerates the upper medium eastward and the lower medium westward.  Momentum flux is dimensionally equivalent to stress and pressure.  In accordance with common usage in geophysical disciplines, flux implies per unit area, called flux density in physics. The total upward eastward momentum flux due to gravity waves is the sum of the fluxes due to orographic gravity waves and nonorographic waves. The upward eastward momentum flux due to orographic gravity waves has the standard name upward_eastward_momentum_flux_in_air_due_to_orographic_gravity_waves. The total upward eastward momentum flux due to nonorographic gravity waves is the sum of the fluxes due to eastward and westward propagating waves. The former has the standard name upward_eastward_momentum_flux_in_air_due_to_nonorographic_eastward _gravity_waves." .

<http://purl.oclc.org/NET/ssnx/cf/cf-property#upward_eastward_momentum_flux_in_air_due_to_orographic_gravity_waves>
  a owl:NamedIndividual, <http://purl.oclc.org/NET/ssnx/qu/dim#StressOrPressure> ;
  rdfs:label "upward eastward momentum flux in air due to orographic gravity waves" ;
  rdfs:isDefinedBy <http://purl.oclc.org/NET/ssnx/cf/cf-property> ;
  rdfs:comment "The specification of a physical process by the phrase due_to_process means that the quantity named is a single term in a sum of terms which together compose the general quantity named by omitting the phrase. Upward indicates a vector component which is positive when directed upward (negative downward).  Eastward indicates a vector component which is positive when directed eastward (negative westward).  Upward eastward indicates the ZX component of a tensor. An upward eastward momentum flux is an upward flux of eastward momentum, which accelerates the upper medium eastward and the lower medium westward.  Momentum flux is dimensionally equivalent to stress and pressure.  In accordance with common usage in geophysical disciplines, flux implies per unit area, called flux density in physics. The total upward eastward momentum flux due to gravity waves is the sum of the fluxes due to orographic gravity waves and nonorographic waves. The total upward eastward momentum flux due to nonorographic gravity waves is the sum of the fluxes due to eastward and westward propagating waves. These quantities have the standard names upward_eastward_momentum_flux_in_air_due_to_nonorographic_eastward_gravity_waves and upward_eastward_momentum_flux_in_air_due_to_nonorographic_westward_gravity_waves, respectively." .

<http://purl.oclc.org/NET/ssnx/cf/cf-property#upward_heat_flux_in_air>
  a owl:NamedIndividual, <http://purl.oclc.org/NET/ssnx/qu/dim#EnergyFlux> ;
  rdfs:label "upward heat flux in air" ;
  rdfs:isDefinedBy <http://purl.oclc.org/NET/ssnx/cf/cf-property> ;
  rdfs:comment "Upward indicates a vector component which is positive when directed upward (negative downward). The vertical heat flux in air is the sum of all heat fluxes i.e. radiative, latent and sensible. In accordance with common usage in geophysical disciplines, flux implies per unit area, called flux density in physics." .

<http://purl.oclc.org/NET/ssnx/cf/cf-property#upward_mass_flux_of_air>
  a owl:NamedIndividual, <http://purl.oclc.org/NET/ssnx/qu/dim#MassPerTimePerArea> ;
  rdfs:label "upward mass flux of air" ;
  rdfs:isDefinedBy <http://purl.oclc.org/NET/ssnx/cf/cf-property> ;
  rdfs:comment "Upward indicates a vector component which is positive when directed upward (negative downward). In accordance with common usage in geophysical disciplines, flux implies per unit area, called flux density in physics." .

<http://purl.oclc.org/NET/ssnx/cf/cf-property#upward_water_vapor_flux_in_air>
  a owl:NamedIndividual, <http://purl.oclc.org/NET/ssnx/qu/dim#MassPerTimePerArea> ;
  rdfs:label "upward water vapor flux in air" ;
  rdfs:isDefinedBy <http://purl.oclc.org/NET/ssnx/cf/cf-property> ;
  rdfs:comment "Upward indicates a vector component which is positive when directed upward (negative downward). In accordance with common usage in geophysical disciplines, flux implies per unit area, called flux density in physics." .

<http://purl.oclc.org/NET/ssnx/cf/cf-property#upward_water_vapor_flux_in_air_due_to_diffusion>
  a owl:NamedIndividual, <http://purl.oclc.org/NET/ssnx/qu/dim#MassPerTimePerArea> ;
  rdfs:label "upward water vapor flux in air due to diffusion" ;
  rdfs:isDefinedBy <http://purl.oclc.org/NET/ssnx/cf/cf-property> ;
  rdfs:comment "The specification of a physical process by the phrase due_to_process means that the quantity named is a single term in a sum of terms which together compose the general quantity named by omitting the phrase. Upward indicates a vector component which is positive when directed upward (negative downward). In accordance with common usage in geophysical disciplines, flux implies per unit area, called flux density in physics." .

<http://purl.oclc.org/NET/ssnx/cf/cf-property#upwelling_longwave_flux_in_air>
  a owl:NamedIndividual, <http://purl.oclc.org/NET/ssnx/qu/dim#EnergyFlux> ;
  rdfs:label "upwelling longwave flux in air" ;
  rdfs:isDefinedBy <http://purl.oclc.org/NET/ssnx/cf/cf-property> ;
  rdfs:comment "longwave means longwave radiation. Upwelling radiation is radiation from below. It does not mean net upward. When thought of as being incident on a surface, a radiative flux is sometimes called irradiance. In addition, it is identical with the quantity measured by a cosine-collector light-meter and sometimes called vector irradiance. In accordance with common usage in geophysical disciplines, flux implies per unit area, called flux density in physics." .

<http://purl.oclc.org/NET/ssnx/cf/cf-property#upwelling_longwave_flux_in_air_assuming_clear_sky>
  a owl:NamedIndividual, <http://purl.oclc.org/NET/ssnx/qu/dim#EnergyFlux> ;
  rdfs:label "upwelling longwave flux in air assuming clear sky" ;
  rdfs:isDefinedBy <http://purl.oclc.org/NET/ssnx/cf/cf-property> ;
  rdfs:comment "Upwelling radiation is radiation from below. It does not mean net upward.  When thought of as being incident on a surface, a radiative flux is sometimes called irradiance.  In addition, it is identical with the quantity measured by a cosine-collector light-meter and sometimes called vector irradiance.  In accordance with common usage in geophysical disciplines, flux implies per unit area, called flux density in physics.  A phrase assuming_condition  indicates that the named quantity is the value which would obtain if all  aspects of the system were unaltered except for the assumption of the  circumstances specified by the condition.  longwave means longwave radiation. " .

<http://purl.oclc.org/NET/ssnx/cf/cf-property#upwelling_longwave_radiance_in_air>
  a owl:NamedIndividual, <http://purl.oclc.org/NET/ssnx/qu/dim#Radiance> ;
  rdfs:label "upwelling longwave radiance in air" ;
  rdfs:isDefinedBy <http://purl.oclc.org/NET/ssnx/cf/cf-property> ;
  rdfs:comment "longwave means longwave radiation. Upwelling radiation is radiation from below. It does not mean net upward. Radiance is the radiative flux in a particular direction, per unit of solid angle. The direction towards which it is going must be specified, for instance with a coordinate of zenith_angle. If the radiation does not depend on direction, a standard name of isotropic radiance should be chosen instead." .

<http://purl.oclc.org/NET/ssnx/cf/cf-property#upwelling_shortwave_flux_in_air>
  a owl:NamedIndividual, <http://purl.oclc.org/NET/ssnx/qu/dim#EnergyFlux> ;
  rdfs:label "upwelling shortwave flux in air" ;
  rdfs:isDefinedBy <http://purl.oclc.org/NET/ssnx/cf/cf-property> ;
  rdfs:comment "shortwave means shortwave radiation. Upwelling radiation is radiation from below. It does not mean net upward. When thought of as being incident on a surface, a radiative flux is sometimes called irradiance. In addition, it is identical with the quantity measured by a cosine-collector light-meter and sometimes called vector irradiance. In accordance with common usage in geophysical disciplines, flux implies per unit area, called flux density in physics." .

<http://purl.oclc.org/NET/ssnx/cf/cf-property#upwelling_shortwave_flux_in_air_assuming_clear_sky>
  a owl:NamedIndividual, <http://purl.oclc.org/NET/ssnx/qu/dim#EnergyFlux> ;
  rdfs:label "upwelling shortwave flux in air assuming clear sky" ;
  rdfs:isDefinedBy <http://purl.oclc.org/NET/ssnx/cf/cf-property> ;
  rdfs:comment "Upwelling radiation is radiation from below. It does not mean net upward.  When thought of as being incident on a surface, a radiative flux is sometimes called irradiance.  In addition, it is identical with the quantity measured by a cosine-collector light-meter and sometimes called vector irradiance.  In accordance with common usage in geophysical disciplines, flux implies per unit area, called flux density in physics.  A phrase assuming_condition  indicates that the named quantity is the value which would obtain if all  aspects of the system were unaltered except for the assumption of the  circumstances specified by the condition.  shortwave means shortwave radiation. " .

<http://purl.oclc.org/NET/ssnx/cf/cf-property#upwelling_shortwave_radiance_in_air>
  a owl:NamedIndividual, <http://purl.oclc.org/NET/ssnx/qu/dim#Radiance> ;
  rdfs:label "upwelling shortwave radiance in air" ;
  rdfs:isDefinedBy <http://purl.oclc.org/NET/ssnx/cf/cf-property> ;
  rdfs:comment "shortwave means shortwave radiation. Upwelling radiation is radiation from below. It does not mean net upward. Radiance is the radiative flux in a particular direction, per unit of solid angle. The direction towards which it is going must be specified, for instance with a coordinate of zenith_angle. If the radiation does not depend on direction, a standard name of isotropic radiance should be chosen instead." .

<http://purl.oclc.org/NET/ssnx/cf/cf-property#visibility_in_air>
  a owl:NamedIndividual, <http://purl.oclc.org/NET/ssnx/qu/dim#Distance> ;
  rdfs:label "visibility in air" ;
  rdfs:isDefinedBy <http://purl.oclc.org/NET/ssnx/cf/cf-property> ;
  rdfs:comment "The visibility is the distance at which something can be" .   

<http://purl.oclc.org/NET/ssnx/cf/cf-property#air_pressure_at_cloud_base>
  a owl:NamedIndividual, <http://purl.oclc.org/NET/ssnx/qu/dim#StressOrPressure> ;
  rdfs:label "air pressure at cloud base" ;
  rdfs:isDefinedBy <http://purl.oclc.org/NET/ssnx/cf/cf-property> ;
  rdfs:comment "cloud_base refers to the base of the lowest cloud." .
  
<http://purl.oclc.org/NET/ssnx/cf/cf-property#air_pressure_at_convective_cloud_top>
  a owl:NamedIndividual, <http://purl.oclc.org/NET/ssnx/qu/dim#StressOrPressure> ;
  rdfs:label "air pressure at convective cloud top" ;
  rdfs:comment "cloud_top refers to the top of the highest cloud. Convective cloud is that produced by the convection schemes in an atmosphere model." ;
  rdfs:isDefinedBy <http://purl.oclc.org/NET/ssnx/cf/cf-property> .

<http://purl.oclc.org/NET/ssnx/cf/cf-property#air_temperature_at_cloud_top>
  a owl:NamedIndividual, <http://purl.oclc.org/NET/ssnx/qu/dim#Temperature> ;
  rdfs:label "air temperature at cloud top" ;
  rdfs:comment "cloud_top refers to the top of the highest cloud. Air temperature is the bulk temperature of the air, not the surface (skin) temperature." ;
  rdfs:isDefinedBy <http://purl.oclc.org/NET/ssnx/cf/cf-property> .

<http://purl.oclc.org/NET/ssnx/cf/cf-property#air_pressure_at_cloud_top>
  a owl:NamedIndividual, <http://purl.oclc.org/NET/ssnx/qu/dim#StressOrPressure> ;
  rdfs:label "air pressure at cloud top" ;
  rdfs:comment "cloud_top refers to the top of the highest cloud." ;
  rdfs:isDefinedBy <http://purl.oclc.org/NET/ssnx/cf/cf-property> .   
  
<http://purl.oclc.org/NET/ssnx/cf/cf-property#air_pressure_at_convective_cloud_base>
  a owl:NamedIndividual, <http://purl.oclc.org/NET/ssnx/qu/dim#StressOrPressure> ;
  rdfs:label "air pressure at convective cloud base" ;
  rdfs:comment "cloud_base refers to the base of the lowest cloud. Convective cloud is that produced by the convection schemes in an atmosphere model." ;
  rdfs:isDefinedBy <http://purl.oclc.org/NET/ssnx/cf/cf-property> .   

<http://purl.oclc.org/NET/ssnx/cf/cf-property#air_pressure_at_freezing_level>
  a owl:NamedIndividual, <http://purl.oclc.org/NET/ssnx/qu/dim#StressOrPressure> ;
  rdfs:label "air pressure at freezing level" ;
  rdfs:isDefinedBy <http://purl.oclc.org/NET/ssnx/cf/cf-property> .    

<http://purl.oclc.org/NET/ssnx/cf/cf-property#tropopause_air_pressure>
  a owl:NamedIndividual, <http://purl.oclc.org/NET/ssnx/qu/dim#StressOrPressure> ;
  rdfs:label "tropopause air pressure" ;
  rdfs:isDefinedBy <http://purl.oclc.org/NET/ssnx/cf/cf-property> .    

<http://purl.oclc.org/NET/ssnx/cf/cf-property#tropopause_air_temperature>
  a owl:NamedIndividual, <http://purl.oclc.org/NET/ssnx/qu/dim#Temperature> ;
  rdfs:label "tropopause air temperature" ;
  rdfs:comment "Air temperature is the bulk temperature of the air, not the surface (skin) temperature." ;
  rdfs:isDefinedBy <http://purl.oclc.org/NET/ssnx/cf/cf-property> .

<http://purl.oclc.org/NET/ssnx/cf/cf-property#minus_one_times_surface_upwelling_longwave_flux_in_air>
  a owl:NamedIndividual, <http://purl.oclc.org/NET/ssnx/qu/dim#EnergyFlux> ;
  rdfs:label "minus one times surface upwelling longwave flux in air" ;
  rdfs:isDefinedBy <http://purl.oclc.org/NET/ssnx/cf/cf-property> ;
  rdfs:comment "Minus one times means that the quantity described takes the opposite sign convention  to that for the quantity which has the same standard name apart from this phrase, i.e. the two quantities differ from one another by a factor of -1. The surface called surface means the lower boundary of the atmosphere. longwave means longwave radiation. Upwelling radiation is radiation from below. It does not mean net upward. When thought of as being incident on a surface, a radiative flux is sometimes called irradiance. In addition, it is identical with the quantity measured by a cosine-collector light-meter and sometimes called vector irradiance. In accordance with common usage in geophysical disciplines, flux implies per unit area, called flux density in physics." .

<http://purl.oclc.org/NET/ssnx/cf/cf-property#minus_one_times_surface_upwelling_shortwave_flux_in_air>
  a owl:NamedIndividual, <http://purl.oclc.org/NET/ssnx/qu/dim#EnergyFlux> ;
  rdfs:label "minus one times surface upwelling shortwave flux in air" ;
  rdfs:isDefinedBy <http://purl.oclc.org/NET/ssnx/cf/cf-property> ;
  rdfs:comment "Minus one times means that the quantity described takes the opposite sign convention  to that for the quantity which has the same standard name apart from this phrase, i.e. the two quantities differ from one another by a factor of -1. The surface called surface means the lower boundary of the atmosphere. shortwave means shortwave radiation. Upwelling radiation is radiation from below. It does not mean net upward. When thought of as being incident on a surface, a radiative flux is sometimes called irradiance. In addition, it is identical with the quantity measured by a cosine-collector light-meter and sometimes called vector irradiance. In accordance with common usage in geophysical disciplines, flux implies per unit area, called flux density in physics." .

<http://purl.oclc.org/NET/ssnx/cf/cf-property#surface_air_pressure>
  a owl:NamedIndividual, <http://purl.oclc.org/NET/ssnx/qu/dim#StressOrPressure> ;
  rdfs:label "surface air pressure" ;
  rdfs:isDefinedBy <http://purl.oclc.org/NET/ssnx/cf/cf-property> ;
  rdfs:comment "The surface called surface means the lower boundary of the atmosphere." .

<http://purl.oclc.org/NET/ssnx/cf/cf-property#surface_diffuse_downwelling_photosynthetic_radiative_flux_in_air>
  a owl:NamedIndividual, <http://purl.oclc.org/NET/ssnx/qu/dim#EnergyFlux> ;
  rdfs:label "surface diffuse downwelling photosynthetic radiative flux in air" ;
  rdfs:isDefinedBy <http://purl.oclc.org/NET/ssnx/cf/cf-property> ;
  rdfs:comment "The surface called surface means the lower boundary of the atmosphere. Downwelling radiation is radiation from above. It does not mean net downward. Radiative flux is the sum of shortwave and longwave radiative fluxes. Photosynthetic radiation is the part of the spectrum which is used in photosynthesis e.g. 300-700 nm. The range of wavelengths could be specified precisely by the bounds of a coordinate of radiation_wavelength. When thought of as being incident on a surface, a radiative flux is sometimes called irradiance. In addition, it is identical with the quantity measured by a cosine-collector light-meter and sometimes called vector irradiance. In accordance with common usage in geophysical disciplines, flux implies per unit area, called flux density in physics." .

<http://purl.oclc.org/NET/ssnx/cf/cf-property#surface_downward_heat_flux_in_air>
  a owl:NamedIndividual, <http://purl.oclc.org/NET/ssnx/qu/dim#EnergyFlux> ;
  rdfs:label "surface downward heat flux in air" ;
  rdfs:isDefinedBy <http://purl.oclc.org/NET/ssnx/cf/cf-property> ;
  rdfs:comment "The surface called surface means the lower boundary of the atmosphere. Downward indicates a vector component which is positive when directed downward (negative upward). The vertical heat flux in air is the sum of all heat fluxes i.e. radiative, latent and sensible. In accordance with common usage in geophysical disciplines, flux implies per unit area, called flux density in physics." .

<http://purl.oclc.org/NET/ssnx/cf/cf-property#surface_downwelling_longwave_flux_in_air>
  a owl:NamedIndividual, <http://purl.oclc.org/NET/ssnx/qu/dim#EnergyFlux> ;
  rdfs:label "surface downwelling longwave flux in air" ;
  rdfs:isDefinedBy <http://purl.oclc.org/NET/ssnx/cf/cf-property> ;
  rdfs:comment "The surface called surface means the lower boundary of the atmosphere. longwave means longwave radiation. Downwelling radiation is radiation from above. It does not mean net downward. When thought of as being incident on a surface, a radiative flux is sometimes called irradiance. In addition, it is identical with the quantity measured by a cosine-collector light-meter and sometimes called vector irradiance. In accordance with common usage in geophysical disciplines, flux implies per unit area, called flux density in physics." .

<http://purl.oclc.org/NET/ssnx/cf/cf-property#surface_downwelling_longwave_flux_in_air_assuming_clear_sky>
  a owl:NamedIndividual, <http://purl.oclc.org/NET/ssnx/qu/dim#EnergyFlux> ;
  rdfs:label "surface downwelling longwave flux in air assuming clear sky" ;
  rdfs:isDefinedBy <http://purl.oclc.org/NET/ssnx/cf/cf-property> ;
  rdfs:comment "The surface called surface means the lower boundary of the atmosphere. A phrase assuming_condition indicates that the named quantity is the value which would obtain if all aspects of the system were unaltered except for the assumption of the circumstances specified by the condition. longwave means longwave radiation. Downwelling radiation is radiation from above. It does not mean net downward. When thought of as being incident on a surface, a radiative flux is sometimes called irradiance. In addition, it is identical with the quantity measured by a cosine-collector light-meter and sometimes called vector irradiance. In accordance with common usage in geophysical disciplines, flux implies per unit area, called flux density in physics." .

<http://purl.oclc.org/NET/ssnx/cf/cf-property#surface_downwelling_photosynthetic_photon_flux_in_air>
  a owl:NamedIndividual, <http://purl.oclc.org/NET/ssnx/qu/dim#PhotonFluxDensity> ;
  rdfs:label "surface downwelling photosynthetic photon flux in air" ;
  rdfs:isDefinedBy <http://purl.oclc.org/NET/ssnx/cf/cf-property> ;
  rdfs:comment "The surface called surface means the lower boundary of the atmosphere. Downwelling radiation is radiation from above. It does not mean net downward. Photosynthetic radiation is the part of the spectrum which is used in photosynthesis e.g. 300-700 nm. The range of wavelengths could be specified precisely by the bounds of a coordinate of radiation_wavelength. A photon flux is specified in terms of numbers of photons expressed in moles. In accordance with common usage in geophysical disciplines, flux implies per unit area, called flux density in physics." .

<http://purl.oclc.org/NET/ssnx/cf/cf-property#surface_downwelling_photosynthetic_radiative_flux_in_air>
  a owl:NamedIndividual, <http://purl.oclc.org/NET/ssnx/qu/dim#EnergyFlux> ;
  rdfs:label "surface downwelling photosynthetic radiative flux in air" ;
  rdfs:isDefinedBy <http://purl.oclc.org/NET/ssnx/cf/cf-property> ;
  rdfs:comment "The surface called surface means the lower boundary of the atmosphere. Downwelling radiation is radiation from above. It does not mean net downward. Radiative flux is the sum of shortwave and longwave radiative fluxes. Photosynthetic radiation is the part of the spectrum which is used in photosynthesis e.g. 300-700 nm. The range of wavelengths could be specified precisely by the bounds of a coordinate of radiation_wavelength. When thought of as being incident on a surface, a radiative flux is sometimes called irradiance. In addition, it is identical with the quantity measured by a cosine-collector light-meter and sometimes called vector irradiance. In accordance with common usage in geophysical disciplines, flux implies per unit area, called flux density in physics." .

<http://purl.oclc.org/NET/ssnx/cf/cf-property#surface_downwelling_shortwave_flux_in_air>
  a owl:NamedIndividual, <http://purl.oclc.org/NET/ssnx/qu/dim#EnergyFlux> ;
  rdfs:label "surface downwelling shortwave flux in air" ;
  rdfs:isDefinedBy <http://purl.oclc.org/NET/ssnx/cf/cf-property> ;
  rdfs:comment "The surface called surface means the lower boundary of the atmosphere. shortwave means shortwave radiation. Downwelling radiation is radiation from above. It does not mean net downward. Surface downwelling shortwave is the sum of direct and diffuse solar radiation incident on the surface, and is sometimes called global radiation. When thought of as being incident on a surface, a radiative flux is sometimes called irradiance. In addition, it is identical with the quantity measured by a cosine-collector light-meter and sometimes called vector irradiance. In accordance with common usage in geophysical disciplines, flux implies per unit area, called flux density in physics." .

<http://purl.oclc.org/NET/ssnx/cf/cf-property#surface_downwelling_shortwave_flux_in_air_assuming_clear_sky>
  a owl:NamedIndividual, <http://purl.oclc.org/NET/ssnx/qu/dim#EnergyFlux> ;
  rdfs:label "surface downwelling shortwave flux in air assuming clear sky" ;
  rdfs:isDefinedBy <http://purl.oclc.org/NET/ssnx/cf/cf-property> ;
  rdfs:comment "The surface called surface means the lower boundary of the atmosphere. A phrase assuming_condition indicates that the named quantity is the value which would obtain if all aspects of the system were unaltered except for the assumption of the circumstances specified by the condition. shortwave means shortwave radiation. Downwelling radiation is radiation from above. It does not mean net downward. Surface downwelling shortwave is the sum of direct and diffuse solar radiation incident on the surface, and is sometimes called global radiation. When thought of as being incident on a surface, a radiative flux is sometimes called irradiance. In addition, it is identical with the quantity measured by a cosine-collector light-meter and sometimes called vector irradiance. In accordance with common usage in geophysical disciplines, flux implies per unit area, called flux density in physics." .

<http://purl.oclc.org/NET/ssnx/cf/cf-property#surface_upward_heat_flux_in_air>
  a owl:NamedIndividual, <http://purl.oclc.org/NET/ssnx/qu/dim#EnergyFlux> ;
  rdfs:label "surface upward heat flux in air" ;
  rdfs:isDefinedBy <http://purl.oclc.org/NET/ssnx/cf/cf-property> ;
  rdfs:comment "The surface called surface means the lower boundary of the atmosphere. Upward indicates a vector component which is positive when directed upward (negative downward). The vertical heat flux in air is the sum of all heat fluxes i.e. radiative, latent and sensible. In accordance with common usage in geophysical disciplines, flux implies per unit area, called flux density in physics." .

<http://purl.oclc.org/NET/ssnx/cf/cf-property#surface_upward_water_vapor_flux_in_air>
  a owl:NamedIndividual, <http://purl.oclc.org/NET/ssnx/qu/dim#MassPerTimePerArea> ;
  rdfs:label "surface upward water vapor flux in air" ;
  rdfs:isDefinedBy <http://purl.oclc.org/NET/ssnx/cf/cf-property> ;
  rdfs:comment "The surface called surface means the lower boundary of the atmosphere.  Upward indicates a vector component which is positive when directed upward (negative downward).  In accordance with common usage in geophysical disciplines, flux implies per unit area, called flux density in physics." .

<http://purl.oclc.org/NET/ssnx/cf/cf-property#surface_upwelling_longwave_flux_in_air>
  a owl:NamedIndividual, <http://purl.oclc.org/NET/ssnx/qu/dim#EnergyFlux> ;
  rdfs:label "surface upwelling longwave flux in air" ;
  rdfs:isDefinedBy <http://purl.oclc.org/NET/ssnx/cf/cf-property> ;
  rdfs:comment "The surface called surface means the lower boundary of the atmosphere. longwave means longwave radiation. Upwelling radiation is radiation from below. It does not mean net upward. When thought of as being incident on a surface, a radiative flux is sometimes called irradiance. In addition, it is identical with the quantity measured by a cosine-collector light-meter and sometimes called vector irradiance. In accordance with common usage in geophysical disciplines, flux implies per unit area, called flux density in physics." .

<http://purl.oclc.org/NET/ssnx/cf/cf-property#surface_upwelling_longwave_flux_in_air_assuming_clear_sky>
  a owl:NamedIndividual, <http://purl.oclc.org/NET/ssnx/qu/dim#EnergyFlux> ;
  rdfs:label "surface upwelling longwave flux in air assuming clear sky" ;
  rdfs:isDefinedBy <http://purl.oclc.org/NET/ssnx/cf/cf-property> ;
  rdfs:comment "The surface called surface means the lower boundary of the atmosphere. A phrase assuming_condition indicates that the named quantity is the value which would obtain if all aspects of the system were unaltered except for the assumption of the circumstances specified by the condition. longwave means longwave radiation. Upwelling radiation is radiation from below. It does not mean net upward. When thought of as being incident on a surface, a radiative flux is sometimes called irradiance. In addition, it is identical with the quantity measured by a cosine-collector light-meter and sometimes called vector irradiance. In accordance with common usage in geophysical disciplines, flux implies per unit area, called flux density in physics." .

<http://purl.oclc.org/NET/ssnx/cf/cf-property#surface_upwelling_photosynthetic_photon_flux_in_air>
  a owl:NamedIndividual, <http://purl.oclc.org/NET/ssnx/qu/dim#PhotonFluxDensity> ;
  rdfs:label "surface upwelling photosynthetic photon flux in air" ;
  rdfs:isDefinedBy <http://purl.oclc.org/NET/ssnx/cf/cf-property> ;
  rdfs:comment "The surface called surface means the lower boundary of the atmosphere. Upwelling radiation is radiation from below. It does not mean net upward. Photosynthetic radiation is the part of the spectrum which is used in photosynthesis e.g. 300-700 nm. The range of wavelengths could be specified precisely by the bounds of a coordinate of radiation_wavelength. A photon flux is specified in terms of numbers of photons expressed in moles. In accordance with common usage in geophysical disciplines, flux implies per unit area, called flux density in physics." .

<http://purl.oclc.org/NET/ssnx/cf/cf-property#surface_upwelling_radiance_in_air>
  a owl:NamedIndividual, <http://purl.oclc.org/NET/ssnx/qu/dim#Radiance> ;
  rdfs:label "surface upwelling radiance in air" ;
  rdfs:isDefinedBy <http://purl.oclc.org/NET/ssnx/cf/cf-property> ;
  rdfs:comment "The surface called surface means the lower boundary of the atmosphere. Upwelling radiation is radiation from below. It does not mean net upward. Radiance is the radiative flux in a particular direction, per unit of solid angle. The direction towards which it is going must be specified, for instance with a coordinate of zenith_angle. If the radiation does not depend on direction, a standard name of isotropic radiance should be chosen instead." .

<http://purl.oclc.org/NET/ssnx/cf/cf-property#surface_upwelling_shortwave_flux_in_air>
  a owl:NamedIndividual, <http://purl.oclc.org/NET/ssnx/qu/dim#EnergyFlux> ;
  rdfs:label "surface upwelling shortwave flux in air" ;
  rdfs:isDefinedBy <http://purl.oclc.org/NET/ssnx/cf/cf-property> ;
  rdfs:comment "The surface called surface means the lower boundary of the atmosphere. shortwave means shortwave radiation. Upwelling radiation is radiation from below. It does not mean net upward. When thought of as being incident on a surface, a radiative flux is sometimes called irradiance. In addition, it is identical with the quantity measured by a cosine-collector light-meter and sometimes called vector irradiance. In accordance with common usage in geophysical disciplines, flux implies per unit area, called flux density in physics." .

<http://purl.oclc.org/NET/ssnx/cf/cf-property#surface_upwelling_shortwave_flux_in_air_assuming_clear_sky>
  a owl:NamedIndividual, <http://purl.oclc.org/NET/ssnx/qu/dim#EnergyFlux> ;
  rdfs:label "surface upwelling shortwave flux in air assuming clear sky" ;
  rdfs:isDefinedBy <http://purl.oclc.org/NET/ssnx/cf/cf-property> ;
  rdfs:comment "The surface called surface means the lower boundary of the atmosphere. A phrase assuming_condition indicates that the named quantity is the value which would obtain if all aspects of the system were unaltered except for the assumption of the circumstances specified by the condition. shortwave means shortwave radiation. Upwelling radiation is radiation from below. It does not mean net upward. When thought of as being incident on a surface, a radiative flux is sometimes called irradiance. In addition, it is identical with the quantity measured by a cosine-collector light-meter and sometimes called vector irradiance. In accordance with common usage in geophysical disciplines, flux implies per unit area, called flux density in" .

<http://purl.oclc.org/NET/ssnx/cf/cf-property#sound_pressure_in_water>
  a <http://purl.oclc.org/NET/ssnx/qu/dim#StressOrPressure> ;
  rdfs:label "sound pressure in water" ;
  rdfs:comment "Sound pressure is the difference from the local ambient pressure caused by a sound wave at a particular location and time." ;
  rdfs:isDefinedBy <http://purl.oclc.org/NET/ssnx/cf/cf-property> .

<http://purl.oclc.org/NET/ssnx/cf/cf-property#sound_intensity_in_water>
  a <http://purl.oclc.org/NET/ssnx/qu/dim#EnergyFlux> ;
  rdfs:label "sound intensity in water" ;
  rdfs:comment "Sound intensity is the sound energy per unit time per unit area." ;
  rdfs:isDefinedBy <http://purl.oclc.org/NET/ssnx/cf/cf-property> .   
