@prefix dct: <http://purl.org/dc/terms/> .
@prefix foaf: <http://xmlns.com/foaf/0.1/> .
@prefix owl: <http://www.w3.org/2002/07/owl#> .
@prefix prov: <http://www.w3.org/ns/prov#> .
@prefix rdfs: <http://www.w3.org/2000/01/rdf-schema#> .
@prefix schema: <https://schema.org/> .
@prefix skos: <http://www.w3.org/2004/02/skos/core#> .
@prefix sosa: <http://www.w3.org/ns/sosa/> .
@prefix xsd: <http://www.w3.org/2001/XMLSchema#> .

<https://raw.githubusercontent.com/opengeospatial/NamingAuthority/master/generic/entailed/properties.ttl> a prov:Entity ;
    dct:format "text/turtle" ;
    dct:hasVersion "git:b179d7ef9e4fdc812747694cefa34b78a0481011" ;
    prov:wasAttributedTo _:Ned287b39fc9b4f7688224933fef20ea7 ;
    prov:wasGeneratedBy [ a prov:Activity ;
            rdfs:label "Entailment and validation" ;
            rdfs:comment "python ogc.na.update_vocabs -w ./rainbow-data rainbow-data/catalog.ttl --use-git-status --update --graph-store https://defs-hosted.opengis.net/fuseki-hosted/data" ;
            prov:endedAtTime "2025-07-09T10:01:25.758137"^^xsd:dateTime ;
            prov:startedAtTime "2025-07-09T10:01:25.526250"^^xsd:dateTime ;
            prov:used [ a prov:Entity ;
                    rdfs:seeAlso <https://datashapes.org/dash.ttl> ],
                [ a prov:Entity ;
                    dct:format "text/turtle" ;
                    dct:hasVersion "git:b179d7ef9e4fdc812747694cefa34b78a0481011" ;
                    rdfs:seeAlso <https://raw.githubusercontent.com/opengeospatial/NamingAuthority/master/catalog.ttl> ],
                [ a prov:Entity ;
                    rdfs:seeAlso <http://www.opengis.net/def/metamodel/profiles/skos_shared> ],
                [ a prov:Entity ;
                    dct:format "text/turtle" ;
                    dct:hasVersion "git:b179d7ef9e4fdc812747694cefa34b78a0481011" ;
                    rdfs:seeAlso <https://raw.githubusercontent.com/opengeospatial/NamingAuthority/master/generic/properties.ttl> ] ;
            prov:wasAssociatedWith _:Ned287b39fc9b4f7688224933fef20ea7 ;
            prov:wasInformedBy [ dct:identifier "ff6b99fb-fe40-4437-9188-33c8a355cbe0" ] ] .

<https://w3id.org/ad4gd/air-quality/properties/CO> a skos:Concept,
        sosa:ObservableProperty ;
    dct:source [ skos:prefLabel "GEMET" ;
            foaf:homepage <https://www.eionet.europa.eu/gemet/en/concept/1173> ] ;
    owl:sameAs <http://purl.org/iot/vocab/iot-taxonomy-lite#ChemicalAgentAtmosphericConcentrationCO>,
        <http://vocabs.lter-europe.net/EnvThes/20809>,
        <https://uk-air.defra.gov.uk/air-pollution/glossary.php?glossary_id=18#18>,
        <https://www.eionet.europa.eu/gemet/en/concept/1173> ;
    skos:definition """Colorless, odourless, tasteless, non-corrosive, highly poisonous gas of about the same density as that of air. Very flammable, burning in air with bright blue flame. Although each molecule of CO has one carbon atom and one oxygen atom, it has a shape similar to that of an oxygen molecule (two atoms of oxygen), which is important with regard to it's lethality.
""" ;
    skos:inScheme <https://w3id.org/ad4gd/air-quality/properties> ;
    skos:prefLabel "CO (Carbon Monoxide)" .

<https://w3id.org/ad4gd/air-quality/properties/CO2> a skos:Concept,
        sosa:ObservableProperty ;
    dct:source [ skos:prefLabel "GEMET" ;
            foaf:homepage <https://www.eionet.europa.eu/gemet/en/concept/1168> ] ;
    owl:sameAs <http://purl.org/iot/vocab/iot-taxonomy-lite#CO2>,
        <http://vocabs.lter-europe.net/EnvThes/20808>,
        <https://www.eionet.europa.eu/gemet/en/concept/1168> ;
    skos:definition """A colourless gas with a faint tingling smell and taste. Atmospheric carbon dioxide is the source of carbon for plants. As carbon dioxide is heavier than air and does not support combustion, it is used in fire extinguishers. It is a normal constituent of the atmosphere, relatively innocuous in itself but playing an important role in the greenhouse effect. It is produced during the combustion of fossil fuels when the carbon content of the fuels reacts with the oxygen during combustion. It is also produced when living organisms respire. It is essential for plant nutrition and in the ocean phytoplankton is capable of absorbing and releasing large quantities of the gas.
""" ;
    skos:inScheme <https://w3id.org/ad4gd/air-quality/properties> ;
    skos:prefLabel "CO2 (Carbon Dioxide)" .

<https://w3id.org/ad4gd/air-quality/properties/H2S> a skos:Concept,
        sosa:ObservableProperty ;
    dct:source [ skos:prefLabel "SLB" ;
            foaf:homepage <https://glossary.slb.com/en/terms/h/h2s> ] ;
    owl:sameAs <https://glossary.slb.com/en/terms/h/h2s> ;
    skos:definition """An extraordinarily poisonous gas with a molecular formula of H2S. At low concentrations, H2S has the odor of rotten eggs, but at higher, lethal concentrations, it is odorless.
""" ;
    skos:inScheme <https://w3id.org/ad4gd/air-quality/properties> ;
    skos:prefLabel "H2S (Hydrogen Sulfide)" .

<https://w3id.org/ad4gd/air-quality/properties/NO2> a skos:Concept,
        sosa:ObservableProperty ;
    dct:source [ skos:prefLabel "AD4GD" ;
            foaf:homepage <https://ad4gd.eu/> ] ;
    owl:sameAs <http://dd.eionet.europa.eu/vocabulary/IEDAnnexIIModule3/EQSAirPollutantsGlassCode/072>,
        <http://dd.eionet.europa.eu/vocabulary/aq/pollutant/8>,
        <http://purl.org/iot/vocab/iot-taxonomy-lite#ChemicalAgentAtmosphericConcentrationNO2>,
        <https://space.oscar.wmo.int/variables/view/no2>,
        <https://uk-air.defra.gov.uk/air-pollution/glossary.php?glossary_id=40#40> ;
    skos:definition "A measurement of the quantity of Nitrogen Dioxide in the air." ;
    skos:inScheme <https://w3id.org/ad4gd/air-quality/properties> ;
    skos:prefLabel "NOâ‚‚ (Nitrogen Dioxide)" .

<https://w3id.org/ad4gd/air-quality/properties/NOx> a skos:Concept,
        sosa:ObservableProperty ;
    dct:source [ skos:prefLabel "DEFRA" ;
            foaf:homepage <https://uk-air.defra.gov.uk/air-pollution/glossary.php?glossary_id=40#40> ] ;
    owl:sameAs <https://uk-air.defra.gov.uk/air-pollution/glossary.php?glossary_id=40#40> ;
    skos:definition """Combustion processes emit a mixture of nitrogen oxides (NOX), primarily nitric oxide (NO) which is quickly oxidised in the atmosphere to nitrogen dioxide (NO2). Nitrogen dioxide has a variety of environmental and health impacts. It is a respiratory irritant which may exacerbate asthma and possibly increase susceptibility to infections. In the presence of sunlight, it reacts with hydrocarbons to produce photochemical pollutants such as ozone. NO2 can be further oxidised in air to acidic gases, which contribute towards the generation of acid rain.
""" ;
    skos:inScheme <https://w3id.org/ad4gd/air-quality/properties> ;
    skos:prefLabel "NOx (Oxides of Nitrogen)" .

<https://w3id.org/ad4gd/air-quality/properties/O3> a skos:Concept,
        sosa:ObservableProperty ;
    dct:source [ skos:prefLabel "AD4GD" ;
            foaf:homepage <https://ad4gd.eu/> ] ;
    owl:sameAs <http://dd.eionet.europa.eu/vocabulary/IEDAnnexIIModule3/EQSAirPollutantsGlassCode/078>,
        <http://purl.org/iot/vocab/iot-taxonomy-lite#ChemicalAgentAtmosphericConcentrationO3>,
        <https://space.oscar.wmo.int/variables/view/o3>,
        <https://uk-air.defra.gov.uk/air-pollution/glossary.php?glossary_id=41#41>,
        <https://vocabs.lter-europe.net/envthes/en/page/20853>,
        <https://www.eionet.europa.eu/gemet/en/concept/5991> ;
    skos:definition "A measurement of the quantity of ozone in the air." ;
    skos:inScheme <https://w3id.org/ad4gd/air-quality/properties> ;
    skos:prefLabel "O3 (Ozone)" .

<https://w3id.org/ad4gd/air-quality/properties/SO2> a skos:Concept,
        sosa:ObservableProperty ;
    dct:source [ skos:prefLabel "DEFRA" ;
            foaf:homepage <https://uk-air.defra.gov.uk/air-pollution/glossary.php?glossary_id=49#49> ] ;
    owl:sameAs <http://dd.eionet.europa.eu/vocabulary/aq/pollutant/1>,
        <http://purl.org/iot/vocab/iot-taxonomy-lite#ChemicalAgentAtmosphericConcentrationSO2>,
        <https://uk-air.defra.gov.uk/air-pollution/glossary.php?glossary_id=49#49> ;
    skos:definition """Sulphur dioxide is a corrosive, acidic gas which combines with water vapour in the atmosphere to produce acid rain. Both wet and dry deposition have been implicated in the damage and destruction of vegetation and in the degradation of soils, building materials and watercourses. SO2 in ambient air is also associated with asthma and chronic bronchitis.
""" ;
    skos:inScheme <https://w3id.org/ad4gd/air-quality/properties> ;
    skos:prefLabel "SO2 (Sulphur Dioxide)" .

<https://w3id.org/ad4gd/air-quality/properties/VOCs> a skos:Concept,
        sosa:ObservableProperty ;
    dct:source [ skos:prefLabel "GEMET" ;
            foaf:homepage <https://www.eionet.europa.eu/gemet/en/concept/8993> ] ;
    owl:sameAs <http://purl.org/iot/vocab/iot-taxonomy-lite#ChemicalAgentAtmosphericConcentrationVOC>,
        <https://uk-air.defra.gov.uk/air-pollution/glossary.php?glossary_id=53#53>,
        <https://www.eionet.europa.eu/gemet/en/concept/8993> ;
    skos:definition """Organic compound readily passing off by evaporation.
""" ;
    skos:inScheme <https://w3id.org/ad4gd/air-quality/properties> ;
    skos:prefLabel "VOCs (Volatile Organic Compounds)" .

<https://w3id.org/ad4gd/air-quality/properties/false> a skos:Concept,
        sosa:ObservableProperty ;
    dct:source [ skos:prefLabel "Wikipedia" ;
            foaf:homepage <https://en.wikipedia.org/wiki/Nitric_oxide> ] ;
    owl:sameAs <https://space.oscar.wmo.int/variables/view/no> ;
    skos:definition "Nitric oxide (nitrogen oxide or nitrogen monoxide) is a colorless gas with the formula NO. It is one of the principal oxides of nitrogen." ;
    skos:inScheme <https://w3id.org/ad4gd/air-quality/properties> ;
    skos:prefLabel "NO (Nitric Oxide)" .

<https://w3id.org/ad4gd/air-quality/properties/humidity> a skos:Concept,
        sosa:ObservableProperty ;
    dct:source [ skos:prefLabel "GEMET" ;
            foaf:homepage <https://www.eionet.europa.eu/gemet/en/concept/626> ] ;
    owl:sameAs <http://dd.eionet.europa.eu/vocabulary/aq/meteoparameter/55>,
        <http://purl.oclc.org/NET/ssnx/cf/cf-feature#Humidity>,
        <https://saref.etsi.org/core/Humidity>,
        <https://vocabs.lter-europe.net/envthes/en/page/22032>,
        <https://www.eionet.europa.eu/gemet/en/concept/626> ;
    skos:definition """A measurable quantity of the moisture content found in the earth's atmosphere.
""" ;
    skos:inScheme <https://w3id.org/ad4gd/air-quality/properties> ;
    skos:prefLabel "Air Humidity" .

<https://w3id.org/ad4gd/air-quality/properties/pm1.0> a skos:Concept,
        sosa:ObservableProperty ;
    dct:source [ skos:prefLabel "AD4GD" ;
            foaf:homepage <https://ad4gd.eu/> ] ;
    rdfs:seeAlso <https://en.wikipedia.org/wiki/Particulates> ;
    owl:sameAs <http://dd.eionet.europa.eu/vocabulary/aq/pollutant/6002>,
        <http://purl.oclc.org/NET/ssnx/cf/cf-property#mass_fraction_of_pm1_ambient_aerosol_in_air>,
        <https://www.iqair.com/us/newsroom/pm1> ;
    skos:definition "The amount of suspended particulates in the air with a diameter of 1 micrometer (Î¼m) or less." ;
    skos:inScheme <https://w3id.org/ad4gd/air-quality/properties> ;
    skos:prefLabel "Particulate matter < 1 Âµm" .

<https://w3id.org/ad4gd/air-quality/properties/pm10> a skos:Concept,
        sosa:ObservableProperty ;
    dct:source [ skos:prefLabel "AD4GD" ;
            foaf:homepage <https://ad4gd.eu/> ] ;
    rdfs:seeAlso <https://en.wikipedia.org/wiki/Particulates> ;
    owl:sameAs <http://dd.eionet.europa.eu/vocabulary/aq/pollutant/5>,
        <http://purl.oclc.org/NET/ssnx/cf/cf-property#mass_fraction_of_pm10_ambient_aerosol_in_air>,
        <https://www.eea.europa.eu/help/glossary/eea-glossary/pm10>,
        <https://www.iqair.com/us/newsroom/pm10> ;
    skos:definition "The amount of suspended particulates in the air with a diameter of 10 micrometers (Î¼m) or less." ;
    skos:inScheme <https://w3id.org/ad4gd/air-quality/properties> ;
    skos:prefLabel "Particulate matter < 10 Âµm" .

<https://w3id.org/ad4gd/air-quality/properties/pm2.5> a skos:Concept,
        sosa:ObservableProperty ;
    dct:source [ skos:prefLabel "AD4GD" ;
            foaf:homepage <https://ad4gd.eu/> ] ;
    rdfs:seeAlso <https://en.wikipedia.org/wiki/Particulates> ;
    owl:sameAs <http://dd.eionet.europa.eu/vocabulary/aq/pollutant/6001>,
        <http://purl.oclc.org/NET/ssnx/cf/cf-property#mass_fraction_of_pm2p5_ambient_aerosol_in_air>,
        <https://www.eea.europa.eu/help/glossary/eea-glossary/pm2.5>,
        <https://www.iqair.com/us/newsroom/pm2-5> ;
    skos:definition "The amount of suspended particulates in the air with a diameter of 2.5 micrometers (Î¼m) or less." ;
    skos:inScheme <https://w3id.org/ad4gd/air-quality/properties> ;
    skos:prefLabel "Particulate matter < 2.5 Âµm" .

<https://w3id.org/ad4gd/air-quality/properties/pressure> a skos:Concept,
        sosa:ObservableProperty ;
    dct:source [ skos:prefLabel "Wikipedia" ;
            foaf:homepage <https://en.wikipedia.org/wiki/Atmospheric_pressure> ] ;
    owl:sameAs <http://purl.oclc.org/NET/ssnx/cf/cf-property#air_pressure>,
        <http://purl.oclc.org/NET/ssnx/qu/quantity#pressure>,
        <http://purl.org/iot/vocab/iot-taxonomy-lite#Pressure>,
        <https://space.oscar.wmo.int/variables/view/air_pressure_near_surface> ;
    skos:definition "Atmospheric pressure, also known as air pressure or barometric pressure (after the barometer), is the pressure within the atmosphere of Earth." ;
    skos:inScheme <https://w3id.org/ad4gd/air-quality/properties> ;
    skos:prefLabel "Air Pressure" .

<https://w3id.org/ad4gd/air-quality/properties/relative-humidity> a skos:Concept,
        sosa:ObservableProperty ;
    dct:source [ skos:prefLabel "OSCAR" ;
            foaf:homepage <https://space.oscar.wmo.int/variables/view/relative_humidity> ] ;
    owl:sameAs <http://dd.eionet.europa.eu/vocabulary/aq/meteoparameter/58>,
        <http://purl.org/iot/vocab/iot-taxonomy-lite#RelativeHumidity>,
        <https://smartdatamodels.org/dataModel.Weather/relativeHumidity>,
        <https://space.oscar.wmo.int/variables/view/relative_humidity> ;
    skos:definition """3D field of relative humidity in the atmosphere. Relative humidity is the ratio of the amount of atmospheric moisture present relative to the amount that would be present if the air were saturated with respct to water or ice to be specified in the metadata .
""" ;
    skos:inScheme <https://w3id.org/ad4gd/air-quality/properties> ;
    skos:prefLabel "Relative Humidity" .

<https://w3id.org/ad4gd/air-quality/properties/temperature> a skos:Concept,
        sosa:ObservableProperty ;
    dct:source [ skos:prefLabel "GEMET" ;
            foaf:homepage <https://www.eionet.europa.eu/gemet/en/concept/281> ] ;
    owl:sameAs <http://dd.eionet.europa.eu/vocabulary/aq/meteoparameter/54>,
        <http://purl.org/iot/vocab/iot-taxonomy-lite#Temperature>,
        <http://vocabs.lter-europe.net/EnvThes/22035>,
        <http://w3id.org/ad4gd/ev/eav/AirTemperature>,
        <https://www.eionet.europa.eu/gemet/en/concept/281> ;
    skos:definition """The temperature of the atmosphere which represents the average kinetic energy of the molecular motion in a small region and is defined in terms of a standard or calibrated thermometer in thermal equilibrium with the air.
""" ;
    skos:inScheme <https://w3id.org/ad4gd/air-quality/properties> ;
    skos:prefLabel "Air Temperature" .

<https://w3id.org/ad4gd/air-quality/properties> a skos:ConceptScheme ;
    dct:source <https://ad4gd.eu/> ;
    skos:prefLabel "AD4GD air quality observable properties" .

[] a prov:Activity ;
    prov:endedAtTime "2025-07-09T10:01:14.285457"^^xsd:dateTime ;
    prov:startedAtTime "2025-07-09T10:01:14.225575"^^xsd:dateTime ;
    prov:used [ a prov:Entity ;
            dct:format "application/json" ;
            dct:hasVersion "git:b179d7ef9e4fdc812747694cefa34b78a0481011" ;
            rdfs:seeAlso <file:///home/runner/work/pilot-3-air-quality/pilot-3-air-quality/rainbow-data/generic/properties.yml> ] ;
    prov:wasAssociatedWith [ a prov:Agent,
                schema:SoftwareApplication ;
            rdfs:label "OGC-NA tools" ;
            dct:hasVersion "0.4" ;
            rdfs:seeAlso <https://github.com/opengeospatial/ogc-na-tools> ] ;
    prov:wasInformedBy [ dct:identifier "a7d93859-2455-482d-bc90-e11a6f873272" ] .

_:Ned287b39fc9b4f7688224933fef20ea7 a prov:Agent,
        schema:SoftwareApplication ;
    rdfs:label "OGC-NA tools" ;
    dct:hasVersion "0.4" ;
    rdfs:comment "ogc.na.update_vocabs version 0.4" ;
    rdfs:seeAlso <https://github.com/opengeospatial/ogc-na-tools> .

