@prefix dct: <http://purl.org/dc/terms/> .
@prefix manuf: <https://w3id.org/ad4gd/air-quality/sensor-manufacturers/> .
@prefix ns1: <foaf:> .
@prefix prov: <http://www.w3.org/ns/prov#> .
@prefix rdfs: <http://www.w3.org/2000/01/rdf-schema#> .
@prefix schema: <https://schema.org/> .
@prefix sensor: <https://w3id.org/ad4gd/air-quality/sensors/> .
@prefix skos: <http://www.w3.org/2004/02/skos/core#> .
@prefix sosa: <http://www.w3.org/ns/sosa/> .
@prefix xsd: <http://www.w3.org/2001/XMLSchema#> .

<https://raw.githubusercontent.com/opengeospatial/NamingAuthority/master/generic/entailed/sensor-platforms.ttl> a prov:Entity ;
    dct:format "text/turtle" ;
    dct:hasVersion "git:b179d7ef9e4fdc812747694cefa34b78a0481011" ;
    prov:wasAttributedTo _:N947529dfa28e41c29b932d1890c52c76 ;
    prov:wasGeneratedBy [ a prov:Activity ;
            rdfs:label "Entailment and validation" ;
            rdfs:comment "python ogc.na.update_vocabs -w ./rainbow-data rainbow-data/catalog.ttl --use-git-status --update --graph-store https://defs-hosted.opengis.net/fuseki-hosted/data" ;
            prov:endedAtTime "2025-07-09T10:01:27.389036"^^xsd:dateTime ;
            prov:startedAtTime "2025-07-09T10:01:27.261197"^^xsd:dateTime ;
            prov:used [ a prov:Entity ;
                    dct:format "text/turtle" ;
                    dct:hasVersion "git:b179d7ef9e4fdc812747694cefa34b78a0481011" ;
                    rdfs:seeAlso <https://raw.githubusercontent.com/opengeospatial/NamingAuthority/master/catalog.ttl> ],
                [ a prov:Entity ;
                    rdfs:seeAlso <https://datashapes.org/dash.ttl> ],
                [ a prov:Entity ;
                    rdfs:seeAlso <http://www.opengis.net/def/metamodel/profiles/skos_shared> ],
                [ a prov:Entity ;
                    dct:format "text/turtle" ;
                    dct:hasVersion "git:b179d7ef9e4fdc812747694cefa34b78a0481011" ;
                    rdfs:seeAlso <https://raw.githubusercontent.com/opengeospatial/NamingAuthority/master/generic/sensor-platforms.ttl> ] ;
            prov:wasAssociatedWith _:N947529dfa28e41c29b932d1890c52c76 ;
            prov:wasInformedBy [ dct:identifier "ff6b99fb-fe40-4437-9188-33c8a355cbe0" ] ] .

<https://w3id.org/ad4gd/air-quality/sensor-platforms/AirRohr> a skos:Concept ;
    dct:description """Build your DIY sensor and become part of the worldwide, opendata & civictech network. With airRohr you can measure air pollution yourself.
""" ;
    dct:source [ ns1:homepage <https://sensor.community/en/sensors/airrohr/> ;
            skos:prefLabel "Sensor.Community" ] ;
    rdfs:seeAlso <https://nettigo.eu/products/sensor-community-kit-sds011-bme280-english-language-harness-cable-edition>,
        <https://sensor.community/en/sensors/airrohr/> ;
    rdfs:subClassOf "sosa:Platform" ;
    skos:inScheme <https://w3id.org/ad4gd/air-quality/sensor-platforms> ;
    skos:prefLabel "AirRohr" ;
    sosa:hosts sensor:BME280,
        sensor:SDS011 ;
    schema:manufacturer manuf:SensorCommunity .

<https://w3id.org/ad4gd/air-quality/sensor-platforms/PlumeFlow2> a skos:Concept ;
    dct:description """The Plume Labs Flow 2 is a wearable air quality sensor that provides real-time measurements of particulate matter (PM1.0, PM2.5 and PM­10) mass concentrations, VOC and NO2 concentrations. Data can be visualized and exported using the phone application for Android and iPhone via Bluetooth.
We created Flow to answer a question: “what is in the air I breathe.” In the spring of 2023 we made the tough decision to dedicate this knowledge, system, and tech to advancing research, raising awareness, and fostering action. As a result Flow and Flow 2 are no longer for sale.    
""" ;
    dct:source [ ns1:homepage <https://www.aqmd.gov/aq-spec/sensordetail/plume-labs---flow-2> ;
            skos:prefLabel "AQMD" ] ;
    rdfs:seeAlso <https://plumelabs.com/en/flow/>,
        <https://www.aqmd.gov/aq-spec/sensordetail/plume-labs---flow-2> ;
    rdfs:subClassOf "sosa:Platform" ;
    skos:inScheme <https://w3id.org/ad4gd/air-quality/sensor-platforms> ;
    skos:prefLabel "PlumeFlow2" ;
    sosa:hosts sensor:PlumeFlow2CO2,
        sensor:PlumeFlow2TH,
        sensor:PlumeFlow2VOC,
        sensor:SDS011 ;
    schema:manufacturer manuf:plume-labs .

<https://w3id.org/ad4gd/air-quality/sensor-platforms/Zephyr> a skos:Concept ;
    dct:description """The Zephyr® is an award-winning, certified, indicative ambient air quality monitor that accurately measures harmful gases and particle matter. 
Zephyr® monitors provide detailed air quality measurements in real-time to help identify pollution hotspots at a localised level such as busy road junctions. Extensive networks can be easily deployed for city-wide pollution data used to aid the development of smarter and cleaner towns and cities.
""" ;
    dct:source [ ns1:homepage <https://www.earthsense.co.uk/_files/ugd/847642_d42371301be448bab9ee526499e1e0bb.pdf> ;
            skos:prefLabel "Earthsense" ] ;
    rdfs:seeAlso <https://www.earthsense.co.uk/_files/ugd/847642_d42371301be448bab9ee526499e1e0bb.pdf>,
        <https://www.earthsense.co.uk/zephyr> ;
    rdfs:subClassOf "sosa:Platform" ;
    skos:inScheme <https://w3id.org/ad4gd/air-quality/sensor-platforms> ;
    skos:prefLabel "Zephyr" ;
    sosa:hosts sensor:ZephyrCO,
        sensor:ZephyrH2S,
        sensor:ZephyrNO,
        sensor:ZephyrO3,
        sensor:ZephyrP,
        sensor:ZephyrPM,
        sensor:ZephyrSO2,
        sensor:ZephyrTH,
        sensor:ZephyrVOC ;
    schema:manufacturer manuf:earthsense .

<https://w3id.org/ad4gd/air-quality/sensor-platforms> a skos:ConceptScheme ;
    dct:source <https://ad4gd.eu/> ;
    skos:prefLabel "AD4GD air quality sensor platforms" .

[] a prov:Activity ;
    prov:endedAtTime "2025-07-09T10:01:14.483684"^^xsd:dateTime ;
    prov:startedAtTime "2025-07-09T10:01:14.428190"^^xsd:dateTime ;
    prov:used [ a prov:Entity ;
            dct:format "application/json" ;
            dct:hasVersion "git:b179d7ef9e4fdc812747694cefa34b78a0481011" ;
            rdfs:seeAlso <file:///home/runner/work/pilot-3-air-quality/pilot-3-air-quality/rainbow-data/generic/sensor-platforms.yml> ] ;
    prov:wasAssociatedWith [ a prov:Agent,
                schema:SoftwareApplication ;
            rdfs:label "OGC-NA tools" ;
            dct:hasVersion "0.4" ;
            rdfs:seeAlso <https://github.com/opengeospatial/ogc-na-tools> ] ;
    prov:wasInformedBy [ dct:identifier "a7d93859-2455-482d-bc90-e11a6f873272" ] .

_:N947529dfa28e41c29b932d1890c52c76 a prov:Agent,
        schema:SoftwareApplication ;
    rdfs:label "OGC-NA tools" ;
    dct:hasVersion "0.4" ;
    rdfs:comment "ogc.na.update_vocabs version 0.4" ;
    rdfs:seeAlso <https://github.com/opengeospatial/ogc-na-tools> .

