@prefix dct: <http://purl.org/dc/terms/> .
@prefix foaf: <http://xmlns.com/foaf/0.1/> .
@prefix ns1: <http://www.opengis.net/def/metamodel/ogc-na/> .
@prefix owl: <http://www.w3.org/2002/07/owl#> .
@prefix prov: <http://www.w3.org/ns/prov#> .
@prefix rdfs: <http://www.w3.org/2000/01/rdf-schema#> .
@prefix schema: <https://schema.org/> .
@prefix skos: <http://www.w3.org/2004/02/skos/core#> .
@prefix sosa: <http://www.w3.org/ns/sosa/> .
@prefix xsd: <http://www.w3.org/2001/XMLSchema#> .

<https://raw.githubusercontent.com/opengeospatial/NamingAuthority/master/generic/entailed/properties.ttl> a prov:Entity ;
    dct:format "text/turtle" ;
    dct:hasVersion "git:d07750e6983a66518d4bb5fd31090cdd5210e7a8" ;
    prov:wasAttributedTo _:N0607bd7e9a6d43ca82eafa45a0bacc71 ;
    prov:wasGeneratedBy [ a prov:Activity ;
            rdfs:label "Entailment and validation" ;
            rdfs:comment "python ogc.na.update_vocabs -w ./rainbow-data rainbow-data/catalog.ttl --use-git-status --update --graph-store https://defs-hosted.opengis.net/fuseki-hosted/data" ;
            prov:endedAtTime "2025-07-23T09:43:07.849041"^^xsd:dateTime ;
            prov:startedAtTime "2025-07-23T09:43:03.532525"^^xsd:dateTime ;
            prov:used [ a prov:Entity ;
                    rdfs:seeAlso <http://www.opengis.net/def/metamodel/profiles/skos_shared> ],
                [ a prov:Entity ;
                    rdfs:seeAlso <http://defs-dev.opengis.net/ogc-na/scripts/skosbasics.shapes.ttl> ],
                [ a prov:Entity ;
                    rdfs:seeAlso <http://defs-dev.opengis.net/ogc-na/scripts/ogc_skos_profile_entailments.ttl> ],
                [ a prov:Entity ;
                    rdfs:seeAlso <http://defs-dev.opengis.net/ogc-na/scripts/ogc_skos_profile.shapes.ttl> ],
                [ a prov:Entity ;
                    rdfs:seeAlso <http://defs-dev.opengis.net/ogc-na/definitions/profiles/resources/skos_shared_shacl.ttl> ],
                [ a prov:Entity ;
                    dct:format "text/turtle" ;
                    dct:hasVersion "git:d07750e6983a66518d4bb5fd31090cdd5210e7a8" ;
                    rdfs:seeAlso <https://raw.githubusercontent.com/opengeospatial/NamingAuthority/master/catalog.ttl> ],
                [ a prov:Entity ;
                    rdfs:seeAlso <https://datashapes.org/dash.ttl> ],
                [ a prov:Entity ;
                    dct:format "text/turtle" ;
                    dct:hasVersion "git:d07750e6983a66518d4bb5fd31090cdd5210e7a8" ;
                    rdfs:seeAlso <https://raw.githubusercontent.com/opengeospatial/NamingAuthority/master/generic/properties.ttl> ] ;
            prov:wasAssociatedWith _:N0607bd7e9a6d43ca82eafa45a0bacc71 ;
            prov:wasInformedBy [ dct:identifier "f9d9d81f-02e8-495b-9512-82b19391f21f" ] ] .

<https://w3id.org/ad4gd/water-quality/properties/> a skos:Collection ;
    dct:provenance "Generated by the OGC Definitions Server to support integration of the elements of this ConceptScheme into bigger collections. ogc_skos_profile_entailements.ttl" ;
    skos:definition "Collection hierarchy for this ConceptScheme" ;
    skos:inScheme <https://w3id.org/ad4gd/water-quality/properties> ;
    skos:prefLabel "Concepts in AD4GD water quality observable properties" .

<https://w3id.org/ad4gd/water-quality/properties/AOX-adsorbable-organic-halides> a skos:Concept,
        sosa:ObservableProperty ;
    dct:source [ skos:prefLabel "DBPedia" ;
            foaf:homepage <https://dbpedia.org/page/Adsorbable_organic_halides> ] ;
    ns1:status <http://www.opengis.net/def/status/valid> ;
    owl:sameAs <https://dbpedia.org/page/Adsorbable_organic_halides> ;
    skos:definition "Adsorbable Organic Halides (AOX) is a measure of the organic halogen load at a sampling site such as soil from a land fill, water, or sewage waste. The procedure measures chlorine, bromine, and iodine as equivalent halogens, but does not measure fluorine levels in the sample." ;
    skos:inScheme <https://w3id.org/ad4gd/water-quality/properties> ;
    skos:prefLabel "AOX (Adsorbable Organic Halides)" ;
    skos:topConceptOf <https://w3id.org/ad4gd/water-quality/properties> .

<https://w3id.org/ad4gd/water-quality/properties/COD-chemical-oxygen-demand> a skos:Concept,
        sosa:ObservableProperty ;
    dct:source [ skos:prefLabel "DBPedia" ;
            foaf:homepage <https://dbpedia.org/page/Chemical_oxygen_demand> ] ;
    ns1:status <http://www.opengis.net/def/status/valid> ;
    rdfs:seeAlso <https://sor.epa.gov/sor_internet/registry/termreg/searchandretrieve/termsandacronyms/search.do?search=&term=chemical%20oxygen%20demand&matchCriteria=Exact&checkedAcronym=true&checkedTerm=true&hasDefinitions=false> ;
    owl:sameAs <http://aims.fao.org/aos/agrovoc/c_15de0183>,
        <https://dbpedia.org/page/Chemical_oxygen_demand>,
        <https://dd.eionet.europa.eu/vocabularyconcept/IEDAnnexIIModule3/EQSWaterPollutantsGlassCode/022/view>,
        <https://dd.eionet.europa.eu/vocabularyconcept/gemet2/concept/1536/view>,
        <https://lod.nal.usda.gov/nalt/24643>,
        <https://sns.uba.de/umthes/de/concepts/_00006030.html> ;
    skos:definition "In environmental chemistry, the chemical oxygen demand (COD) is an indicative measure of the amount of oxygen that can be consumed by reactions in a measured solution. It is commonly expressed in mass of oxygen consumed over volume of solution which in SI units is milligrams per litre (mg/L). A COD test can be used to easily quantify the amount of organics in water. The most common application of COD is in quantifying the amount of oxidizable pollutants found in surface water (e.g. lakes and rivers) or wastewater. COD is useful in terms of water quality by providing a metric to determine the effect an effluent will have on the receiving body, much like biochemical oxygen demand (BOD)." ;
    skos:inScheme <https://w3id.org/ad4gd/water-quality/properties> ;
    skos:prefLabel "COD (Chemical Oxygen Demand)" ;
    skos:topConceptOf <https://w3id.org/ad4gd/water-quality/properties> .

<https://w3id.org/ad4gd/water-quality/properties/DOC-dissolved-organic-carbon> a skos:Concept,
        sosa:ObservableProperty ;
    dct:source [ skos:prefLabel "EIONET" ;
            foaf:homepage <http://www.eionet.europa.eu/gemet/concept/2259> ] ;
    ns1:status <http://www.opengis.net/def/status/valid> ;
    rdfs:seeAlso <https://sor.epa.gov/sor_internet/registry/termreg/searchandretrieve/termsandacronyms/search.do?search=&term=Dissolved%20organic%20carbon&matchCriteria=Exact&checkedAcronym=true&checkedTerm=true&hasDefinitions=false> ;
    owl:sameAs <http://aims.fao.org/aos/agrovoc/c_02b11638>,
        <http://vocabulary.worldbank.org/thesaurus/1644123>,
        <http://www.eionet.europa.eu/gemet/concept/2259>,
        <https://lod.nal.usda.gov/nalt/34079>,
        <https://sns.uba.de/umthes/de/concepts/_00500166.html> ;
    skos:definition "The fraction of total organic carbon (all carbon atoms covalently bonded in organic molecules) in water that passes through a 0.45 micron pore-diameter filter." ;
    skos:inScheme <https://w3id.org/ad4gd/water-quality/properties> ;
    skos:prefLabel "DOC (Dissolved Organic Carbon)" ;
    skos:relatedMatch "https://dbpedia.org/page/Dissolved_organic_carbon" ;
    skos:topConceptOf <https://w3id.org/ad4gd/water-quality/properties> .

<https://w3id.org/ad4gd/water-quality/properties/H4O4Si-silicic-acid> a skos:Concept,
        sosa:ObservableProperty ;
    dct:source [ skos:prefLabel "DBPedia" ;
            foaf:homepage <https://dbpedia.org/page/Silicic_acid> ] ;
    ns1:status <http://www.opengis.net/def/status/valid> ;
    owl:sameAs <https://dbpedia.org/page/Silicic_acid> ;
    skos:definition "In chemistry, a silicic acid (/sɪˈlɪsɪk/) is any chemical compound containing the element silicon attached to oxide (=O) and hydroxyl (−OH) groups, with the general formula [H2xSiOx+2]n or, equivalently, [SiOx(OH)4-2x]n. Orthosilicic acid is a representative example. Silicic acids are rarely observed in isolation, but are thought to exist in aqueous solutions, including seawater, and play a role in biomineralization. They are typically colorless weak acids that are sparingly soluble in water. Like the silicate anions, which are their better known conjugate bases, silicic acids are proposed to be oligomeric or polymeric. No simple silicic acid has ever been identified, since these species being primarily of theoretical interest." ;
    skos:inScheme <https://w3id.org/ad4gd/water-quality/properties> ;
    skos:prefLabel "H4O4Si (Silicic Acid)" ;
    skos:topConceptOf <https://w3id.org/ad4gd/water-quality/properties> .

<https://w3id.org/ad4gd/water-quality/properties/ORP-oxidation-reduction-potential> a skos:Concept,
        sosa:ObservableProperty ;
    dct:source [ skos:prefLabel "DBPedia" ;
            foaf:homepage <https://dbpedia.org/page/Reduction_potential> ] ;
    ns1:status <http://www.opengis.net/def/status/valid> ;
    rdfs:seeAlso <https://sor.epa.gov/sor_internet/registry/termreg/searchandretrieve/termsandacronyms/search.do?search=&term=Oxidation-Reduction%20potential&matchCriteria=Exact&checkedAcronym=true&checkedTerm=true&hasDefinitions=false> ;
    owl:sameAs <http://aims.fao.org/aos/agrovoc/c_6482>,
        <https://d-nb.info/gnd/4076577-5>,
        <https://dbpedia.org/page/Reduction_potential>,
        <https://lod.nal.usda.gov/nalt/56439>,
        <https://sns.uba.de/umthes/de/concepts/_00020545.html> ;
    skos:definition "Redox potential (also known as oxidation / reduction potential, ORP, pe, , or ) is a measure of the tendency of a chemical species to acquire electrons from or lose electrons to an electrode and thereby be reduced or oxidised respectively. Redox potential is expressed in volts (V). Each species has its own intrinsic redox potential; for example, the more positive the reduction potential (reduction potential is more often used due to general formalism in electrochemistry), the greater the species' affinity for electrons and tendency to be reduced." ;
    skos:inScheme <https://w3id.org/ad4gd/water-quality/properties> ;
    skos:prefLabel "ORP (Oxidation-Reduction Potential)" ;
    skos:topConceptOf <https://w3id.org/ad4gd/water-quality/properties> .

<https://w3id.org/ad4gd/water-quality/properties/TNb-total-nitrogen-bound> a skos:Concept,
        sosa:ObservableProperty ;
    dct:source [ skos:prefLabel "ISO 23697-1:2023(en)" ;
            foaf:homepage <https://www.iso.org/obp/ui/#iso:std:iso:23697:-1:ed-1:v1:en> ] ;
    ns1:status <http://www.opengis.net/def/status/valid> ;
    owl:sameAs <https://www.iso.org/obp/ui/#iso:std:iso:23697:-1:ed-1:v1:en> ;
    skos:definition "Total bound nitrogen (ST-TNb) includes all inorganic forms, nitric nitrogen, nitrous nitrogen, ammoniacal nitrogen and all organic forms of nitrogen in a water sample. Nitrate in particular is one of the fundamental nutrients of algae which, in the presence of sufficient quantities of phosphates and other favourable conditions, determine the eutrophication of water. The main sources of nitrogen are both natural and anthropogenic. Of the anthropogenic sources, particular importance can be attributed to domestic wastewater and the use of fertilizers in agriculture. Reduction of nitrogen load is carried out in domestic and industrial wastewater treatment plants through special denitrification processes. The presence of significant concentrations of nitrogenous substances in water can indicate pollution and pose a risk to health and environment." ;
    skos:inScheme <https://w3id.org/ad4gd/water-quality/properties> ;
    skos:prefLabel "TNb (Total Nitrogen Bound)" ;
    skos:topConceptOf <https://w3id.org/ad4gd/water-quality/properties> .

<https://w3id.org/ad4gd/water-quality/properties/ammonia-concentration> a skos:Concept,
        sosa:ObservableProperty ;
    dct:source [ skos:prefLabel "KWB" ;
            foaf:homepage <https://www.kompetenz-wasser.de/en> ] ;
    ns1:status <http://www.opengis.net/def/status/valid> ;
    rdfs:seeAlso <https://github.com/smart-data-models/dataModel.WaterQuality/blob/master/WaterQualityObserved/doc/spec.md>,
        <https://wq.moenv.gov.tw/EWQP/en/Encyclopedia/NounDefinition/Pedia_08.aspx>,
        <https://wqa.org/resources/ammonia/> ;
    skos:definition "Property of the water indicating its concentration of ammonia." ;
    skos:inScheme <https://w3id.org/ad4gd/water-quality/properties> ;
    skos:prefLabel "Ammonia Concentration" ;
    skos:relatedMatch "http://aims.fao.org/aos/agrovoc/c_349",
        "http://purl.org/bncf/tid/22283",
        "http://www.eionet.europa.eu/gemet/concept/375",
        "http://zbw.eu/stw/descriptor/14636-6",
        "https://d-nb.info/gnd/4001735-7",
        "https://dbpedia.org/page/Ammonia",
        "https://lod.nal.usda.gov/nalt/7925",
        "https://sns.uba.de/umthes/de/concepts/_00001875.html",
        "https://vocabularyserver.com/cnr/ml/earth/en/xml.php?skosTema=64510" ;
    skos:topConceptOf <https://w3id.org/ad4gd/water-quality/properties> .

<https://w3id.org/ad4gd/water-quality/properties/ammonium-concentration> a skos:Concept,
        sosa:ObservableProperty ;
    dct:source [ skos:prefLabel "SAREF extension for water" ;
            foaf:homepage <https://saref.etsi.org/saref4watr/Ammonium> ] ;
    ns1:status <http://www.opengis.net/def/status/valid> ;
    rdfs:seeAlso <https://github.com/smart-data-models/dataModel.WaterQuality/blob/master/WaterQualityObserved/doc/spec.md>,
        <https://sor.epa.gov/sor_internet/registry/termreg/searchandretrieve/termsandacronyms/search.do?search=&term=ammonium&matchCriteria=Exact&checkedAcronym=true&checkedTerm=true&hasDefinitions=false> ;
    owl:sameAs <https://saref.etsi.org/saref4watr/Ammonium> ;
    skos:definition "Property of the water indicating its concentration of ammonium." ;
    skos:inScheme <https://w3id.org/ad4gd/water-quality/properties> ;
    skos:prefLabel "Ammonium Concentration" ;
    skos:relatedMatch "http://aims.fao.org/aos/agrovoc/c_32634",
        "http://purl.org/bncf/tid/31172",
        "http://www.eionet.europa.eu/gemet/concept/379",
        "https://dbpedia.org/page/Ammonium",
        "https://vocabularyserver.com/cnr/ml/earth/en/xml.php?skosTema=42940" ;
    skos:topConceptOf <https://w3id.org/ad4gd/water-quality/properties> .

<https://w3id.org/ad4gd/water-quality/properties/animals-in-near-the-water> a skos:Concept,
        sosa:ObservableProperty ;
    dct:source [ skos:prefLabel "CrowdWater" ;
            foaf:homepage <https://crowdwater.ch/en/start/> ] ;
    ns1:status <http://www.opengis.net/def/status/valid> ;
    skos:definition """App question: What animals do you see in/near the water?
Options label: Animals in/near the water
Options: Fish; Amphibians; Dragonflies; Water birds; No animals visible
Multiple response question
""" ;
    skos:inScheme <https://w3id.org/ad4gd/water-quality/properties> ;
    skos:prefLabel "Animals in/near the Water" ;
    skos:topConceptOf <https://w3id.org/ad4gd/water-quality/properties> .

<https://w3id.org/ad4gd/water-quality/properties/biochemical-oxygen-demand-5> a skos:Concept,
        sosa:ObservableProperty ;
    dct:source [ skos:prefLabel "Environmental Water Quality Information" ;
            foaf:homepage <https://wq.moenv.gov.tw/EWQP/en/Encyclopedia/NounDefinition/Pedia_04.aspx> ] ;
    ns1:status <http://www.opengis.net/def/status/valid> ;
    rdfs:seeAlso <https://github.com/smart-data-models/dataModel.WaterQuality/blob/master/WaterQualityObserved/doc/spec.md>,
        <https://wq.moenv.gov.tw/EWQP/en/Encyclopedia/NounDefinition/Pedia_04.aspx>,
        <https://www.epa.gov/sites/default/files/2014-12/documents/wqsglossary9-2012.pdf> ;
    skos:definition "Biochemical oxygen demand (BOD) refers to the amount of dissolved oxygen needed by microbes to break down organic material present in a given water sample at certain temperature over a specific time period. BOD is measured in a water sample during 5 days of incubation at 20℃, known as BOD5. BOD represents the amount of organic matter which can be decomposed by aquatic organisms. It also indirectly represents the degree of organic pollution of the water." ;
    skos:inScheme <https://w3id.org/ad4gd/water-quality/properties> ;
    skos:prefLabel "Biochemical Oxygen Demand in 5 Days" ;
    skos:topConceptOf <https://w3id.org/ad4gd/water-quality/properties> .

<https://w3id.org/ad4gd/water-quality/properties/carbonate-hardness> a skos:Concept,
        sosa:ObservableProperty ;
    dct:source [ skos:prefLabel "DBPedia" ;
            foaf:homepage <https://dbpedia.org/page/Carbonate_hardness> ] ;
    ns1:status <http://www.opengis.net/def/status/valid> ;
    owl:sameAs <https://dbpedia.org/page/Carbonate_hardness> ;
    skos:definition "Carbonate hardness, is a measure of the water hardness caused by the presence of carbonate (CO2−3) and bicarbonate (HCO−3) anions. Carbonate hardness is usually expressed either in degrees KH (dKH) (from the German \"Karbonathärte\"), or in parts per million calcium carbonate ( ppm CaCO3 or grams CaCO3 per litre|mg/L). One dKH is equal to 17.848 mg/L (ppm) CaCO3, e.g. one dKH corresponds to the carbonate and bicarbonate ions found in a solution of approximately 17.848 milligrams of calcium carbonate(CaCO3) per litre of water (17.848 ppm). Both measurements (mg/L or KH) are usually expressed as mg/L CaCO3 – meaning the concentration of carbonate expressed as if calcium carbonate were the sole source of carbonate ions." ;
    skos:inScheme <https://w3id.org/ad4gd/water-quality/properties> ;
    skos:prefLabel "Carbonate Hardness" ;
    skos:topConceptOf <https://w3id.org/ad4gd/water-quality/properties> .

<https://w3id.org/ad4gd/water-quality/properties/dead-wood-protrudes> a skos:Concept,
        sosa:ObservableProperty ;
    dct:source [ skos:prefLabel "CrowdWater" ;
            foaf:homepage <https://crowdwater.ch/en/start/> ] ;
    ns1:status <http://www.opengis.net/def/status/valid> ;
    skos:definition """App question: Is dead wood protruding from the shore into the water?
Options label: Dead wood protrudes into the water
Options: Yes, a lot; Yes, a little; No
Single response question
""" ;
    skos:inScheme <https://w3id.org/ad4gd/water-quality/properties> ;
    skos:prefLabel "Dead Wood Protrudes into the Water" ;
    skos:topConceptOf <https://w3id.org/ad4gd/water-quality/properties> .

<https://w3id.org/ad4gd/water-quality/properties/direct-normal-irradiance> a skos:Concept,
        sosa:ObservableProperty ;
    dct:source [ skos:prefLabel "Open Meteo" ;
            foaf:homepage <https://open-meteo.com/en/docs> ] ;
    ns1:status <http://www.opengis.net/def/status/valid> ;
    rdfs:seeAlso <https://open-meteo.com/en/docs> ;
    skos:definition "Direct solar radiation as average of the preceding hour on the horizontal plane and the normal plane (perpendicular to the sun)." ;
    skos:inScheme <https://w3id.org/ad4gd/water-quality/properties> ;
    skos:prefLabel "Direct Normal Irradiance" ;
    skos:topConceptOf <https://w3id.org/ad4gd/water-quality/properties> .

<https://w3id.org/ad4gd/water-quality/properties/dissolved-boron-concentration> a skos:Concept,
        sosa:ObservableProperty ;
    dct:source [ skos:prefLabel "SAREF extension for water" ;
            foaf:homepage <https://saref.etsi.org/saref4watr/Boron> ] ;
    ns1:status <http://www.opengis.net/def/status/valid> ;
    rdfs:seeAlso <https://github.com/smart-data-models/dataModel.WaterQuality/blob/master/WaterQualityObserved/doc/spec.md> ;
    owl:sameAs <https://saref.etsi.org/saref4watr/Boron> ;
    skos:definition "Property of the water indicating its concentration of boron." ;
    skos:inScheme <https://w3id.org/ad4gd/water-quality/properties> ;
    skos:prefLabel "Dissolved Boron Concentration" ;
    skos:relatedMatch "http://purl.org/bncf/tid/31249",
        "http://www.eionet.europa.eu/gemet/concept/965",
        "https://d-nb.info/gnd/4007709-3",
        "https://dbpedia.org/page/Boron",
        "https://lod.nal.usda.gov/nalt/18678",
        "https://sns.uba.de/umthes/de/concepts/_00005488.html",
        "https://vocabularyserver.com/cnr/ml/earth/en/xml.php?skosTema=52040" ;
    skos:topConceptOf <https://w3id.org/ad4gd/water-quality/properties> .

<https://w3id.org/ad4gd/water-quality/properties/dissolved-chloride-concentration> a skos:Concept,
        sosa:ObservableProperty ;
    dct:source [ skos:prefLabel "SAREF extension for water" ;
            foaf:homepage <https://saref.etsi.org/saref4watr/Chloride> ] ;
    ns1:status <http://www.opengis.net/def/status/valid> ;
    rdfs:seeAlso <https://github.com/smart-data-models/dataModel.WaterQuality/blob/master/WaterQualityObserved/doc/spec.md>,
        <https://sor.epa.gov/sor_internet/registry/termreg/searchandretrieve/termsandacronyms/search.do?search=&term=Chloride&matchCriteria=Exact&checkedAcronym=true&checkedTerm=true&hasDefinitions=false>,
        <https://wq.moenv.gov.tw/EWQP/en/Encyclopedia/NounDefinition/Pedia_28.aspx> ;
    owl:sameAs <https://saref.etsi.org/saref4watr/Chloride> ;
    skos:definition "Property of the water indicating its concentration of chloride." ;
    skos:inScheme <https://w3id.org/ad4gd/water-quality/properties> ;
    skos:prefLabel "Dissolved Chloride Concentration" ;
    skos:relatedMatch "http://aims.fao.org/aos/agrovoc/c_1567",
        "http://www.eionet.europa.eu/gemet/concept/1366",
        "https://dbpedia.org/page/Chloride",
        "https://lod.nal.usda.gov/nalt/7277",
        "https://sns.uba.de/umthes/de/concepts/_00028727.html" ;
    skos:topConceptOf <https://w3id.org/ad4gd/water-quality/properties> .

<https://w3id.org/ad4gd/water-quality/properties/dissolved-iron3-concentration> a skos:Concept,
        sosa:ObservableProperty ;
    dct:source [ skos:prefLabel "SAREF extension for water" ;
            foaf:homepage <https://saref.etsi.org/saref4watr/Iron> ] ;
    ns1:status <http://www.opengis.net/def/status/valid> ;
    rdfs:seeAlso <https://github.com/smart-data-models/dataModel.WaterQuality/blob/master/WaterQualityObserved/doc/spec.md>,
        <https://sor.epa.gov/sor_internet/registry/termreg/searchandretrieve/termsandacronyms/search.do?search=&term=Iron&matchCriteria=Exact&checkedAcronym=true&checkedTerm=true&hasDefinitions=false>,
        <https://wq.moenv.gov.tw/EWQP/en/Encyclopedia/NounDefinition/Pedia_15.aspx> ;
    owl:sameAs <https://saref.etsi.org/saref4watr/Iron> ;
    skos:definition "Property of the water indicating its concentration of iron." ;
    skos:inScheme <https://w3id.org/ad4gd/water-quality/properties> ;
    skos:prefLabel "Dissolved Iron3 Concentration" ;
    skos:relatedMatch "http://aims.fao.org/aos/agrovoc/c_3950",
        "http://eurovoc.europa.eu/981",
        "http://purl.org/bncf/tid/474",
        "http://www.eionet.europa.eu/gemet/concept/4498",
        "https://d-nb.info/gnd/4014002-7",
        "https://lod.nal.usda.gov/nalt/33434",
        "https://sns.uba.de/umthes/de/concepts/_00028823.html",
        "https://vocabularyserver.com/cnr/ml/earth/en/xml.php?skosTema=50410" ;
    skos:topConceptOf <https://w3id.org/ad4gd/water-quality/properties> .

<https://w3id.org/ad4gd/water-quality/properties/dissolved-manganese-concentration> a skos:Concept,
        sosa:ObservableProperty ;
    dct:source [ skos:prefLabel "SAREF extension for water" ;
            foaf:homepage <https://saref.etsi.org/saref4watr/Manganese> ] ;
    ns1:status <http://www.opengis.net/def/status/valid> ;
    rdfs:seeAlso <https://sor.epa.gov/sor_internet/registry/termreg/searchandretrieve/termsandacronyms/search.do?search=&term=Manganese&matchCriteria=Exact&checkedAcronym=true&checkedTerm=true&hasDefinitions=false>,
        <https://wq.moenv.gov.tw/EWQP/en/Encyclopedia/NounDefinition/Pedia_45.aspx> ;
    owl:sameAs <https://saref.etsi.org/saref4watr/Manganese> ;
    skos:definition "Property of the water indicating its concentration of manganese." ;
    skos:inScheme <https://w3id.org/ad4gd/water-quality/properties> ;
    skos:prefLabel "Dissolved Manganese Concentration" ;
    skos:relatedMatch "http://aims.fao.org/aos/agrovoc/c_4570",
        "http://eurovoc.europa.eu/1779",
        "http://purl.org/bncf/tid/25173",
        "http://zbw.eu/stw/descriptor/14301-2",
        "https://d-nb.info/gnd/4037315-0",
        "https://dbpedia.org/page/Manganese",
        "https://lod.nal.usda.gov/nalt/33435",
        "https://sns.uba.de/umthes/de/concepts/_00016555.html" ;
    skos:topConceptOf <https://w3id.org/ad4gd/water-quality/properties> .

<https://w3id.org/ad4gd/water-quality/properties/dissolved-oxygen-concentration> a skos:Concept,
        sosa:ObservableProperty ;
    dct:source [ skos:prefLabel "KWB" ;
            foaf:homepage <https://www.kompetenz-wasser.de/en> ] ;
    ns1:status <http://www.opengis.net/def/status/valid> ;
    owl:sameAs <https://sns.uba.de/umthes/de/concepts/_00021376.html> ;
    skos:definition "Property of the water indicating its concentration of dissolved oxygen." ;
    skos:inScheme <https://w3id.org/ad4gd/water-quality/properties> ;
    skos:prefLabel "Dissolved Oxygen Concentration" ;
    skos:relatedMatch "https://dbpedia.org/page/Oxygen_concentration" ;
    skos:topConceptOf <https://w3id.org/ad4gd/water-quality/properties> .

<https://w3id.org/ad4gd/water-quality/properties/duckweed> a skos:Concept,
        sosa:ObservableProperty ;
    dct:source [ skos:prefLabel "CrowdWater" ;
            foaf:homepage <https://crowdwater.ch/en/start/> ] ;
    ns1:status <http://www.opengis.net/def/status/valid> ;
    skos:definition """App question: How much of the water surface is covered with duckweed?
Options label: Duckweed
Options: 0; approx. 1/4; approx. half; approx. 3/4; Complete
Single response question
""" ;
    skos:inScheme <https://w3id.org/ad4gd/water-quality/properties> ;
    skos:prefLabel "Duckweed" ;
    skos:topConceptOf <https://w3id.org/ad4gd/water-quality/properties> .

<https://w3id.org/ad4gd/water-quality/properties/floating-leaf-plants> a skos:Concept,
        sosa:ObservableProperty ;
    dct:source [ skos:prefLabel "CrowdWater" ;
            foaf:homepage <https://crowdwater.ch/en/start/> ] ;
    ns1:status <http://www.opengis.net/def/status/valid> ;
    skos:definition """Question: Are floating leaf plants (e.g. water lilies) recognizable?
Options: Yes; No
Single response question
""" ;
    skos:inScheme <https://w3id.org/ad4gd/water-quality/properties> ;
    skos:prefLabel "Floating Leaf Plants" ;
    skos:topConceptOf <https://w3id.org/ad4gd/water-quality/properties> .

<https://w3id.org/ad4gd/water-quality/properties/gauge-datum> a skos:Concept,
        sosa:ObservableProperty ;
    dct:source [ skos:prefLabel "ISO 772:2022(en)" ;
            foaf:homepage <https://www.iso.org/obp/ui/#iso:std:iso:772:ed-6:v1:en> ] ;
    ns1:status <http://www.opengis.net/def/status/valid> ;
    rdfs:seeAlso <https://www.iso.org/obp/ui/#iso:std:iso:772:ed-6:v1:en>,
        <https://www.nchm.gov.bt/attachment/ckfinder/userfiles/files/PR-HWRSD-01%20(Hydrological%20Observation).pdf> ;
    skos:definition "Elevation of the zero of the gauge (3.40) to which the level of the liquid surface is referred." ;
    skos:inScheme <https://w3id.org/ad4gd/water-quality/properties> ;
    skos:prefLabel "Gauge Datum" ;
    skos:topConceptOf <https://w3id.org/ad4gd/water-quality/properties> .

<https://w3id.org/ad4gd/water-quality/properties/go-swimming> a skos:Concept,
        sosa:ObservableProperty ;
    dct:source [ skos:prefLabel "CrowdWater" ;
            foaf:homepage <https://crowdwater.ch/en/start/> ] ;
    ns1:status <http://www.opengis.net/def/status/valid> ;
    skos:definition """Question: Would you swim in the water?
Options: Yes; No
Single response question
""" ;
    skos:inScheme <https://w3id.org/ad4gd/water-quality/properties> ;
    skos:prefLabel "Go Swimming" ;
    skos:topConceptOf <https://w3id.org/ad4gd/water-quality/properties> .

<https://w3id.org/ad4gd/water-quality/properties/lake-access> a skos:Concept,
        sosa:ObservableProperty ;
    dct:source [ skos:prefLabel "CrowdWater" ;
            foaf:homepage <https://crowdwater.ch/en/start/> ] ;
    ns1:status <http://www.opengis.net/def/status/valid> ;
    skos:definition """Question: Is the lake shore accessible?
Options: Yes; No
Single response question
""" ;
    skos:inScheme <https://w3id.org/ad4gd/water-quality/properties> ;
    skos:prefLabel "Lake Access" ;
    skos:topConceptOf <https://w3id.org/ad4gd/water-quality/properties> .

<https://w3id.org/ad4gd/water-quality/properties/lake-dries-out> a skos:Concept,
        sosa:ObservableProperty ;
    dct:source [ skos:prefLabel "CrowdWater" ;
            foaf:homepage <https://crowdwater.ch/en/start/> ] ;
    ns1:status <http://www.opengis.net/def/status/valid> ;
    skos:definition """App question: Does the lake sometimes dry out?
Options label: Lake sometimes dries out
Options: Yes; No; I don’t know
Single response question
""" ;
    skos:inScheme <https://w3id.org/ad4gd/water-quality/properties> ;
    skos:prefLabel "Lake Dries Out" ;
    skos:topConceptOf <https://w3id.org/ad4gd/water-quality/properties> .

<https://w3id.org/ad4gd/water-quality/properties/lake-usage> a skos:Concept,
        sosa:ObservableProperty ;
    dct:source [ skos:prefLabel "CrowdWater" ;
            foaf:homepage <https://crowdwater.ch/en/start/> ] ;
    ns1:status <http://www.opengis.net/def/status/valid> ;
    skos:definition """Question: How is the lake being used?
Options label: Lake usage
Options: Bathing; Dog bathing place; Water sports; Fishing; Shore usage (Picknicks, sunbathing,...); No visible usage
Multiple response question
""" ;
    skos:inScheme <https://w3id.org/ad4gd/water-quality/properties> ;
    skos:prefLabel "Lake Usage" ;
    skos:topConceptOf <https://w3id.org/ad4gd/water-quality/properties> .

<https://w3id.org/ad4gd/water-quality/properties/lakeshore-vegetation> a skos:Concept,
        sosa:ObservableProperty ;
    dct:source [ skos:prefLabel "CrowdWater" ;
            foaf:homepage <https://crowdwater.ch/en/start/> ] ;
    ns1:status <http://www.opengis.net/def/status/valid> ;
    skos:definition """Question: Which lakeshore vegetation can be identified?
Options label: Lakeshore vegetation
Options: Reeds; Trees; Grass; Other; None
Multiple response question
""" ;
    skos:inScheme <https://w3id.org/ad4gd/water-quality/properties> ;
    skos:prefLabel "Lakeshore Vegetation" ;
    skos:topConceptOf <https://w3id.org/ad4gd/water-quality/properties> .

<https://w3id.org/ad4gd/water-quality/properties/lakewater-smell> a skos:Concept,
        sosa:ObservableProperty ;
    dct:source [ skos:prefLabel "CrowdWater" ;
            foaf:homepage <https://crowdwater.ch/en/start/> ] ;
    ns1:status <http://www.opengis.net/def/status/valid> ;
    skos:definition """Question: Does the water have a smell?
Options label: Lakewater smell
Options: No smell; Rotten eggs; Moldy; Fishy; Other sewage smell; Other noticeable Smell
Single response question
""" ;
    skos:inScheme <https://w3id.org/ad4gd/water-quality/properties> ;
    skos:prefLabel "Lakewater Smell" ;
    skos:relatedMatch "https://saref.etsi.org/saref4watr/Odour" ;
    skos:topConceptOf <https://w3id.org/ad4gd/water-quality/properties> .

<https://w3id.org/ad4gd/water-quality/properties/litter-in-water> a skos:Concept,
        sosa:ObservableProperty ;
    dct:source [ skos:prefLabel "CrowdWater" ;
            foaf:homepage <https://crowdwater.ch/en/start/> ] ;
    ns1:status <http://www.opengis.net/def/status/valid> ;
    skos:definition """Question: Is there litter in the water?
Options: No litter; Some litter, but not prominent; Abundant litter
Single response question
""" ;
    skos:inScheme <https://w3id.org/ad4gd/water-quality/properties> ;
    skos:prefLabel "Litter in Water" ;
    skos:topConceptOf <https://w3id.org/ad4gd/water-quality/properties> .

<https://w3id.org/ad4gd/water-quality/properties/mussels> a skos:Concept,
        sosa:ObservableProperty ;
    dct:source [ skos:prefLabel "CrowdWater" ;
            foaf:homepage <https://crowdwater.ch/en/start/> ] ;
    ns1:status <http://www.opengis.net/def/status/valid> ;
    skos:definition """App question: Do you see mussels on the shore?
Options: Large mussels; Triangular mussel; Others; No mussels visible
Single response question
""" ;
    skos:inScheme <https://w3id.org/ad4gd/water-quality/properties> ;
    skos:prefLabel "Mussels" ;
    skos:topConceptOf <https://w3id.org/ad4gd/water-quality/properties> .

<https://w3id.org/ad4gd/water-quality/properties/nitrate-concentration> a skos:Concept,
        sosa:ObservableProperty ;
    dct:source [ skos:prefLabel "SAREF extension for water" ;
            foaf:homepage <https://saref.etsi.org/saref4watr/Nitrate> ] ;
    ns1:status <http://www.opengis.net/def/status/valid> ;
    rdfs:seeAlso <https://github.com/smart-data-models/dataModel.WaterQuality/blob/master/WaterQualityObserved/doc/spec.md>,
        <https://sor.epa.gov/sor_internet/registry/termreg/searchandretrieve/termsandacronyms/search.do?search=&term=Nitrate&matchCriteria=Exact&checkedAcronym=true&checkedTerm=true&hasDefinitions=false>,
        <https://wq.moenv.gov.tw/EWQP/en/Encyclopedia/NounDefinition/Pedia_31.aspx>,
        <https://wqa.org/resources/nitrites-nitrates/>,
        <https://www.mysuwanneeriver.com/419/Nitrate-Concentration> ;
    owl:sameAs <https://saref.etsi.org/saref4watr/Nitrate> ;
    skos:definition "Property of the water indicating its concentration of nitrate." ;
    skos:inScheme <https://w3id.org/ad4gd/water-quality/properties> ;
    skos:prefLabel "Nitrate Concentration" ;
    skos:relatedMatch "http://aims.fao.org/aos/agrovoc/c_0e5d9815",
        "http://www.eionet.europa.eu/gemet/concept/5593",
        "https://dbpedia.org/page/Nitrate",
        "https://sns.uba.de/umthes/de/concepts/_00028736.html" ;
    skos:topConceptOf <https://w3id.org/ad4gd/water-quality/properties> .

<https://w3id.org/ad4gd/water-quality/properties/nitrite-concentration> a skos:Concept,
        sosa:ObservableProperty ;
    dct:source [ skos:prefLabel "SAREF extension for water" ;
            foaf:homepage <https://saref.etsi.org/saref4watr/Nitrite> ] ;
    ns1:status <http://www.opengis.net/def/status/valid> ;
    rdfs:seeAlso <https://wq.moenv.gov.tw/EWQP/en/Encyclopedia/NounDefinition/Pedia_27.aspx>,
        <https://wqa.org/resources/nitrites-nitrates/> ;
    owl:sameAs <https://saref.etsi.org/saref4watr/Nitrite> ;
    skos:definition "Property of the water indicating its concentration of nitrite." ;
    skos:inScheme <https://w3id.org/ad4gd/water-quality/properties> ;
    skos:prefLabel "Nitrite Concentration" ;
    skos:relatedMatch "http://aims.fao.org/aos/agrovoc/c_5190",
        "http://purl.org/bncf/tid/37366",
        "https://dbpedia.org/page/Nitrite",
        "https://lod.nal.usda.gov/nalt/30836",
        "https://sns.uba.de/umthes/de/concepts/_00018171.html" ;
    skos:topConceptOf <https://w3id.org/ad4gd/water-quality/properties> .

<https://w3id.org/ad4gd/water-quality/properties/orthophosphate-concentration> a skos:Concept,
        sosa:ObservableProperty ;
    dct:source [ skos:prefLabel "KWB" ;
            foaf:homepage <https://www.kompetenz-wasser.de/en> ] ;
    ns1:status <http://www.opengis.net/def/status/valid> ;
    rdfs:seeAlso <https://sor.epa.gov/sor_internet/registry/termreg/searchandretrieve/termsandacronyms/search.do?search=&term=orthoPhosphate&matchCriteria=Exact&checkedAcronym=true&checkedTerm=true&hasDefinitions=false> ;
    skos:definition "Property of the water indicating its concentration of orthophosphate." ;
    skos:inScheme <https://w3id.org/ad4gd/water-quality/properties> ;
    skos:prefLabel "Orthophosphate Concentration" ;
    skos:relatedMatch "http://aims.fao.org/aos/agrovoc/c_35986",
        "http://purl.org/bncf/tid/21193",
        "http://zbw.eu/stw/descriptor/14646-3",
        "https://d-nb.info/gnd/4134029-2",
        "https://dbpedia.org/page/Phosphate",
        "https://lod.nal.usda.gov/nalt/7280",
        "https://sns.uba.de/umthes/de/concepts/_00019272.html" ;
    skos:topConceptOf <https://w3id.org/ad4gd/water-quality/properties> .

<https://w3id.org/ad4gd/water-quality/properties/oxygen-saturation> a skos:Concept,
        sosa:ObservableProperty ;
    dct:source [ skos:prefLabel "DBPedia" ;
            foaf:homepage <https://dbpedia.org/page/Oxygen_saturation> ] ;
    ns1:status <http://www.opengis.net/def/status/valid> ;
    rdfs:seeAlso <https://sor.epa.gov/sor_internet/registry/termreg/searchandretrieve/termsandacronyms/search.do?search=&term=Oxygen%20Saturation&matchCriteria=Exact&checkedAcronym=true&checkedTerm=true&hasDefinitions=false> ;
    owl:sameAs <http://dd.eionet.europa.eu/vocabulary/wise/ObservedProperty/EEA_3131-01-9>,
        <http://dd.eionet.europa.eu/vocabulary/wise/WFDQualityElement/QE3-1-3-1>,
        <https://dbpedia.org/page/Oxygen_saturation>,
        <https://saref.etsi.org/saref4watr/Oxygen>,
        <https://sns.uba.de/umthes/de/concepts/_00021379.html> ;
    skos:definition "Oxygen saturation (symbol SO2) is a relative measure of the concentration of oxygen that is dissolved or carried in a given medium as a proportion of the maximal concentration that can be dissolved in that medium at the given temperature. It can be measured with a dissolved oxygen probe such as an oxygen sensor or an optode in liquid media, usually water. The standard unit of oxygen saturation is percent (%)." ;
    skos:inScheme <https://w3id.org/ad4gd/water-quality/properties> ;
    skos:prefLabel "Oxygen Saturation" ;
    skos:topConceptOf <https://w3id.org/ad4gd/water-quality/properties> .

<https://w3id.org/ad4gd/water-quality/properties/pH> a skos:Concept,
        sosa:ObservableProperty ;
    dct:source [ skos:prefLabel "DBPedia" ;
            foaf:homepage <https://dbpedia.org/page/PH> ] ;
    ns1:status <http://www.opengis.net/def/status/valid> ;
    rdfs:seeAlso <https://sor.epa.gov/sor_internet/registry/termreg/searchandretrieve/termsandacronyms/search.do?search=&term=pH&matchCriteria=Exact&checkedAcronym=true&checkedTerm=true&hasDefinitions=false>,
        <https://wq.moenv.gov.tw/EWQP/en/Encyclopedia/NounDefinition/Pedia_47.aspx>,
        <https://www.epa.gov/sites/default/files/2014-12/documents/wqsglossary9-2012.pdf> ;
    owl:sameAs <http://aims.fao.org/aos/agrovoc/c_5753>,
        <http://purl.org/bncf/tid/32910>,
        <http://www.eionet.europa.eu/gemet/concept/47>,
        <https://d-nb.info/gnd/4189273-2>,
        <https://dbpedia.org/page/PH>,
        <https://lod.nal.usda.gov/nalt/2772>,
        <https://sns.uba.de/umthes/de/concepts/_00019242.html>,
        <https://vocabularyserver.com/cnr/ml/earth/en/xml.php?skosTema=33090> ;
    skos:definition "In chemistry, pH (/piːˈeɪtʃ/), historically denoting \"potential of hydrogen\" (or \"power of hydrogen\"), is a scale used to specify the acidity or basicity of an aqueous solution. Acidic solutions (solutions with higher concentrations of H+ ions) are measured to have lower pH values than basic or alkaline solutions. The pH scale is logarithmic and inversely indicates the concentration of hydrogen ions in the solution." ;
    skos:inScheme <https://w3id.org/ad4gd/water-quality/properties> ;
    skos:prefLabel "pH" ;
    skos:topConceptOf <https://w3id.org/ad4gd/water-quality/properties> .

<https://w3id.org/ad4gd/water-quality/properties/plants-under-water> a skos:Concept,
        sosa:ObservableProperty ;
    dct:source [ skos:prefLabel "CrowdWater" ;
            foaf:homepage <https://crowdwater.ch/en/start/> ] ;
    ns1:status <http://www.opengis.net/def/status/valid> ;
    skos:definition """Question: Are plants under water recognizable?
Options: Yes; No
Single response question
""" ;
    skos:inScheme <https://w3id.org/ad4gd/water-quality/properties> ;
    skos:prefLabel "Plants Under Water" ;
    skos:topConceptOf <https://w3id.org/ad4gd/water-quality/properties> .

<https://w3id.org/ad4gd/water-quality/properties/potential-evapotranspiration> a skos:Concept,
        sosa:ObservableProperty ;
    dct:source [ skos:prefLabel "Open Meteo" ;
            foaf:homepage <https://open-meteo.com/en/docs> ] ;
    ns1:status <http://www.opengis.net/def/status/valid> ;
    rdfs:seeAlso <https://open-meteo.com/en/docs>,
        <https://sor.epa.gov/sor_internet/registry/termreg/searchandretrieve/termsandacronyms/search.do?search=&term=evapotranspiration&matchCriteria=Exact&checkedAcronym=true&checkedTerm=true&hasDefinitions=false> ;
    skos:definition "Evapotranspration from land surface and plants that weather models assumes for this location. Available soil water is considered. 1 mm evapotranspiration per hour equals 1 liter of water per spare meter." ;
    skos:inScheme <https://w3id.org/ad4gd/water-quality/properties> ;
    skos:prefLabel "Potential-Evapotranspiration" ;
    skos:topConceptOf <https://w3id.org/ad4gd/water-quality/properties> .

<https://w3id.org/ad4gd/water-quality/properties/precipitation> a skos:Concept,
        sosa:ObservableProperty ;
    dct:source [ skos:prefLabel "EPA Terminology Services" ;
            foaf:homepage <https://sor.epa.gov/sor_internet/registry/termreg/searchandretrieve/termsandacronyms/search.do?search=&term=precipitation&matchCriteria=Exact&checkedAcronym=true&checkedTerm=true&hasDefinitions=false> ] ;
    ns1:status <http://www.opengis.net/def/status/valid> ;
    rdfs:seeAlso <https://sor.epa.gov/sor_internet/registry/termreg/searchandretrieve/termsandacronyms/search.do?search=&term=precipitation&matchCriteria=Exact&checkedAcronym=true&checkedTerm=true&hasDefinitions=false> ;
    owl:sameAs <https://saref.etsi.org/saref4watr/Precipitation> ;
    skos:definition "In analytic chemistry, the process of producing a separable solid phase within a liquid medium." ;
    skos:inScheme <https://w3id.org/ad4gd/water-quality/properties> ;
    skos:prefLabel "Precipitation" ;
    skos:topConceptOf <https://w3id.org/ad4gd/water-quality/properties> .

<https://w3id.org/ad4gd/water-quality/properties/reference-evapotranspiration> a skos:Concept,
        sosa:ObservableProperty ;
    dct:source [ skos:prefLabel "Open Meteo" ;
            foaf:homepage <https://open-meteo.com/en/docs> ] ;
    ns1:status <http://www.opengis.net/def/status/valid> ;
    rdfs:seeAlso <https://open-meteo.com/en/docs> ;
    skos:definition "ET0 Reference Evapotranspiration of a well watered grass field. Based on FAO-56 Penman-Monteith equations ET0 is calculated from temperature, wind speed, humidity and solar radiation. Unlimited soil water is assumed. ET0 is commonly used to estimate the required irrigation for plants." ;
    skos:inScheme <https://w3id.org/ad4gd/water-quality/properties> ;
    skos:prefLabel "Reference-Evapotranspiration" ;
    skos:topConceptOf <https://w3id.org/ad4gd/water-quality/properties> .

<https://w3id.org/ad4gd/water-quality/properties/shore-properties> a skos:Concept,
        sosa:ObservableProperty ;
    dct:source [ skos:prefLabel "CrowdWater" ;
            foaf:homepage <https://crowdwater.ch/en/start/> ] ;
    ns1:status <http://www.opengis.net/def/status/valid> ;
    skos:definition """Question: What is the condition of the shore?
Options: Natural; Partially built up; Built up
Single response question
""" ;
    skos:inScheme <https://w3id.org/ad4gd/water-quality/properties> ;
    skos:prefLabel "Shore Properties" ;
    skos:topConceptOf <https://w3id.org/ad4gd/water-quality/properties> .

<https://w3id.org/ad4gd/water-quality/properties/specific-conductivity> a skos:Concept,
        sosa:ObservableProperty ;
    dct:source [ skos:prefLabel "KWB" ;
            foaf:homepage <https://www.kompetenz-wasser.de/en> ] ;
    ns1:status <http://www.opengis.net/def/status/valid> ;
    rdfs:seeAlso <https://en.wikipedia.org/wiki/Conductivity_(electrolytic)>,
        <https://sor.epa.gov/sor_internet/registry/termreg/searchandretrieve/termsandacronyms/search.do?search=&term=specific%20conductance&matchCriteria=Exact&checkedAcronym=true&checkedTerm=true&hasDefinitions=false> ;
    skos:definition "Conductivity of water at 25 degrees Celsius (25 C)." ;
    skos:inScheme <https://w3id.org/ad4gd/water-quality/properties> ;
    skos:prefLabel "Specific Conductivity" ;
    skos:relatedMatch "https://sns.uba.de/umthes/de/concepts/_00016073.html" ;
    skos:topConceptOf <https://w3id.org/ad4gd/water-quality/properties> .

<https://w3id.org/ad4gd/water-quality/properties/sulphate-concentration> a skos:Concept,
        sosa:ObservableProperty ;
    dct:source [ skos:prefLabel "KWB" ;
            foaf:homepage <https://www.kompetenz-wasser.de/en> ] ;
    ns1:status <http://www.opengis.net/def/status/valid> ;
    rdfs:seeAlso <https://github.com/smart-data-models/dataModel.WaterQuality/blob/master/WaterQualityObserved/doc/spec.md>,
        <https://wq.moenv.gov.tw/EWQP/en/Encyclopedia/NounDefinition/Pedia_20.aspx> ;
    skos:definition "Property of the water indicating its concentration of sulphate." ;
    skos:inScheme <https://w3id.org/ad4gd/water-quality/properties> ;
    skos:prefLabel "Sulphate Concentration" ;
    skos:relatedMatch "http://aims.fao.org/aos/agrovoc/c_7510",
        "http://www.eionet.europa.eu/gemet/concept/8190",
        "https://sns.uba.de/umthes/de/concepts/_00028731.html" ;
    skos:topConceptOf <https://w3id.org/ad4gd/water-quality/properties> .

<https://w3id.org/ad4gd/water-quality/properties/surface-reflectance> a skos:Concept,
        sosa:ObservableProperty ;
    dct:source [ skos:prefLabel "USGS" ;
            foaf:homepage <https://www.usgs.gov/landsat-missions/landsat-collection-1-surface-reflectance> ] ;
    ns1:status <http://www.opengis.net/def/status/valid> ;
    rdfs:seeAlso <https://www.usgs.gov/landsat-missions/landsat-collection-1-surface-reflectance> ;
    skos:definition "Surface reflectance is the amount of light reflected by the surface of the Earth. It is a ratio of surface radiance to surface irradiance, and as such is unitless, with values between 0 and 1." ;
    skos:inScheme <https://w3id.org/ad4gd/water-quality/properties> ;
    skos:prefLabel "Surface Reflectance" ;
    skos:topConceptOf <https://w3id.org/ad4gd/water-quality/properties> .

<https://w3id.org/ad4gd/water-quality/properties/total-organic-carbon> a skos:Concept,
        sosa:ObservableProperty ;
    dct:source [ skos:prefLabel "DBPedia" ;
            foaf:homepage <https://dbpedia.org/page/Total_organic_carbon> ] ;
    ns1:status <http://www.opengis.net/def/status/valid> ;
    rdfs:seeAlso <https://saref.etsi.org/saref4watr/TotalOrganicCarbon>,
        <https://sor.epa.gov/sor_internet/registry/termreg/searchandretrieve/termsandacronyms/search.do?search=&term=Total%20organic%20carbon&matchCriteria=Exact&checkedAcronym=true&checkedTerm=true&hasDefinitions=false>,
        <https://wq.moenv.gov.tw/EWQP/en/Encyclopedia/NounDefinition/Pedia_13.aspx> ;
    owl:sameAs <http://aims.fao.org/aos/agrovoc/c_c35fdd26>,
        <http://vocabulary.worldbank.org/thesaurus/1644128>,
        <http://www.eionet.europa.eu/gemet/concept/11779>,
        <https://dbpedia.org/page/Total_organic_carbon>,
        <https://lod.nal.usda.gov/nalt/325123>,
        <https://sns.uba.de/umthes/de/concepts/_00657196.html> ;
    skos:definition "Total organic carbon (TOC) is the amount of carbon found in an organic compound and is often used as a non-specific indicator of water quality or cleanliness of pharmaceutical manufacturing equipment. TOC may also refer to the amount of organic carbon in soil, or in a geological formation, particularly the source rock for a petroleum play; 2% is a rough minimum. For marine surface sediments average TOC content is 0.5% in the deep ocean, and 2% along the eastern margins." ;
    skos:inScheme <https://w3id.org/ad4gd/water-quality/properties> ;
    skos:prefLabel "Total Organic Carbon" ;
    skos:topConceptOf <https://w3id.org/ad4gd/water-quality/properties> .

<https://w3id.org/ad4gd/water-quality/properties/total-phosphorus> a skos:Concept,
        sosa:ObservableProperty ;
    dct:source [ skos:prefLabel "Smart Data Models" ;
            foaf:homepage <https://github.com/smart-data-models/dataModel.WaterQuality/blob/master/WaterQualityObserved/doc/spec.md> ] ;
    ns1:status <http://www.opengis.net/def/status/valid> ;
    rdfs:seeAlso <https://github.com/smart-data-models/dataModel.WaterQuality/blob/master/WaterQualityObserved/doc/spec.md>,
        <https://sor.epa.gov/sor_internet/registry/termreg/searchandretrieve/termsandacronyms/search.do?search=&term=Total%20phosphorus&matchCriteria=Exact&checkedAcronym=true&checkedTerm=true&hasDefinitions=false> ;
    owl:sameAs <https://sns.uba.de/umthes/de/concepts/_00011161.html> ;
    skos:definition "Total phosphorus is a measure of all forms of phosphorus in the water, including dissolved and particulate, organic and inorganic." ;
    skos:inScheme <https://w3id.org/ad4gd/water-quality/properties> ;
    skos:prefLabel "Total Phosphorus" ;
    skos:topConceptOf <https://w3id.org/ad4gd/water-quality/properties> .

<https://w3id.org/ad4gd/water-quality/properties/total-suspended-solids> a skos:Concept,
        sosa:ObservableProperty ;
    dct:source [ skos:prefLabel "DBPedia" ;
            foaf:homepage <https://dbpedia.org/page/Total_suspended_solids> ] ;
    ns1:status <http://www.opengis.net/def/status/valid> ;
    rdfs:seeAlso <https://github.com/smart-data-models/dataModel.WaterQuality/blob/master/WaterQualityObserved/doc/spec.md>,
        <https://sor.epa.gov/sor_internet/registry/termreg/searchandretrieve/termsandacronyms/search.do?search=&term=Total%20suspended%20solids&matchCriteria=Exact&checkedAcronym=true&checkedTerm=true&hasDefinitions=false> ;
    owl:sameAs <http://aims.fao.org/aos/agrovoc/c_3c8040e9>,
        <http://dd.eionet.europa.eu/vocabulary/IEDAnnexIIModule3/EQSWaterPollutantsGlassCode/109>,
        <http://dd.eionet.europa.eu/vocabulary/wise/ObservedProperty/EEA_31-02-7>,
        <https://dbpedia.org/page/Total_suspended_solids>,
        <https://saref.etsi.org/saref4watr/TotalSuspendedSolids>,
        <https://sns.uba.de/umthes/de/concepts/_00022057.html> ;
    skos:definition "Total suspended solids (TSS) is the dry-weight of suspended particles, that are not dissolved, in a sample of water that can be trapped by a filter that is analyzed using a filtration apparatus known as sintered glass crucible. TSS is a water quality parameter used to assess the quality of a specimen of any type of water or water body, ocean water for example, or wastewater after treatment in a wastewater treatment plant. It is listed as a conventional pollutant in the U.S. Clean Water Act. Total dissolved solids is another parameter acquired through a separate analysis which is also used to determine water quality based on the total substances that are fully dissolved within the water, rather than undissolved suspended particles." ;
    skos:inScheme <https://w3id.org/ad4gd/water-quality/properties> ;
    skos:prefLabel "Total Suspended Solids" ;
    skos:topConceptOf <https://w3id.org/ad4gd/water-quality/properties> .

<https://w3id.org/ad4gd/water-quality/properties/water-color> a skos:Concept,
        sosa:ObservableProperty ;
    dct:source [ skos:prefLabel "CrowdWater" ;
            foaf:homepage <https://crowdwater.ch/en/start/> ] ;
    ns1:status <http://www.opengis.net/def/status/valid> ;
    skos:definition """Question: How would you describe the water color?
Options label: Water colour
Options: Clear (no color); Green; Beige (like cappuccino); Brown (like black tea); Gray or milky; Reddish; Blue
Single response question
""" ;
    skos:inScheme <https://w3id.org/ad4gd/water-quality/properties> ;
    skos:prefLabel "Water Color" ;
    skos:relatedMatch "https://saref.etsi.org/saref4watr/Colour" ;
    skos:topConceptOf <https://w3id.org/ad4gd/water-quality/properties> .

<https://w3id.org/ad4gd/water-quality/properties/water-hardness> a skos:Concept,
        sosa:ObservableProperty ;
    dct:source [ skos:prefLabel "SAREF extension for water" ;
            foaf:homepage <https://saref.etsi.org/saref4watr/Hardness> ] ;
    ns1:status <http://www.opengis.net/def/status/valid> ;
    rdfs:seeAlso <https://sor.epa.gov/sor_internet/registry/termreg/searchandretrieve/termsandacronyms/search.do?search=&term=Water%20hardness&matchCriteria=Exact&checkedAcronym=true&checkedTerm=true&hasDefinitions=false>,
        <https://wq.moenv.gov.tw/EWQP/en/Encyclopedia/NounDefinition/Pedia_11.aspx>,
        <https://www.epa.gov/sites/default/files/2014-12/documents/wqsglossary9-2012.pdf> ;
    owl:sameAs <http://aims.fao.org/aos/agrovoc/c_25423>,
        <http://vocabulary.worldbank.org/thesaurus/1612631>,
        <https://lod.nal.usda.gov/nalt/67253>,
        <https://saref.etsi.org/saref4watr/Hardness>,
        <https://sns.uba.de/umthes/de/concepts/_00027253.html>,
        <https://vocabularyserver.com/cnr/ml/earth/en/xml.php?skosTema=52920> ;
    skos:definition "Property of the water indicating its hardness." ;
    skos:inScheme <https://w3id.org/ad4gd/water-quality/properties> ;
    skos:prefLabel "Water Hardness" ;
    skos:relatedMatch "http://www.eionet.europa.eu/gemet/concept/9184" ;
    skos:topConceptOf <https://w3id.org/ad4gd/water-quality/properties> .

<https://w3id.org/ad4gd/water-quality/properties/water-level> a skos:Concept,
        sosa:ObservableProperty ;
    dct:source [ skos:prefLabel "EIONET" ;
            foaf:homepage <http://www.eionet.europa.eu/gemet/concept/9190> ] ;
    ns1:status <http://www.opengis.net/def/status/valid> ;
    rdfs:seeAlso <https://sor.epa.gov/sor_internet/registry/termreg/searchandretrieve/termsandacronyms/search.do?search=&term=Water%20level&matchCriteria=Exact&checkedAcronym=true&checkedTerm=true&hasDefinitions=false> ;
    owl:sameAs <http://aims.fao.org/aos/agrovoc/c_29685>,
        <http://www.eionet.europa.eu/gemet/concept/9190>,
        <https://d-nb.info/gnd/4189260-4>,
        <https://sns.uba.de/umthes/de/concepts/_00027345.html>,
        <https://vocabularyserver.com/cnr/ml/earth/en/xml.php?skosTema=21430> ;
    skos:definition "The level reached by the surface of a body of water." ;
    skos:inScheme <https://w3id.org/ad4gd/water-quality/properties> ;
    skos:prefLabel "Water Level" ;
    skos:topConceptOf <https://w3id.org/ad4gd/water-quality/properties> .

<https://w3id.org/ad4gd/water-quality/properties/water-level-above-sea-level> a skos:Concept,
        sosa:ObservableProperty ;
    dct:source [ skos:prefLabel "KWB" ;
            foaf:homepage <https://www.kompetenz-wasser.de/en> ] ;
    ns1:status <http://www.opengis.net/def/status/valid> ;
    skos:definition "Property of the water indicating its level above sea level." ;
    skos:inScheme <https://w3id.org/ad4gd/water-quality/properties> ;
    skos:prefLabel "Water Level Above Sea Level" ;
    skos:topConceptOf <https://w3id.org/ad4gd/water-quality/properties> .

<https://w3id.org/ad4gd/water-quality/properties/water-level-change> a skos:Concept,
        sosa:ObservableProperty ;
    dct:source [ skos:prefLabel "CrowdWater" ;
            foaf:homepage <https://crowdwater.ch/en/start/> ] ;
    ns1:status <http://www.opengis.net/def/status/valid> ;
    skos:definition """App question: Are there water level changes in the lake?
Options label: Water level change
Options: Yes, large; Yes, small; No; No idea
Single response question
""" ;
    skos:inScheme <https://w3id.org/ad4gd/water-quality/properties> ;
    skos:prefLabel "Water Level Change" ;
    skos:topConceptOf <https://w3id.org/ad4gd/water-quality/properties> .

<https://w3id.org/ad4gd/water-quality/properties/water-temperature> a skos:Concept,
        sosa:ObservableProperty ;
    dct:source [ skos:prefLabel "EPA Terminology Services" ;
            foaf:homepage <https://sor.epa.gov/sor_internet/registry/termreg/searchandretrieve/termsandacronyms/search.do?search=&term=Water%20temperature&matchCriteria=Exact&checkedAcronym=true&checkedTerm=true&hasDefinitions=false> ] ;
    ns1:status <http://www.opengis.net/def/status/valid> ;
    rdfs:seeAlso <https://sor.epa.gov/sor_internet/registry/termreg/searchandretrieve/termsandacronyms/search.do?search=&term=Water%20temperature&matchCriteria=Exact&checkedAcronym=true&checkedTerm=true&hasDefinitions=false>,
        <https://wq.moenv.gov.tw/EWQP/en/Encyclopedia/NounDefinition/Pedia_17.aspx> ;
    owl:sameAs <http://aims.fao.org/aos/agrovoc/c_16063>,
        <http://dd.eionet.europa.eu/vocabulary/wise/ObservedProperty/EEA_3121-01-5>,
        <http://dd.eionet.europa.eu/vocabulary/wise/WFDQualityElement/QE3-1-2-1>,
        <https://d-nb.info/gnd/4234773-7>,
        <https://lod.nal.usda.gov/nalt/65553>,
        <https://saref.etsi.org/saref4watr/Temperature>,
        <https://sns.uba.de/umthes/de/concepts/_00027358.html>,
        <https://vocabularyserver.com/cnr/ml/earth/en/xml.php?skosTema=91090> ;
    skos:definition "Water temperature is a physical property expressing how hot or cold water is. Temperature is an important factor to consider when assessing water quality. Many fish and other aquatic animals are sensitive to changes in water temperature and require a certain temperature range to survive. If water temperature goes outside that range for too long, they can become sick or die." ;
    skos:inScheme <https://w3id.org/ad4gd/water-quality/properties> ;
    skos:prefLabel "Water Temperature" ;
    skos:topConceptOf <https://w3id.org/ad4gd/water-quality/properties> .

<https://w3id.org/ad4gd/water-quality/properties/water-transparency> a skos:Concept,
        sosa:ObservableProperty ;
    dct:source [ skos:prefLabel "CrowdWater" ;
            foaf:homepage <https://crowdwater.ch/en/start/> ] ;
    ns1:status <http://www.opengis.net/def/status/valid> ;
    skos:definition """Question: How deep can you see?
Options label: Water transparency 
Options: a few cm; 20 – 50 cm; 50 cm – 1 m; deeper than 1 m
Single response question
""" ;
    skos:inScheme <https://w3id.org/ad4gd/water-quality/properties> ;
    skos:prefLabel "Water Transparency" ;
    skos:topConceptOf <https://w3id.org/ad4gd/water-quality/properties> .

<https://w3id.org/ad4gd/water-quality/properties/wind-speed> a skos:Concept,
        sosa:ObservableProperty ;
    dct:source [ skos:prefLabel "Open Meteo" ;
            foaf:homepage <https://open-meteo.com/en/docs> ] ;
    ns1:status <http://www.opengis.net/def/status/valid> ;
    rdfs:seeAlso <https://open-meteo.com/en/docs> ;
    skos:definition "Wind speed at different heights above ground. Wind speed on 10 meters is the standard level." ;
    skos:inScheme <https://w3id.org/ad4gd/water-quality/properties> ;
    skos:prefLabel "Wind Speed" ;
    skos:topConceptOf <https://w3id.org/ad4gd/water-quality/properties> .

<https://w3id.org/ad4gd/water-quality/properties> a skos:ConceptScheme ;
    dct:source <https://ad4gd.eu/> ;
    ns1:collectionView <https://w3id.org/ad4gd/water-quality/properties/> ;
    skos:hasTopConcept <https://w3id.org/ad4gd/water-quality/properties/AOX-adsorbable-organic-halides>,
        <https://w3id.org/ad4gd/water-quality/properties/COD-chemical-oxygen-demand>,
        <https://w3id.org/ad4gd/water-quality/properties/DOC-dissolved-organic-carbon>,
        <https://w3id.org/ad4gd/water-quality/properties/H4O4Si-silicic-acid>,
        <https://w3id.org/ad4gd/water-quality/properties/ORP-oxidation-reduction-potential>,
        <https://w3id.org/ad4gd/water-quality/properties/TNb-total-nitrogen-bound>,
        <https://w3id.org/ad4gd/water-quality/properties/ammonia-concentration>,
        <https://w3id.org/ad4gd/water-quality/properties/ammonium-concentration>,
        <https://w3id.org/ad4gd/water-quality/properties/animals-in-near-the-water>,
        <https://w3id.org/ad4gd/water-quality/properties/biochemical-oxygen-demand-5>,
        <https://w3id.org/ad4gd/water-quality/properties/carbonate-hardness>,
        <https://w3id.org/ad4gd/water-quality/properties/dead-wood-protrudes>,
        <https://w3id.org/ad4gd/water-quality/properties/direct-normal-irradiance>,
        <https://w3id.org/ad4gd/water-quality/properties/dissolved-boron-concentration>,
        <https://w3id.org/ad4gd/water-quality/properties/dissolved-chloride-concentration>,
        <https://w3id.org/ad4gd/water-quality/properties/dissolved-iron3-concentration>,
        <https://w3id.org/ad4gd/water-quality/properties/dissolved-manganese-concentration>,
        <https://w3id.org/ad4gd/water-quality/properties/dissolved-oxygen-concentration>,
        <https://w3id.org/ad4gd/water-quality/properties/duckweed>,
        <https://w3id.org/ad4gd/water-quality/properties/floating-leaf-plants>,
        <https://w3id.org/ad4gd/water-quality/properties/gauge-datum>,
        <https://w3id.org/ad4gd/water-quality/properties/go-swimming>,
        <https://w3id.org/ad4gd/water-quality/properties/lake-access>,
        <https://w3id.org/ad4gd/water-quality/properties/lake-dries-out>,
        <https://w3id.org/ad4gd/water-quality/properties/lake-usage>,
        <https://w3id.org/ad4gd/water-quality/properties/lakeshore-vegetation>,
        <https://w3id.org/ad4gd/water-quality/properties/lakewater-smell>,
        <https://w3id.org/ad4gd/water-quality/properties/litter-in-water>,
        <https://w3id.org/ad4gd/water-quality/properties/mussels>,
        <https://w3id.org/ad4gd/water-quality/properties/nitrate-concentration>,
        <https://w3id.org/ad4gd/water-quality/properties/nitrite-concentration>,
        <https://w3id.org/ad4gd/water-quality/properties/orthophosphate-concentration>,
        <https://w3id.org/ad4gd/water-quality/properties/oxygen-saturation>,
        <https://w3id.org/ad4gd/water-quality/properties/pH>,
        <https://w3id.org/ad4gd/water-quality/properties/plants-under-water>,
        <https://w3id.org/ad4gd/water-quality/properties/potential-evapotranspiration>,
        <https://w3id.org/ad4gd/water-quality/properties/precipitation>,
        <https://w3id.org/ad4gd/water-quality/properties/reference-evapotranspiration>,
        <https://w3id.org/ad4gd/water-quality/properties/shore-properties>,
        <https://w3id.org/ad4gd/water-quality/properties/specific-conductivity>,
        <https://w3id.org/ad4gd/water-quality/properties/sulphate-concentration>,
        <https://w3id.org/ad4gd/water-quality/properties/surface-reflectance>,
        <https://w3id.org/ad4gd/water-quality/properties/total-organic-carbon>,
        <https://w3id.org/ad4gd/water-quality/properties/total-phosphorus>,
        <https://w3id.org/ad4gd/water-quality/properties/total-suspended-solids>,
        <https://w3id.org/ad4gd/water-quality/properties/water-color>,
        <https://w3id.org/ad4gd/water-quality/properties/water-hardness>,
        <https://w3id.org/ad4gd/water-quality/properties/water-level>,
        <https://w3id.org/ad4gd/water-quality/properties/water-level-above-sea-level>,
        <https://w3id.org/ad4gd/water-quality/properties/water-level-change>,
        <https://w3id.org/ad4gd/water-quality/properties/water-temperature>,
        <https://w3id.org/ad4gd/water-quality/properties/water-transparency>,
        <https://w3id.org/ad4gd/water-quality/properties/wind-speed> ;
    skos:prefLabel "AD4GD water quality observable properties" .

[] a prov:Activity ;
    prov:endedAtTime "2025-07-23T09:42:50.626173"^^xsd:dateTime ;
    prov:startedAtTime "2025-07-23T09:42:50.552568"^^xsd:dateTime ;
    prov:used [ a prov:Entity ;
            dct:format "application/json" ;
            dct:hasVersion "git:d07750e6983a66518d4bb5fd31090cdd5210e7a8" ;
            rdfs:seeAlso <file:///home/runner/work/pilot-1-water-quality/pilot-1-water-quality/rainbow-data/generic/properties.yml> ] ;
    prov:wasAssociatedWith [ a prov:Agent,
                schema:SoftwareApplication ;
            rdfs:label "OGC-NA tools" ;
            dct:hasVersion "0.5.dev3+g1871e64" ;
            rdfs:seeAlso <https://github.com/opengeospatial/ogc-na-tools> ] ;
    prov:wasInformedBy [ dct:identifier "22e78aa4-3930-44b3-9fbd-6e04fc3fc7cd" ] .

_:N0607bd7e9a6d43ca82eafa45a0bacc71 a prov:Agent,
        schema:SoftwareApplication ;
    rdfs:label "OGC-NA tools" ;
    dct:hasVersion "0.5.dev3+g1871e64" ;
    rdfs:comment "ogc.na.update_vocabs version 0.5.dev3+g1871e64" ;
    rdfs:seeAlso <https://github.com/opengeospatial/ogc-na-tools> .

