@prefix ad4gd-procedure: <https://w3id.org/ad4gd/air-quality/procedures/> .
@prefix ad4gd-prop: <https://w3id.org/ad4gd/air-quality/properties/> .
@prefix dct: <http://purl.org/dc/terms/> .
@prefix manuf: <https://w3id.org/ad4gd/air-quality/sensor-manufacturers/> .
@prefix ns1: <http://www.opengis.net/def/metamodel/ogc-na/> .
@prefix owl: <http://www.w3.org/2002/07/owl#> .
@prefix prov: <http://www.w3.org/ns/prov#> .
@prefix qb: <http://purl.org/linked-data/cube#> .
@prefix qudt: <http://qudt.org/schema/qudt/> .
@prefix rdfs: <http://www.w3.org/2000/01/rdf-schema#> .
@prefix sdo: <https://schema.org/> .
@prefix skos: <http://www.w3.org/2004/02/skos/core#> .
@prefix sosa: <http://www.w3.org/ns/sosa/> .
@prefix ssn: <http://www.w3.org/ns/ssn/> .
@prefix unit: <http://qudt.org/vocab/unit/> .
@prefix xsd: <http://www.w3.org/2001/XMLSchema#> .

<https://raw.githubusercontent.com/opengeospatial/NamingAuthority/master/generic/entailed/sensors.ttl> a prov:Entity ;
    dct:format "text/turtle" ;
    dct:hasVersion "git:dd39b657e7d09026ea1600203fae9883db7d74c1" ;
    prov:wasAttributedTo _:N5cd6a0cbbd7f45bebe384b4800ba7259 ;
    prov:wasGeneratedBy [ a prov:Activity ;
            rdfs:label "Entailment and validation" ;
            rdfs:comment "python ogc.na.update_vocabs -w ./rainbow rainbow/catalog.ttl --use-git-status --update --graph-store https://defs-dev.opengis.net/fuseki-hosted/data" ;
            prov:endedAtTime "2024-09-04T08:46:44.928895"^^xsd:dateTime ;
            prov:startedAtTime "2024-09-04T08:46:41.966662"^^xsd:dateTime ;
            prov:used [ a prov:Entity ;
                    rdfs:seeAlso <http://defs-dev.opengis.net/ogc-na/scripts/ogc_skos_profile_entailments.ttl> ],
                [ a prov:Entity ;
                    rdfs:seeAlso <http://defs-dev.opengis.net/ogc-na/definitions/profiles/resources/skos_shared_shacl.ttl> ],
                [ a prov:Entity ;
                    rdfs:seeAlso <http://defs-dev.opengis.net/ogc-na/scripts/ogc_skos_profile.shapes.ttl> ],
                [ a prov:Entity ;
                    dct:format "text/turtle" ;
                    dct:hasVersion "git:dd39b657e7d09026ea1600203fae9883db7d74c1" ;
                    rdfs:seeAlso <https://raw.githubusercontent.com/opengeospatial/NamingAuthority/master/catalog.ttl> ],
                [ a prov:Entity ;
                    rdfs:seeAlso <http://defs-dev.opengis.net/def/metamodel/profiles/skos_shared?_profile=shacl&_mediatype=text/turtle> ],
                [ a prov:Entity ;
                    rdfs:seeAlso <https://datashapes.org/dash.ttl> ],
                [ a prov:Entity ;
                    dct:format "text/turtle" ;
                    dct:hasVersion "git:dd39b657e7d09026ea1600203fae9883db7d74c1" ;
                    rdfs:seeAlso <https://raw.githubusercontent.com/opengeospatial/NamingAuthority/master/generic/sensors.ttl> ],
                [ a prov:Entity ;
                    rdfs:seeAlso <http://defs-dev.opengis.net/ogc-na/scripts/skosbasics.shapes.ttl> ],
                [ a prov:Entity ;
                    rdfs:seeAlso <http://www.opengis.net/def/metamodel/profiles/skos_shared> ] ;
            prov:wasAssociatedWith _:N5cd6a0cbbd7f45bebe384b4800ba7259 ;
            prov:wasInformedBy [ dct:identifier "de537cd7-2b2c-476f-833b-a92f5bdaa250" ] ] .

<https://w3id.org/ad4gd/air-quality/sensors/> a skos:Collection ;
    dct:provenance "Generated by the OGC Definitions Server to support integration of the elements of this ConceptScheme into bigger collections. ogc_skos_profile_entailements.ttl" ;
    skos:definition "Collection hierarchy for this ConceptScheme" ;
    skos:inScheme <https://w3id.org/ad4gd/air-quality/sensors> ;
    skos:prefLabel "Concepts in AD4GD air quality sensors" .

<https://w3id.org/ad4gd/air-quality/sensors/BME280> a owl:Class,
        skos:Concept ;
    dct:description """This precision sensor from Bosch is the best low-cost sensing solution for measuring humidity with ±3% accuracy,
barometric pressure with ±1 hPa absolute accuraccy, and temperature with ±1.0°C accuracy. Because pressure changes with altitude,
and the pressure measurements are so good, you can also use it as an altimeter with  ±1 meter or better accuracy! 

From: https://www.adafruit.com/product/2652'
""" ;
    ns1:status <http://www.opengis.net/def/status/valid> ;
    rdfs:seeAlso <https://www.adafruit.com/product/2652> ;
    rdfs:subClassOf sosa:Sensor ;
    skos:inScheme <https://w3id.org/ad4gd/air-quality/sensors> ;
    skos:prefLabel "BME280" ;
    skos:topConceptOf <https://w3id.org/ad4gd/air-quality/sensors> ;
    sosa:observes [ qudt:hasUnit unit:DEG_C ;
            skos:broader ad4gd-prop:temperature ],
        [ qudt:hasUnit unit:PA ;
            skos:broader ad4gd-prop:pressure ],
        [ qudt:hasUnit unit:PERCENT_RH ;
            skos:broader ad4gd-prop:relative-humidity ] ;
    sdo:manufacturer manuf:bosch .

<https://w3id.org/ad4gd/air-quality/sensors/BMP180> a owl:Class,
        skos:Concept ;
    dct:description """The BMP180 is the function compatible successor of the BMP085, a new generation of high precision digital pressure sensors for consumer applications. 
From: https://cdn-shop.adafruit.com/datasheets/BST-BMP180-DS000-09.pdf
""" ;
    ns1:status <http://www.opengis.net/def/status/valid> ;
    rdfs:seeAlso <https://cdn-shop.adafruit.com/datasheets/BST-BMP180-DS000-09.pdf> ;
    rdfs:subClassOf sosa:Sensor ;
    skos:inScheme <https://w3id.org/ad4gd/air-quality/sensors> ;
    skos:prefLabel "BMP180" ;
    skos:topConceptOf <https://w3id.org/ad4gd/air-quality/sensors> ;
    sosa:observes [ qudt:hasUnit unit:DEG_C ;
            skos:broader ad4gd-prop:temperature ],
        [ qudt:hasUnit unit:PA ;
            skos:broader ad4gd-prop:pressure ] ;
    sdo:manufacturer manuf:bosch .

<https://w3id.org/ad4gd/air-quality/sensors/BMP280> a owl:Class,
        skos:Concept ;
    dct:description """The BMP280 is an absolute barometric pressure sensor, which is especially feasible for mobile applications. Its small dimensions and its low power consumption allow for the implementation in battery-powered devices such as mobile phones, GPS modules or watches. The BMP280 is based on Bosch’s proven piezo-resistive pressure sensor technology featuring high accuracy and linearity as well as long-term stability and high EMC robustness. Numerous device operation options guarantee for highest flexibility. The device is optimized in terms of power consumption, resolution and filter performance.
From: https://www.bosch-sensortec.com/products/environmental-sensors/pressure-sensors/bmp280/
""" ;
    ns1:status <http://www.opengis.net/def/status/valid> ;
    rdfs:seeAlso <https://www.bosch-sensortec.com/products/environmental-sensors/pressure-sensors/bmp280/> ;
    rdfs:subClassOf sosa:Sensor ;
    skos:inScheme <https://w3id.org/ad4gd/air-quality/sensors> ;
    skos:prefLabel "BMP280" ;
    skos:topConceptOf <https://w3id.org/ad4gd/air-quality/sensors> ;
    sosa:observes [ qudt:hasUnit unit:PA ;
            skos:broader ad4gd-prop:pressure ] ;
    sdo:manufacturer manuf:bosch .

<https://w3id.org/ad4gd/air-quality/sensors/DHT22> a owl:Class,
        skos:Concept ;
    dct:description """The DHT22 is a basic, low-cost digital temperature and humidity sensor. It uses a capacitive humidity sensor and a thermistor to measure
the surrounding air and spits out a digital signal on the data pin (no analog input pins needed). It's fairly simple to use but requires
careful timing to grab data. The only real downside of this sensor is you can only get new data from it once every 2 seconds, so when using
our library, sensor readings can be up to 2 seconds old.

Low cost
Good for 0-100% humidity readings with 2-5% accuracy
Good for -40 to 80°C temperature readings ±0.5°C accuracy
No more than 0.5 Hz sampling rate (once every 2 seconds)
From: https://www.adafruit.com/product/385
""" ;
    ns1:status <http://www.opengis.net/def/status/valid> ;
    rdfs:seeAlso <https://www.adafruit.com/product/385> ;
    rdfs:subClassOf sosa:Sensor ;
    skos:inScheme <https://w3id.org/ad4gd/air-quality/sensors> ;
    skos:prefLabel "DHT22" ;
    skos:topConceptOf <https://w3id.org/ad4gd/air-quality/sensors> ;
    sosa:observes [ qudt:hasUnit unit:PERCENT_RH ;
            skos:broader ad4gd-prop:relative-humidity ],
        [ qudt:hasUnit unit:DEG_C ;
            skos:broader ad4gd-prop:temperature ] ;
    sdo:manufacturer manuf:various .

<https://w3id.org/ad4gd/air-quality/sensors/DS18B20> a owl:Class,
        skos:Concept ;
    dct:description """The DS18B20 digital thermometer provides 9-bit to 12-bit Celsius temperature measurements and has an alarm function with nonvolatile user-programmable upper and lower trigger points. The DS18B20 communicates over a 1-Wire bus that by definition requires only one data line (and ground) for communication with a central microprocessor. In addition, the DS18B20 can derive power directly from the data line (“parasite power”), eliminating the need for an external power supply.
From: https://www.analog.com/media/en/technical-documentation/data-sheets/ds18b20.pdf
""" ;
    ns1:status <http://www.opengis.net/def/status/valid> ;
    rdfs:seeAlso <https://www.analog.com/media/en/technical-documentation/data-sheets/ds18b20.pdf> ;
    rdfs:subClassOf sosa:Sensor ;
    skos:inScheme <https://w3id.org/ad4gd/air-quality/sensors> ;
    skos:prefLabel "DS18B20" ;
    skos:topConceptOf <https://w3id.org/ad4gd/air-quality/sensors> ;
    sosa:observes [ qudt:hasUnit unit:DEG_C ;
            skos:broader ad4gd-prop:temperature ] ;
    sdo:manufacturer manuf:dallas-semiconductor .

<https://w3id.org/ad4gd/air-quality/sensors/HPM> a owl:Class,
        skos:Concept ;
    dct:description """Honeywell HPM Particulate Matter Sensors detect and count particles by using light scattering, enhancing the ability to more accurately monitor environmental particulates. These laser-based sensors feature a 0µg/m3 to 1000µg/m3 detection range, <6s response time, and ±15% accuracy. The modules are fully calibrated and offer an 80mA maximum supply current. Honeywell HPM Particulate Matter Sensors are well-suited for HVAC systems, air quality monitors, and air purifiers.
Laser-based light scattering particle sensing
0µg/m3 to 1000µg/m3 concentration range
Fully calibrated
EMC: Heavy industrial level IEC61000
<6s response time
80mA maximum supply current
Output signal: universal asynchronous receiver / transmitter (UART)
PM2.5, PM10 output (standard); PM1.0, PM2.5, PM4.0, PM10 output (compact)
RoHS and REACH compliant
From: https://www.mouser.co.uk/new/honeywell/honeywell-hpm-particulate-matter-sensors/
""" ;
    ns1:status <http://www.opengis.net/def/status/valid> ;
    rdfs:seeAlso <https://www.mouser.co.uk/new/honeywell/honeywell-hpm-particulate-matter-sensors/> ;
    rdfs:subClassOf sosa:Sensor ;
    skos:inScheme <https://w3id.org/ad4gd/air-quality/sensors> ;
    skos:prefLabel "HPM" ;
    skos:topConceptOf <https://w3id.org/ad4gd/air-quality/sensors> ;
    sosa:observes [ qudt:hasUnit unit:MicroGM-PER-M3 ;
            skos:broader ad4gd-prop:pm1 ],
        [ qudt:hasUnit unit:MicroGM-PER-M3 ;
            skos:broader ad4gd-prop:pm10 ],
        [ qudt:hasUnit unit:MicroGM-PER-M3 ;
            skos:broader ad4gd-prop:pm4 ],
        [ qudt:hasUnit unit:MicroGM-PER-M3 ;
            skos:broader ad4gd-prop:pm2.5 ] ;
    sdo:manufacturer manuf:honeywell .

<https://w3id.org/ad4gd/air-quality/sensors/HTU21D> a owl:Class,
        skos:Concept ;
    dct:description """The HTU21D(F) is a new digital humidity sensor with temperature output by MEAS. Setting new standards in terms of size and intelligence, it is embedded in a reflow solderable Dual Flat No leads (DFN) package with a small 3 x 3 x 0.9 mm footprint. This sensor provides calibrated, linearized signals in digital, I²C format.
From: https://cdn-shop.adafruit.com/datasheets/1899_HTU21D.pdf
""" ;
    ns1:status <http://www.opengis.net/def/status/valid> ;
    rdfs:seeAlso <https://cdn-shop.adafruit.com/datasheets/1899_HTU21D.pdf> ;
    rdfs:subClassOf sosa:Sensor ;
    skos:inScheme <https://w3id.org/ad4gd/air-quality/sensors> ;
    skos:prefLabel "HTU21D" ;
    skos:topConceptOf <https://w3id.org/ad4gd/air-quality/sensors> ;
    sosa:observes [ qudt:hasUnit unit:DEG_C ;
            skos:broader ad4gd-prop:temperature ],
        [ qudt:hasUnit unit:PERCENT_RH ;
            skos:broader ad4gd-prop:relative-humidity ] ;
    sdo:manufacturer manuf:measurement-specialties .

<https://w3id.org/ad4gd/air-quality/sensors/NextPM> a owl:Class,
        skos:Concept ;
    dct:description """Designed for environmental monitoring and smart cities application, NextPM provides real time PM1, PM2.5 and PM10 measurements in µg/m3 and pcs/L.
With its patented air flow control technology, NextPM provides up to 10 years of monitoring without maintenance, even in an atmosphere with high pollution and humidity levels.
From: https://tera-sensor.com/product/nextpm/
""" ;
    ns1:status <http://www.opengis.net/def/status/valid> ;
    rdfs:seeAlso <https://tera-sensor.com/product/nextpm/> ;
    rdfs:subClassOf sosa:Sensor ;
    skos:inScheme <https://w3id.org/ad4gd/air-quality/sensors> ;
    skos:prefLabel "NextPM" ;
    skos:topConceptOf <https://w3id.org/ad4gd/air-quality/sensors> ;
    sosa:observes [ qudt:hasUnit unit:MicroGM-PER-M3 ;
            skos:broader ad4gd-prop:pm2.5 ],
        [ qudt:hasUnit unit:MicroGM-PER-M3 ;
            skos:broader ad4gd-prop:pm10 ],
        [ qudt:hasUnit unit:MicroGM-PER-M3 ;
            skos:broader ad4gd-prop:pm1 ] ;
    sdo:manufacturer manuf:TERA-Sensor .

<https://w3id.org/ad4gd/air-quality/sensors/PMS1003> a owl:Class,
        skos:Concept ;
    dct:description """The PMS 1003 Sensor is a recent laser based Air Quality Sensor developped by plantower (chinese name: 攀藤 (pānténg))
and used inside a numerous number of air quality sensing devices. It is also sometimes refered as HK 5001, or labelled
under the "oneair" brand, but it is indeed developped and produced by plantower (a Shenzhen based company with office in Beijing).

Measuring range: 0.3 to 1.0, 1.0 ~ 2.5, 2.5 to 10 microns (um)
Range: 0 ~ 500 ug / m3
Counting accuracy of 50% @ 0.3um, 98% @ ≥0.5 um said the quasi-volume : 0.1 liters (L)
Response time: ≤10 seconds (s)

From: https://aqicn.org/sensor/pms1003/
""" ;
    ns1:status <http://www.opengis.net/def/status/valid> ;
    rdfs:seeAlso <https://aqicn.org/sensor/pms1003/> ;
    rdfs:subClassOf sosa:Sensor ;
    skos:inScheme <https://w3id.org/ad4gd/air-quality/sensors> ;
    skos:prefLabel "PMS1003" ;
    skos:topConceptOf <https://w3id.org/ad4gd/air-quality/sensors> ;
    sosa:observes [ qudt:hasUnit unit:MicroGM-PER-M3 ;
            skos:broader ad4gd-prop:pm2.5 ],
        [ qudt:hasUnit unit:MicroGM-PER-M3 ;
            skos:broader ad4gd-prop:pm10 ],
        [ qudt:hasUnit unit:MicroGM-PER-M3 ;
            skos:broader ad4gd-prop:pm1 ] ;
    sdo:manufacturer manuf:plantower .

<https://w3id.org/ad4gd/air-quality/sensors/PMS3003> a owl:Class,
        skos:Concept ;
    dct:description """The PMS 3003 Sensor is the third generation evolution of the PMS1003 developped by plantower (chinese name: 攀藤 (pānténg).
Measuring range :0.3 to 1.0 ; 1.0 to 2.5 ; 2.5 to 10  (mm)
Counting efficiency :50%@0.3um 98% @> = 0.5 um 
Response time :≤ 10  sec
DC supply voltage :5 V
Operating current :120  mA
Standby Current :≤ 200  µA
Data interface level :L <0.8 @ 3.3 H> 2.7@3.3  V
Operating temperature range :-20 ~ + 50  °C
Operating humidity range :0 to 99% 
MTBF :≥ 3  Year
Size :65 × 42 × 23  mm
From: https://aqicn.org/sensor/pms3003/
""" ;
    ns1:status <http://www.opengis.net/def/status/valid> ;
    rdfs:seeAlso <https://aqicn.org/sensor/pms3003/> ;
    rdfs:subClassOf sosa:Sensor ;
    skos:inScheme <https://w3id.org/ad4gd/air-quality/sensors> ;
    skos:prefLabel "PMS3003" ;
    skos:topConceptOf <https://w3id.org/ad4gd/air-quality/sensors> ;
    sosa:observes [ qudt:hasUnit unit:MicroGM-PER-M3 ;
            skos:broader ad4gd-prop:pm1 ],
        [ qudt:hasUnit unit:MicroGM-PER-M3 ;
            skos:broader ad4gd-prop:pm10 ],
        [ qudt:hasUnit unit:MicroGM-PER-M3 ;
            skos:broader ad4gd-prop:pm2.5 ] ;
    sdo:manufacturer manuf:plantower .

<https://w3id.org/ad4gd/air-quality/sensors/PMS5003> a owl:Class,
        skos:Concept ;
    dct:description """The PMS 7003 and PMS 5003 sensors are the 7th resp 5th generation of the PMSx003 series developed by Plantower (chinese name 攀藤).
Range of measurement: 0.3~1.0; 1.0~2.5; 2.5~10 μ m
Effective Range: 0~500 μ g/m³
Maximum Range: * ≥1000 μ g/m³
Resolution: 1 μ g/m³
Standard Volume: 0.1L

From: https://aqicn.org/sensor/pms5003-7003/
""" ;
    ns1:status <http://www.opengis.net/def/status/valid> ;
    rdfs:seeAlso <https://aqicn.org/sensor/pms5003-7003/>,
        <https://www.adafruit.com/product/3686> ;
    rdfs:subClassOf sosa:Sensor ;
    skos:inScheme <https://w3id.org/ad4gd/air-quality/sensors> ;
    skos:prefLabel "PMS5003" ;
    skos:topConceptOf <https://w3id.org/ad4gd/air-quality/sensors> ;
    sosa:observes [ qudt:hasUnit unit:MicroGM-PER-M3 ;
            skos:broader ad4gd-prop:pm10 ],
        [ qudt:hasUnit unit:MicroGM-PER-M3 ;
            skos:broader ad4gd-prop:pm1 ],
        [ qudt:hasUnit unit:MicroGM-PER-M3 ;
            skos:broader ad4gd-prop:pm2.5 ] ;
    sdo:manufacturer manuf:plantower .

<https://w3id.org/ad4gd/air-quality/sensors/PMS6003> a owl:Class,
        skos:Concept ;
    dct:description """Particle Range of measurement 0.3~1.0; 1.0~2.5; 2.5~10 Micrometer（μm）
Particle Counting Efficiency 50%@0.3µm 98%@≥0.5µm	
Particle Effective Range (PM2.5 standard）	0~500 μg/m³
Particle Maximum Range (PM2.5 standard）*	≥1000 μg/m³
Working Temperature Range	-10~+60 ℃
Working Humidity Range 0~95%（No condensation）	
Storage Temperature Range -40~+85 ℃ 
MTTF ≥10 Year
Physical Size 50mm×38mm×21mm mm
From: https://www.plantower.com/en/products_33/75.html
""" ;
    ns1:status <http://www.opengis.net/def/status/valid> ;
    rdfs:seeAlso <https://www.plantower.com/en/products_33/75.html> ;
    rdfs:subClassOf sosa:Sensor ;
    skos:inScheme <https://w3id.org/ad4gd/air-quality/sensors> ;
    skos:prefLabel "PMS6003" ;
    skos:topConceptOf <https://w3id.org/ad4gd/air-quality/sensors> ;
    sosa:observes [ qudt:hasUnit unit:MicroGM-PER-M3 ;
            skos:broader ad4gd-prop:pm2.5 ],
        [ qudt:hasUnit unit:MicroGM-PER-M3 ;
            skos:broader ad4gd-prop:pm10 ],
        [ qudt:hasUnit unit:MicroGM-PER-M3 ;
            skos:broader ad4gd-prop:pm1 ] ;
    sdo:manufacturer manuf:plantower .

<https://w3id.org/ad4gd/air-quality/sensors/PMS7003> a owl:Class,
        skos:Concept ;
    dct:description """The PMS 7003 and PMS 5003 sensors are the 7th resp 5th generation of the PMSx003 series developed by Plantower (chinese name 攀藤).
Range of measurement: 0.3~1.0; 1.0~2.5; 2.5~10 μ m
Effective Range: 0~500 μ g/m³
Maximum Range: * ≥1000 μ g/m³
Resolution: 1 μ g/m³
Standard Volume: 0.1L

From: https://aqicn.org/sensor/pms5003-7003/
""" ;
    ns1:status <http://www.opengis.net/def/status/valid> ;
    rdfs:seeAlso <https://aqicn.org/sensor/pms5003-7003/>,
        <https://www.adafruit.com/product/3686> ;
    rdfs:subClassOf sosa:Sensor ;
    skos:inScheme <https://w3id.org/ad4gd/air-quality/sensors> ;
    skos:prefLabel "PMS7003" ;
    skos:topConceptOf <https://w3id.org/ad4gd/air-quality/sensors> ;
    sosa:observes [ qudt:hasUnit unit:MicroGM-PER-M3 ;
            skos:broader ad4gd-prop:pm2.5 ],
        [ qudt:hasUnit unit:MicroGM-PER-M3 ;
            skos:broader ad4gd-prop:pm10 ],
        [ qudt:hasUnit unit:MicroGM-PER-M3 ;
            skos:broader ad4gd-prop:pm1 ] ;
    sdo:manufacturer manuf:plantower .

<https://w3id.org/ad4gd/air-quality/sensors/PPD42NS> a owl:Class,
        skos:Concept ;
    dct:description """Manufacturer: SHINYEI Technology Co. LTD.
Model: PPD42 (PPD42NS / PPD42NJ)
Detectable Particle Size: Over 1.0µm
Supply Voltage: DC 5V（4.75~5.75V）
Operating Temperature Range: 0 to 45℃
Operating Humidity Range: Less than 95%rh (No Condensation)
Output Method: Digital (Pulse) - PWM
Dimensions: 59(W) x 45(H) x 22(D) mm
Weight: 24g (Approx.)
""" ;
    ns1:status <http://www.opengis.net/def/status/valid> ;
    rdfs:seeAlso <https://aqicn.org/sensor/shinyei/>,
        <https://nettigo.eu/products/shinyei-ppd42-air-quality-sensor> ;
    rdfs:subClassOf sosa:Sensor ;
    skos:inScheme <https://w3id.org/ad4gd/air-quality/sensors> ;
    skos:prefLabel "PPD42NS" ;
    skos:topConceptOf <https://w3id.org/ad4gd/air-quality/sensors> ;
    sosa:observes [ qudt:hasUnit unit:MicroGM-PER-M3 ;
            skos:broader ad4gd-prop:pm2.5 ],
        [ qudt:hasUnit unit:MicroGM-PER-M3 ;
            skos:broader ad4gd-prop:pm10 ] ;
    sdo:manufacturer manuf:shinyei .

<https://w3id.org/ad4gd/air-quality/sensors/PlumeFlow2CO2> a owl:Class,
        skos:Concept ;
    dct:description """This is a placeholder for PlumeFlow2 carbon dioxide (CO2) sensor. The type of sensor used is unknown.
""" ;
    ns1:status <http://www.opengis.net/def/status/valid> ;
    rdfs:seeAlso <https://plumelabs.com/en/flow/>,
        <https://www.aqmd.gov/aq-spec/sensordetail/plume-labs---flow-2> ;
    rdfs:subClassOf sosa:Sensor ;
    skos:inScheme <https://w3id.org/ad4gd/air-quality/sensors> ;
    skos:prefLabel "Plume Flow 2 Carbon Dioxide (CO2) sensor" ;
    skos:topConceptOf <https://w3id.org/ad4gd/air-quality/sensors> ;
    sosa:observes [ qudt:hasUnit unit:PPM ;
            skos:broader ad4gd-prop:CO2 ] ;
    sdo:manufacturer manuf:plume-labs .

<https://w3id.org/ad4gd/air-quality/sensors/PlumeFlow2TH> a owl:Class,
        skos:Concept ;
    dct:description """This is a placeholder for PlumeFlow2 temperature and humidity sensor. The type of sensor used is unknown.
""" ;
    ns1:status <http://www.opengis.net/def/status/valid> ;
    rdfs:seeAlso <https://plumelabs.com/en/flow/>,
        <https://www.aqmd.gov/aq-spec/sensordetail/plume-labs---flow-2> ;
    rdfs:subClassOf sosa:Sensor ;
    skos:inScheme <https://w3id.org/ad4gd/air-quality/sensors> ;
    skos:prefLabel "Plume Flow 2 Air Temperature and Air Humidity sensor sensor" ;
    skos:topConceptOf <https://w3id.org/ad4gd/air-quality/sensors> ;
    sosa:observes [ qudt:hasUnit unit:DEG_C ;
            skos:broader ad4gd-prop:temperature ],
        [ qudt:hasUnit unit:PERCENT_RH ;
            skos:broader ad4gd-prop:relative-humidity ] ;
    sdo:manufacturer manuf:plume-labs .

<https://w3id.org/ad4gd/air-quality/sensors/PlumeFlow2VOC> a owl:Class,
        skos:Concept ;
    dct:description """This is a placeholder for PlumeFlow2 Volatile Organic Compounds (VOCs) sensor. The type of sensor used is unknown.
""" ;
    ns1:status <http://www.opengis.net/def/status/valid> ;
    rdfs:seeAlso <https://plumelabs.com/en/flow/>,
        <https://www.aqmd.gov/aq-spec/sensordetail/plume-labs---flow-2> ;
    rdfs:subClassOf sosa:Sensor ;
    skos:inScheme <https://w3id.org/ad4gd/air-quality/sensors> ;
    skos:prefLabel "Plume Flow 2 Volatile Organic Compounds (VOCs) sensor" ;
    skos:topConceptOf <https://w3id.org/ad4gd/air-quality/sensors> ;
    sosa:observes [ qudt:hasUnit unit:PPB ;
            skos:broader ad4gd-prop:VOC ] ;
    sdo:manufacturer manuf:plume-labs .

<https://w3id.org/ad4gd/air-quality/sensors/SCD30> a owl:Class,
        skos:Concept ;
    dct:description """CO₂ accuracy of ±(30 ppm + 3% MV) @400-10000 ppm
The SCD30 is a highly accurate CO2 sensor module based on our patented CMOSens® Technology for IR detection that includes a best-in-class humidity and temperature sensor. This allows ambient humidity and temperature to be outputted through modeling and compensating of external heat sources without the requirement for any additional components. The module’s dual-channel principle enables excellent long-term stability by design, and its ultra-thin package size allows easy integration into even the most demanding applications. 
From: https://sensirion.com/products/catalog/SCD30
""" ;
    ns1:status <http://www.opengis.net/def/status/valid> ;
    rdfs:seeAlso <https://sensirion.com/products/catalog/SCD30> ;
    rdfs:subClassOf sosa:Sensor ;
    skos:inScheme <https://w3id.org/ad4gd/air-quality/sensors> ;
    skos:prefLabel "SCD30" ;
    skos:topConceptOf <https://w3id.org/ad4gd/air-quality/sensors> ;
    sosa:observes [ qudt:hasUnit unit:DEG_C ;
            skos:broader ad4gd-prop:temperature ],
        [ qudt:hasUnit unit:PPM ;
            skos:broader ad4gd-prop:CO2 ],
        [ qudt:hasUnit unit:PERCENT_RH ;
            skos:broader ad4gd-prop:relative-humidity ] ;
    sdo:manufacturer manuf:sensirion-AG .

<https://w3id.org/ad4gd/air-quality/sensors/SDS011> a owl:Class,
        skos:Concept ;
    dct:description """This is the specification for the SDS011. One should not consider all those values for granted as there is quite often a big difference
 between what is said to be possible and what is actually possible (and this is why we are setting up all our experiments).
  Output: PM2.5, PM10
  Measuring Range: 0.0-999.9μg/m3
  Response Time 1 second
  Serial Data Output Frequency: 1 time/second
  Particle Diameter Resolution: ≤0.3μm
  Relative Error:10%
  Temperature Range:-20~50°C

Note that the SDS011 humidity working range is 0-70%. Above 70% humidity the readings become unreliable.

From: https://aqicn.org/sensor/sds011/
""" ;
    ns1:status <http://www.opengis.net/def/status/valid> ;
    rdfs:seeAlso <https://aqicn.org/sensor/sds011/> ;
    rdfs:subClassOf sosa:Sensor ;
    skos:inScheme <https://w3id.org/ad4gd/air-quality/sensors> ;
    skos:prefLabel "SDS011" ;
    skos:topConceptOf <https://w3id.org/ad4gd/air-quality/sensors> ;
    sosa:observes [ qudt:hasUnit unit:MicroGM-PER-M3 ;
            skos:broader ad4gd-prop:pm2.5 ;
            ssn:implements [ qb:order 1 ;
                    skos:broader ad4gd-procedure:pm-humidity-correction ] ],
        [ qudt:hasUnit unit:MicroGM-PER-M3 ;
            skos:broader ad4gd-prop:pm10 ;
            ssn:implements [ qb:order 1 ;
                    skos:broader ad4gd-procedure:pm-humidity-correction ] ] ;
    sdo:manufacturer manuf:nova-fitness .

<https://w3id.org/ad4gd/air-quality/sensors/SDS021> a owl:Class,
        skos:Concept ;
    dct:description """The SDS021 using principle of laser scattering,can get theparticleconcentration between 0.3 to 10μm in the air. It with digital outputandbuilt-in fan is stable and reliable.Product has passed the CE, FCCandRoHS certification.
From: https://cdn.sparkfun.com/assets/parts/1/2/2/7/5/SDS021_laser_PM2.5_sensor_specification-V1.0.pdf
""" ;
    ns1:status <http://www.opengis.net/def/status/valid> ;
    rdfs:seeAlso <https://aqicn.org/sensor/sds021/>,
        <https://cdn.sparkfun.com/assets/parts/1/2/2/7/5/SDS021_laser_PM2.5_sensor_specification-V1.0.pdf> ;
    rdfs:subClassOf sosa:Sensor ;
    skos:inScheme <https://w3id.org/ad4gd/air-quality/sensors> ;
    skos:prefLabel "SDS021" ;
    skos:topConceptOf <https://w3id.org/ad4gd/air-quality/sensors> ;
    sosa:observes [ qudt:hasUnit unit:MicroGM-PER-M3 ;
            skos:broader ad4gd-prop:pm10 ],
        [ qudt:hasUnit unit:MicroGM-PER-M3 ;
            skos:broader ad4gd-prop:pm2.5 ] ;
    sdo:manufacturer manuf:nova-fitness .

<https://w3id.org/ad4gd/air-quality/sensors/SHT11> a owl:Class,
        skos:Concept ;
    dct:description """±3% Digital humidity and temperature sensor
The SHT1x digital humidity sensor is a reflow solderable sensor. The SHT1x series consists of a low-cost version with the SHT10 humidity sensor, a standard version with the SHT11 humidity sensor, and a high-end version with the SHT15 humidity sensor. 
As with every other Sensirion sensor type from the SHTxx humidity sensor family, they are fully calibrated and provide a digital output.
From: https://sensirion.com/products/catalog/SHT11
""" ;
    ns1:status <http://www.opengis.net/def/status/valid> ;
    rdfs:seeAlso <https://sensirion.com/products/catalog/SHT11> ;
    rdfs:subClassOf sosa:Sensor ;
    skos:inScheme <https://w3id.org/ad4gd/air-quality/sensors> ;
    skos:prefLabel "SHT11" ;
    skos:topConceptOf <https://w3id.org/ad4gd/air-quality/sensors> ;
    sosa:observes [ qudt:hasUnit unit:PERCENT_RH ;
            skos:broader ad4gd-prop:relative-humidity ],
        [ qudt:hasUnit unit:DEG_C ;
            skos:broader ad4gd-prop:temperature ] ;
    sdo:manufacturer manuf:sensirion-AG .

<https://w3id.org/ad4gd/air-quality/sensors/SHT30> a owl:Class,
        skos:Concept ;
    dct:description """SHT3x-DIS is the next generation of Sensirion’s temperature and humidity sensors. It builds on a new CMOSens® sensor chip that is at the heart of Sensirion’s new humidity and temperature platform. The SHT3x-DIS has increased intelligence, reliability and improved accuracy specifications compared to its predecessor. Its functionality includes enhanced signal processing, two distinctive and user selectable I2C addresses and communication speeds of up to 1 MHz. 
From: https://www.farnell.com/datasheets/2901984.pdf
""" ;
    ns1:status <http://www.opengis.net/def/status/valid> ;
    rdfs:seeAlso <https://www.farnell.com/datasheets/2901984.pdf> ;
    rdfs:subClassOf sosa:Sensor ;
    skos:inScheme <https://w3id.org/ad4gd/air-quality/sensors> ;
    skos:prefLabel "SHT30" ;
    skos:topConceptOf <https://w3id.org/ad4gd/air-quality/sensors> ;
    sosa:observes [ qudt:hasUnit unit:PERCENT_RH ;
            skos:broader ad4gd-prop:relative-humidity ],
        [ qudt:hasUnit unit:DEG_C ;
            skos:broader ad4gd-prop:temperature ] ;
    sdo:manufacturer manuf:sensirion-AG .

<https://w3id.org/ad4gd/air-quality/sensors/SHT31> a owl:Class,
        skos:Concept ;
    dct:description """The SHT31-D sensor has an excellent ±2% relative humidity and ±0.3°C accuracy for most uses.
From: https://www.adafruit.com/product/2857'
""" ;
    ns1:status <http://www.opengis.net/def/status/valid> ;
    rdfs:seeAlso <https://www.adafruit.com/product/2857> ;
    rdfs:subClassOf sosa:Sensor ;
    skos:inScheme <https://w3id.org/ad4gd/air-quality/sensors> ;
    skos:prefLabel "SHT31" ;
    skos:topConceptOf <https://w3id.org/ad4gd/air-quality/sensors> ;
    sosa:observes [ qudt:hasUnit unit:PERCENT_RH ;
            skos:broader ad4gd-prop:relative-humidity ],
        [ qudt:hasUnit unit:DEG_C ;
            skos:broader ad4gd-prop:temperature ] ;
    sdo:manufacturer manuf:sensirion-AG .

<https://w3id.org/ad4gd/air-quality/sensors/SHT35> a owl:Class,
        skos:Concept ;
    dct:description """±1.5% Digital humidity and temperature sensor, filter membrane
The digital SHT3x humidity sensor series takes sensor technology to a new level. As the successor of the SHT2x series it sets the industry standard in humidity sensing. The SHT3x humidity sensor series consists of a low-cost version with the SHT30 humidity sensor, a standard version with the SHT31 humidity sensor, and a high-end version with the SHT35 humidity sensor.
Humidity:
Typ. relative humidity accuracy 1.5 %RH	
Operating relative humidity range 0 - 100 %RH	
Response time (τ63%) 8s	
Protective option	Filter membrane		
Calibration certificate Factory calibration	
Temperature:
Typ. temperature accuracy 0.1 °C	
Operating temperature range -40 - 125 °C	
Response time (τ63%) > 2 s	
From: https://sensirion.com/products/catalog/SHT35-DIS-F
""" ;
    ns1:status <http://www.opengis.net/def/status/valid> ;
    rdfs:seeAlso <https://sensirion.com/products/catalog/SHT35-DIS-F> ;
    rdfs:subClassOf sosa:Sensor ;
    skos:inScheme <https://w3id.org/ad4gd/air-quality/sensors> ;
    skos:prefLabel "SHT35" ;
    skos:topConceptOf <https://w3id.org/ad4gd/air-quality/sensors> ;
    sosa:observes [ qudt:hasUnit unit:DEG_C ;
            skos:broader ad4gd-prop:temperature ],
        [ qudt:hasUnit unit:PERCENT_RH ;
            skos:broader ad4gd-prop:relative-humidity ] ;
    sdo:manufacturer manuf:sensirion-AG .

<https://w3id.org/ad4gd/air-quality/sensors/SHT85> a owl:Class,
        skos:Concept ;
    dct:description """SHT85 is Sensirion’s best-in-class humidity sensor with pin-type connector for easy integration and replacement. It builds on a highly accurate and long-term stable SHT3x sensor that is at the heart of Sensirion’s new humidity and temperature platform. The unique package design allows for the best possible thermal coupling to the environment and decoupling from potential heat sources on the main board. The SHT85 features a PTFE membrane dedicated to protect the sensor opening from liquids and dust according to IP67, without affecting the response time of the RH signal. It thus allows for sensor use under harsh environmental conditions,(such as spray water and high exposure to dust). Final accuracy testing on product level ensures best performance, making the SHT85 the ultimate choice for even the most demanding applications. 
From: https://www.mouser.com/catalog/specsheets/Sensirion_10022018_HT_DS_SHT85_V0.9_D1.pdf
""" ;
    ns1:status <http://www.opengis.net/def/status/valid> ;
    rdfs:seeAlso <https://www.mouser.com/catalog/specsheets/Sensirion_10022018_HT_DS_SHT85_V0.9_D1.pdf> ;
    rdfs:subClassOf sosa:Sensor ;
    skos:inScheme <https://w3id.org/ad4gd/air-quality/sensors> ;
    skos:prefLabel "SHT85" ;
    skos:topConceptOf <https://w3id.org/ad4gd/air-quality/sensors> ;
    sosa:observes [ qudt:hasUnit unit:DEG_C ;
            skos:broader ad4gd-prop:temperature ],
        [ qudt:hasUnit unit:PERCENT_RH ;
            skos:broader ad4gd-prop:relative-humidity ] ;
    sdo:manufacturer manuf:sensirion-AG .

<https://w3id.org/ad4gd/air-quality/sensors/SPS30> a owl:Class,
        skos:Concept ;
    dct:description """PM2.5 Sensor for HVAC and air quality applications SPS30
The MCERTS-certified SPS30 particulate matter (PM) sensor marks a new technological breakthrough in optical PM sensors. Its measurement principle is based on laser scattering and makes use of Sensirion's innovative contamination-resistance technology. This technology, together with high-quality and long-lasting components, enables precise measurements from the device's first operation and throughout its lifetime of more than ten years.
Mass concentration precision ±10	%	
Mass concentration range 0 - 1000 μg/m³	
Lifetime > 10 years	
Particle size range PM1.0, PM2.5, PM4 and PM10
From: https://sensirion.com/products/catalog/SPS30
""" ;
    ns1:status <http://www.opengis.net/def/status/valid> ;
    rdfs:seeAlso <https://sensirion.com/products/catalog/SPS30> ;
    rdfs:subClassOf sosa:Sensor ;
    skos:inScheme <https://w3id.org/ad4gd/air-quality/sensors> ;
    skos:prefLabel "SPS30" ;
    skos:topConceptOf <https://w3id.org/ad4gd/air-quality/sensors> ;
    sosa:observes [ qudt:hasUnit unit:MicroGM-PER-M3 ;
            skos:broader ad4gd-prop:pm1 ],
        [ qudt:hasUnit unit:MicroGM-PER-M3 ;
            skos:broader ad4gd-prop:pm10 ],
        [ qudt:hasUnit unit:MicroGM-PER-M3 ;
            skos:broader ad4gd-prop:pm4 ],
        [ qudt:hasUnit unit:MicroGM-PER-M3 ;
            skos:broader ad4gd-prop:pm2.5 ] ;
    sdo:manufacturer manuf:sensirion-AG .

<https://w3id.org/ad4gd/air-quality/sensors/ZephyrCO> a owl:Class,
        skos:Concept ;
    dct:description """This is a placeholder for Zephyr Carbon Monoxide (CO) and Carbon Dioxide (CO2) sensor. The type of sensor used is unknown.
Carbon Monoxide and Carbon Dioxide sensor, measures CO and CO2 with 0.3 mg/m3 and 30 ppmV estimated accuracy respectively.
From: https://www.earthsense.co.uk/_files/ugd/847642_d42371301be448bab9ee526499e1e0bb.pdf
""" ;
    ns1:status <http://www.opengis.net/def/status/valid> ;
    rdfs:seeAlso <https://www.earthsense.co.uk/_files/ugd/847642_d42371301be448bab9ee526499e1e0bb.pdf>,
        <https://www.earthsense.co.uk/zephyr> ;
    rdfs:subClassOf sosa:Sensor ;
    skos:inScheme <https://w3id.org/ad4gd/air-quality/sensors> ;
    skos:prefLabel "Zephyr Carbon Monoxide (CO) and Carbon Dioxide (CO2) sensor" ;
    skos:topConceptOf <https://w3id.org/ad4gd/air-quality/sensors> ;
    sosa:observes [ qudt:hasUnit unit:PPM ;
            skos:broader ad4gd-prop:CO2 ],
        [ qudt:hasUnit unit:MilliGM-PER-M3 ;
            skos:broader ad4gd-prop:CO ] ;
    sdo:manufacturer manuf:earthsense .

<https://w3id.org/ad4gd/air-quality/sensors/ZephyrH2S> a owl:Class,
        skos:Concept ;
    dct:description """This is a placeholder for Zephyr Hydrogen Sulfide (H2S) sensor. The type of sensor used is unknown.
Hydrogen Sulfide (H2S) sensor, measures Hydrogen Sulfide with 5 µg/m3 estimated accuracy.
From: https://www.earthsense.co.uk/_files/ugd/847642_d42371301be448bab9ee526499e1e0bb.pdf
""" ;
    ns1:status <http://www.opengis.net/def/status/valid> ;
    rdfs:seeAlso <https://www.earthsense.co.uk/_files/ugd/847642_d42371301be448bab9ee526499e1e0bb.pdf>,
        <https://www.earthsense.co.uk/zephyr> ;
    rdfs:subClassOf sosa:Sensor ;
    skos:inScheme <https://w3id.org/ad4gd/air-quality/sensors> ;
    skos:prefLabel "Zephyr Hydrogen Sulfide (H2S) sensor" ;
    skos:topConceptOf <https://w3id.org/ad4gd/air-quality/sensors> ;
    sosa:observes [ qudt:hasUnit unit:MicroGM-PER-M3 ;
            skos:broader ad4gd-prop:H2S ] ;
    sdo:manufacturer manuf:earthsense .

<https://w3id.org/ad4gd/air-quality/sensors/ZephyrNO> a owl:Class,
        skos:Concept ;
    dct:description """This is a placeholder for Zephyr Nitric Oxide (NO) and Nitrogen Dioxide (NO2) sensor. The type of sensor used is unknown.
Nitric Oxide and Nitrogen Dioxide sensor, measures Nitrogen Oxides with 10 µg/m3 estimated accuracy
From: https://www.earthsense.co.uk/_files/ugd/847642_d42371301be448bab9ee526499e1e0bb.pdf
""" ;
    ns1:status <http://www.opengis.net/def/status/valid> ;
    rdfs:seeAlso <https://www.earthsense.co.uk/_files/ugd/847642_d42371301be448bab9ee526499e1e0bb.pdf>,
        <https://www.earthsense.co.uk/zephyr> ;
    rdfs:subClassOf sosa:Sensor ;
    skos:inScheme <https://w3id.org/ad4gd/air-quality/sensors> ;
    skos:prefLabel "Zephyr Nitric Oxide (NO) and Nitrogen Dioxide (NO2) sensor" ;
    skos:topConceptOf <https://w3id.org/ad4gd/air-quality/sensors> ;
    sosa:observes [ qudt:hasUnit unit:MicroGM-PER-M3 ;
            skos:broader false ],
        [ qudt:hasUnit unit:MicroGM-PER-M3 ;
            skos:broader ad4gd-prop:NO2 ] ;
    sdo:manufacturer manuf:earthsense .

<https://w3id.org/ad4gd/air-quality/sensors/ZephyrO3> a owl:Class,
        skos:Concept ;
    dct:description """This is a placeholder for Zephyr Ozone (O3) sensor. The type of sensor used is unknown.
Ozone (O3) sensor, measures Ozone with 15 µg/m3 estimated accuracy.
From: https://www.earthsense.co.uk/_files/ugd/847642_d42371301be448bab9ee526499e1e0bb.pdf
""" ;
    ns1:status <http://www.opengis.net/def/status/valid> ;
    rdfs:seeAlso <https://www.earthsense.co.uk/_files/ugd/847642_d42371301be448bab9ee526499e1e0bb.pdf>,
        <https://www.earthsense.co.uk/zephyr> ;
    rdfs:subClassOf sosa:Sensor ;
    skos:inScheme <https://w3id.org/ad4gd/air-quality/sensors> ;
    skos:prefLabel "Zephyr Ozone (O3) sensor" ;
    skos:topConceptOf <https://w3id.org/ad4gd/air-quality/sensors> ;
    sosa:observes [ qudt:hasUnit unit:MicroGM-PER-M3 ;
            skos:broader ad4gd-prop:O3 ] ;
    sdo:manufacturer manuf:earthsense .

<https://w3id.org/ad4gd/air-quality/sensors/ZephyrP> a owl:Class,
        skos:Concept ;
    dct:description """This is a placeholder for Zephyr pressure sensor. The type of sensor used is unknown.
Pressure sensor, measures pressure with 1.2 hPa esitmated accuracy.
From: https://www.earthsense.co.uk/_files/ugd/847642_d42371301be448bab9ee526499e1e0bb.pdf
""" ;
    ns1:status <http://www.opengis.net/def/status/valid> ;
    rdfs:seeAlso <https://www.earthsense.co.uk/_files/ugd/847642_d42371301be448bab9ee526499e1e0bb.pdf>,
        <https://www.earthsense.co.uk/zephyr> ;
    rdfs:subClassOf sosa:Sensor ;
    skos:inScheme <https://w3id.org/ad4gd/air-quality/sensors> ;
    skos:prefLabel "Zephyr Air Pressure sensor" ;
    skos:topConceptOf <https://w3id.org/ad4gd/air-quality/sensors> ;
    sosa:observes [ qudt:hasUnit unit:PA ;
            skos:broader ad4gd-prop:pressure ] ;
    sdo:manufacturer manuf:earthsense .

<https://w3id.org/ad4gd/air-quality/sensors/ZephyrPM> a owl:Class,
        skos:Concept ;
    dct:description """This is a placeholder for Zephyr particulate matter (PM) sensor. The type of sensor used is unknown.
Particulate sensor (laser), measures PM1, PM2.5, PM10 with 5 µg/m3 estimated accuracy.
From: https://www.earthsense.co.uk/_files/ugd/847642_d42371301be448bab9ee526499e1e0bb.pdf
""" ;
    ns1:status <http://www.opengis.net/def/status/valid> ;
    rdfs:seeAlso <https://www.earthsense.co.uk/_files/ugd/847642_d42371301be448bab9ee526499e1e0bb.pdf>,
        <https://www.earthsense.co.uk/zephyr> ;
    rdfs:subClassOf sosa:Sensor ;
    skos:inScheme <https://w3id.org/ad4gd/air-quality/sensors> ;
    skos:prefLabel "Zephyr particulate matter (PM) sensor" ;
    skos:topConceptOf <https://w3id.org/ad4gd/air-quality/sensors> ;
    sosa:observes [ qudt:hasUnit unit:MicroGM-PER-M3 ;
            skos:broader ad4gd-prop:pm2.5 ],
        [ qudt:hasUnit unit:MicroGM-PER-M3 ;
            skos:broader ad4gd-prop:pm1 ],
        [ qudt:hasUnit unit:MicroGM-PER-M3 ;
            skos:broader ad4gd-prop:pm10 ] ;
    sdo:manufacturer manuf:earthsense .

<https://w3id.org/ad4gd/air-quality/sensors/ZephyrSO2> a owl:Class,
        skos:Concept ;
    dct:description """This is a placeholder for Zephyr Sulphur Dioxide (SO2) sensor. The type of sensor used is unknown.
Sulphur Dioxide (SO2) sensor, measures Sulphur Dioxide with 20 µg/m3 estimated accuracy.
From: https://www.earthsense.co.uk/_files/ugd/847642_d42371301be448bab9ee526499e1e0bb.pdf
""" ;
    ns1:status <http://www.opengis.net/def/status/valid> ;
    rdfs:seeAlso <https://www.earthsense.co.uk/_files/ugd/847642_d42371301be448bab9ee526499e1e0bb.pdf>,
        <https://www.earthsense.co.uk/zephyr> ;
    rdfs:subClassOf sosa:Sensor ;
    skos:inScheme <https://w3id.org/ad4gd/air-quality/sensors> ;
    skos:prefLabel "Zephyr Sulphur Dioxide (SO2) sensor" ;
    skos:topConceptOf <https://w3id.org/ad4gd/air-quality/sensors> ;
    sosa:observes [ qudt:hasUnit unit:MicroGM-PER-M3 ;
            skos:broader ad4gd-prop:SO2 ] ;
    sdo:manufacturer manuf:earthsense .

<https://w3id.org/ad4gd/air-quality/sensors/ZephyrTH> a owl:Class,
        skos:Concept ;
    dct:description """This is a placeholder for Zephyr temperature and humidity sensor. The type of sensor used is unknown.
Temperature and humidity sensor, measures ambient temperature and humidity with 5ºC and 5% esitmated accuracy respectively.
From: https://www.earthsense.co.uk/_files/ugd/847642_d42371301be448bab9ee526499e1e0bb.pdf
""" ;
    ns1:status <http://www.opengis.net/def/status/valid> ;
    rdfs:seeAlso <https://www.earthsense.co.uk/_files/ugd/847642_d42371301be448bab9ee526499e1e0bb.pdf>,
        <https://www.earthsense.co.uk/zephyr> ;
    rdfs:subClassOf sosa:Sensor ;
    skos:inScheme <https://w3id.org/ad4gd/air-quality/sensors> ;
    skos:prefLabel "Zephyr Air Temperature and Air Humidity sensor" ;
    skos:topConceptOf <https://w3id.org/ad4gd/air-quality/sensors> ;
    sosa:observes [ qudt:hasUnit unit:PERCENT_RH ;
            skos:broader ad4gd-prop:relative-humidity ],
        [ qudt:hasUnit unit:DEG_C ;
            skos:broader ad4gd-prop:temperature ] ;
    sdo:manufacturer manuf:earthsense .

<https://w3id.org/ad4gd/air-quality/sensors/ZephyrVOC> a owl:Class,
        skos:Concept ;
    dct:description """This is a placeholder for Zephyr Volatile Organic Compounds (VOCs) sensor. The type of sensor used is unknown.
Volatile organic compounds (VOCs) sensor, measures VOC with a range of 0 - 15,000 ppbV c.
From: https://www.earthsense.co.uk/_files/ugd/847642_d42371301be448bab9ee526499e1e0bb.pdf
""" ;
    ns1:status <http://www.opengis.net/def/status/valid> ;
    rdfs:seeAlso <https://www.earthsense.co.uk/_files/ugd/847642_d42371301be448bab9ee526499e1e0bb.pdf>,
        <https://www.earthsense.co.uk/zephyr> ;
    rdfs:subClassOf sosa:Sensor ;
    skos:inScheme <https://w3id.org/ad4gd/air-quality/sensors> ;
    skos:prefLabel "Zephyr Volatile Organic Compounds (VOCs) sensor" ;
    skos:topConceptOf <https://w3id.org/ad4gd/air-quality/sensors> ;
    sosa:observes [ qudt:hasUnit unit:PPB ;
            skos:broader ad4gd-prop:VOC ] ;
    sdo:manufacturer manuf:earthsense .

<https://w3id.org/ad4gd/air-quality/sensors> a skos:ConceptScheme ;
    dct:source <https://ad4gd.eu/> ;
    ns1:collectionView <https://w3id.org/ad4gd/air-quality/sensors/> ;
    skos:hasTopConcept <https://w3id.org/ad4gd/air-quality/sensors/BME280>,
        <https://w3id.org/ad4gd/air-quality/sensors/BMP180>,
        <https://w3id.org/ad4gd/air-quality/sensors/BMP280>,
        <https://w3id.org/ad4gd/air-quality/sensors/DHT22>,
        <https://w3id.org/ad4gd/air-quality/sensors/DS18B20>,
        <https://w3id.org/ad4gd/air-quality/sensors/HPM>,
        <https://w3id.org/ad4gd/air-quality/sensors/HTU21D>,
        <https://w3id.org/ad4gd/air-quality/sensors/NextPM>,
        <https://w3id.org/ad4gd/air-quality/sensors/PMS1003>,
        <https://w3id.org/ad4gd/air-quality/sensors/PMS3003>,
        <https://w3id.org/ad4gd/air-quality/sensors/PMS5003>,
        <https://w3id.org/ad4gd/air-quality/sensors/PMS6003>,
        <https://w3id.org/ad4gd/air-quality/sensors/PMS7003>,
        <https://w3id.org/ad4gd/air-quality/sensors/PPD42NS>,
        <https://w3id.org/ad4gd/air-quality/sensors/PlumeFlow2CO2>,
        <https://w3id.org/ad4gd/air-quality/sensors/PlumeFlow2TH>,
        <https://w3id.org/ad4gd/air-quality/sensors/PlumeFlow2VOC>,
        <https://w3id.org/ad4gd/air-quality/sensors/SCD30>,
        <https://w3id.org/ad4gd/air-quality/sensors/SDS011>,
        <https://w3id.org/ad4gd/air-quality/sensors/SDS021>,
        <https://w3id.org/ad4gd/air-quality/sensors/SHT11>,
        <https://w3id.org/ad4gd/air-quality/sensors/SHT30>,
        <https://w3id.org/ad4gd/air-quality/sensors/SHT31>,
        <https://w3id.org/ad4gd/air-quality/sensors/SHT35>,
        <https://w3id.org/ad4gd/air-quality/sensors/SHT85>,
        <https://w3id.org/ad4gd/air-quality/sensors/SPS30>,
        <https://w3id.org/ad4gd/air-quality/sensors/ZephyrCO>,
        <https://w3id.org/ad4gd/air-quality/sensors/ZephyrH2S>,
        <https://w3id.org/ad4gd/air-quality/sensors/ZephyrNO>,
        <https://w3id.org/ad4gd/air-quality/sensors/ZephyrO3>,
        <https://w3id.org/ad4gd/air-quality/sensors/ZephyrP>,
        <https://w3id.org/ad4gd/air-quality/sensors/ZephyrPM>,
        <https://w3id.org/ad4gd/air-quality/sensors/ZephyrSO2>,
        <https://w3id.org/ad4gd/air-quality/sensors/ZephyrTH>,
        <https://w3id.org/ad4gd/air-quality/sensors/ZephyrVOC> ;
    skos:prefLabel "AD4GD air quality sensors" .

[] a prov:Activity ;
    prov:endedAtTime "2024-09-04T08:46:35.940993"^^xsd:dateTime ;
    prov:startedAtTime "2024-09-04T08:46:35.867534"^^xsd:dateTime ;
    prov:used [ a prov:Entity ;
            dct:format "application/json" ;
            dct:hasVersion "git:dd39b657e7d09026ea1600203fae9883db7d74c1" ;
            rdfs:seeAlso <file:///home/runner/work/pilot-3-air-quality/pilot-3-air-quality/rainbow/generic/sensors.yml> ] ;
    prov:wasAssociatedWith [ a prov:Agent,
                sdo:SoftwareApplication ;
            rdfs:label "OGC-NA tools" ;
            dct:hasVersion "0.3.51" ;
            rdfs:seeAlso <https://github.com/opengeospatial/ogc-na-tools> ] ;
    prov:wasInformedBy [ dct:identifier "fe36114d-db76-4d46-91ec-4c00ead00e60" ] .

_:N5cd6a0cbbd7f45bebe384b4800ba7259 a prov:Agent,
        sdo:SoftwareApplication ;
    rdfs:label "OGC-NA tools" ;
    dct:hasVersion "0.3.51" ;
    rdfs:comment "ogc.na.update_vocabs version 0.3.51" ;
    rdfs:seeAlso <https://github.com/opengeospatial/ogc-na-tools> .

